@prefix dct: <http://purl.org/dc/terms/> .
@prefix dqm: <http://www.opengis.net/def/metamodel/isodqm/> .
@prefix ns1: <https://standards.isotc211.org/19157/-3/1/dqc/content/> .
@prefix policy: <http://www.opengis.net/def/metamodel/ogc-na/> .
@prefix prov: <http://www.w3.org/ns/prov#> .
@prefix rdfs: <http://www.w3.org/2000/01/rdf-schema#> .
@prefix schema: <https://schema.org/> .
@prefix skos: <http://www.w3.org/2004/02/skos/core#> .
@prefix xsd: <http://www.w3.org/2001/XMLSchema#> .

<https://raw.githubusercontent.com/ogcincubator/iso19157-3-dqm-register/master/entailed/entailed/dqm-master.csv.ttl> a prov:Entity ;
    dct:format "text/turtle" ;
    dct:hasVersion "git:af8a68942a51ba1c1b6f0d83684f014c48d6b039" ;
    prov:wasAttributedTo _:N37c06c812c314898acd2944a2c992aa9 ;
    prov:wasGeneratedBy [ a prov:Activity ;
            rdfs:label "Entailment and validation" ;
            rdfs:comment "python ogc.na.update_vocabs -w . .ogc/catalog.ttl --batch --base-uri https://raw.githubusercontent.com/ogcincubator/iso19157-3-dqm-register/master --update --graph-store http://defs-dev.opengis.net:8061/fuseki-hosted/data" ;
            prov:endedAtTime "2024-06-22T13:25:42.866232"^^xsd:dateTime ;
            prov:startedAtTime "2024-06-22T13:25:42.848167"^^xsd:dateTime ;
            prov:used [ a prov:Entity ;
                    dct:format "text/turtle" ;
                    dct:hasVersion "git:af8a68942a51ba1c1b6f0d83684f014c48d6b039" ;
                    rdfs:seeAlso <https://raw.githubusercontent.com/ogcincubator/iso19157-3-dqm-register/master/.ogc/catalog.ttl> ],
                [ a prov:Entity ;
                    dct:format "text/turtle" ;
                    dct:hasVersion "git:af8a68942a51ba1c1b6f0d83684f014c48d6b039" ;
                    rdfs:seeAlso <https://raw.githubusercontent.com/ogcincubator/iso19157-3-dqm-register/master/entailed/dqm-master.csv.ttl> ] ;
            prov:wasAssociatedWith _:N37c06c812c314898acd2944a2c992aa9 ;
            prov:wasInformedBy [ dct:identifier "9d4cd726-f4f0-4bb7-b94c-2e769932ab25" ] ] .

<https://standards.isotc211.org/19157/-1/1/dqc/content/qualityMeasure/101> a skos:Concept ;
    dct:description "The measure will take the  value true if all the requirements in the referred data product specification are fulfilled" ;
    dct:hasVersion "1.0" ;
    policy:status <http://www.opengis.net/def/status/valid> ;
    skos:definition "indication that all requirements in the referred data product specification are fulfilled" ;
    skos:inScheme ns1:qualityMeasure ;
    skos:notation "101" ;
    skos:prefLabel "data product specification passed" .

<https://standards.isotc211.org/19157/-1/1/dqc/content/qualityMeasure/102> a skos:Concept ;
    dct:hasVersion "1.0" ;
    policy:status <http://www.opengis.net/def/status/valid> ;
    skos:definition "number of data product specification requirements that are not fulfilled by the current product/dataset" ;
    skos:inScheme ns1:qualityMeasure ;
    skos:notation "102" ;
    skos:prefLabel "data product specification fail count" .

<https://standards.isotc211.org/19157/-1/1/dqc/content/qualityMeasure/11> a skos:Concept ;
    dct:description "Which surfaces may overlap and which shall not is application dependent. Not all overlapping surfaces are necessarily erroneous. When reporting this data quality measure, the types of feature classes corresponding to the illegal overlapping surfaces shall be reported as well. See also: https://standards.isotc211.org/19157/-1/1/dqc/content/qualityMeasure/204" ;
    dct:hasVersion "1.0" ;
    dqm:elementName "conceptual consistency" ;
    policy:status <http://www.opengis.net/def/status/valid> ;
    skos:altLabel "overlapping surfaces" ;
    skos:definition "total number of erroneous overlaps within the data" ;
    skos:example """Search for surfaces that are not allowed to overlap according to the conceptual schema. In this case, forest and built-up-area are not allowed to overlap
D13288XZ.EPS""" ;
    skos:inScheme ns1:qualityMeasure ;
    skos:notation "11" ;
    skos:prefLabel "number of invalid overlaps of surfaces" .

<https://standards.isotc211.org/19157/-1/1/dqc/content/qualityMeasure/119> a skos:Concept ;
    dct:description "The value true indicates physical structure conflict" ;
    dct:hasVersion "1.0" ;
    dqm:elementName "format consistency" ;
    policy:status <http://www.opengis.net/def/status/retired> ;
    skos:definition "indication that items are stored in conflict with the physical structure of the dataset" ;
    skos:example "True (the dataset is stored in wrong file format, a shape file instead of gml)" ;
    skos:inScheme ns1:qualityMeasure ;
    skos:notation "119" ;
    skos:prefLabel "physical structure conflicts" .

<https://standards.isotc211.org/19157/-1/1/dqc/content/qualityMeasure/12> a skos:Concept ;
    dct:description "The value indicates number of items in the dataset that are not compliant with the rules of the conceptual schema in relation to the total number of these items supposed to be in the dataset" ;
    dct:hasVersion "1.0" ;
    dqm:elementName "conceptual consistency" ;
    policy:status <http://www.opengis.net/def/status/draft> ;
    skos:definition "number of items in the dataset that are not compliant with the rules of the conceptual schema in relation to the total number of these items supposed to be in the dataset" ;
    skos:example "0,02 (in a test area there is 227 objects coded as living houses in the dataset but in the universe of discourse there are 231 objects that should be coded as living houses, 4 of them was coded as farm buildings)" ;
    skos:inScheme ns1:qualityMeasure ;
    skos:notation "12" ;
    skos:prefLabel "non-compliance rate with respect to the rules of the conceptual schema" .

<https://standards.isotc211.org/19157/-1/1/dqc/content/qualityMeasure/14> a skos:Concept ;
    dct:description "The value true indicates that an item is not in conformance with its value domain)" ;
    dct:hasVersion "1.0" ;
    dqm:elementName "domain consistency" ;
    policy:status <http://www.opengis.net/def/status/valid> ;
    skos:definition "indication of if an item is not in conformance with its value domain" ;
    skos:example "True – a feature with attribute colour has the value ‘blau’, but it does not exist in the specified value domain: red, green, blue, yellow" ;
    skos:inScheme ns1:qualityMeasure ;
    skos:notation "14" ;
    skos:prefLabel "value domain non-conformance" .

<https://standards.isotc211.org/19157/-1/1/dqc/content/qualityMeasure/21> a skos:Concept ;
    dct:description "A point-curve connection exists where different curves touch. These curves have an intrinsic topological relationship that shall reflect the true constellation. If the point-curve connection contradicts the universe of discourse, the point-curve connection is faulty with respect to this data quality measure. The data quality measure counts the number of errors of this kind." ;
    dct:hasVersion "1.0" ;
    dqm:elementName "topological consistency" ;
    policy:status <http://www.opengis.net/def/status/valid> ;
    skos:altLabel "extraneous nodes" ;
    skos:definition "number of faulty point-curve connections in the dataset" ;
    skos:example "Count the number of wrong curve connections - e.g. two-point curve connections exist where only one should be present, or count all curves with more than the threshold value of 500 vertices (in which system automatically places point-curve based on vertices limitation built into software code where no spatial justification for point-curve exists)." ;
    skos:inScheme ns1:qualityMeasure ;
    skos:notation "21" ;
    skos:prefLabel "number of faulty point-curve connections" .

<https://standards.isotc211.org/19157/-1/1/dqc/content/qualityMeasure/28> a skos:Concept ;
    dct:description """https://standards.isotc211.org/19157/-3/1/dqc/content/measureDescription/MD28_1
https://standards.isotc211.org/19157/-3/1/dqc/content/measureDescription/MD28_2
https://standards.isotc211.org/19157/-3/1/dqc/content/measureDescription/MD28_3
https://standards.isotc211.org/19157/-3/1/dqc/content/measureDescription/MD28_4""" ;
    dct:hasVersion "1.0" ;
    dqm:elementName "absolute or external accuracy" ;
    policy:status <http://www.opengis.net/def/status/superseded> ;
    skos:inScheme ns1:qualityMeasure ;
    skos:notation "28" ;
    skos:prefLabel "mean value of positional uncertainties (1D, 2D and 3D)" .

<https://standards.isotc211.org/19157/-1/1/dqc/content/qualityMeasure/4> a skos:Concept ;
    dct:description "https://standards.isotc211.org/19157/-3/1/dqc/content/measureDescription/MD4" ;
    dct:hasVersion "1.0" ;
    dct:source "ISO/TS 19138 (modified)" ;
    dqm:elementName "commission" ;
    policy:status <http://www.opengis.net/def/status/valid> ;
    skos:definition "total number of exact duplications of feature instances within the data" ;
    skos:example """Features with identical attribution and identical coordinates representing the same real object, for example: two (or more) points collected on top of each other
D13288RZ.EPS two (or more) curves collected on top of each other
D13288SZ.EPS two (or more) surfaces collected on top of each other.""" ;
    skos:inScheme ns1:qualityMeasure ;
    skos:notation "4" ;
    skos:prefLabel "number of duplicate feature instances" .

<https://standards.isotc211.org/19157/-1/1/dqc/content/qualityMeasure/47> a skos:Concept ;
    dct:description "The true values of the observed coordinates X and Y are known as xt and yt. From this the estimator" ;
    dct:hasVersion "2.0" ;
    dqm:elementName "absolute or external accuracy" ;
    policy:status <http://www.opengis.net/def/status/superseded> ;
    skos:altLabel "RMSEP" ;
    skos:definition "radius of a circle around the given point, in which the true value lies with probability P" ;
    skos:inScheme ns1:qualityMeasure ;
    skos:notation "47" ;
    skos:prefLabel "root mean square error of planimetry" .

<https://standards.isotc211.org/19157/-1/1/dqc/content/qualityMeasure/49> a skos:Concept ;
    dct:description "https://standards.isotc211.org/19157/-3/1/dqc/content/measureDescription/MD49" ;
    dct:hasVersion "1.0" ;
    dqm:elementName "absolute or external accuracy" ;
    policy:status <http://www.opengis.net/def/status/valid> ;
    skos:altLabel "ACE" ;
    skos:definition "absolute horizontal accuracy of the data’s coordinates, expressed in terms of circular error at 90 % probability given that a bias is present" ;
    skos:inScheme ns1:qualityMeasure ;
    skos:notation "49" ;
    skos:prefLabel "absolute circular error at 90 % significance level of biased data" .

<https://standards.isotc211.org/19157/-1/1/dqc/content/qualityMeasure/59> a skos:Concept ;
    dct:description "The value indicates the probability for the true value of being within a lower and the upper limit of the interval." ;
    dct:hasVersion "1.0" ;
    dqm:elementName "accuracy of a time measurement" ;
    policy:status <http://www.opengis.net/def/status/valid> ;
    skos:definition "half length of the interval defined by an upper and a lower limit, in which the true value for the time instance lies with probability 99,8 %" ;
    skos:inScheme ns1:qualityMeasure ;
    skos:notation "59" ;
    skos:prefLabel "time accuracy at 99,8 % significance level" .

<https://standards.isotc211.org/19157/-1/1/dqc/content/qualityMeasure/62> a skos:Concept ;
    dct:description "https://standards.isotc211.org/19157/-3/1/dqc/content/measureDescription/MD62" ;
    dct:hasVersion "1.0" ;
    dqm:elementName "classification correctness" ;
    dqm:valueStructure "Matrix (n × n)" ;
    policy:status <http://www.opengis.net/def/status/valid> ;
    skos:altLabel "confusion matrix" ;
    skos:definition "matrix that indicates the number of items of class (i) classified as class (j)" ;
    skos:inScheme ns1:qualityMeasure ;
    skos:notation "62" ;
    skos:prefLabel "misclassification matrix" ;
    ns1:qualityMeasureParameter <https://standards.isotc211.org/19157/-1/1/dqc/content/measureParameter/MP2> .

<https://raw.githubusercontent.com/ogcincubator/iso19157-3-dqm-register/master/entailed/dqm-master.csv.ttl> a prov:Entity ;
    dct:format "text/turtle" ;
    dct:hasVersion "git:551a12d2398dad51a829a05cbb51d65f86bc74fa" ;
    prov:wasAttributedTo _:n83f2eec0677e48de9ae773dfd525f84ab1 ;
    prov:wasGeneratedBy [ a prov:Activity ;
            rdfs:label "Entailment and validation" ;
            rdfs:comment "python ogc.na.update_vocabs -w . .ogc/catalog.ttl --batch --base-uri https://raw.githubusercontent.com/ogcincubator/iso19157-3-dqm-register/master --update --graph-store http://defs-dev.opengis.net:8061/fuseki-hosted/data" ;
            prov:endedAtTime "2023-10-01T07:58:01.438516"^^xsd:dateTime ;
            prov:startedAtTime "2023-10-01T07:58:01.417145"^^xsd:dateTime ;
            prov:used [ a prov:Entity ;
                    dct:format "text/turtle" ;
                    dct:hasVersion "git:551a12d2398dad51a829a05cbb51d65f86bc74fa" ;
                    rdfs:seeAlso <https://raw.githubusercontent.com/ogcincubator/iso19157-3-dqm-register/master/ISO19157-3/dqm-master.csv.ttl> ],
                [ a prov:Entity ;
                    dct:format "text/turtle" ;
                    dct:hasVersion "git:551a12d2398dad51a829a05cbb51d65f86bc74fa" ;
                    rdfs:seeAlso <https://raw.githubusercontent.com/ogcincubator/iso19157-3-dqm-register/master/.ogc/catalog.ttl> ] ;
            prov:wasAssociatedWith _:n83f2eec0677e48de9ae773dfd525f84ab1 ;
            prov:wasInformedBy [ dct:identifier "e911eaa9-9aea-4ede-92d7-199b5054b2ad" ] ] .

ns1:qualityMeasure a skos:ConceptScheme ;
    skos:prefLabel "ISO19157-3 quality measures" .

[] a prov:Activity ;
    prov:endedAtTime "2023-09-29T12:53:03.753916"^^xsd:dateTime ;
    prov:startedAtTime "2023-09-29T12:53:03.661143"^^xsd:dateTime ;
    prov:used [ a prov:Entity ;
            dct:format "application/json" ;
            dct:hasVersion "git:64cd1c4cad8cbac4166de7abbc029b8bd1ef68a3" ;
            rdfs:seeAlso <file:///home/runner/work/iso19157-3-dqm-register/iso19157-3-dqm-register/ISO19157-3/dqm-master.csv.json> ] ;
    prov:wasAssociatedWith [ a prov:Agent,
                schema:SoftwareApplication ;
            rdfs:label "OGC-NA tools" ;
            dct:hasVersion "0.3.14" ;
            rdfs:seeAlso <https://github.com/opengeospatial/ogc-na-tools> ] ;
    prov:wasInformedBy [ dct:identifier "744d179b-e5c7-47fb-927c-da35b4cdb274" ] .

_:N37c06c812c314898acd2944a2c992aa9 a prov:Agent,
        schema:SoftwareApplication ;
    rdfs:label "OGC-NA tools" ;
    dct:hasVersion "0.3.47.dev1+g5249c1b" ;
    rdfs:comment "ogc.na.update_vocabs version 0.3.47.dev1+g5249c1b" ;
    rdfs:seeAlso <https://github.com/opengeospatial/ogc-na-tools> .

_:n83f2eec0677e48de9ae773dfd525f84ab1 a prov:Agent,
        schema:SoftwareApplication ;
    rdfs:label "OGC-NA tools" ;
    dct:hasVersion "0.3.14" ;
    rdfs:comment "ogc.na.update_vocabs version 0.3.14" ;
    rdfs:seeAlso <https://github.com/opengeospatial/ogc-na-tools> .

