<?xml version="1.0" encoding="utf-8"?>
<rdf:RDF
   xmlns:dct="http://purl.org/dc/terms/"
   xmlns:dqm="http://www.opengis.net/def/metamodel/isodqm/"
   xmlns:ns1="https://standards.isotc211.org/19157/-3/1/dqc/content/"
   xmlns:policy="http://www.opengis.net/def/metamodel/ogc-na/"
   xmlns:prov="http://www.w3.org/ns/prov#"
   xmlns:rdf="http://www.w3.org/1999/02/22-rdf-syntax-ns#"
   xmlns:rdfs="http://www.w3.org/2000/01/rdf-schema#"
   xmlns:skos="http://www.w3.org/2004/02/skos/core#"
>
  <rdf:Description rdf:about="https://standards.isotc211.org/19157/-1/1/dqc/content/qualityMeasure/4">
    <dct:hasVersion>1.0</dct:hasVersion>
    <dqm:elementName>commission</dqm:elementName>
    <skos:example>Features with identical attribution and identical coordinates representing the same real object, for example: two (or more) points collected on top of each other
D13288RZ.EPS two (or more) curves collected on top of each other
D13288SZ.EPS two (or more) surfaces collected on top of each other.</skos:example>
    <skos:notation>4</skos:notation>
    <dct:description>https://standards.isotc211.org/19157/-3/1/dqc/content/measureDescription/MD4</dct:description>
    <skos:definition>total number of exact duplications of feature instances within the data</skos:definition>
    <skos:inScheme rdf:resource="https://standards.isotc211.org/19157/-3/1/dqc/content/qualityMeasure"/>
    <skos:prefLabel>number of duplicate feature instances</skos:prefLabel>
    <rdf:type rdf:resource="http://www.w3.org/2004/02/skos/core#Concept"/>
    <dct:source>ISO/TS 19138 (modified)</dct:source>
    <policy:status rdf:resource="http://www.opengis.net/def/status/valid"/>
  </rdf:Description>
  <rdf:Description rdf:about="https://standards.isotc211.org/19157/-1/1/dqc/content/qualityMeasure/12">
    <dqm:elementName>conceptual consistency</dqm:elementName>
    <skos:inScheme rdf:resource="https://standards.isotc211.org/19157/-3/1/dqc/content/qualityMeasure"/>
    <policy:status rdf:resource="http://www.opengis.net/def/status/draft"/>
    <skos:notation>12</skos:notation>
    <rdf:type rdf:resource="http://www.w3.org/2004/02/skos/core#Concept"/>
    <dct:description>The value indicates number of items in the dataset that are not compliant with the rules of the conceptual schema in relation to the total number of these items supposed to be in the dataset</dct:description>
    <skos:example>0,02 (in a test area there is 227 objects coded as living houses in the dataset but in the universe of discourse there are 231 objects that should be coded as living houses, 4 of them was coded as farm buildings)</skos:example>
    <dct:hasVersion>1.0</dct:hasVersion>
    <skos:prefLabel>non-compliance rate with respect to the rules of the conceptual schema</skos:prefLabel>
    <skos:definition>number of items in the dataset that are not compliant with the rules of the conceptual schema in relation to the total number of these items supposed to be in the dataset</skos:definition>
  </rdf:Description>
  <rdf:Description rdf:nodeID="N7f0333a428ed4b3caf347c9286d182ef">
    <dct:format>text/turtle</dct:format>
    <rdfs:seeAlso rdf:resource="https://raw.githubusercontent.com/ogcincubator/iso19157-3-dqm-register/master/ISO19157-3/dqm-master.csv.ttl"/>
    <dct:hasVersion>git:a7dd9d78bc4a51b0d2167d32caf25ac459410f44</dct:hasVersion>
    <rdf:type rdf:resource="http://www.w3.org/ns/prov#Entity"/>
  </rdf:Description>
  <rdf:Description rdf:about="https://standards.isotc211.org/19157/-1/1/dqc/content/qualityMeasure/59">
    <skos:prefLabel>time accuracy at 99,8 % significance level</skos:prefLabel>
    <rdf:type rdf:resource="http://www.w3.org/2004/02/skos/core#Concept"/>
    <policy:status rdf:resource="http://www.opengis.net/def/status/valid"/>
    <dct:hasVersion>1.0</dct:hasVersion>
    <skos:inScheme rdf:resource="https://standards.isotc211.org/19157/-3/1/dqc/content/qualityMeasure"/>
    <skos:definition>half length of the interval defined by an upper and a lower limit, in which the true value for the time instance lies with probability 99,8 %</skos:definition>
    <skos:notation>59</skos:notation>
    <dqm:elementName>accuracy of a time measurement</dqm:elementName>
    <dct:description>The value indicates the probability for the true value of being within a lower and the upper limit of the interval.</dct:description>
  </rdf:Description>
  <rdf:Description rdf:about="https://standards.isotc211.org/19157/-1/1/dqc/content/qualityMeasure/14">
    <dct:description>The value true indicates that an item is not in conformance with its value domain)</dct:description>
    <skos:example>True – a feature with attribute colour has the value ‘blau’, but it does not exist in the specified value domain: red, green, blue, yellow</skos:example>
    <policy:status rdf:resource="http://www.opengis.net/def/status/valid"/>
    <dct:hasVersion>1.0</dct:hasVersion>
    <skos:notation>14</skos:notation>
    <skos:inScheme rdf:resource="https://standards.isotc211.org/19157/-3/1/dqc/content/qualityMeasure"/>
    <dqm:elementName>domain consistency</dqm:elementName>
    <skos:prefLabel>value domain non-conformance</skos:prefLabel>
    <skos:definition>indication of if an item is not in conformance with its value domain</skos:definition>
    <rdf:type rdf:resource="http://www.w3.org/2004/02/skos/core#Concept"/>
  </rdf:Description>
  <rdf:Description rdf:nodeID="n5d85183356704f96b0ccf6426e8d716ab2">
    <dct:format>application/json</dct:format>
    <rdf:type rdf:resource="http://www.w3.org/ns/prov#Entity"/>
    <dct:hasVersion>git:64cd1c4cad8cbac4166de7abbc029b8bd1ef68a3</dct:hasVersion>
    <rdfs:seeAlso rdf:resource="file:///home/runner/work/iso19157-3-dqm-register/iso19157-3-dqm-register/ISO19157-3/dqm-master.csv.json"/>
  </rdf:Description>
  <rdf:Description rdf:about="https://raw.githubusercontent.com/ogcincubator/iso19157-3-dqm-register/master/entailed/dqm-master.csv.ttl">
    <dct:hasVersion>git:a7dd9d78bc4a51b0d2167d32caf25ac459410f44</dct:hasVersion>
    <prov:wasGeneratedBy rdf:nodeID="Nc055ef04a57c49d09bf472a88464e0fe"/>
    <prov:wasAttributedTo rdf:nodeID="N8fc05cdcc9fe49debd52eae31414ea01"/>
    <rdf:type rdf:resource="http://www.w3.org/ns/prov#Entity"/>
    <dct:format>text/turtle</dct:format>
  </rdf:Description>
  <rdf:Description rdf:nodeID="n5d85183356704f96b0ccf6426e8d716ab1">
    <prov:startedAtTime rdf:datatype="http://www.w3.org/2001/XMLSchema#dateTime">2023-09-29T12:53:03.661143</prov:startedAtTime>
    <prov:endedAtTime rdf:datatype="http://www.w3.org/2001/XMLSchema#dateTime">2023-09-29T12:53:03.753916</prov:endedAtTime>
    <prov:wasInformedBy rdf:nodeID="n5d85183356704f96b0ccf6426e8d716ab4"/>
    <prov:wasAssociatedWith rdf:nodeID="n5d85183356704f96b0ccf6426e8d716ab3"/>
    <rdf:type rdf:resource="http://www.w3.org/ns/prov#Activity"/>
    <prov:used rdf:nodeID="n5d85183356704f96b0ccf6426e8d716ab2"/>
  </rdf:Description>
  <rdf:Description rdf:nodeID="N8fc05cdcc9fe49debd52eae31414ea01">
    <rdfs:seeAlso rdf:resource="https://github.com/opengeospatial/ogc-na-tools"/>
    <rdfs:comment>ogc.na.update_vocabs version 0.3.14</rdfs:comment>
    <rdf:type rdf:resource="http://www.w3.org/ns/prov#Agent"/>
    <rdf:type rdf:resource="https://schema.org/SoftwareApplication"/>
    <dct:hasVersion>0.3.14</dct:hasVersion>
    <rdfs:label>OGC-NA tools</rdfs:label>
  </rdf:Description>
  <rdf:Description rdf:about="https://standards.isotc211.org/19157/-1/1/dqc/content/qualityMeasure/21">
    <skos:inScheme rdf:resource="https://standards.isotc211.org/19157/-3/1/dqc/content/qualityMeasure"/>
    <skos:definition>number of faulty point-curve connections in the dataset</skos:definition>
    <dct:description>A point-curve connection exists where different curves touch. These curves have an intrinsic topological relationship that shall reflect the true constellation. If the point-curve connection contradicts the universe of discourse, the point-curve connection is faulty with respect to this data quality measure. The data quality measure counts the number of errors of this kind.</dct:description>
    <skos:notation>21</skos:notation>
    <policy:status rdf:resource="http://www.opengis.net/def/status/valid"/>
    <dct:hasVersion>1.0</dct:hasVersion>
    <skos:altLabel>extraneous nodes</skos:altLabel>
    <skos:example>Count the number of wrong curve connections - e.g. two-point curve connections exist where only one should be present, or count all curves with more than the threshold value of 500 vertices (in which system automatically places point-curve based on vertices limitation built into software code where no spatial justification for point-curve exists).</skos:example>
    <dqm:elementName>topological consistency</dqm:elementName>
    <skos:prefLabel>number of faulty point-curve connections</skos:prefLabel>
    <rdf:type rdf:resource="http://www.w3.org/2004/02/skos/core#Concept"/>
  </rdf:Description>
  <rdf:Description rdf:nodeID="N42109d1c4e9a45cf93da7f893f8bb8ef">
    <rdfs:seeAlso rdf:resource="https://github.com/opengeospatial/ogc-na-tools"/>
    <rdf:type rdf:resource="http://www.w3.org/ns/prov#Agent"/>
    <rdf:type rdf:resource="https://schema.org/SoftwareApplication"/>
    <rdfs:label>OGC-NA tools</rdfs:label>
    <rdfs:comment>ogc.na.update_vocabs version 0.3.14</rdfs:comment>
    <dct:hasVersion>0.3.14</dct:hasVersion>
  </rdf:Description>
  <rdf:Description rdf:about="https://standards.isotc211.org/19157/-1/1/dqc/content/qualityMeasure/119">
    <policy:status rdf:resource="http://www.opengis.net/def/status/retired"/>
    <dct:hasVersion>1.0</dct:hasVersion>
    <dct:description>The value true indicates physical structure conflict</dct:description>
    <skos:definition>indication that items are stored in conflict with the physical structure of the dataset</skos:definition>
    <skos:inScheme rdf:resource="https://standards.isotc211.org/19157/-3/1/dqc/content/qualityMeasure"/>
    <skos:example>True (the dataset is stored in wrong file format, a shape file instead of gml)</skos:example>
    <skos:notation>119</skos:notation>
    <dqm:elementName>format consistency</dqm:elementName>
    <rdf:type rdf:resource="http://www.w3.org/2004/02/skos/core#Concept"/>
    <skos:prefLabel>physical structure conflicts</skos:prefLabel>
  </rdf:Description>
  <rdf:Description rdf:about="https://standards.isotc211.org/19157/-1/1/dqc/content/qualityMeasure/28">
    <dqm:elementName>absolute or external accuracy</dqm:elementName>
    <dct:hasVersion>1.0</dct:hasVersion>
    <policy:status rdf:resource="http://www.opengis.net/def/status/superseded"/>
    <dct:description>https://standards.isotc211.org/19157/-3/1/dqc/content/measureDescription/MD28_1
https://standards.isotc211.org/19157/-3/1/dqc/content/measureDescription/MD28_2
https://standards.isotc211.org/19157/-3/1/dqc/content/measureDescription/MD28_3
https://standards.isotc211.org/19157/-3/1/dqc/content/measureDescription/MD28_4</dct:description>
    <skos:prefLabel>mean value of positional uncertainties (1D, 2D and 3D)</skos:prefLabel>
    <skos:notation>28</skos:notation>
    <rdf:type rdf:resource="http://www.w3.org/2004/02/skos/core#Concept"/>
    <skos:inScheme rdf:resource="https://standards.isotc211.org/19157/-3/1/dqc/content/qualityMeasure"/>
  </rdf:Description>
  <rdf:Description rdf:about="https://standards.isotc211.org/19157/-1/1/dqc/content/qualityMeasure/11">
    <skos:prefLabel>number of invalid overlaps of surfaces</skos:prefLabel>
    <skos:example>Search for surfaces that are not allowed to overlap according to the conceptual schema. In this case, forest and built-up-area are not allowed to overlap
D13288XZ.EPS</skos:example>
    <dqm:elementName>conceptual consistency</dqm:elementName>
    <policy:status rdf:resource="http://www.opengis.net/def/status/valid"/>
    <skos:inScheme rdf:resource="https://standards.isotc211.org/19157/-3/1/dqc/content/qualityMeasure"/>
    <skos:definition>total number of erroneous overlaps within the data</skos:definition>
    <dct:description>Which surfaces may overlap and which shall not is application dependent. Not all overlapping surfaces are necessarily erroneous. When reporting this data quality measure, the types of feature classes corresponding to the illegal overlapping surfaces shall be reported as well. See also: https://standards.isotc211.org/19157/-1/1/dqc/content/qualityMeasure/204</dct:description>
    <rdf:type rdf:resource="http://www.w3.org/2004/02/skos/core#Concept"/>
    <dct:hasVersion>1.0</dct:hasVersion>
    <skos:altLabel>overlapping surfaces</skos:altLabel>
    <skos:notation>11</skos:notation>
  </rdf:Description>
  <rdf:Description rdf:nodeID="Na8958dc30dfe4704a4d156ce8dab77d4">
    <dct:hasVersion>git:a7dd9d78bc4a51b0d2167d32caf25ac459410f44</dct:hasVersion>
    <rdfs:seeAlso rdf:resource="https://raw.githubusercontent.com/ogcincubator/iso19157-3-dqm-register/master/.ogc/catalog.ttl"/>
    <dct:format>text/turtle</dct:format>
    <rdf:type rdf:resource="http://www.w3.org/ns/prov#Entity"/>
  </rdf:Description>
  <rdf:Description rdf:about="https://standards.isotc211.org/19157/-1/1/dqc/content/qualityMeasure/102">
    <skos:inScheme rdf:resource="https://standards.isotc211.org/19157/-3/1/dqc/content/qualityMeasure"/>
    <skos:notation>102</skos:notation>
    <skos:prefLabel>data product specification fail count</skos:prefLabel>
    <policy:status rdf:resource="http://www.opengis.net/def/status/valid"/>
    <rdf:type rdf:resource="http://www.w3.org/2004/02/skos/core#Concept"/>
    <skos:definition>number of data product specification requirements that are not fulfilled by the current product/dataset</skos:definition>
    <dct:hasVersion>1.0</dct:hasVersion>
  </rdf:Description>
  <rdf:Description rdf:about="https://standards.isotc211.org/19157/-1/1/dqc/content/qualityMeasure/62">
    <dct:description>https://standards.isotc211.org/19157/-3/1/dqc/content/measureDescription/MD62</dct:description>
    <dct:hasVersion>1.0</dct:hasVersion>
    <dqm:valueStructure>Matrix (n × n)</dqm:valueStructure>
    <ns1:qualityMeasureParameter rdf:resource="https://standards.isotc211.org/19157/-1/1/dqc/content/measureParameter/MP2"/>
    <policy:status rdf:resource="http://www.opengis.net/def/status/valid"/>
    <skos:definition>matrix that indicates the number of items of class (i) classified as class (j)</skos:definition>
    <skos:prefLabel>misclassification matrix</skos:prefLabel>
    <skos:altLabel>confusion matrix</skos:altLabel>
    <rdf:type rdf:resource="http://www.w3.org/2004/02/skos/core#Concept"/>
    <dqm:elementName>classification correctness</dqm:elementName>
    <skos:notation>62</skos:notation>
    <skos:inScheme rdf:resource="https://standards.isotc211.org/19157/-3/1/dqc/content/qualityMeasure"/>
  </rdf:Description>
  <rdf:Description rdf:about="https://standards.isotc211.org/19157/-1/1/dqc/content/qualityMeasure/49">
    <skos:inScheme rdf:resource="https://standards.isotc211.org/19157/-3/1/dqc/content/qualityMeasure"/>
    <skos:prefLabel>absolute circular error at 90 % significance level of biased data</skos:prefLabel>
    <skos:definition>absolute horizontal accuracy of the data’s coordinates, expressed in terms of circular error at 90 % probability given that a bias is present</skos:definition>
    <dct:description>https://standards.isotc211.org/19157/-3/1/dqc/content/measureDescription/MD49</dct:description>
    <policy:status rdf:resource="http://www.opengis.net/def/status/valid"/>
    <dct:hasVersion>1.0</dct:hasVersion>
    <dqm:elementName>absolute or external accuracy</dqm:elementName>
    <rdf:type rdf:resource="http://www.w3.org/2004/02/skos/core#Concept"/>
    <skos:notation>49</skos:notation>
    <skos:altLabel>ACE</skos:altLabel>
  </rdf:Description>
  <rdf:Description rdf:about="https://standards.isotc211.org/19157/-1/1/dqc/content/qualityMeasure/47">
    <dct:description>The true values of the observed coordinates X and Y are known as xt and yt. From this the estimator</dct:description>
    <skos:definition>radius of a circle around the given point, in which the true value lies with probability P</skos:definition>
    <dct:hasVersion>2.0</dct:hasVersion>
    <skos:notation>47</skos:notation>
    <skos:prefLabel>root mean square error of planimetry</skos:prefLabel>
    <dqm:elementName>absolute or external accuracy</dqm:elementName>
    <rdf:type rdf:resource="http://www.w3.org/2004/02/skos/core#Concept"/>
    <skos:altLabel>RMSEP</skos:altLabel>
    <policy:status rdf:resource="http://www.opengis.net/def/status/superseded"/>
    <skos:inScheme rdf:resource="https://standards.isotc211.org/19157/-3/1/dqc/content/qualityMeasure"/>
  </rdf:Description>
  <rdf:Description rdf:about="https://standards.isotc211.org/19157/-1/1/dqc/content/qualityMeasure/101">
    <skos:inScheme rdf:resource="https://standards.isotc211.org/19157/-3/1/dqc/content/qualityMeasure"/>
    <skos:prefLabel>data product specification passed</skos:prefLabel>
    <policy:status rdf:resource="http://www.opengis.net/def/status/valid"/>
    <skos:definition>indication that all requirements in the referred data product specification are fulfilled</skos:definition>
    <rdf:type rdf:resource="http://www.w3.org/2004/02/skos/core#Concept"/>
    <skos:notation>101</skos:notation>
    <dct:description>The measure will take the  value true if all the requirements in the referred data product specification are fulfilled</dct:description>
    <dct:hasVersion>1.0</dct:hasVersion>
  </rdf:Description>
  <rdf:Description rdf:about="https://standards.isotc211.org/19157/-3/1/dqc/content/qualityMeasure">
    <skos:prefLabel>ISO19157-3 quality measures</skos:prefLabel>
    <rdf:type rdf:resource="http://www.w3.org/2004/02/skos/core#ConceptScheme"/>
  </rdf:Description>
  <rdf:Description rdf:nodeID="Nc055ef04a57c49d09bf472a88464e0fe">
    <prov:wasAssociatedWith rdf:nodeID="N8fc05cdcc9fe49debd52eae31414ea01"/>
    <prov:used rdf:nodeID="N7f0333a428ed4b3caf347c9286d182ef"/>
    <prov:used rdf:nodeID="Na8958dc30dfe4704a4d156ce8dab77d4"/>
    <rdf:type rdf:resource="http://www.w3.org/ns/prov#Activity"/>
    <prov:wasInformedBy rdf:nodeID="N7ae89eaaabf342df90d2bdbff1846ed8"/>
    <prov:endedAtTime rdf:datatype="http://www.w3.org/2001/XMLSchema#dateTime">2023-09-29T12:53:57.378784</prov:endedAtTime>
    <rdfs:comment>python ogc.na.update_vocabs -w . .ogc/catalog.ttl --batch --base-uri https://raw.githubusercontent.com/ogcincubator/iso19157-3-dqm-register/master --update --graph-store http://defs-dev.opengis.net:8061/fuseki-hosted/data</rdfs:comment>
    <prov:startedAtTime rdf:datatype="http://www.w3.org/2001/XMLSchema#dateTime">2023-09-29T12:53:57.352456</prov:startedAtTime>
    <rdfs:label>Entailment and validation</rdfs:label>
  </rdf:Description>
  <rdf:Description rdf:nodeID="N833d9b2e1f804682884fbc056cbd52d1">
    <prov:used rdf:nodeID="Nde18822a43234b4d9950c7041fd364c4"/>
    <prov:used rdf:nodeID="Nbd602e9f28c34bbcab46bd1b65b43e39"/>
    <rdf:type rdf:resource="http://www.w3.org/ns/prov#Activity"/>
    <rdfs:label>Entailment and validation</rdfs:label>
    <prov:startedAtTime rdf:datatype="http://www.w3.org/2001/XMLSchema#dateTime">2023-09-29T12:53:57.352456</prov:startedAtTime>
    <prov:endedAtTime rdf:datatype="http://www.w3.org/2001/XMLSchema#dateTime">2023-09-29T12:53:57.400719</prov:endedAtTime>
    <prov:wasInformedBy rdf:nodeID="Nc213c642d97047528bd7573d94bdb7aa"/>
    <rdfs:comment>python ogc.na.update_vocabs -w . .ogc/catalog.ttl --batch --base-uri https://raw.githubusercontent.com/ogcincubator/iso19157-3-dqm-register/master --update --graph-store http://defs-dev.opengis.net:8061/fuseki-hosted/data</rdfs:comment>
    <prov:wasAssociatedWith rdf:nodeID="N42109d1c4e9a45cf93da7f893f8bb8ef"/>
  </rdf:Description>
  <rdf:Description rdf:nodeID="Nbd602e9f28c34bbcab46bd1b65b43e39">
    <rdfs:seeAlso rdf:resource="https://raw.githubusercontent.com/ogcincubator/iso19157-3-dqm-register/master/.ogc/catalog.ttl"/>
    <dct:hasVersion>git:a7dd9d78bc4a51b0d2167d32caf25ac459410f44</dct:hasVersion>
    <rdf:type rdf:resource="http://www.w3.org/ns/prov#Entity"/>
    <dct:format>text/turtle</dct:format>
  </rdf:Description>
  <rdf:Description rdf:nodeID="n5d85183356704f96b0ccf6426e8d716ab3">
    <dct:hasVersion>0.3.14</dct:hasVersion>
    <rdf:type rdf:resource="http://www.w3.org/ns/prov#Agent"/>
    <rdf:type rdf:resource="https://schema.org/SoftwareApplication"/>
    <rdfs:seeAlso rdf:resource="https://github.com/opengeospatial/ogc-na-tools"/>
    <rdfs:label>OGC-NA tools</rdfs:label>
  </rdf:Description>
  <rdf:Description rdf:about="https://raw.githubusercontent.com/ogcincubator/iso19157-3-dqm-register/master/entailed/dqm-master.csv.rdf">
    <dct:hasVersion>git:a7dd9d78bc4a51b0d2167d32caf25ac459410f44</dct:hasVersion>
    <rdf:type rdf:resource="http://www.w3.org/ns/prov#Entity"/>
    <dct:format>application/rdf+xml</dct:format>
    <prov:wasGeneratedBy rdf:nodeID="N833d9b2e1f804682884fbc056cbd52d1"/>
    <prov:wasAttributedTo rdf:nodeID="N42109d1c4e9a45cf93da7f893f8bb8ef"/>
  </rdf:Description>
  <rdf:Description rdf:nodeID="Nde18822a43234b4d9950c7041fd364c4">
    <rdfs:seeAlso rdf:resource="https://raw.githubusercontent.com/ogcincubator/iso19157-3-dqm-register/master/ISO19157-3/dqm-master.csv.ttl"/>
    <dct:hasVersion>git:a7dd9d78bc4a51b0d2167d32caf25ac459410f44</dct:hasVersion>
    <rdf:type rdf:resource="http://www.w3.org/ns/prov#Entity"/>
    <dct:format>text/turtle</dct:format>
  </rdf:Description>
  <rdf:Description rdf:nodeID="N7ae89eaaabf342df90d2bdbff1846ed8">
    <dct:identifier>e954b39d-4c0f-49f9-8ecd-f1db8e95e509</dct:identifier>
  </rdf:Description>
  <rdf:Description rdf:nodeID="Nc213c642d97047528bd7573d94bdb7aa">
    <dct:identifier>e954b39d-4c0f-49f9-8ecd-f1db8e95e509</dct:identifier>
  </rdf:Description>
  <rdf:Description rdf:nodeID="n5d85183356704f96b0ccf6426e8d716ab4">
    <dct:identifier>744d179b-e5c7-47fb-927c-da35b4cdb274</dct:identifier>
  </rdf:Description>
</rdf:RDF>
