@prefix dcterms: <http://purl.org/dc/terms/> .
@prefix ns1: <http://www.opengis.net/def/metamodel/isodqm/> .
@prefix prov: <http://www.w3.org/ns/prov#> .
@prefix rdfs: <http://www.w3.org/2000/01/rdf-schema#> .
@prefix schema: <https://schema.org/> .
@prefix skos: <http://www.w3.org/2004/02/skos/core#> .
@prefix xsd: <http://www.w3.org/2001/XMLSchema#> .

<https://raw.githubusercontent.com/ogcincubator/iso19157-3-dqm-register/master/sources/entailed/BasicMeasures.csv.ttl> a prov:Entity ;
    dcterms:format "text/turtle" ;
    dcterms:hasVersion "git:4f17dcac9447f6d217612ec525843df2f94db721" ;
    prov:wasAttributedTo _:N326f6e8523af4d04800a69910af3888a ;
    prov:wasGeneratedBy [ a prov:Activity ;
            rdfs:label "Entailment and validation" ;
            rdfs:comment "python ogc.na.update_vocabs -w . .ogc/catalog.ttl --batch --base-uri https://raw.githubusercontent.com/ogcincubator/iso19157-3-dqm-register/master --update --graph-store http://defs-dev.opengis.net:8061/fuseki-hosted/data" ;
            prov:endedAtTime "2024-09-11T12:20:18.559794"^^xsd:dateTime ;
            prov:startedAtTime "2024-09-11T12:20:17.380209"^^xsd:dateTime ;
            prov:used [ a prov:Entity ;
                    dcterms:format "text/turtle" ;
                    dcterms:hasVersion "git:4f17dcac9447f6d217612ec525843df2f94db721" ;
                    rdfs:seeAlso <https://raw.githubusercontent.com/ogcincubator/iso19157-3-dqm-register/master/sources/BasicMeasures.csv.ttl> ],
                [ a prov:Entity ;
                    rdfs:seeAlso <entailments.shapes.ttl> ],
                [ a prov:Entity ;
                    dcterms:format "text/turtle" ;
                    dcterms:hasVersion "git:4f17dcac9447f6d217612ec525843df2f94db721" ;
                    rdfs:seeAlso <https://raw.githubusercontent.com/ogcincubator/iso19157-3-dqm-register/master/.ogc/catalog.ttl> ] ;
            prov:wasAssociatedWith _:N326f6e8523af4d04800a69910af3888a ;
            prov:wasInformedBy [ dcterms:identifier "fd69c946-3328-4566-8849-8d051541eb48" ] ] .

<https://standards.isotc211.org/19157/-3/1/dqc/content/basicMeasure/BM1> a skos:Concept ;
    ns1:measureDescription <https://standards.isotc211.org/19157/-3/1/dqc/content/measureDescription/MDBM1> ;
    ns1:valueType <http://def.isotc211.org/iso19103/2015/PrimitiveTypes/Boolean> ;
    skos:definition "Indicator that an item is in error." ;
    skos:example "False" ;
    skos:inScheme <https://standards.isotc211.org/19157/-3/1/dqc/content/basicMeasure> ;
    skos:prefLabel "error indicator" .

<https://standards.isotc211.org/19157/-3/1/dqc/content/basicMeasure/BM2> a skos:Concept ;
    ns1:measureDescription <https://standards.isotc211.org/19157/-3/1/dqc/content/measureDescription/MDBM2> ;
    ns1:valueType <http://def.isotc211.org/iso19103/2015/PrimitiveTypes/Real> ;
    skos:definition "Number of the erroneous items with respect to the total number of items that should have been present." ;
    skos:example "MD2bme" ;
    skos:inScheme <https://standards.isotc211.org/19157/-3/1/dqc/content/basicMeasure> ;
    skos:prefLabel "error rate" .

<https://standards.isotc211.org/19157/-3/1/dqc/content/basicMeasure/BM3> a skos:Concept ;
    ns1:measureDescription <https://standards.isotc211.org/19157/-3/1/dqc/content/measureDescription/MDBM3> ;
    ns1:valueType <http://def.isotc211.org/iso19103/2015/PrimitiveTypes/Integer> ;
    skos:definition "Total number of items that are subject to an error of a specified type." ;
    skos:example "11" ;
    skos:inScheme <https://standards.isotc211.org/19157/-3/1/dqc/content/basicMeasure> ;
    skos:prefLabel "error count" .

<https://standards.isotc211.org/19157/-3/1/dqc/content/basicMeasure/BM4> a skos:Concept ;
    ns1:measureDescription <https://standards.isotc211.org/19157/-3/1/dqc/content/measureDescription/MDBM4> ;
    ns1:valueType <http://def.isotc211.org/iso19103/2015/PrimitiveTypes/Boolean> ;
    skos:definition "Indicator that an item is correct." ;
    skos:example "True" ;
    skos:inScheme <https://standards.isotc211.org/19157/-3/1/dqc/content/basicMeasure> ;
    skos:prefLabel "correctness indicator" .

<https://standards.isotc211.org/19157/-3/1/dqc/content/basicMeasure/BM5> a skos:Concept ;
    ns1:measureDescription <https://standards.isotc211.org/19157/-3/1/dqc/content/measureDescription/MDBM5> ;
    ns1:valueType <http://def.isotc211.org/iso19103/2015/PrimitiveTypes/Integer> ;
    skos:definition "Total number of items that are free of errors of a specified type." ;
    skos:example "571" ;
    skos:inScheme <https://standards.isotc211.org/19157/-3/1/dqc/content/basicMeasure> ;
    skos:prefLabel "correct items count" .

<https://standards.isotc211.org/19157/-3/1/dqc/content/basicMeasure/BM6> a skos:Concept ;
    ns1:measureDescription <https://standards.isotc211.org/19157/-3/1/dqc/content/measureDescription/MDBM6> ;
    ns1:valueType <http://def.isotc211.org/iso19103/2015/PrimitiveTypes/Real> ;
    skos:definition "Number of the correct items with respect to the total number of items that should have been present." ;
    skos:example "0.9811" ;
    skos:inScheme <https://standards.isotc211.org/19157/-3/1/dqc/content/basicMeasure> ;
    skos:prefLabel "correct items rate" .

<https://standards.isotc211.org/19157/-3/1/dqc/content/basicMeasure/CE39.4> a skos:Concept ;
    ns1:measureDescription <https://standards.isotc211.org/19157/-3/1/dqc/content/measureDescription/MDsd1xy_CE39.4> ;
    ns1:valueType <http://def.isotc211.org/iso19103/2015/PrimitiveTypes/Measure> ;
    skos:definition "confidence interval in two dimensions given by the probability P=39,4 % of the true value within an area" ;
    skos:inScheme <https://standards.isotc211.org/19157/-3/1/dqc/content/basicMeasure> ;
    skos:prefLabel "2D random variable 39.4 % probability" .

<https://standards.isotc211.org/19157/-3/1/dqc/content/basicMeasure/CE50> a skos:Concept ;
    ns1:measureDescription <https://standards.isotc211.org/19157/-3/1/dqc/content/measureDescription/MDsd1xy_CE50> ;
    ns1:valueType <http://def.isotc211.org/iso19103/2015/PrimitiveTypes/Measure> ;
    skos:definition "2D random variable 50 % probability" ;
    skos:inScheme <https://standards.isotc211.org/19157/-3/1/dqc/content/basicMeasure> ;
    skos:prefLabel "2D random variable 50 % probability" .

<https://standards.isotc211.org/19157/-3/1/dqc/content/basicMeasure/CE90> a skos:Concept ;
    ns1:measureDescription <https://standards.isotc211.org/19157/-3/1/dqc/content/measureDescription/MDsd1xy_CE90> ;
    ns1:valueType <http://def.isotc211.org/iso19103/2015/PrimitiveTypes/Measure> ;
    skos:definition "2D random variable 90 % probability" ;
    skos:inScheme <https://standards.isotc211.org/19157/-3/1/dqc/content/basicMeasure> ;
    skos:prefLabel "2D random variable 90 % probability" .

<https://standards.isotc211.org/19157/-3/1/dqc/content/basicMeasure/CE95> a skos:Concept ;
    ns1:measureDescription <https://standards.isotc211.org/19157/-3/1/dqc/content/measureDescription/MDsd1xy_CE95> ;
    ns1:valueType <http://def.isotc211.org/iso19103/2015/PrimitiveTypes/Measure> ;
    skos:definition "2D random variable 95 % probability" ;
    skos:inScheme <https://standards.isotc211.org/19157/-3/1/dqc/content/basicMeasure> ;
    skos:prefLabel "2D random variable 95 % probability" .

<https://standards.isotc211.org/19157/-3/1/dqc/content/basicMeasure/CE99.8> a skos:Concept ;
    ns1:measureDescription <https://standards.isotc211.org/19157/-3/1/dqc/content/measureDescription/MDsd1xy_CE99.8> ;
    ns1:valueType <http://def.isotc211.org/iso19103/2015/PrimitiveTypes/Measure> ;
    skos:definition "2D random variable 99.8 % probability" ;
    skos:inScheme <https://standards.isotc211.org/19157/-3/1/dqc/content/basicMeasure> ;
    skos:prefLabel "2D random variable 99.8 % probability" .

<https://standards.isotc211.org/19157/-3/1/dqc/content/basicMeasure/LE50> a skos:Concept ;
    ns1:measureDescription <https://standards.isotc211.org/19157/-3/1/dqc/content/measureDescription/MDsd1_LE50> ;
    ns1:valueType <http://def.isotc211.org/iso19103/2015/PrimitiveTypes/Measure> ;
    skos:definition "Confidence interval given by the probability P=50 % of the true value being between the lower and upper limit." ;
    skos:inScheme <https://standards.isotc211.org/19157/-3/1/dqc/content/basicMeasure> ;
    skos:prefLabel "1D variable 50 % probability" .

<https://standards.isotc211.org/19157/-3/1/dqc/content/basicMeasure/LE50r1> a skos:Concept ;
    ns1:measureDescription <https://standards.isotc211.org/19157/-3/1/dqc/content/measureDescription/MDsd2_LE50r1> ;
    ns1:valueType <http://def.isotc211.org/iso19103/2015/PrimitiveTypes/Measure> ;
    skos:definition "Confidence interval for probability P=50 % derived from t-distribution by 1 redundant measurement." ;
    skos:inScheme <https://standards.isotc211.org/19157/-3/1/dqc/content/basicMeasure> ;
    skos:prefLabel "1D variable 50 % probability; 1 redundant measurement" .

<https://standards.isotc211.org/19157/-3/1/dqc/content/basicMeasure/LE50r10> a skos:Concept ;
    ns1:measureDescription <https://standards.isotc211.org/19157/-3/1/dqc/content/measureDescription/MDsd2_LE50r10> ;
    ns1:valueType <http://def.isotc211.org/iso19103/2015/PrimitiveTypes/Measure> ;
    skos:definition "Confidence interval for probability P=50 % derived from t-distribution by 10 redundant measurements." ;
    skos:inScheme <https://standards.isotc211.org/19157/-3/1/dqc/content/basicMeasure> ;
    skos:prefLabel "1D variable 50 % probability; 10 redundant measurements" .

<https://standards.isotc211.org/19157/-3/1/dqc/content/basicMeasure/LE50r2> a skos:Concept ;
    ns1:measureDescription <https://standards.isotc211.org/19157/-3/1/dqc/content/measureDescription/MDsd2_LE50r2> ;
    ns1:valueType <http://def.isotc211.org/iso19103/2015/PrimitiveTypes/Measure> ;
    skos:definition "Confidence interval for probability P=50 % derived from t-distribution by 2 redundant measurements." ;
    skos:inScheme <https://standards.isotc211.org/19157/-3/1/dqc/content/basicMeasure> ;
    skos:prefLabel "1D variable 50 % probability; 2 redundant measurements" .

<https://standards.isotc211.org/19157/-3/1/dqc/content/basicMeasure/LE50r3> a skos:Concept ;
    ns1:measureDescription <https://standards.isotc211.org/19157/-3/1/dqc/content/measureDescription/MDsd2_LE50r3> ;
    ns1:valueType <http://def.isotc211.org/iso19103/2015/PrimitiveTypes/Measure> ;
    skos:definition "Confidence interval for probability P=50 % derived from t-distribution by 3 redundant measurements." ;
    skos:inScheme <https://standards.isotc211.org/19157/-3/1/dqc/content/basicMeasure> ;
    skos:prefLabel "1D variable 50 % probability; 3 redundant measurements" .

<https://standards.isotc211.org/19157/-3/1/dqc/content/basicMeasure/LE50r4> a skos:Concept ;
    ns1:measureDescription <https://standards.isotc211.org/19157/-3/1/dqc/content/measureDescription/MDsd2_LE50r4> ;
    ns1:valueType <http://def.isotc211.org/iso19103/2015/PrimitiveTypes/Measure> ;
    skos:definition "Confidence interval for probability P=50 % derived from t-distribution by 4 redundant measurements." ;
    skos:inScheme <https://standards.isotc211.org/19157/-3/1/dqc/content/basicMeasure> ;
    skos:prefLabel "1D variable 50 % probability; 4 redundant measurements" .

<https://standards.isotc211.org/19157/-3/1/dqc/content/basicMeasure/LE50r5> a skos:Concept ;
    ns1:measureDescription <https://standards.isotc211.org/19157/-3/1/dqc/content/measureDescription/MDsd2_LE50r5> ;
    ns1:valueType <http://def.isotc211.org/iso19103/2015/PrimitiveTypes/Measure> ;
    skos:definition "Confidence interval for probability P=50 % derived from t-distribution by 5 redundant measurements." ;
    skos:inScheme <https://standards.isotc211.org/19157/-3/1/dqc/content/basicMeasure> ;
    skos:prefLabel "1D variable 50 % probability; 5 redundant measurements" .

<https://standards.isotc211.org/19157/-3/1/dqc/content/basicMeasure/LE68.3> a skos:Concept ;
    ns1:measureDescription <https://standards.isotc211.org/19157/-3/1/dqc/content/measureDescription/MDsd1_LE68.3> ;
    ns1:valueType <http://def.isotc211.org/iso19103/2015/PrimitiveTypes/Measure> ;
    skos:definition "Confidence interval given by the probability P=68,3 % of the true value being between the lower and upper limit" ;
    skos:inScheme <https://standards.isotc211.org/19157/-3/1/dqc/content/basicMeasure> ;
    skos:prefLabel "1D variable 68.3 % probability" .

<https://standards.isotc211.org/19157/-3/1/dqc/content/basicMeasure/LE68.3r1> a skos:Concept ;
    ns1:measureDescription <https://standards.isotc211.org/19157/-3/1/dqc/content/measureDescription/MDsd2_LE68.3r1> ;
    ns1:valueType <http://def.isotc211.org/iso19103/2015/PrimitiveTypes/Measure> ;
    skos:definition "Confidence interval for probability P=68,3 % derived from t-distribution by 1 redundant measurement." ;
    skos:inScheme <https://standards.isotc211.org/19157/-3/1/dqc/content/basicMeasure> ;
    skos:prefLabel "1D variable 68.3 % probability; 1 redundant measurement" .

<https://standards.isotc211.org/19157/-3/1/dqc/content/basicMeasure/LE68.3r10> a skos:Concept ;
    ns1:measureDescription <https://standards.isotc211.org/19157/-3/1/dqc/content/measureDescription/MDsd2_LE68.3r10> ;
    ns1:valueType <http://def.isotc211.org/iso19103/2015/PrimitiveTypes/Measure> ;
    skos:definition "Confidence interval for probability P=68,3 % derived from t-distribution by 10 redundant measurements." ;
    skos:inScheme <https://standards.isotc211.org/19157/-3/1/dqc/content/basicMeasure> ;
    skos:prefLabel "1D variable 68.3 % probability; 10 redundant measurements" .

<https://standards.isotc211.org/19157/-3/1/dqc/content/basicMeasure/LE68.3r2> a skos:Concept ;
    ns1:measureDescription <https://standards.isotc211.org/19157/-3/1/dqc/content/measureDescription/MDsd2_LE68.3r2> ;
    ns1:valueType <http://def.isotc211.org/iso19103/2015/PrimitiveTypes/Measure> ;
    skos:definition "Confidence interval for probability P=68,3 % derived from t-distribution by 2 redundant measurements." ;
    skos:inScheme <https://standards.isotc211.org/19157/-3/1/dqc/content/basicMeasure> ;
    skos:prefLabel "1D variable 68.3 % probability; 2 redundant measurements" .

<https://standards.isotc211.org/19157/-3/1/dqc/content/basicMeasure/LE68.3r3> a skos:Concept ;
    ns1:measureDescription <https://standards.isotc211.org/19157/-3/1/dqc/content/measureDescription/MDsd2_LE68.3r3> ;
    ns1:valueType <http://def.isotc211.org/iso19103/2015/PrimitiveTypes/Measure> ;
    skos:definition "Confidence interval for probability P=68,3 % derived from t-distribution by 3 redundant measurements." ;
    skos:inScheme <https://standards.isotc211.org/19157/-3/1/dqc/content/basicMeasure> ;
    skos:prefLabel "1D variable 68.3 % probability; 3 redundant measurements" .

<https://standards.isotc211.org/19157/-3/1/dqc/content/basicMeasure/LE68.3r4> a skos:Concept ;
    ns1:measureDescription <https://standards.isotc211.org/19157/-3/1/dqc/content/measureDescription/MDsd2_LE68.3r4> ;
    ns1:valueType <http://def.isotc211.org/iso19103/2015/PrimitiveTypes/Measure> ;
    skos:definition "Confidence interval for probability P=68,3 % derived from t-distribution by 4 redundant measurements." ;
    skos:inScheme <https://standards.isotc211.org/19157/-3/1/dqc/content/basicMeasure> ;
    skos:prefLabel "1D variable 68.3 % probability; 4 redundant measurements" .

<https://standards.isotc211.org/19157/-3/1/dqc/content/basicMeasure/LE68.3r5> a skos:Concept ;
    ns1:measureDescription <https://standards.isotc211.org/19157/-3/1/dqc/content/measureDescription/MDsd2_LE68.3r5> ;
    ns1:valueType <http://def.isotc211.org/iso19103/2015/PrimitiveTypes/Measure> ;
    skos:definition "Confidence interval for probability P=68,3 % derived from t-distribution by 5 redundant measurements." ;
    skos:inScheme <https://standards.isotc211.org/19157/-3/1/dqc/content/basicMeasure> ;
    skos:prefLabel "1D variable 68.3 % probability; 5 redundant measurements" .

<https://standards.isotc211.org/19157/-3/1/dqc/content/basicMeasure/LE90> a skos:Concept ;
    ns1:measureDescription <https://standards.isotc211.org/19157/-3/1/dqc/content/measureDescription/MDsd1_LE90> ;
    ns1:valueType <http://def.isotc211.org/iso19103/2015/PrimitiveTypes/Measure> ;
    skos:definition "Confidence interval given by the probability P=90 % of the true value being between the lower and upper limit." ;
    skos:inScheme <https://standards.isotc211.org/19157/-3/1/dqc/content/basicMeasure> ;
    skos:prefLabel "1D variable 90 % probability" .

<https://standards.isotc211.org/19157/-3/1/dqc/content/basicMeasure/LE90r1> a skos:Concept ;
    ns1:measureDescription <https://standards.isotc211.org/19157/-3/1/dqc/content/measureDescription/MDsd2_LE90r1> ;
    ns1:valueType <http://def.isotc211.org/iso19103/2015/PrimitiveTypes/Measure> ;
    skos:definition "Confidence interval for probability P=90 % derived from t-distribution by 1 redundant measurement." ;
    skos:inScheme <https://standards.isotc211.org/19157/-3/1/dqc/content/basicMeasure> ;
    skos:prefLabel "1D variable 90 % probability; 1 redundant measurement" .

<https://standards.isotc211.org/19157/-3/1/dqc/content/basicMeasure/LE90r10> a skos:Concept ;
    ns1:measureDescription <https://standards.isotc211.org/19157/-3/1/dqc/content/measureDescription/MDsd2_LE90r10> ;
    ns1:valueType <http://def.isotc211.org/iso19103/2015/PrimitiveTypes/Measure> ;
    skos:definition "Confidence interval for probability P=90 % derived from t-distribution by 10 redundant measurements." ;
    skos:inScheme <https://standards.isotc211.org/19157/-3/1/dqc/content/basicMeasure> ;
    skos:prefLabel "1D variable 90 % probability; 10 redundant measurements" .

<https://standards.isotc211.org/19157/-3/1/dqc/content/basicMeasure/LE90r2> a skos:Concept ;
    ns1:measureDescription <https://standards.isotc211.org/19157/-3/1/dqc/content/measureDescription/MDsd2_LE90r2> ;
    ns1:valueType <http://def.isotc211.org/iso19103/2015/PrimitiveTypes/Measure> ;
    skos:definition "Confidence interval for probability P=90 % derived from t-distribution by 2 redundant measurements." ;
    skos:inScheme <https://standards.isotc211.org/19157/-3/1/dqc/content/basicMeasure> ;
    skos:prefLabel "1D variable 90 % probability; 2 redundant measurements" .

<https://standards.isotc211.org/19157/-3/1/dqc/content/basicMeasure/LE90r3> a skos:Concept ;
    ns1:measureDescription <https://standards.isotc211.org/19157/-3/1/dqc/content/measureDescription/MDsd2_LE90r3> ;
    ns1:valueType <http://def.isotc211.org/iso19103/2015/PrimitiveTypes/Measure> ;
    skos:definition "Confidence interval for probability P=90 % derived from t-distribution by 3 redundant measurements." ;
    skos:inScheme <https://standards.isotc211.org/19157/-3/1/dqc/content/basicMeasure> ;
    skos:prefLabel "1D variable 90 % probability; 3 redundant measurements" .

<https://standards.isotc211.org/19157/-3/1/dqc/content/basicMeasure/LE90r4> a skos:Concept ;
    ns1:measureDescription <https://standards.isotc211.org/19157/-3/1/dqc/content/measureDescription/MDsd2_LE90r4> ;
    ns1:valueType <http://def.isotc211.org/iso19103/2015/PrimitiveTypes/Measure> ;
    skos:definition "Confidence interval for probability P=90 % derived from t-distribution by 4 redundant measurements." ;
    skos:inScheme <https://standards.isotc211.org/19157/-3/1/dqc/content/basicMeasure> ;
    skos:prefLabel "1D variable 90 % probability; 4 redundant measurements" .

<https://standards.isotc211.org/19157/-3/1/dqc/content/basicMeasure/LE90r5> a skos:Concept ;
    ns1:measureDescription <https://standards.isotc211.org/19157/-3/1/dqc/content/measureDescription/MDsd2_LE90r5> ;
    ns1:valueType <http://def.isotc211.org/iso19103/2015/PrimitiveTypes/Measure> ;
    skos:definition "Confidence interval for probability P=90 % derived from t-distribution by 5 redundant measurements." ;
    skos:inScheme <https://standards.isotc211.org/19157/-3/1/dqc/content/basicMeasure> ;
    skos:prefLabel "1D variable 90 % probability; 5 redundant measurements" .

<https://standards.isotc211.org/19157/-3/1/dqc/content/basicMeasure/LE95> a skos:Concept ;
    ns1:measureDescription <https://standards.isotc211.org/19157/-3/1/dqc/content/measureDescription/MDsd1_LE95> ;
    ns1:valueType <http://def.isotc211.org/iso19103/2015/PrimitiveTypes/Measure> ;
    skos:definition "Confidence interval given by the probability P=95 % of the true value being between the lower and upper limit." ;
    skos:inScheme <https://standards.isotc211.org/19157/-3/1/dqc/content/basicMeasure> ;
    skos:prefLabel "1D variable 95 % probability" .

<https://standards.isotc211.org/19157/-3/1/dqc/content/basicMeasure/LE95r1> a skos:Concept ;
    ns1:measureDescription <https://standards.isotc211.org/19157/-3/1/dqc/content/measureDescription/MDsd2_LE95r1> ;
    ns1:valueType <http://def.isotc211.org/iso19103/2015/PrimitiveTypes/Measure> ;
    skos:definition "Confidence interval for probability P=95 % derived from t-distribution by 1 redundant measurement." ;
    skos:inScheme <https://standards.isotc211.org/19157/-3/1/dqc/content/basicMeasure> ;
    skos:prefLabel "1D variable 95 % probability; 1 redundant measurement" .

<https://standards.isotc211.org/19157/-3/1/dqc/content/basicMeasure/LE95r10> a skos:Concept ;
    ns1:measureDescription <https://standards.isotc211.org/19157/-3/1/dqc/content/measureDescription/MDsd2_LE95r10> ;
    ns1:valueType <http://def.isotc211.org/iso19103/2015/PrimitiveTypes/Measure> ;
    skos:definition "Confidence interval for probability P=95 % derived from t-distribution by 10 redundant measurements." ;
    skos:inScheme <https://standards.isotc211.org/19157/-3/1/dqc/content/basicMeasure> ;
    skos:prefLabel "1D variable 95 % probability; 10 redundant measurements" .

<https://standards.isotc211.org/19157/-3/1/dqc/content/basicMeasure/LE95r2> a skos:Concept ;
    ns1:measureDescription <https://standards.isotc211.org/19157/-3/1/dqc/content/measureDescription/MDsd2_LE95r2> ;
    ns1:valueType <http://def.isotc211.org/iso19103/2015/PrimitiveTypes/Measure> ;
    skos:definition "Confidence interval for probability P=95 % derived from t-distribution by 2 redundant measurements." ;
    skos:inScheme <https://standards.isotc211.org/19157/-3/1/dqc/content/basicMeasure> ;
    skos:prefLabel "1D variable 95 % probability; 2 redundant measurements" .

<https://standards.isotc211.org/19157/-3/1/dqc/content/basicMeasure/LE95r3> a skos:Concept ;
    ns1:measureDescription <https://standards.isotc211.org/19157/-3/1/dqc/content/measureDescription/MDsd2_LE95r3> ;
    ns1:valueType <http://def.isotc211.org/iso19103/2015/PrimitiveTypes/Measure> ;
    skos:definition "Confidence interval for probability P=95 % derived from t-distribution by 3 redundant measurements." ;
    skos:inScheme <https://standards.isotc211.org/19157/-3/1/dqc/content/basicMeasure> ;
    skos:prefLabel "1D variable 95 % probability; 3 redundant measurements" .

<https://standards.isotc211.org/19157/-3/1/dqc/content/basicMeasure/LE95r4> a skos:Concept ;
    ns1:measureDescription <https://standards.isotc211.org/19157/-3/1/dqc/content/measureDescription/MDsd2_LE95r4> ;
    ns1:valueType <http://def.isotc211.org/iso19103/2015/PrimitiveTypes/Measure> ;
    skos:definition "Confidence interval for probability P=95 % derived from t-distribution by 4 redundant measurements." ;
    skos:inScheme <https://standards.isotc211.org/19157/-3/1/dqc/content/basicMeasure> ;
    skos:prefLabel "1D variable 95 % probability; 4 redundant measurements" .

<https://standards.isotc211.org/19157/-3/1/dqc/content/basicMeasure/LE95r5> a skos:Concept ;
    ns1:measureDescription <https://standards.isotc211.org/19157/-3/1/dqc/content/measureDescription/MDsd2_LE95r5> ;
    ns1:valueType <http://def.isotc211.org/iso19103/2015/PrimitiveTypes/Measure> ;
    skos:definition "Confidence interval for probability P=95 % derived from t-distribution by 5 redundant measurements." ;
    skos:inScheme <https://standards.isotc211.org/19157/-3/1/dqc/content/basicMeasure> ;
    skos:prefLabel "1D variable 95 % probability; 5 redundant measurements" .

<https://standards.isotc211.org/19157/-3/1/dqc/content/basicMeasure/LE99> a skos:Concept ;
    ns1:measureDescription <https://standards.isotc211.org/19157/-3/1/dqc/content/measureDescription/MDsd1_LE99> ;
    ns1:valueType <http://def.isotc211.org/iso19103/2015/PrimitiveTypes/Measure> ;
    skos:definition "Confidence interval given by the probability P=99 % of the true value being between the lower and upper limit." ;
    skos:inScheme <https://standards.isotc211.org/19157/-3/1/dqc/content/basicMeasure> ;
    skos:prefLabel "1D variable 99 % probability" .

<https://standards.isotc211.org/19157/-3/1/dqc/content/basicMeasure/LE99.8> a skos:Concept ;
    ns1:measureDescription <https://standards.isotc211.org/19157/-3/1/dqc/content/measureDescription/MDsd1_LE99.8> ;
    ns1:valueType <http://def.isotc211.org/iso19103/2015/PrimitiveTypes/Measure> ;
    skos:definition "confidence interval given by the probability P=99,8 % of the true value being between the lower and upper limit" ;
    skos:inScheme <https://standards.isotc211.org/19157/-3/1/dqc/content/basicMeasure> ;
    skos:prefLabel "One dimensional variable 99,8 % probability" .

<https://standards.isotc211.org/19157/-3/1/dqc/content/basicMeasure/LE99.8r1> a skos:Concept ;
    ns1:measureDescription <https://standards.isotc211.org/19157/-3/1/dqc/content/measureDescription/MDsd2_LE99.8r1> ;
    ns1:valueType <http://def.isotc211.org/iso19103/2015/PrimitiveTypes/Measure> ;
    skos:definition "Confidence interval for probability P=99,8 % derived from t-distribution by 1 redundant measurement." ;
    skos:inScheme <https://standards.isotc211.org/19157/-3/1/dqc/content/basicMeasure> ;
    skos:prefLabel "1D variable 99.8 % probability; 1 redundant measurement" .

<https://standards.isotc211.org/19157/-3/1/dqc/content/basicMeasure/LE99.8r10> a skos:Concept ;
    ns1:measureDescription <https://standards.isotc211.org/19157/-3/1/dqc/content/measureDescription/MDsd2_LE99.8r10> ;
    ns1:valueType <http://def.isotc211.org/iso19103/2015/PrimitiveTypes/Measure> ;
    skos:definition "Confidence interval for probability P=99,8 % derived from t-distribution by 10 redundant measurements." ;
    skos:inScheme <https://standards.isotc211.org/19157/-3/1/dqc/content/basicMeasure> ;
    skos:prefLabel "1D variable 99.8 % probability; 10 redundant measurements" .

<https://standards.isotc211.org/19157/-3/1/dqc/content/basicMeasure/LE99.8r2> a skos:Concept ;
    ns1:measureDescription <https://standards.isotc211.org/19157/-3/1/dqc/content/measureDescription/MDsd2_LE99.8r2> ;
    ns1:valueType <http://def.isotc211.org/iso19103/2015/PrimitiveTypes/Measure> ;
    skos:definition "Confidence interval for probability P=99,8 % derived from t-distribution by 2 redundant measurements." ;
    skos:inScheme <https://standards.isotc211.org/19157/-3/1/dqc/content/basicMeasure> ;
    skos:prefLabel "1D variable 99.8 % probability; 2 redundant measurements" .

<https://standards.isotc211.org/19157/-3/1/dqc/content/basicMeasure/LE99.8r3> a skos:Concept ;
    ns1:measureDescription <https://standards.isotc211.org/19157/-3/1/dqc/content/measureDescription/MDsd2_LE99.8r3> ;
    ns1:valueType <http://def.isotc211.org/iso19103/2015/PrimitiveTypes/Measure> ;
    skos:definition "Confidence interval for probability P=99,8 % derived from t-distribution by 3 redundant measurements." ;
    skos:inScheme <https://standards.isotc211.org/19157/-3/1/dqc/content/basicMeasure> ;
    skos:prefLabel "1D variable 99.8 % probability; 3 redundant measurements" .

<https://standards.isotc211.org/19157/-3/1/dqc/content/basicMeasure/LE99.8r4> a skos:Concept ;
    ns1:measureDescription <https://standards.isotc211.org/19157/-3/1/dqc/content/measureDescription/MDsd2_LE99.8r4> ;
    ns1:valueType <http://def.isotc211.org/iso19103/2015/PrimitiveTypes/Measure> ;
    skos:definition "Confidence interval for probability P=99,8 % derived from t-distribution by 4 redundant measurements." ;
    skos:inScheme <https://standards.isotc211.org/19157/-3/1/dqc/content/basicMeasure> ;
    skos:prefLabel "1D variable 99.8 % probability; 4 redundant measurements" .

<https://standards.isotc211.org/19157/-3/1/dqc/content/basicMeasure/LE99.8r5> a skos:Concept ;
    ns1:measureDescription <https://standards.isotc211.org/19157/-3/1/dqc/content/measureDescription/MDsd2_LE99.8r5> ;
    ns1:valueType <http://def.isotc211.org/iso19103/2015/PrimitiveTypes/Measure> ;
    skos:definition "Confidence interval for probability P=99,8 % derived from t-distribution by 5 redundant measurements." ;
    skos:inScheme <https://standards.isotc211.org/19157/-3/1/dqc/content/basicMeasure> ;
    skos:prefLabel "1D variable 99.8 % probability; 5 redundant measurements" .

<https://standards.isotc211.org/19157/-3/1/dqc/content/basicMeasure/LE99r1> a skos:Concept ;
    ns1:measureDescription <https://standards.isotc211.org/19157/-3/1/dqc/content/measureDescription/MDsd2_LE99r1> ;
    ns1:valueType <http://def.isotc211.org/iso19103/2015/PrimitiveTypes/Measure> ;
    skos:definition "Confidence interval for probability P=99 % derived from t-distribution by 1 redundant measurement." ;
    skos:inScheme <https://standards.isotc211.org/19157/-3/1/dqc/content/basicMeasure> ;
    skos:prefLabel "1D variable 99 % probability; 1 redundant measurement" .

<https://standards.isotc211.org/19157/-3/1/dqc/content/basicMeasure/LE99r10> a skos:Concept ;
    ns1:measureDescription <https://standards.isotc211.org/19157/-3/1/dqc/content/measureDescription/MDsd2_LE99r10> ;
    ns1:valueType <http://def.isotc211.org/iso19103/2015/PrimitiveTypes/Measure> ;
    skos:definition "Confidence interval for probability P=99 % derived from t-distribution by 10 redundant measurements." ;
    skos:inScheme <https://standards.isotc211.org/19157/-3/1/dqc/content/basicMeasure> ;
    skos:prefLabel "1D variable 99 % probability; 10 redundant measurements" .

<https://standards.isotc211.org/19157/-3/1/dqc/content/basicMeasure/LE99r2> a skos:Concept ;
    ns1:measureDescription <https://standards.isotc211.org/19157/-3/1/dqc/content/measureDescription/MDsd2_LE99r> ;
    ns1:valueType <http://def.isotc211.org/iso19103/2015/PrimitiveTypes/Measure> ;
    skos:definition "Confidence interval for probability P=99 % derived from t-distribution by 2 redundant measurements." ;
    skos:inScheme <https://standards.isotc211.org/19157/-3/1/dqc/content/basicMeasure> ;
    skos:prefLabel "1D variable 99 % probability; 2 redundant measurements" .

<https://standards.isotc211.org/19157/-3/1/dqc/content/basicMeasure/LE99r3> a skos:Concept ;
    ns1:measureDescription <https://standards.isotc211.org/19157/-3/1/dqc/content/measureDescription/MDsd2_LE99r3> ;
    ns1:valueType <http://def.isotc211.org/iso19103/2015/PrimitiveTypes/Measure> ;
    skos:definition "Confidence interval for probability P=99 % derived from t-distribution by 3 redundant measurements." ;
    skos:inScheme <https://standards.isotc211.org/19157/-3/1/dqc/content/basicMeasure> ;
    skos:prefLabel "1D variable 99 % probability; 3 redundant measurements" .

<https://standards.isotc211.org/19157/-3/1/dqc/content/basicMeasure/LE99r4> a skos:Concept ;
    ns1:measureDescription <https://standards.isotc211.org/19157/-3/1/dqc/content/measureDescription/MDsd2_LE99r4> ;
    ns1:valueType <http://def.isotc211.org/iso19103/2015/PrimitiveTypes/Measure> ;
    skos:definition "Confidence interval for probability P=99 % derived from t-distribution by 4 redundant measurements." ;
    skos:inScheme <https://standards.isotc211.org/19157/-3/1/dqc/content/basicMeasure> ;
    skos:prefLabel "1D variable 99 % probability; 4 redundant measurements" .

<https://standards.isotc211.org/19157/-3/1/dqc/content/basicMeasure/LE99r5> a skos:Concept ;
    ns1:measureDescription <https://standards.isotc211.org/19157/-3/1/dqc/content/measureDescription/MDsd2_LE99r5> ;
    ns1:valueType <http://def.isotc211.org/iso19103/2015/PrimitiveTypes/Measure> ;
    skos:definition "Confidence interval for probability P=99 % derived from t-distribution by 5 redundant measurements." ;
    skos:inScheme <https://standards.isotc211.org/19157/-3/1/dqc/content/basicMeasure> ;
    skos:prefLabel "1D variable 99 % probability; 5 redundant measurements" .

<https://standards.isotc211.org/19157/-3/1/dqc/content/basicMeasure/MRSE> a skos:Concept ;
    ns1:measureDescription <https://standards.isotc211.org/19157/-3/1/dqc/content/measureDescription/MDsd1xyz_MRSE> ;
    ns1:valueType <http://def.isotc211.org/iso19103/2015/PrimitiveTypes/Measure> ;
    skos:definition "Radius of sphere centered at the true position, containing the position estimate in 3D with probability of 61%." ;
    skos:inScheme <https://standards.isotc211.org/19157/-3/1/dqc/content/basicMeasure> ;
    skos:prefLabel "Mean radial spherical error" .

<https://standards.isotc211.org/19157/-3/1/dqc/content/basicMeasure/SAS90> a skos:Concept ;
    ns1:measureDescription <https://standards.isotc211.org/19157/-3/1/dqc/content/measureDescription/MDsd1xyz_SAS90> ;
    ns1:valueType <http://def.isotc211.org/iso19103/2015/PrimitiveTypes/Measure> ;
    skos:definition "Radius of sphere centered at the true position, containing the position estimate in 3D with probability of 90%." ;
    skos:inScheme <https://standards.isotc211.org/19157/-3/1/dqc/content/basicMeasure> ;
    skos:prefLabel "90% spherical accuracy standard" .

<https://standards.isotc211.org/19157/-3/1/dqc/content/basicMeasure/SAS99> a skos:Concept ;
    ns1:measureDescription <https://standards.isotc211.org/19157/-3/1/dqc/content/measureDescription/MDsd1xyz_SAS99> ;
    ns1:valueType <http://def.isotc211.org/iso19103/2015/PrimitiveTypes/Measure> ;
    skos:definition "Radius of sphere centered at the true position, containing the position estimate in 3D with probability of 99%." ;
    skos:inScheme <https://standards.isotc211.org/19157/-3/1/dqc/content/basicMeasure> ;
    skos:prefLabel "99% spherical accuracy standard" .

<https://standards.isotc211.org/19157/-3/1/dqc/content/basicMeasure/SD1> a skos:Concept ;
    ns1:measureDescription <https://standards.isotc211.org/19157/-3/1/dqc/content/measureDescription/MDsd1> ;
    ns1:valueType <http://def.isotc211.org/iso19103/2015/PrimitiveTypes/Measure> ;
    skos:definition "Standard deviation for observations or measurements where the true value known." ;
    skos:inScheme <https://standards.isotc211.org/19157/-3/1/dqc/content/basicMeasure> ;
    skos:prefLabel "Standard deviation - true value known" .

<https://standards.isotc211.org/19157/-3/1/dqc/content/basicMeasure/SD1x> a skos:Concept ;
    ns1:measureDescription <https://standards.isotc211.org/19157/-3/1/dqc/content/measureDescription/MDsd1x> ;
    ns1:valueType <http://def.isotc211.org/iso19103/2015/PrimitiveTypes/Measure> ;
    skos:definition "Standard deviation for observations or measurements where the true value known." ;
    skos:inScheme <https://standards.isotc211.org/19157/-3/1/dqc/content/basicMeasure> ;
    skos:prefLabel "Standard deviation in x-direction - true value known" .

<https://standards.isotc211.org/19157/-3/1/dqc/content/basicMeasure/SD1y> a skos:Concept ;
    ns1:measureDescription <https://standards.isotc211.org/19157/-3/1/dqc/content/measureDescription/MDsd1y> ;
    ns1:valueType <http://def.isotc211.org/iso19103/2015/PrimitiveTypes/Measure> ;
    skos:definition "Standard deviation for observations or measurements where the true value known." ;
    skos:inScheme <https://standards.isotc211.org/19157/-3/1/dqc/content/basicMeasure> ;
    skos:prefLabel "Standard deviation in y-direction - true value known" .

<https://standards.isotc211.org/19157/-3/1/dqc/content/basicMeasure/SD1z> a skos:Concept ;
    ns1:measureDescription <https://standards.isotc211.org/19157/-3/1/dqc/content/measureDescription/MDsd1z> ;
    ns1:valueType <http://def.isotc211.org/iso19103/2015/PrimitiveTypes/Measure> ;
    skos:definition "Standard deviation for observations or measurements where the true value known." ;
    skos:inScheme <https://standards.isotc211.org/19157/-3/1/dqc/content/basicMeasure> ;
    skos:prefLabel "Standard deviation in z-direction - true value known" .

<https://standards.isotc211.org/19157/-3/1/dqc/content/basicMeasure/SD2> a skos:Concept ;
    ns1:measureDescription <https://standards.isotc211.org/19157/-3/1/dqc/content/measureDescription/MDsd2> ;
    ns1:valueType <http://def.isotc211.org/iso19103/2015/PrimitiveTypes/Measure> ;
    skos:definition "Standard deviation for observations or measurements where the true value unknown." ;
    skos:inScheme <https://standards.isotc211.org/19157/-3/1/dqc/content/basicMeasure> ;
    skos:prefLabel "Standard deviation - true value unknown" .

<https://standards.isotc211.org/19157/-3/1/dqc/content/basicMeasure/SEP> a skos:Concept ;
    ns1:measureDescription <https://standards.isotc211.org/19157/-3/1/dqc/content/measureDescription/MDsd1xyz_SEP> ;
    ns1:valueType <http://def.isotc211.org/iso19103/2015/PrimitiveTypes/Measure> ;
    skos:definition "Radius of sphere centered at the true position, containing the position estimate in 3D with probability of 50%." ;
    skos:inScheme <https://standards.isotc211.org/19157/-3/1/dqc/content/basicMeasure> ;
    skos:prefLabel "Spherical error probable" .

<https://standards.isotc211.org/19157/-3/1/dqc/content/basicMeasure> a skos:ConceptScheme ;
    skos:definition "ISO19157-3 basic quality measures" ;
    skos:prefLabel "ISO19157-3 basic quality measures" .

[] a prov:Activity ;
    prov:endedAtTime "2024-09-10T13:09:32.550934"^^xsd:dateTime ;
    prov:startedAtTime "2024-09-10T13:09:32.445415"^^xsd:dateTime ;
    prov:used [ a prov:Entity ;
            dcterms:format "application/json" ;
            dcterms:hasVersion "git:57794f311633719a6690d7986204bd7c6f8c06f7" ;
            rdfs:seeAlso <file:///home/runner/work/iso19157-3-dqm-register/iso19157-3-dqm-register/sources/BasicMeasures.csv.json> ] ;
    prov:wasAssociatedWith [ a prov:Agent,
                schema:SoftwareApplication ;
            rdfs:label "OGC-NA tools" ;
            dcterms:hasVersion "0.3.51" ;
            rdfs:seeAlso <https://github.com/opengeospatial/ogc-na-tools> ] ;
    prov:wasInformedBy [ dcterms:identifier "8a487b7b-3e4a-4497-9a66-83a6075bf59a" ] .

_:N326f6e8523af4d04800a69910af3888a a prov:Agent,
        schema:SoftwareApplication ;
    rdfs:label "OGC-NA tools" ;
    dcterms:hasVersion "0.3.51" ;
    rdfs:comment "ogc.na.update_vocabs version 0.3.51" ;
    rdfs:seeAlso <https://github.com/opengeospatial/ogc-na-tools> .

