<?xml version="1.0" encoding="utf-8"?>
<rdf:RDF
   xmlns:dct="http://purl.org/dc/terms/"
   xmlns:ns1="http://www.opengis.net/def/metamodel/isodqm/"
   xmlns:prov="http://www.w3.org/ns/prov#"
   xmlns:rdf="http://www.w3.org/1999/02/22-rdf-syntax-ns#"
   xmlns:rdfs="http://www.w3.org/2000/01/rdf-schema#"
   xmlns:skos="http://www.w3.org/2004/02/skos/core#"
>
  <rdf:Description rdf:about="https://standards.isotc211.org/19157/-3/1/dqc/content/basicMeasure/SD1z">
    <rdf:type rdf:resource="http://www.w3.org/2004/02/skos/core#Concept"/>
    <ns1:valueType rdf:resource="http://def.isotc211.org/iso19103/2015/PrimitiveTypes/Measure"/>
    <skos:inScheme rdf:resource="https://standards.isotc211.org/19157/-3/1/dqc/content/basicMeasure"/>
    <ns1:measureDescription rdf:resource="https://standards.isotc211.org/19157/-3/1/dqc/content/measureDescription/MDsd1z"/>
    <skos:definition>Standard deviation for observations or measurements where the true value known.</skos:definition>
  </rdf:Description>
  <rdf:Description rdf:about="https://standards.isotc211.org/19157/-3/1/dqc/content/basicMeasure/LE90r5">
    <rdf:type rdf:resource="http://www.w3.org/2004/02/skos/core#Concept"/>
    <skos:inScheme rdf:resource="https://standards.isotc211.org/19157/-3/1/dqc/content/basicMeasure"/>
    <ns1:valueType rdf:resource="http://def.isotc211.org/iso19103/2015/PrimitiveTypes/Measure"/>
    <skos:definition>Confidence interval for probability P=90 % derived from t-distribution by 5 redundant measurements.</skos:definition>
    <ns1:measureDescription rdf:resource="https://standards.isotc211.org/19157/-3/1/dqc/content/measureDescription/MDsd2_LE90r5"/>
  </rdf:Description>
  <rdf:Description rdf:about="https://standards.isotc211.org/19157/-3/1/dqc/content/basicMeasure/LE68.3r10">
    <rdf:type rdf:resource="http://www.w3.org/2004/02/skos/core#Concept"/>
    <skos:definition>Confidence interval for probability P=68,3 % derived from t-distribution by 10 redundant measurements.</skos:definition>
    <ns1:valueType rdf:resource="http://def.isotc211.org/iso19103/2015/PrimitiveTypes/Measure"/>
    <skos:inScheme rdf:resource="https://standards.isotc211.org/19157/-3/1/dqc/content/basicMeasure"/>
    <ns1:measureDescription rdf:resource="https://standards.isotc211.org/19157/-3/1/dqc/content/measureDescription/MDsd2_LE68.3r10"/>
  </rdf:Description>
  <rdf:Description rdf:about="https://standards.isotc211.org/19157/-3/1/dqc/content/basicMeasure/LE95r2">
    <rdf:type rdf:resource="http://www.w3.org/2004/02/skos/core#Concept"/>
    <ns1:measureDescription rdf:resource="https://standards.isotc211.org/19157/-3/1/dqc/content/measureDescription/MDsd2_LE95r2"/>
    <skos:definition>Confidence interval for probability P=95 % derived from t-distribution by 2 redundant measurements.</skos:definition>
    <ns1:valueType rdf:resource="http://def.isotc211.org/iso19103/2015/PrimitiveTypes/Measure"/>
    <skos:inScheme rdf:resource="https://standards.isotc211.org/19157/-3/1/dqc/content/basicMeasure"/>
  </rdf:Description>
  <rdf:Description rdf:about="https://standards.isotc211.org/19157/-3/1/dqc/content/basicMeasure/LE99r10">
    <ns1:measureDescription rdf:resource="https://standards.isotc211.org/19157/-3/1/dqc/content/measureDescription/MDsd2_LE99r10"/>
    <rdf:type rdf:resource="http://www.w3.org/2004/02/skos/core#Concept"/>
    <ns1:valueType rdf:resource="http://def.isotc211.org/iso19103/2015/PrimitiveTypes/Measure"/>
    <skos:inScheme rdf:resource="https://standards.isotc211.org/19157/-3/1/dqc/content/basicMeasure"/>
    <skos:definition>Confidence interval for probability P=99 % derived from t-distribution by 10 redundant measurements.</skos:definition>
  </rdf:Description>
  <rdf:Description rdf:about="https://standards.isotc211.org/19157/-3/1/dqc/content/basicMeasure">
    <skos:prefLabel>ISO19157-3 basic quality measures</skos:prefLabel>
    <rdf:type rdf:resource="http://www.w3.org/2004/02/skos/core#ConceptScheme"/>
  </rdf:Description>
  <rdf:Description rdf:about="https://standards.isotc211.org/19157/-3/1/dqc/content/basicMeasure/LE99.8r4">
    <ns1:measureDescription rdf:resource="https://standards.isotc211.org/19157/-3/1/dqc/content/measureDescription/MDsd2_LE99.8r4"/>
    <rdf:type rdf:resource="http://www.w3.org/2004/02/skos/core#Concept"/>
    <ns1:valueType rdf:resource="http://def.isotc211.org/iso19103/2015/PrimitiveTypes/Measure"/>
    <skos:inScheme rdf:resource="https://standards.isotc211.org/19157/-3/1/dqc/content/basicMeasure"/>
    <skos:definition>Confidence interval for probability P=99,8 % derived from t-distribution by 4 redundant measurements.</skos:definition>
  </rdf:Description>
  <rdf:Description rdf:about="https://standards.isotc211.org/19157/-3/1/dqc/content/basicMeasure/MRSE">
    <rdf:type rdf:resource="http://www.w3.org/2004/02/skos/core#Concept"/>
    <ns1:valueType rdf:resource="http://def.isotc211.org/iso19103/2015/PrimitiveTypes/Measure"/>
    <skos:definition>Radius of sphere centered at the true position, containing the position estimate in 3D with probability of 61%.</skos:definition>
    <skos:inScheme rdf:resource="https://standards.isotc211.org/19157/-3/1/dqc/content/basicMeasure"/>
    <ns1:measureDescription rdf:resource="https://standards.isotc211.org/19157/-3/1/dqc/content/measureDescription/MDsd1xyz_MRSE"/>
  </rdf:Description>
  <rdf:Description rdf:nodeID="n094311d70f484125972e72e6cdff08ecb1">
    <prov:wasAssociatedWith rdf:nodeID="n094311d70f484125972e72e6cdff08ecb3"/>
    <prov:startedAtTime rdf:datatype="http://www.w3.org/2001/XMLSchema#dateTime">2024-09-10T07:37:28.336928</prov:startedAtTime>
    <prov:endedAtTime rdf:datatype="http://www.w3.org/2001/XMLSchema#dateTime">2024-09-10T07:37:28.439181</prov:endedAtTime>
    <prov:used rdf:nodeID="n094311d70f484125972e72e6cdff08ecb2"/>
    <rdf:type rdf:resource="http://www.w3.org/ns/prov#Activity"/>
    <prov:wasInformedBy rdf:nodeID="n094311d70f484125972e72e6cdff08ecb4"/>
  </rdf:Description>
  <rdf:Description rdf:about="https://standards.isotc211.org/19157/-3/1/dqc/content/basicMeasure/BM1">
    <rdf:type rdf:resource="http://www.w3.org/2004/02/skos/core#Concept"/>
    <skos:inScheme rdf:resource="https://standards.isotc211.org/19157/-3/1/dqc/content/basicMeasure"/>
    <ns1:valueType rdf:resource="http://def.isotc211.org/iso19103/2015/PrimitiveTypes/Boolean"/>
    <skos:example>False</skos:example>
    <ns1:measureDescription rdf:resource="https://standards.isotc211.org/19157/-3/1/dqc/content/measureDescription/MDBM1"/>
    <skos:definition>Indicator that an item is in error.</skos:definition>
  </rdf:Description>
  <rdf:Description rdf:about="https://standards.isotc211.org/19157/-3/1/dqc/content/basicMeasure/LE95r4">
    <ns1:valueType rdf:resource="http://def.isotc211.org/iso19103/2015/PrimitiveTypes/Measure"/>
    <skos:inScheme rdf:resource="https://standards.isotc211.org/19157/-3/1/dqc/content/basicMeasure"/>
    <ns1:measureDescription rdf:resource="https://standards.isotc211.org/19157/-3/1/dqc/content/measureDescription/MDsd2_LE95r4"/>
    <skos:definition>Confidence interval for probability P=95 % derived from t-distribution by 4 redundant measurements.</skos:definition>
    <rdf:type rdf:resource="http://www.w3.org/2004/02/skos/core#Concept"/>
  </rdf:Description>
  <rdf:Description rdf:about="https://standards.isotc211.org/19157/-3/1/dqc/content/basicMeasure/LE95r5">
    <skos:definition>Confidence interval for probability P=95 % derived from t-distribution by 5 redundant measurements.</skos:definition>
    <ns1:valueType rdf:resource="http://def.isotc211.org/iso19103/2015/PrimitiveTypes/Measure"/>
    <skos:inScheme rdf:resource="https://standards.isotc211.org/19157/-3/1/dqc/content/basicMeasure"/>
    <ns1:measureDescription rdf:resource="https://standards.isotc211.org/19157/-3/1/dqc/content/measureDescription/MDsd2_LE95r5"/>
    <rdf:type rdf:resource="http://www.w3.org/2004/02/skos/core#Concept"/>
  </rdf:Description>
  <rdf:Description rdf:about="https://standards.isotc211.org/19157/-3/1/dqc/content/basicMeasure/SAS90">
    <rdf:type rdf:resource="http://www.w3.org/2004/02/skos/core#Concept"/>
    <ns1:valueType rdf:resource="http://def.isotc211.org/iso19103/2015/PrimitiveTypes/Measure"/>
    <skos:inScheme rdf:resource="https://standards.isotc211.org/19157/-3/1/dqc/content/basicMeasure"/>
    <skos:definition>Radius of sphere centered at the true position, containing the position estimate in 3D with probability of 90%.</skos:definition>
    <ns1:measureDescription rdf:resource="https://standards.isotc211.org/19157/-3/1/dqc/content/measureDescription/MDsd1xyz_SAS90"/>
  </rdf:Description>
  <rdf:Description rdf:about="https://raw.githubusercontent.com/ogcincubator/iso19157-3-dqm-register/master/sources/entailed/BasicMeasures.csv.ttl">
    <dct:hasVersion>git:8ffe5454e3163ff74d6b3fec2f4a0b65f7f0bbc7</dct:hasVersion>
    <rdf:type rdf:resource="http://www.w3.org/ns/prov#Entity"/>
    <dct:format>text/turtle</dct:format>
    <prov:wasGeneratedBy rdf:nodeID="N139d0c338782434d83541cdd6d487f6b"/>
    <prov:wasAttributedTo rdf:nodeID="N3fe2b4c62e514d5cada6e979eb040b96"/>
  </rdf:Description>
  <rdf:Description rdf:about="https://standards.isotc211.org/19157/-3/1/dqc/content/basicMeasure/LE90r1">
    <ns1:measureDescription rdf:resource="https://standards.isotc211.org/19157/-3/1/dqc/content/measureDescription/MDsd2_LE90r1"/>
    <skos:definition>Confidence interval for probability P=90 % derived from t-distribution by 1 redundant measurement.</skos:definition>
    <rdf:type rdf:resource="http://www.w3.org/2004/02/skos/core#Concept"/>
    <ns1:valueType rdf:resource="http://def.isotc211.org/iso19103/2015/PrimitiveTypes/Measure"/>
    <skos:inScheme rdf:resource="https://standards.isotc211.org/19157/-3/1/dqc/content/basicMeasure"/>
  </rdf:Description>
  <rdf:Description rdf:nodeID="N9beec3b395e14df18b5be288cd81bc86">
    <prov:used rdf:nodeID="N9ffd7253b62b426aa71993d816916639"/>
    <prov:used rdf:nodeID="N4e79c82277024efc9f0ddd49cf7d45ff"/>
    <rdf:type rdf:resource="http://www.w3.org/ns/prov#Activity"/>
    <rdfs:label>Entailment and validation</rdfs:label>
    <prov:startedAtTime rdf:datatype="http://www.w3.org/2001/XMLSchema#dateTime">2024-09-10T07:40:46.456580</prov:startedAtTime>
    <prov:endedAtTime rdf:datatype="http://www.w3.org/2001/XMLSchema#dateTime">2024-09-10T07:40:46.505773</prov:endedAtTime>
    <prov:wasInformedBy rdf:nodeID="N9d9fc1b99e2d448f9f57eb06ee001d97"/>
    <rdfs:comment>python ogc.na.update_vocabs -w . .ogc/catalog.ttl --batch --base-uri https://raw.githubusercontent.com/ogcincubator/iso19157-3-dqm-register/master --update --graph-store http://defs-dev.opengis.net:8061/fuseki-hosted/data</rdfs:comment>
    <prov:wasAssociatedWith rdf:nodeID="Na0e88bd4c53641b698ce629c5d87852a"/>
  </rdf:Description>
  <rdf:Description rdf:nodeID="n094311d70f484125972e72e6cdff08ecb3">
    <rdf:type rdf:resource="http://www.w3.org/ns/prov#Agent"/>
    <rdf:type rdf:resource="https://schema.org/SoftwareApplication"/>
    <dct:hasVersion>0.3.51</dct:hasVersion>
    <rdfs:label>OGC-NA tools</rdfs:label>
    <rdfs:seeAlso rdf:resource="https://github.com/opengeospatial/ogc-na-tools"/>
  </rdf:Description>
  <rdf:Description rdf:about="https://standards.isotc211.org/19157/-3/1/dqc/content/basicMeasure/LE99.8r2">
    <ns1:measureDescription rdf:resource="https://standards.isotc211.org/19157/-3/1/dqc/content/measureDescription/MDsd2_LE99.8r2"/>
    <skos:definition>Confidence interval for probability P=99,8 % derived from t-distribution by 2 redundant measurements.</skos:definition>
    <rdf:type rdf:resource="http://www.w3.org/2004/02/skos/core#Concept"/>
    <ns1:valueType rdf:resource="http://def.isotc211.org/iso19103/2015/PrimitiveTypes/Measure"/>
    <skos:inScheme rdf:resource="https://standards.isotc211.org/19157/-3/1/dqc/content/basicMeasure"/>
  </rdf:Description>
  <rdf:Description rdf:about="https://standards.isotc211.org/19157/-3/1/dqc/content/basicMeasure/CE39.4">
    <rdf:type rdf:resource="http://www.w3.org/2004/02/skos/core#Concept"/>
    <skos:definition>confidence interval in two dimensions given by the probability P=39,4 % of the true value within an area</skos:definition>
    <ns1:measureDescription rdf:resource="https://standards.isotc211.org/19157/-3/1/dqc/content/measureDescription/MDsd1xy_CE39.4"/>
    <ns1:valueType rdf:resource="http://def.isotc211.org/iso19103/2015/PrimitiveTypes/Measure"/>
    <skos:inScheme rdf:resource="https://standards.isotc211.org/19157/-3/1/dqc/content/basicMeasure"/>
  </rdf:Description>
  <rdf:Description rdf:about="https://standards.isotc211.org/19157/-3/1/dqc/content/basicMeasure/LE68.3r4">
    <ns1:measureDescription rdf:resource="https://standards.isotc211.org/19157/-3/1/dqc/content/measureDescription/MDsd2_LE68.3r4"/>
    <rdf:type rdf:resource="http://www.w3.org/2004/02/skos/core#Concept"/>
    <ns1:valueType rdf:resource="http://def.isotc211.org/iso19103/2015/PrimitiveTypes/Measure"/>
    <skos:inScheme rdf:resource="https://standards.isotc211.org/19157/-3/1/dqc/content/basicMeasure"/>
    <skos:definition>Confidence interval for probability P=68,3 % derived from t-distribution by 4 redundant measurements.</skos:definition>
  </rdf:Description>
  <rdf:Description rdf:nodeID="N4e79c82277024efc9f0ddd49cf7d45ff">
    <rdfs:seeAlso rdf:resource="https://raw.githubusercontent.com/ogcincubator/iso19157-3-dqm-register/master/.ogc/catalog.ttl"/>
    <dct:hasVersion>git:8ffe5454e3163ff74d6b3fec2f4a0b65f7f0bbc7</dct:hasVersion>
    <rdf:type rdf:resource="http://www.w3.org/ns/prov#Entity"/>
    <dct:format>text/turtle</dct:format>
  </rdf:Description>
  <rdf:Description rdf:about="https://standards.isotc211.org/19157/-3/1/dqc/content/basicMeasure/SEP">
    <skos:definition>Radius of sphere centered at the true position, containing the position estimate in 3D with probability of 50%.</skos:definition>
    <ns1:measureDescription rdf:resource="https://standards.isotc211.org/19157/-3/1/dqc/content/measureDescription/MDsd1xyz_SEP"/>
    <rdf:type rdf:resource="http://www.w3.org/2004/02/skos/core#Concept"/>
    <ns1:valueType rdf:resource="http://def.isotc211.org/iso19103/2015/PrimitiveTypes/Measure"/>
    <skos:inScheme rdf:resource="https://standards.isotc211.org/19157/-3/1/dqc/content/basicMeasure"/>
  </rdf:Description>
  <rdf:Description rdf:about="https://standards.isotc211.org/19157/-3/1/dqc/content/basicMeasure/LE90">
    <rdf:type rdf:resource="http://www.w3.org/2004/02/skos/core#Concept"/>
    <skos:definition>Confidence interval given by the probability P=90 % of the true value being between the lower and upper limit.</skos:definition>
    <ns1:valueType rdf:resource="http://def.isotc211.org/iso19103/2015/PrimitiveTypes/Measure"/>
    <skos:inScheme rdf:resource="https://standards.isotc211.org/19157/-3/1/dqc/content/basicMeasure"/>
    <ns1:measureDescription rdf:resource="https://standards.isotc211.org/19157/-3/1/dqc/content/measureDescription/MDsd1_LE90"/>
  </rdf:Description>
  <rdf:Description rdf:about="https://standards.isotc211.org/19157/-3/1/dqc/content/basicMeasure/BM3">
    <ns1:measureDescription rdf:resource="https://standards.isotc211.org/19157/-3/1/dqc/content/measureDescription/MDBM3"/>
    <skos:inScheme rdf:resource="https://standards.isotc211.org/19157/-3/1/dqc/content/basicMeasure"/>
    <skos:example>11</skos:example>
    <ns1:valueType rdf:resource="http://def.isotc211.org/iso19103/2015/PrimitiveTypes/Integer"/>
    <skos:definition>Total number of items that are subject to an error of a specified type.</skos:definition>
    <rdf:type rdf:resource="http://www.w3.org/2004/02/skos/core#Concept"/>
  </rdf:Description>
  <rdf:Description rdf:about="https://standards.isotc211.org/19157/-3/1/dqc/content/basicMeasure/LE99r5">
    <ns1:valueType rdf:resource="http://def.isotc211.org/iso19103/2015/PrimitiveTypes/Measure"/>
    <skos:inScheme rdf:resource="https://standards.isotc211.org/19157/-3/1/dqc/content/basicMeasure"/>
    <skos:definition>Confidence interval for probability P=99 % derived from t-distribution by 5 redundant measurements.</skos:definition>
    <ns1:measureDescription rdf:resource="https://standards.isotc211.org/19157/-3/1/dqc/content/measureDescription/MDsd2_LE99r5"/>
    <rdf:type rdf:resource="http://www.w3.org/2004/02/skos/core#Concept"/>
  </rdf:Description>
  <rdf:Description rdf:nodeID="Na0e88bd4c53641b698ce629c5d87852a">
    <rdfs:seeAlso rdf:resource="https://github.com/opengeospatial/ogc-na-tools"/>
    <rdf:type rdf:resource="http://www.w3.org/ns/prov#Agent"/>
    <rdf:type rdf:resource="https://schema.org/SoftwareApplication"/>
    <rdfs:label>OGC-NA tools</rdfs:label>
    <rdfs:comment>ogc.na.update_vocabs version 0.3.51</rdfs:comment>
    <dct:hasVersion>0.3.51</dct:hasVersion>
  </rdf:Description>
  <rdf:Description rdf:about="https://raw.githubusercontent.com/ogcincubator/iso19157-3-dqm-register/master/sources/entailed/BasicMeasures.csv.rdf">
    <dct:hasVersion>git:8ffe5454e3163ff74d6b3fec2f4a0b65f7f0bbc7</dct:hasVersion>
    <rdf:type rdf:resource="http://www.w3.org/ns/prov#Entity"/>
    <dct:format>application/rdf+xml</dct:format>
    <prov:wasGeneratedBy rdf:nodeID="N9beec3b395e14df18b5be288cd81bc86"/>
    <prov:wasAttributedTo rdf:nodeID="Na0e88bd4c53641b698ce629c5d87852a"/>
  </rdf:Description>
  <rdf:Description rdf:about="https://standards.isotc211.org/19157/-3/1/dqc/content/basicMeasure/LE50r10">
    <ns1:valueType rdf:resource="http://def.isotc211.org/iso19103/2015/PrimitiveTypes/Measure"/>
    <skos:inScheme rdf:resource="https://standards.isotc211.org/19157/-3/1/dqc/content/basicMeasure"/>
    <rdf:type rdf:resource="http://www.w3.org/2004/02/skos/core#Concept"/>
    <skos:definition>Confidence interval for probability P=50 % derived from t-distribution by 10 redundant measurements.</skos:definition>
    <ns1:measureDescription rdf:resource="https://standards.isotc211.org/19157/-3/1/dqc/content/measureDescription/MDsd2_LE50r10"/>
  </rdf:Description>
  <rdf:Description rdf:about="https://standards.isotc211.org/19157/-3/1/dqc/content/basicMeasure/LE95">
    <ns1:valueType rdf:resource="http://def.isotc211.org/iso19103/2015/PrimitiveTypes/Measure"/>
    <skos:inScheme rdf:resource="https://standards.isotc211.org/19157/-3/1/dqc/content/basicMeasure"/>
    <ns1:measureDescription rdf:resource="https://standards.isotc211.org/19157/-3/1/dqc/content/measureDescription/MDsd1_LE95"/>
    <rdf:type rdf:resource="http://www.w3.org/2004/02/skos/core#Concept"/>
    <skos:definition>Confidence interval given by the probability P=95 % of the true value being between the lower and upper limit.</skos:definition>
  </rdf:Description>
  <rdf:Description rdf:about="https://standards.isotc211.org/19157/-3/1/dqc/content/basicMeasure/LE50r4">
    <skos:definition>Confidence interval for probability P=50 % derived from t-distribution by 4 redundant measurements.</skos:definition>
    <ns1:valueType rdf:resource="http://def.isotc211.org/iso19103/2015/PrimitiveTypes/Measure"/>
    <skos:inScheme rdf:resource="https://standards.isotc211.org/19157/-3/1/dqc/content/basicMeasure"/>
    <ns1:measureDescription rdf:resource="https://standards.isotc211.org/19157/-3/1/dqc/content/measureDescription/MDsd2_LE50r4"/>
    <rdf:type rdf:resource="http://www.w3.org/2004/02/skos/core#Concept"/>
  </rdf:Description>
  <rdf:Description rdf:about="https://standards.isotc211.org/19157/-3/1/dqc/content/basicMeasure/SD1x">
    <ns1:measureDescription rdf:resource="https://standards.isotc211.org/19157/-3/1/dqc/content/measureDescription/MDsd1x"/>
    <ns1:valueType rdf:resource="http://def.isotc211.org/iso19103/2015/PrimitiveTypes/Measure"/>
    <skos:inScheme rdf:resource="https://standards.isotc211.org/19157/-3/1/dqc/content/basicMeasure"/>
    <rdf:type rdf:resource="http://www.w3.org/2004/02/skos/core#Concept"/>
    <skos:definition>Standard deviation for observations or measurements where the true value known.</skos:definition>
  </rdf:Description>
  <rdf:Description rdf:about="https://standards.isotc211.org/19157/-3/1/dqc/content/basicMeasure/LE99r4">
    <skos:definition>Confidence interval for probability P=99 % derived from t-distribution by 4 redundant measurements.</skos:definition>
    <skos:inScheme rdf:resource="https://standards.isotc211.org/19157/-3/1/dqc/content/basicMeasure"/>
    <rdf:type rdf:resource="http://www.w3.org/2004/02/skos/core#Concept"/>
    <ns1:valueType rdf:resource="http://def.isotc211.org/iso19103/2015/PrimitiveTypes/Measure"/>
    <ns1:measureDescription rdf:resource="https://standards.isotc211.org/19157/-3/1/dqc/content/measureDescription/MDsd2_LE99r4"/>
  </rdf:Description>
  <rdf:Description rdf:about="https://standards.isotc211.org/19157/-3/1/dqc/content/basicMeasure/LE50r2">
    <ns1:valueType rdf:resource="http://def.isotc211.org/iso19103/2015/PrimitiveTypes/Measure"/>
    <skos:inScheme rdf:resource="https://standards.isotc211.org/19157/-3/1/dqc/content/basicMeasure"/>
    <ns1:measureDescription rdf:resource="https://standards.isotc211.org/19157/-3/1/dqc/content/measureDescription/MDsd2_LE50r2"/>
    <skos:definition>Confidence interval for probability P=50 % derived from t-distribution by 2 redundant measurements.</skos:definition>
    <rdf:type rdf:resource="http://www.w3.org/2004/02/skos/core#Concept"/>
  </rdf:Description>
  <rdf:Description rdf:about="https://standards.isotc211.org/19157/-3/1/dqc/content/basicMeasure/SD2">
    <ns1:valueType rdf:resource="http://def.isotc211.org/iso19103/2015/PrimitiveTypes/Measure"/>
    <skos:inScheme rdf:resource="https://standards.isotc211.org/19157/-3/1/dqc/content/basicMeasure"/>
    <skos:definition>Standard deviation for observations or measurements where the true value unknown.</skos:definition>
    <ns1:measureDescription rdf:resource="https://standards.isotc211.org/19157/-3/1/dqc/content/measureDescription/MDsd2"/>
    <rdf:type rdf:resource="http://www.w3.org/2004/02/skos/core#Concept"/>
  </rdf:Description>
  <rdf:Description rdf:about="https://standards.isotc211.org/19157/-3/1/dqc/content/basicMeasure/SAS99">
    <ns1:measureDescription rdf:resource="https://standards.isotc211.org/19157/-3/1/dqc/content/measureDescription/MDsd1xyz_SAS99"/>
    <rdf:type rdf:resource="http://www.w3.org/2004/02/skos/core#Concept"/>
    <skos:definition>Radius of sphere centered at the true position, containing the position estimate in 3D with probability of 99%.</skos:definition>
    <skos:inScheme rdf:resource="https://standards.isotc211.org/19157/-3/1/dqc/content/basicMeasure"/>
    <ns1:valueType rdf:resource="http://def.isotc211.org/iso19103/2015/PrimitiveTypes/Measure"/>
  </rdf:Description>
  <rdf:Description rdf:about="https://standards.isotc211.org/19157/-3/1/dqc/content/basicMeasure/BM4">
    <skos:inScheme rdf:resource="https://standards.isotc211.org/19157/-3/1/dqc/content/basicMeasure"/>
    <skos:definition>Indicator that an item is correct.</skos:definition>
    <ns1:valueType rdf:resource="http://def.isotc211.org/iso19103/2015/PrimitiveTypes/Boolean"/>
    <skos:example>True</skos:example>
    <rdf:type rdf:resource="http://www.w3.org/2004/02/skos/core#Concept"/>
    <ns1:measureDescription rdf:resource="https://standards.isotc211.org/19157/-3/1/dqc/content/measureDescription/MDBM4"/>
  </rdf:Description>
  <rdf:Description rdf:about="https://standards.isotc211.org/19157/-3/1/dqc/content/basicMeasure/LE90r3">
    <ns1:measureDescription rdf:resource="https://standards.isotc211.org/19157/-3/1/dqc/content/measureDescription/MDsd2_LE90r3"/>
    <rdf:type rdf:resource="http://www.w3.org/2004/02/skos/core#Concept"/>
    <ns1:valueType rdf:resource="http://def.isotc211.org/iso19103/2015/PrimitiveTypes/Measure"/>
    <skos:inScheme rdf:resource="https://standards.isotc211.org/19157/-3/1/dqc/content/basicMeasure"/>
    <skos:definition>Confidence interval for probability P=90 % derived from t-distribution by 3 redundant measurements.</skos:definition>
  </rdf:Description>
  <rdf:Description rdf:about="https://standards.isotc211.org/19157/-3/1/dqc/content/basicMeasure/LE99r1">
    <skos:definition>Confidence interval for probability P=99 % derived from t-distribution by 1 redundant measurement.</skos:definition>
    <rdf:type rdf:resource="http://www.w3.org/2004/02/skos/core#Concept"/>
    <ns1:valueType rdf:resource="http://def.isotc211.org/iso19103/2015/PrimitiveTypes/Measure"/>
    <ns1:measureDescription rdf:resource="https://standards.isotc211.org/19157/-3/1/dqc/content/measureDescription/MDsd2_LE99r1"/>
    <skos:inScheme rdf:resource="https://standards.isotc211.org/19157/-3/1/dqc/content/basicMeasure"/>
  </rdf:Description>
  <rdf:Description rdf:about="https://standards.isotc211.org/19157/-3/1/dqc/content/basicMeasure/LE99.8r3">
    <ns1:valueType rdf:resource="http://def.isotc211.org/iso19103/2015/PrimitiveTypes/Measure"/>
    <skos:inScheme rdf:resource="https://standards.isotc211.org/19157/-3/1/dqc/content/basicMeasure"/>
    <ns1:measureDescription rdf:resource="https://standards.isotc211.org/19157/-3/1/dqc/content/measureDescription/MDsd2_LE99.8r3"/>
    <skos:definition>Confidence interval for probability P=99,8 % derived from t-distribution by 3 redundant measurements.</skos:definition>
    <rdf:type rdf:resource="http://www.w3.org/2004/02/skos/core#Concept"/>
  </rdf:Description>
  <rdf:Description rdf:about="https://standards.isotc211.org/19157/-3/1/dqc/content/basicMeasure/LE68.3r3">
    <rdf:type rdf:resource="http://www.w3.org/2004/02/skos/core#Concept"/>
    <ns1:valueType rdf:resource="http://def.isotc211.org/iso19103/2015/PrimitiveTypes/Measure"/>
    <skos:inScheme rdf:resource="https://standards.isotc211.org/19157/-3/1/dqc/content/basicMeasure"/>
    <skos:definition>Confidence interval for probability P=68,3 % derived from t-distribution by 3 redundant measurements.</skos:definition>
    <ns1:measureDescription rdf:resource="https://standards.isotc211.org/19157/-3/1/dqc/content/measureDescription/MDsd2_LE68.3r3"/>
  </rdf:Description>
  <rdf:Description rdf:about="https://standards.isotc211.org/19157/-3/1/dqc/content/basicMeasure/LE68.3">
    <ns1:valueType rdf:resource="http://def.isotc211.org/iso19103/2015/PrimitiveTypes/Measure"/>
    <ns1:measureDescription rdf:resource="https://standards.isotc211.org/19157/-3/1/dqc/content/measureDescription/MDsd1_LE68.3"/>
    <rdf:type rdf:resource="http://www.w3.org/2004/02/skos/core#Concept"/>
    <skos:definition>Confidence interval given by the probability P=68,3 % of the true value being between the lower and upper limit</skos:definition>
    <skos:inScheme rdf:resource="https://standards.isotc211.org/19157/-3/1/dqc/content/basicMeasure"/>
  </rdf:Description>
  <rdf:Description rdf:about="https://standards.isotc211.org/19157/-3/1/dqc/content/basicMeasure/LE99">
    <ns1:measureDescription rdf:resource="https://standards.isotc211.org/19157/-3/1/dqc/content/measureDescription/MDsd1_LE99"/>
    <skos:inScheme rdf:resource="https://standards.isotc211.org/19157/-3/1/dqc/content/basicMeasure"/>
    <rdf:type rdf:resource="http://www.w3.org/2004/02/skos/core#Concept"/>
    <skos:definition>Confidence interval given by the probability P=99 % of the true value being between the lower and upper limit.</skos:definition>
    <ns1:valueType rdf:resource="http://def.isotc211.org/iso19103/2015/PrimitiveTypes/Measure"/>
  </rdf:Description>
  <rdf:Description rdf:nodeID="N3fe2b4c62e514d5cada6e979eb040b96">
    <rdfs:seeAlso rdf:resource="https://github.com/opengeospatial/ogc-na-tools"/>
    <rdf:type rdf:resource="https://schema.org/SoftwareApplication"/>
    <rdf:type rdf:resource="http://www.w3.org/ns/prov#Agent"/>
    <rdfs:comment>ogc.na.update_vocabs version 0.3.51</rdfs:comment>
    <dct:hasVersion>0.3.51</dct:hasVersion>
    <rdfs:label>OGC-NA tools</rdfs:label>
  </rdf:Description>
  <rdf:Description rdf:about="https://standards.isotc211.org/19157/-3/1/dqc/content/basicMeasure/BM2">
    <skos:example>MD2bme</skos:example>
    <ns1:measureDescription rdf:resource="https://standards.isotc211.org/19157/-3/1/dqc/content/measureDescription/MDBM2"/>
    <ns1:valueType rdf:resource="http://def.isotc211.org/iso19103/2015/PrimitiveTypes/Real"/>
    <rdf:type rdf:resource="http://www.w3.org/2004/02/skos/core#Concept"/>
    <skos:definition>Number of the erroneous items with respect to the total number of items that should have been present.</skos:definition>
    <skos:inScheme rdf:resource="https://standards.isotc211.org/19157/-3/1/dqc/content/basicMeasure"/>
  </rdf:Description>
  <rdf:Description rdf:about="https://standards.isotc211.org/19157/-3/1/dqc/content/basicMeasure/LE99.8r5">
    <ns1:measureDescription rdf:resource="https://standards.isotc211.org/19157/-3/1/dqc/content/measureDescription/MDsd2_LE99.8r5"/>
    <ns1:valueType rdf:resource="http://def.isotc211.org/iso19103/2015/PrimitiveTypes/Measure"/>
    <skos:inScheme rdf:resource="https://standards.isotc211.org/19157/-3/1/dqc/content/basicMeasure"/>
    <skos:definition>Confidence interval for probability P=99,8 % derived from t-distribution by 5 redundant measurements.</skos:definition>
    <rdf:type rdf:resource="http://www.w3.org/2004/02/skos/core#Concept"/>
  </rdf:Description>
  <rdf:Description rdf:about="https://standards.isotc211.org/19157/-3/1/dqc/content/basicMeasure/LE95r10">
    <ns1:measureDescription rdf:resource="https://standards.isotc211.org/19157/-3/1/dqc/content/measureDescription/MDsd2_LE95r10"/>
    <rdf:type rdf:resource="http://www.w3.org/2004/02/skos/core#Concept"/>
    <ns1:valueType rdf:resource="http://def.isotc211.org/iso19103/2015/PrimitiveTypes/Measure"/>
    <skos:inScheme rdf:resource="https://standards.isotc211.org/19157/-3/1/dqc/content/basicMeasure"/>
    <skos:definition>Confidence interval for probability P=95 % derived from t-distribution by 10 redundant measurements.</skos:definition>
  </rdf:Description>
  <rdf:Description rdf:about="https://standards.isotc211.org/19157/-3/1/dqc/content/basicMeasure/LE90r2">
    <skos:definition>Confidence interval for probability P=90 % derived from t-distribution by 2 redundant measurements.</skos:definition>
    <ns1:measureDescription rdf:resource="https://standards.isotc211.org/19157/-3/1/dqc/content/measureDescription/MDsd2_LE90r2"/>
    <rdf:type rdf:resource="http://www.w3.org/2004/02/skos/core#Concept"/>
    <skos:inScheme rdf:resource="https://standards.isotc211.org/19157/-3/1/dqc/content/basicMeasure"/>
    <ns1:valueType rdf:resource="http://def.isotc211.org/iso19103/2015/PrimitiveTypes/Measure"/>
  </rdf:Description>
  <rdf:Description rdf:about="https://standards.isotc211.org/19157/-3/1/dqc/content/basicMeasure/LE50r5">
    <rdf:type rdf:resource="http://www.w3.org/2004/02/skos/core#Concept"/>
    <ns1:valueType rdf:resource="http://def.isotc211.org/iso19103/2015/PrimitiveTypes/Measure"/>
    <skos:inScheme rdf:resource="https://standards.isotc211.org/19157/-3/1/dqc/content/basicMeasure"/>
    <ns1:measureDescription rdf:resource="https://standards.isotc211.org/19157/-3/1/dqc/content/measureDescription/MDsd2_LE50r5"/>
    <skos:definition>Confidence interval for probability P=50 % derived from t-distribution by 5 redundant measurements.</skos:definition>
  </rdf:Description>
  <rdf:Description rdf:about="https://standards.isotc211.org/19157/-3/1/dqc/content/basicMeasure/LE68.3r2">
    <ns1:valueType rdf:resource="http://def.isotc211.org/iso19103/2015/PrimitiveTypes/Measure"/>
    <skos:inScheme rdf:resource="https://standards.isotc211.org/19157/-3/1/dqc/content/basicMeasure"/>
    <ns1:measureDescription rdf:resource="https://standards.isotc211.org/19157/-3/1/dqc/content/measureDescription/MDsd2_LE68.3r2"/>
    <rdf:type rdf:resource="http://www.w3.org/2004/02/skos/core#Concept"/>
    <skos:definition>Confidence interval for probability P=68,3 % derived from t-distribution by 2 redundant measurements.</skos:definition>
  </rdf:Description>
  <rdf:Description rdf:about="https://standards.isotc211.org/19157/-3/1/dqc/content/basicMeasure/LE99.8r10">
    <skos:definition>Confidence interval for probability P=99,8 % derived from t-distribution by 10 redundant measurements.</skos:definition>
    <rdf:type rdf:resource="http://www.w3.org/2004/02/skos/core#Concept"/>
    <ns1:valueType rdf:resource="http://def.isotc211.org/iso19103/2015/PrimitiveTypes/Measure"/>
    <skos:inScheme rdf:resource="https://standards.isotc211.org/19157/-3/1/dqc/content/basicMeasure"/>
    <ns1:measureDescription rdf:resource="https://standards.isotc211.org/19157/-3/1/dqc/content/measureDescription/MDsd2_LE99.8r10"/>
  </rdf:Description>
  <rdf:Description rdf:about="https://standards.isotc211.org/19157/-3/1/dqc/content/basicMeasure/BM6">
    <skos:definition>Number of the correct items with respect to the total number of items that should have been present.</skos:definition>
    <skos:example>0.9811</skos:example>
    <rdf:type rdf:resource="http://www.w3.org/2004/02/skos/core#Concept"/>
    <ns1:measureDescription rdf:resource="https://standards.isotc211.org/19157/-3/1/dqc/content/measureDescription/MDBM6"/>
    <skos:inScheme rdf:resource="https://standards.isotc211.org/19157/-3/1/dqc/content/basicMeasure"/>
    <ns1:valueType rdf:resource="http://def.isotc211.org/iso19103/2015/PrimitiveTypes/Real"/>
  </rdf:Description>
  <rdf:Description rdf:about="https://standards.isotc211.org/19157/-3/1/dqc/content/basicMeasure/LE99r2">
    <ns1:measureDescription rdf:resource="https://standards.isotc211.org/19157/-3/1/dqc/content/measureDescription/MDsd2_LE99r"/>
    <ns1:valueType rdf:resource="http://def.isotc211.org/iso19103/2015/PrimitiveTypes/Measure"/>
    <skos:inScheme rdf:resource="https://standards.isotc211.org/19157/-3/1/dqc/content/basicMeasure"/>
    <skos:definition>Confidence interval for probability P=99 % derived from t-distribution by 2 redundant measurements.</skos:definition>
    <rdf:type rdf:resource="http://www.w3.org/2004/02/skos/core#Concept"/>
  </rdf:Description>
  <rdf:Description rdf:about="https://standards.isotc211.org/19157/-3/1/dqc/content/basicMeasure/LE68.3r5">
    <ns1:valueType rdf:resource="http://def.isotc211.org/iso19103/2015/PrimitiveTypes/Measure"/>
    <skos:inScheme rdf:resource="https://standards.isotc211.org/19157/-3/1/dqc/content/basicMeasure"/>
    <ns1:measureDescription rdf:resource="https://standards.isotc211.org/19157/-3/1/dqc/content/measureDescription/MDsd2_LE68.3r5"/>
    <skos:definition>Confidence interval for probability P=68,3 % derived from t-distribution by 5 redundant measurements.</skos:definition>
    <rdf:type rdf:resource="http://www.w3.org/2004/02/skos/core#Concept"/>
  </rdf:Description>
  <rdf:Description rdf:about="https://standards.isotc211.org/19157/-3/1/dqc/content/basicMeasure/SD1y">
    <rdf:type rdf:resource="http://www.w3.org/2004/02/skos/core#Concept"/>
    <skos:definition>Standard deviation for observations or measurements where the true value known.</skos:definition>
    <ns1:valueType rdf:resource="http://def.isotc211.org/iso19103/2015/PrimitiveTypes/Measure"/>
    <skos:inScheme rdf:resource="https://standards.isotc211.org/19157/-3/1/dqc/content/basicMeasure"/>
    <ns1:measureDescription rdf:resource="https://standards.isotc211.org/19157/-3/1/dqc/content/measureDescription/MDsd1y"/>
  </rdf:Description>
  <rdf:Description rdf:nodeID="N9ffd7253b62b426aa71993d816916639">
    <rdfs:seeAlso rdf:resource="https://raw.githubusercontent.com/ogcincubator/iso19157-3-dqm-register/master/sources/BasicMeasures.csv.ttl"/>
    <dct:hasVersion>git:8ffe5454e3163ff74d6b3fec2f4a0b65f7f0bbc7</dct:hasVersion>
    <rdf:type rdf:resource="http://www.w3.org/ns/prov#Entity"/>
    <dct:format>text/turtle</dct:format>
  </rdf:Description>
  <rdf:Description rdf:about="https://standards.isotc211.org/19157/-3/1/dqc/content/basicMeasure/LE95r3">
    <ns1:measureDescription rdf:resource="https://standards.isotc211.org/19157/-3/1/dqc/content/measureDescription/MDsd2_LE95r3"/>
    <rdf:type rdf:resource="http://www.w3.org/2004/02/skos/core#Concept"/>
    <skos:definition>Confidence interval for probability P=95 % derived from t-distribution by 3 redundant measurements.</skos:definition>
    <ns1:valueType rdf:resource="http://def.isotc211.org/iso19103/2015/PrimitiveTypes/Measure"/>
    <skos:inScheme rdf:resource="https://standards.isotc211.org/19157/-3/1/dqc/content/basicMeasure"/>
  </rdf:Description>
  <rdf:Description rdf:about="https://standards.isotc211.org/19157/-3/1/dqc/content/basicMeasure/LE99r3">
    <ns1:measureDescription rdf:resource="https://standards.isotc211.org/19157/-3/1/dqc/content/measureDescription/MDsd2_LE99r3"/>
    <skos:definition>Confidence interval for probability P=99 % derived from t-distribution by 3 redundant measurements.</skos:definition>
    <rdf:type rdf:resource="http://www.w3.org/2004/02/skos/core#Concept"/>
    <ns1:valueType rdf:resource="http://def.isotc211.org/iso19103/2015/PrimitiveTypes/Measure"/>
    <skos:inScheme rdf:resource="https://standards.isotc211.org/19157/-3/1/dqc/content/basicMeasure"/>
  </rdf:Description>
  <rdf:Description rdf:about="https://standards.isotc211.org/19157/-3/1/dqc/content/basicMeasure/LE90r4">
    <skos:definition>Confidence interval for probability P=90 % derived from t-distribution by 4 redundant measurements.</skos:definition>
    <ns1:measureDescription rdf:resource="https://standards.isotc211.org/19157/-3/1/dqc/content/measureDescription/MDsd2_LE90r4"/>
    <rdf:type rdf:resource="http://www.w3.org/2004/02/skos/core#Concept"/>
    <ns1:valueType rdf:resource="http://def.isotc211.org/iso19103/2015/PrimitiveTypes/Measure"/>
    <skos:inScheme rdf:resource="https://standards.isotc211.org/19157/-3/1/dqc/content/basicMeasure"/>
  </rdf:Description>
  <rdf:Description rdf:about="https://standards.isotc211.org/19157/-3/1/dqc/content/basicMeasure/BM5">
    <skos:definition>Total number of items that are free of errors of a specified type.</skos:definition>
    <ns1:valueType rdf:resource="http://def.isotc211.org/iso19103/2015/PrimitiveTypes/Integer"/>
    <rdf:type rdf:resource="http://www.w3.org/2004/02/skos/core#Concept"/>
    <ns1:measureDescription rdf:resource="https://standards.isotc211.org/19157/-3/1/dqc/content/measureDescription/MDBM5"/>
    <skos:inScheme rdf:resource="https://standards.isotc211.org/19157/-3/1/dqc/content/basicMeasure"/>
    <skos:example>571</skos:example>
  </rdf:Description>
  <rdf:Description rdf:about="https://standards.isotc211.org/19157/-3/1/dqc/content/basicMeasure/SD1">
    <skos:definition>Standard deviation for observations or measurements where the true value known.</skos:definition>
    <ns1:measureDescription rdf:resource="https://standards.isotc211.org/19157/-3/1/dqc/content/measureDescription/MDsd1"/>
    <rdf:type rdf:resource="http://www.w3.org/2004/02/skos/core#Concept"/>
    <ns1:valueType rdf:resource="http://def.isotc211.org/iso19103/2015/PrimitiveTypes/Measure"/>
    <skos:inScheme rdf:resource="https://standards.isotc211.org/19157/-3/1/dqc/content/basicMeasure"/>
  </rdf:Description>
  <rdf:Description rdf:about="https://standards.isotc211.org/19157/-3/1/dqc/content/basicMeasure/LE95r1">
    <skos:definition>Confidence interval for probability P=95 % derived from t-distribution by 1 redundant measurement.</skos:definition>
    <rdf:type rdf:resource="http://www.w3.org/2004/02/skos/core#Concept"/>
    <ns1:valueType rdf:resource="http://def.isotc211.org/iso19103/2015/PrimitiveTypes/Measure"/>
    <skos:inScheme rdf:resource="https://standards.isotc211.org/19157/-3/1/dqc/content/basicMeasure"/>
    <ns1:measureDescription rdf:resource="https://standards.isotc211.org/19157/-3/1/dqc/content/measureDescription/MDsd2_LE95r1"/>
  </rdf:Description>
  <rdf:Description rdf:nodeID="n094311d70f484125972e72e6cdff08ecb4">
    <dct:identifier>448c53c2-a49f-425a-9db8-ba365856db2f</dct:identifier>
  </rdf:Description>
  <rdf:Description rdf:about="https://standards.isotc211.org/19157/-3/1/dqc/content/basicMeasure/LE99.8r1">
    <rdf:type rdf:resource="http://www.w3.org/2004/02/skos/core#Concept"/>
    <skos:definition>Confidence interval for probability P=99,8 % derived from t-distribution by 1 redundant measurement.</skos:definition>
    <skos:inScheme rdf:resource="https://standards.isotc211.org/19157/-3/1/dqc/content/basicMeasure"/>
    <ns1:measureDescription rdf:resource="https://standards.isotc211.org/19157/-3/1/dqc/content/measureDescription/MDsd2_LE99.8r1"/>
    <ns1:valueType rdf:resource="http://def.isotc211.org/iso19103/2015/PrimitiveTypes/Measure"/>
  </rdf:Description>
  <rdf:Description rdf:nodeID="N139d0c338782434d83541cdd6d487f6b">
    <prov:wasAssociatedWith rdf:nodeID="N3fe2b4c62e514d5cada6e979eb040b96"/>
    <prov:startedAtTime rdf:datatype="http://www.w3.org/2001/XMLSchema#dateTime">2024-09-10T07:40:46.456580</prov:startedAtTime>
    <rdfs:label>Entailment and validation</rdfs:label>
    <prov:used rdf:nodeID="N86841db65b904213b6ddaba6f3de405e"/>
    <prov:used rdf:nodeID="N9054391109e54d4a8b84d4d51dc5c8e7"/>
    <prov:wasInformedBy rdf:nodeID="Ncaac0dbd36b7499599e6550b37b3ff43"/>
    <rdfs:comment>python ogc.na.update_vocabs -w . .ogc/catalog.ttl --batch --base-uri https://raw.githubusercontent.com/ogcincubator/iso19157-3-dqm-register/master --update --graph-store http://defs-dev.opengis.net:8061/fuseki-hosted/data</rdfs:comment>
    <rdf:type rdf:resource="http://www.w3.org/ns/prov#Activity"/>
    <prov:endedAtTime rdf:datatype="http://www.w3.org/2001/XMLSchema#dateTime">2024-09-10T07:40:46.480286</prov:endedAtTime>
  </rdf:Description>
  <rdf:Description rdf:nodeID="n094311d70f484125972e72e6cdff08ecb2">
    <dct:format>application/json</dct:format>
    <rdf:type rdf:resource="http://www.w3.org/ns/prov#Entity"/>
    <dct:hasVersion>git:42bcfe51b78c60e40f5a3a34781b955fe1d1c51e</dct:hasVersion>
    <rdfs:seeAlso rdf:resource="file:///home/runner/work/iso19157-3-dqm-register/iso19157-3-dqm-register/sources/BasicMeasures.csv.json"/>
  </rdf:Description>
  <rdf:Description rdf:about="https://standards.isotc211.org/19157/-3/1/dqc/content/basicMeasure/CE95">
    <ns1:measureDescription rdf:resource="https://standards.isotc211.org/19157/-3/1/dqc/content/measureDescription/MDsd1xy_CE95"/>
    <rdf:type rdf:resource="http://www.w3.org/2004/02/skos/core#Concept"/>
    <ns1:valueType rdf:resource="http://def.isotc211.org/iso19103/2015/PrimitiveTypes/Measure"/>
    <skos:inScheme rdf:resource="https://standards.isotc211.org/19157/-3/1/dqc/content/basicMeasure"/>
  </rdf:Description>
  <rdf:Description rdf:about="https://standards.isotc211.org/19157/-3/1/dqc/content/basicMeasure/LE50">
    <rdf:type rdf:resource="http://www.w3.org/2004/02/skos/core#Concept"/>
    <skos:definition>Confidence interval given by the probability P=50 % of the true value being between the lower and upper limit.</skos:definition>
    <ns1:valueType rdf:resource="http://def.isotc211.org/iso19103/2015/PrimitiveTypes/Measure"/>
    <skos:inScheme rdf:resource="https://standards.isotc211.org/19157/-3/1/dqc/content/basicMeasure"/>
    <ns1:measureDescription rdf:resource="https://standards.isotc211.org/19157/-3/1/dqc/content/measureDescription/MDsd1_LE50"/>
  </rdf:Description>
  <rdf:Description rdf:about="https://standards.isotc211.org/19157/-3/1/dqc/content/basicMeasure/LE90r10">
    <rdf:type rdf:resource="http://www.w3.org/2004/02/skos/core#Concept"/>
    <ns1:measureDescription rdf:resource="https://standards.isotc211.org/19157/-3/1/dqc/content/measureDescription/MDsd2_LE90r10"/>
    <ns1:valueType rdf:resource="http://def.isotc211.org/iso19103/2015/PrimitiveTypes/Measure"/>
    <skos:inScheme rdf:resource="https://standards.isotc211.org/19157/-3/1/dqc/content/basicMeasure"/>
    <skos:definition>Confidence interval for probability P=90 % derived from t-distribution by 10 redundant measurements.</skos:definition>
  </rdf:Description>
  <rdf:Description rdf:nodeID="N86841db65b904213b6ddaba6f3de405e">
    <dct:format>text/turtle</dct:format>
    <dct:hasVersion>git:8ffe5454e3163ff74d6b3fec2f4a0b65f7f0bbc7</dct:hasVersion>
    <rdf:type rdf:resource="http://www.w3.org/ns/prov#Entity"/>
    <rdfs:seeAlso rdf:resource="https://raw.githubusercontent.com/ogcincubator/iso19157-3-dqm-register/master/.ogc/catalog.ttl"/>
  </rdf:Description>
  <rdf:Description rdf:about="https://standards.isotc211.org/19157/-3/1/dqc/content/basicMeasure/CE50">
    <rdf:type rdf:resource="http://www.w3.org/2004/02/skos/core#Concept"/>
    <ns1:measureDescription rdf:resource="https://standards.isotc211.org/19157/-3/1/dqc/content/measureDescription/MDsd1xy_CE50"/>
    <ns1:valueType rdf:resource="http://def.isotc211.org/iso19103/2015/PrimitiveTypes/Measure"/>
    <skos:inScheme rdf:resource="https://standards.isotc211.org/19157/-3/1/dqc/content/basicMeasure"/>
  </rdf:Description>
  <rdf:Description rdf:about="https://standards.isotc211.org/19157/-3/1/dqc/content/basicMeasure/LE99.8">
    <ns1:measureDescription rdf:resource="https://standards.isotc211.org/19157/-3/1/dqc/content/measureDescription/MDsd1_LE99.8"/>
    <rdf:type rdf:resource="http://www.w3.org/2004/02/skos/core#Concept"/>
    <skos:definition>confidence interval given by the probability P=99,8 % of the true value being between the lower and upper limit</skos:definition>
    <ns1:valueType rdf:resource="http://def.isotc211.org/iso19103/2015/PrimitiveTypes/Measure"/>
    <skos:inScheme rdf:resource="https://standards.isotc211.org/19157/-3/1/dqc/content/basicMeasure"/>
  </rdf:Description>
  <rdf:Description rdf:about="https://standards.isotc211.org/19157/-3/1/dqc/content/basicMeasure/LE50r3">
    <rdf:type rdf:resource="http://www.w3.org/2004/02/skos/core#Concept"/>
    <ns1:valueType rdf:resource="http://def.isotc211.org/iso19103/2015/PrimitiveTypes/Measure"/>
    <skos:inScheme rdf:resource="https://standards.isotc211.org/19157/-3/1/dqc/content/basicMeasure"/>
    <skos:definition>Confidence interval for probability P=50 % derived from t-distribution by 3 redundant measurements.</skos:definition>
    <ns1:measureDescription rdf:resource="https://standards.isotc211.org/19157/-3/1/dqc/content/measureDescription/MDsd2_LE50r3"/>
  </rdf:Description>
  <rdf:Description rdf:about="https://standards.isotc211.org/19157/-3/1/dqc/content/basicMeasure/CE99.8">
    <skos:inScheme rdf:resource="https://standards.isotc211.org/19157/-3/1/dqc/content/basicMeasure"/>
    <rdf:type rdf:resource="http://www.w3.org/2004/02/skos/core#Concept"/>
    <ns1:valueType rdf:resource="http://def.isotc211.org/iso19103/2015/PrimitiveTypes/Measure"/>
    <ns1:measureDescription rdf:resource="https://standards.isotc211.org/19157/-3/1/dqc/content/measureDescription/MDsd1xy_CE99.8"/>
  </rdf:Description>
  <rdf:Description rdf:nodeID="N9054391109e54d4a8b84d4d51dc5c8e7">
    <dct:hasVersion>git:8ffe5454e3163ff74d6b3fec2f4a0b65f7f0bbc7</dct:hasVersion>
    <rdf:type rdf:resource="http://www.w3.org/ns/prov#Entity"/>
    <dct:format>text/turtle</dct:format>
    <rdfs:seeAlso rdf:resource="https://raw.githubusercontent.com/ogcincubator/iso19157-3-dqm-register/master/sources/BasicMeasures.csv.ttl"/>
  </rdf:Description>
  <rdf:Description rdf:about="https://standards.isotc211.org/19157/-3/1/dqc/content/basicMeasure/LE50r1">
    <rdf:type rdf:resource="http://www.w3.org/2004/02/skos/core#Concept"/>
    <ns1:measureDescription rdf:resource="https://standards.isotc211.org/19157/-3/1/dqc/content/measureDescription/MDsd2_LE50r1"/>
    <skos:definition>Confidence interval for probability P=50 % derived from t-distribution by 1 redundant measurement.</skos:definition>
    <ns1:valueType rdf:resource="http://def.isotc211.org/iso19103/2015/PrimitiveTypes/Measure"/>
    <skos:inScheme rdf:resource="https://standards.isotc211.org/19157/-3/1/dqc/content/basicMeasure"/>
  </rdf:Description>
  <rdf:Description rdf:about="https://standards.isotc211.org/19157/-3/1/dqc/content/basicMeasure/CE90">
    <rdf:type rdf:resource="http://www.w3.org/2004/02/skos/core#Concept"/>
    <ns1:measureDescription rdf:resource="https://standards.isotc211.org/19157/-3/1/dqc/content/measureDescription/MDsd1xy_CE90"/>
    <ns1:valueType rdf:resource="http://def.isotc211.org/iso19103/2015/PrimitiveTypes/Measure"/>
    <skos:inScheme rdf:resource="https://standards.isotc211.org/19157/-3/1/dqc/content/basicMeasure"/>
  </rdf:Description>
  <rdf:Description rdf:about="https://standards.isotc211.org/19157/-3/1/dqc/content/basicMeasure/LE68.3r1">
    <ns1:measureDescription rdf:resource="https://standards.isotc211.org/19157/-3/1/dqc/content/measureDescription/MDsd2_LE68.3r1"/>
    <rdf:type rdf:resource="http://www.w3.org/2004/02/skos/core#Concept"/>
    <skos:definition>Confidence interval for probability P=68,3 % derived from t-distribution by 1 redundant measurement.</skos:definition>
    <ns1:valueType rdf:resource="http://def.isotc211.org/iso19103/2015/PrimitiveTypes/Measure"/>
    <skos:inScheme rdf:resource="https://standards.isotc211.org/19157/-3/1/dqc/content/basicMeasure"/>
  </rdf:Description>
  <rdf:Description rdf:nodeID="Ncaac0dbd36b7499599e6550b37b3ff43">
    <dct:identifier>872ee265-40d8-4878-81cc-d63caa9a8845</dct:identifier>
  </rdf:Description>
  <rdf:Description rdf:nodeID="N9d9fc1b99e2d448f9f57eb06ee001d97">
    <dct:identifier>872ee265-40d8-4878-81cc-d63caa9a8845</dct:identifier>
  </rdf:Description>
</rdf:RDF>
