<?xml version="1.0" encoding="utf-8"?>
<rdf:RDF
   xmlns:dcterms="http://purl.org/dc/terms/"
   xmlns:dqm="http://www.opengis.net/def/metamodel/isodqm/"
   xmlns:foaf="http://xmlns.com/foaf/0.1/"
   xmlns:prov="http://www.w3.org/ns/prov#"
   xmlns:rdf="http://www.w3.org/1999/02/22-rdf-syntax-ns#"
   xmlns:rdfs="http://www.w3.org/2000/01/rdf-schema#"
   xmlns:skos="http://www.w3.org/2004/02/skos/core#"
>
  <rdf:Description rdf:about="https://standards.isotc211.org/19157/-3/1/dqc/content/measureDescription/MD202">
    <rdf:type rdf:resource="http://www.w3.org/2004/02/skos/core#Concept"/>
    <skos:inScheme rdf:resource="https://standards.isotc211.org/19157/-3/1/dqc/content/measureDescription"/>
    <skos:definition>The principle of geometric fidelity is that any real world alignment or shape, when viewed at the source survey scale, shall be accurately reflected in the data to the required specification.</skos:definition>
    <skos:prefLabel>MD202</skos:prefLabel>
  </rdf:Description>
  <rdf:Description rdf:about="https://standards.isotc211.org/19157/-3/1/dqc/content/measureDescription/MDsd2_LE95r4">
    <skos:inScheme rdf:resource="https://standards.isotc211.org/19157/-3/1/dqc/content/measureDescription"/>
    <skos:prefLabel>MDsd2_LE95r4</skos:prefLabel>
    <skos:definition>Standard deviation - true value unknown; significance level 95%; 4 redundant measurements.</skos:definition>
    <dqm:formula rdf:resource="https://standards.isotc211.org/19157/-3/1/dqc/content/formulaType/FTsd2_LE95r4"/>
    <rdf:type rdf:resource="http://www.w3.org/2004/02/skos/core#Concept"/>
  </rdf:Description>
  <rdf:Description rdf:nodeID="Nf7095029aaba4a9a838915a8d4aa2ea2">
    <rdfs:seeAlso rdf:resource="https://raw.githubusercontent.com/ogcincubator/iso19157-3-dqm-register/master/sources/MeasureDescription.csv.ttl"/>
    <dcterms:hasVersion>git:4f17dcac9447f6d217612ec525843df2f94db721</dcterms:hasVersion>
    <rdf:type rdf:resource="http://www.w3.org/ns/prov#Entity"/>
    <dcterms:format>text/turtle</dcterms:format>
  </rdf:Description>
  <rdf:Description rdf:about="https://standards.isotc211.org/19157/-3/1/dqc/content/measureDescription/MD8e">
    <rdf:type rdf:resource="http://www.w3.org/2004/02/skos/core#Concept"/>
    <skos:prefLabel>MD8e</skos:prefLabel>
    <skos:inScheme rdf:resource="https://standards.isotc211.org/19157/-3/1/dqc/content/measureDescription"/>
    <skos:definition>True (One feature relationship exists which is not defined in the conceptual schema).</skos:definition>
  </rdf:Description>
  <rdf:Description rdf:about="https://standards.isotc211.org/19157/-3/1/dqc/content/measureDescription/MD40">
    <skos:inScheme rdf:resource="https://standards.isotc211.org/19157/-3/1/dqc/content/measureDescription"/>
    <dqm:formula rdf:resource="https://standards.isotc211.org/19157/-3/1/dqc/content/formulaType/FT40_4"/>
    <dqm:formula rdf:resource="https://standards.isotc211.org/19157/-3/1/dqc/content/formulaType/FT40_5"/>
    <dqm:formula rdf:resource="https://standards.isotc211.org/19157/-3/1/dqc/content/formulaType/FT40_3"/>
    <dqm:formula rdf:resource="https://standards.isotc211.org/19157/-3/1/dqc/content/formulaType/FT40_6"/>
    <dqm:formula rdf:resource="https://standards.isotc211.org/19157/-3/1/dqc/content/formulaType/FT40_7"/>
    <dqm:formula rdf:resource="https://standards.isotc211.org/19157/-3/1/dqc/content/formulaType/FT40_1"/>
    <dqm:formula rdf:resource="https://standards.isotc211.org/19157/-3/1/dqc/content/formulaType/FT40_8"/>
    <dqm:formula rdf:resource="https://standards.isotc211.org/19157/-3/1/dqc/content/formulaType/FT40_2"/>
    <rdf:type rdf:resource="http://www.w3.org/2004/02/skos/core#Concept"/>
    <skos:definition>A manner of calculating the comparison of the data (source) and the control (reference).</skos:definition>
    <skos:prefLabel>MD40</skos:prefLabel>
  </rdf:Description>
  <rdf:Description rdf:about="https://standards.isotc211.org/19157/-3/1/dqc/content/measureDescription/MD23">
    <rdf:type rdf:resource="http://www.w3.org/2004/02/skos/core#Concept"/>
    <skos:inScheme rdf:resource="https://standards.isotc211.org/19157/-3/1/dqc/content/measureDescription"/>
    <skos:prefLabel>MD23</skos:prefLabel>
    <skos:definition>Search distance as defined in the specification.</skos:definition>
  </rdf:Description>
  <rdf:Description rdf:about="https://standards.isotc211.org/19157/-3/1/dqc/content/measureDescription/MD26e">
    <foaf:depiction rdf:resource="https://ogcincubator.github.io/iso19157-3-dqm-register/ISO19157-3/img/26e.PNG"/>
    <skos:prefLabel>MD26e</skos:prefLabel>
    <skos:inScheme rdf:resource="https://standards.isotc211.org/19157/-3/1/dqc/content/measureDescription"/>
    <rdf:type rdf:resource="http://www.w3.org/2004/02/skos/core#Concept"/>
    <skos:definition>Key: 1) Building 1
2) illegal intersection (loop)</skos:definition>
  </rdf:Description>
  <rdf:Description rdf:about="https://standards.isotc211.org/19157/-3/1/dqc/content/measureDescription/MDsd1xy_CE95">
    <skos:prefLabel>MDsd1xy_CE95</skos:prefLabel>
    <skos:inScheme rdf:resource="https://standards.isotc211.org/19157/-3/1/dqc/content/measureDescription"/>
    <skos:definition>Standard deviation 2D - true value known; significance level 95%.</skos:definition>
    <rdf:type rdf:resource="http://www.w3.org/2004/02/skos/core#Concept"/>
    <dqm:formula rdf:resource="https://standards.isotc211.org/19157/-3/1/dqc/content/formulaType/FTsd1xy_CE95"/>
  </rdf:Description>
  <rdf:Description rdf:about="https://standards.isotc211.org/19157/-3/1/dqc/content/measureDescription/MD208e2">
    <skos:prefLabel>MD208e2</skos:prefLabel>
    <rdf:type rdf:resource="http://www.w3.org/2004/02/skos/core#Concept"/>
    <skos:inScheme rdf:resource="https://standards.isotc211.org/19157/-3/1/dqc/content/measureDescription"/>
    <foaf:depiction rdf:resource="https://ogcincubator.github.io/iso19157-3-dqm-register/ISO19157-3/img/MD208e2.png"/>
    <skos:definition>Calculate the rate of omission of street view imagery coverage against a reference area. The street view imagery is represented as constructed buffers of imagery points with a radius, and the reference area is a rectangular grid cell of area A1.</skos:definition>
  </rdf:Description>
  <rdf:Description rdf:about="https://standards.isotc211.org/19157/-3/1/dqc/content/measureDescription/MD32_1">
    <skos:inScheme rdf:resource="https://standards.isotc211.org/19157/-3/1/dqc/content/measureDescription"/>
    <skos:definition>The covariance matrix generalizes the concept of variance from one to n dimensions, i.e. from scalar-valued random variables to vector-valued random variables (tuples of scalar random variables).</skos:definition>
    <rdf:type rdf:resource="http://www.w3.org/2004/02/skos/core#Concept"/>
    <skos:prefLabel>MD32_1</skos:prefLabel>
    <dqm:formula rdf:resource="https://standards.isotc211.org/19157/-3/1/dqc/content/formulaType/FT32_2"/>
    <dqm:formula rdf:resource="https://standards.isotc211.org/19157/-3/1/dqc/content/formulaType/FT32_3"/>
    <dqm:formula rdf:resource="https://standards.isotc211.org/19157/-3/1/dqc/content/formulaType/FT32_4"/>
    <dqm:formula rdf:resource="https://standards.isotc211.org/19157/-3/1/dqc/content/formulaType/FT32_1"/>
    <dqm:sequence>1</dqm:sequence>
  </rdf:Description>
  <rdf:Description rdf:about="https://standards.isotc211.org/19157/-3/1/dqc/content/measureDescription/MD1e">
    <rdf:type rdf:resource="http://www.w3.org/2004/02/skos/core#Concept"/>
    <skos:definition>True (a house is present in the dataset, but does not exists in the universe of discourse).</skos:definition>
    <skos:inScheme rdf:resource="https://standards.isotc211.org/19157/-3/1/dqc/content/measureDescription"/>
    <skos:prefLabel>MD1e</skos:prefLabel>
  </rdf:Description>
  <rdf:Description rdf:about="https://standards.isotc211.org/19157/-3/1/dqc/content/measureDescription/MD19e">
    <skos:definition>5 (5 living quarters type code is coded on more than 3 characters although the requirement in data product specification is 3).</skos:definition>
    <skos:prefLabel>MD19e</skos:prefLabel>
    <skos:inScheme rdf:resource="https://standards.isotc211.org/19157/-3/1/dqc/content/measureDescription"/>
    <rdf:type rdf:resource="http://www.w3.org/2004/02/skos/core#Concept"/>
  </rdf:Description>
  <rdf:Description rdf:about="https://standards.isotc211.org/19157/-3/1/dqc/content/measureDescription/MDsd1x">
    <dqm:formula rdf:resource="https://standards.isotc211.org/19157/-3/1/dqc/content/formulaType/FTsd1x"/>
    <skos:inScheme rdf:resource="https://standards.isotc211.org/19157/-3/1/dqc/content/measureDescription"/>
    <rdf:type rdf:resource="http://www.w3.org/2004/02/skos/core#Concept"/>
    <skos:prefLabel>MDsd1x</skos:prefLabel>
    <skos:definition>Standard deviation 2D - true value known; direction x.</skos:definition>
  </rdf:Description>
  <rdf:Description rdf:about="https://standards.isotc211.org/19157/-3/1/dqc/content/measureDescription/MDBM1">
    <skos:prefLabel>MDBM1</skos:prefLabel>
    <rdf:type rdf:resource="http://www.w3.org/2004/02/skos/core#Concept"/>
    <skos:inScheme rdf:resource="https://standards.isotc211.org/19157/-3/1/dqc/content/measureDescription"/>
    <skos:definition>Boolean value expressing the item is indicated an error.</skos:definition>
  </rdf:Description>
  <rdf:Description rdf:about="https://standards.isotc211.org/19157/-3/1/dqc/content/measureDescription/MDsd2_LE90r5">
    <skos:definition>Standard deviation - true value unknown; significance level 90%; 5 redundant measurements.</skos:definition>
    <skos:prefLabel>MDsd2_LE90r5</skos:prefLabel>
    <dqm:formula rdf:resource="https://standards.isotc211.org/19157/-3/1/dqc/content/formulaType/FTsd2_LE90r5"/>
    <skos:inScheme rdf:resource="https://standards.isotc211.org/19157/-3/1/dqc/content/measureDescription"/>
    <rdf:type rdf:resource="http://www.w3.org/2004/02/skos/core#Concept"/>
  </rdf:Description>
  <rdf:Description rdf:about="https://standards.isotc211.org/19157/-3/1/dqc/content/measureDescription/MD32_2">
    <skos:definition>The covariance matrix generalizes the concept of variance from one to n dimensions, i.e. from scalar-valued random variables to vector-valued random variables (tuples of scalar random variables).</skos:definition>
    <skos:prefLabel>MD32_2</skos:prefLabel>
    <dqm:sequence>2</dqm:sequence>
    <skos:inScheme rdf:resource="https://standards.isotc211.org/19157/-3/1/dqc/content/measureDescription"/>
    <rdf:type rdf:resource="http://www.w3.org/2004/02/skos/core#Concept"/>
    <dqm:formula rdf:resource="https://standards.isotc211.org/19157/-3/1/dqc/content/formulaType/FT32_5"/>
    <dqm:formula rdf:resource="https://standards.isotc211.org/19157/-3/1/dqc/content/formulaType/FT32_6"/>
  </rdf:Description>
  <rdf:Description rdf:nodeID="N6b0aa890b3f44184ab68539d5d3b19e6">
    <dcterms:identifier>fd69c946-3328-4566-8849-8d051541eb48</dcterms:identifier>
  </rdf:Description>
  <rdf:Description rdf:about="https://standards.isotc211.org/19157/-3/1/dqc/content/measureDescription/MDsd2_LE50r4">
    <skos:definition>Standard deviation - true value unknown; significance level 50%; 4 redundant measurements.</skos:definition>
    <skos:prefLabel>MDsd2_LE50r4</skos:prefLabel>
    <skos:inScheme rdf:resource="https://standards.isotc211.org/19157/-3/1/dqc/content/measureDescription"/>
    <rdf:type rdf:resource="http://www.w3.org/2004/02/skos/core#Concept"/>
    <dqm:formula rdf:resource="https://standards.isotc211.org/19157/-3/1/dqc/content/formulaType/FTsd2_LE50r4"/>
  </rdf:Description>
  <rdf:Description rdf:about="https://standards.isotc211.org/19157/-3/1/dqc/content/measureDescription/MDsd2_LE99.8r3">
    <dqm:formula rdf:resource="https://standards.isotc211.org/19157/-3/1/dqc/content/formulaType/FTsd2_LE99.8r3"/>
    <skos:definition>Standard deviation - true value unknown; significance level 99.8%; 3 redundant measurements.</skos:definition>
    <skos:prefLabel>MDsd2_LE99.8r3</skos:prefLabel>
    <rdf:type rdf:resource="http://www.w3.org/2004/02/skos/core#Concept"/>
    <skos:inScheme rdf:resource="https://standards.isotc211.org/19157/-3/1/dqc/content/measureDescription"/>
  </rdf:Description>
  <rdf:Description rdf:about="https://standards.isotc211.org/19157/-3/1/dqc/content/measureDescription/MD13">
    <skos:definition>Conceptual schema describes the rules and content of the dataset.</skos:definition>
    <skos:inScheme rdf:resource="https://standards.isotc211.org/19157/-3/1/dqc/content/measureDescription"/>
    <rdf:type rdf:resource="http://www.w3.org/2004/02/skos/core#Concept"/>
    <skos:prefLabel>MD13</skos:prefLabel>
  </rdf:Description>
  <rdf:Description rdf:about="https://standards.isotc211.org/19157/-3/1/dqc/content/measureDescription/MDBM3">
    <rdf:type rdf:resource="http://www.w3.org/2004/02/skos/core#Concept"/>
    <skos:inScheme rdf:resource="https://standards.isotc211.org/19157/-3/1/dqc/content/measureDescription"/>
    <skos:prefLabel>MDBM3</skos:prefLabel>
    <skos:definition>The data product specification shall describe the features and how items shall be typed.</skos:definition>
  </rdf:Description>
  <rdf:Description rdf:nodeID="N1eb0b1d7f55640ed87322f7fa3c19b95">
    <rdfs:comment>python ogc.na.update_vocabs -w . .ogc/catalog.ttl --batch --base-uri https://raw.githubusercontent.com/ogcincubator/iso19157-3-dqm-register/master --update --graph-store http://defs-dev.opengis.net:8061/fuseki-hosted/data</rdfs:comment>
    <prov:wasInformedBy rdf:nodeID="Nb13b972d4e744b04a38526c2a2ae7942"/>
    <rdf:type rdf:resource="http://www.w3.org/ns/prov#Activity"/>
    <prov:used rdf:nodeID="N85163b0296794a67b860b276db2c284c"/>
    <prov:used rdf:nodeID="Ndd11de545b8f4594afde58b69b5ba57d"/>
    <prov:used rdf:nodeID="N54101fafc1ba44c2aa5e49528e77a94c"/>
    <prov:wasAssociatedWith rdf:nodeID="N4df3e8306032451892eef51fe2cba317"/>
    <prov:startedAtTime rdf:datatype="http://www.w3.org/2001/XMLSchema#dateTime">2024-09-11T12:20:22.049559</prov:startedAtTime>
    <prov:endedAtTime rdf:datatype="http://www.w3.org/2001/XMLSchema#dateTime">2024-09-11T12:20:25.434218</prov:endedAtTime>
    <rdfs:label>Entailment and validation</rdfs:label>
  </rdf:Description>
  <rdf:Description rdf:nodeID="Nb31b7c799d2f441180f7235d2e01478a">
    <rdfs:seeAlso rdf:resource="https://raw.githubusercontent.com/ogcincubator/iso19157-3-dqm-register/master/.ogc/catalog.ttl"/>
    <dcterms:hasVersion>git:4f17dcac9447f6d217612ec525843df2f94db721</dcterms:hasVersion>
    <rdf:type rdf:resource="http://www.w3.org/ns/prov#Entity"/>
    <dcterms:format>text/turtle</dcterms:format>
  </rdf:Description>
  <rdf:Description rdf:about="https://standards.isotc211.org/19157/-3/1/dqc/content/measureDescription/MD7">
    <skos:definition>Divide number of item not present in the dataset in relation to number of items in the universe of discourse.</skos:definition>
    <skos:inScheme rdf:resource="https://standards.isotc211.org/19157/-3/1/dqc/content/measureDescription"/>
    <rdf:type rdf:resource="http://www.w3.org/2004/02/skos/core#Concept"/>
    <skos:prefLabel>MD7</skos:prefLabel>
  </rdf:Description>
  <rdf:Description rdf:about="https://standards.isotc211.org/19157/-3/1/dqc/content/measureDescription/MD206">
    <skos:definition>Mean time from when an object has been changed until its updated in the data base.</skos:definition>
    <skos:inScheme rdf:resource="https://standards.isotc211.org/19157/-3/1/dqc/content/measureDescription"/>
    <rdf:type rdf:resource="http://www.w3.org/2004/02/skos/core#Concept"/>
    <skos:prefLabel>MD206</skos:prefLabel>
  </rdf:Description>
  <rdf:Description rdf:about="https://standards.isotc211.org/19157/-3/1/dqc/content/measureDescription/MD61">
    <rdf:type rdf:resource="http://www.w3.org/2004/02/skos/core#Concept"/>
    <skos:inScheme rdf:resource="https://standards.isotc211.org/19157/-3/1/dqc/content/measureDescription"/>
    <skos:prefLabel>MD61</skos:prefLabel>
    <skos:definition>Number of incorrectly classified features compared to the specification. Features and the classification method as defined in the specification.</skos:definition>
  </rdf:Description>
  <rdf:Description rdf:about="https://standards.isotc211.org/19157/-3/1/dqc/content/measureDescription/MDsd1_LE99">
    <skos:prefLabel>MDsd1_LE99</skos:prefLabel>
    <dqm:formula rdf:resource="https://standards.isotc211.org/19157/-3/1/dqc/content/formulaType/FTsd1_LE99"/>
    <skos:definition>Standard deviation - true value known; significance level 99%.</skos:definition>
    <skos:inScheme rdf:resource="https://standards.isotc211.org/19157/-3/1/dqc/content/measureDescription"/>
    <rdf:type rdf:resource="http://www.w3.org/2004/02/skos/core#Concept"/>
  </rdf:Description>
  <rdf:Description rdf:about="https://standards.isotc211.org/19157/-3/1/dqc/content/measureDescription/MD207e">
    <skos:definition>The timetable of a railway station shall be updated with the frequency required to allow passengers to take a train even if the scheduled time or platform change.</skos:definition>
    <rdf:type rdf:resource="http://www.w3.org/2004/02/skos/core#Concept"/>
    <skos:inScheme rdf:resource="https://standards.isotc211.org/19157/-3/1/dqc/content/measureDescription"/>
    <skos:prefLabel>MD207e</skos:prefLabel>
  </rdf:Description>
  <rdf:Description rdf:about="https://standards.isotc211.org/19157/-3/1/dqc/content/measureDescription/MD29_2">
    <dqm:formula rdf:resource="https://standards.isotc211.org/19157/-3/1/dqc/content/formulaType/FT29_2"/>
    <rdf:type rdf:resource="http://www.w3.org/2004/02/skos/core#Concept"/>
    <skos:prefLabel>MD29_2</skos:prefLabel>
    <skos:inScheme rdf:resource="https://standards.isotc211.org/19157/-3/1/dqc/content/measureDescription"/>
    <skos:definition>A criterion for the establishing of correspondence should also be stated (e.g. allowing for correspondence to the closest position, correspondence on vertices or along lines). The criteria for finding the corresponding points shall be reported with the data quality evaluation result.</skos:definition>
    <dqm:sequence>2</dqm:sequence>
  </rdf:Description>
  <rdf:Description rdf:about="https://standards.isotc211.org/19157/-3/1/dqc/content/measureDescription/MD21e">
    <foaf:depiction rdf:resource="https://ogcincubator.github.io/iso19157-3-dqm-register/ISO19157-3/img/21e_1.PNG"/>
    <foaf:depiction rdf:resource="https://ogcincubator.github.io/iso19157-3-dqm-register/ISO19157-3/img/21e_2.PNG"/>
    <skos:definition>Count the number of wrong curve connections - e.g. two-point curve connections exist where only one should be present, or count all curves with more than the threshold value of 500 vertices (in which system automatically places point-curve based on vertices limitation built into software code where no spatial justification for point-curve exists).
</skos:definition>
    <skos:prefLabel>MD21e</skos:prefLabel>
    <rdf:type rdf:resource="http://www.w3.org/2004/02/skos/core#Concept"/>
    <skos:inScheme rdf:resource="https://standards.isotc211.org/19157/-3/1/dqc/content/measureDescription"/>
  </rdf:Description>
  <rdf:Description rdf:about="https://standards.isotc211.org/19157/-3/1/dqc/content/measureDescription/MD208_2">
    <skos:prefLabel>MD208_2</skos:prefLabel>
    <rdf:type rdf:resource="http://www.w3.org/2004/02/skos/core#Concept"/>
    <skos:inScheme rdf:resource="https://standards.isotc211.org/19157/-3/1/dqc/content/measureDescription"/>
    <skos:definition>If reference data is in line geometry:
Where l’ is the length of each segment of reference data that is not captured by the coverage of the source data, n is the total number of uncovered segments, and L is the total length of all reference line features. </skos:definition>
    <dqm:sequence>2</dqm:sequence>
    <dqm:formula rdf:resource="https://standards.isotc211.org/19157/-3/1/dqc/content/formulaType/FT208_L"/>
  </rdf:Description>
  <rdf:Description rdf:about="https://standards.isotc211.org/19157/-3/1/dqc/content/measureDescription/MD48">
    <dqm:formula rdf:resource="https://standards.isotc211.org/19157/-3/1/dqc/content/formulaType/FT48_6"/>
    <dqm:formula rdf:resource="https://standards.isotc211.org/19157/-3/1/dqc/content/formulaType/FT48_3"/>
    <dqm:formula rdf:resource="https://standards.isotc211.org/19157/-3/1/dqc/content/formulaType/FT48_2"/>
    <dqm:formula rdf:resource="https://standards.isotc211.org/19157/-3/1/dqc/content/formulaType/FT48_5"/>
    <dqm:formula rdf:resource="https://standards.isotc211.org/19157/-3/1/dqc/content/formulaType/FT48_4"/>
    <dqm:formula rdf:resource="https://standards.isotc211.org/19157/-3/1/dqc/content/formulaType/FT48_1"/>
    <skos:prefLabel>MD48</skos:prefLabel>
    <skos:definition>Absolute horizontal accuracy of the data coordinates, expressed in terms of circular error at 90 % probability given that a bias is present. A manner of calculating the comparison of the data (source) and the control (reference).</skos:definition>
    <rdf:type rdf:resource="http://www.w3.org/2004/02/skos/core#Concept"/>
    <skos:inScheme rdf:resource="https://standards.isotc211.org/19157/-3/1/dqc/content/measureDescription"/>
  </rdf:Description>
  <rdf:Description rdf:about="https://standards.isotc211.org/19157/-3/1/dqc/content/measureDescription/MD208e">
    <foaf:depiction rdf:resource="https://ogcincubator.github.io/iso19157-3-dqm-register/ISO19157-3/img/MD208e.png"/>
    <rdf:type rdf:resource="http://www.w3.org/2004/02/skos/core#Concept"/>
    <skos:prefLabel>MD208e</skos:prefLabel>
    <skos:inScheme rdf:resource="https://standards.isotc211.org/19157/-3/1/dqc/content/measureDescription"/>
    <skos:definition>Calculate the rate of omission of street view imagery (SVI) coverage using street network as the reference data. In the example, street view imagery is represented as points (circular dots in the figure), and the reference street network consists of seven line features of length L1, L2, … L7. 
Step 1: Snap each point to the nearest location on the street it is closest to. Snapped locations are marked by red crosses in the figure.
Step 2: Split the lines at the snapped locations and calculate the length of each split segment. Segments with a length longer than a certain threshold (e.g. 50 m) where no SVI is found are deemed as uncovered. In this example, we identify four segments with lengths l 1, l 2, l 3, and l 4 as uncovered segments.
Step 3: Rate of omission is thus calculated as the sum of lengths of uncovered segments, divided by the sum of lengths of all segments.
The example demonstrates a way to calculate the omission rate for the whole dataset. Besides, the omission rate can also be calculated at a finer spatial scale, i.e. for each geometry unit. For instance, it can be calculated at the street level, where the omission rate is calculated for each street segment.</skos:definition>
  </rdf:Description>
  <rdf:Description rdf:about="https://standards.isotc211.org/19157/-3/1/dqc/content/measureDescription/MD213">
    <skos:prefLabel>MD213</skos:prefLabel>
    <rdf:type rdf:resource="http://www.w3.org/2004/02/skos/core#Concept"/>
    <skos:inScheme rdf:resource="https://standards.isotc211.org/19157/-3/1/dqc/content/measureDescription"/>
    <skos:definition>The quantity of data where sensitive information is present, divided by the total quantity of data.</skos:definition>
  </rdf:Description>
  <rdf:Description rdf:about="https://standards.isotc211.org/19157/-3/1/dqc/content/measureDescription/MD205">
    <skos:prefLabel>MD205</skos:prefLabel>
    <skos:definition>The update frequency as shown in metadata.</skos:definition>
    <rdf:type rdf:resource="http://www.w3.org/2004/02/skos/core#Concept"/>
    <skos:inScheme rdf:resource="https://standards.isotc211.org/19157/-3/1/dqc/content/measureDescription"/>
  </rdf:Description>
  <rdf:Description rdf:about="https://standards.isotc211.org/19157/-3/1/dqc/content/measureDescription/MD15e">
    <skos:prefLabel>MD15e</skos:prefLabel>
    <skos:inScheme rdf:resource="https://standards.isotc211.org/19157/-3/1/dqc/content/measureDescription"/>
    <rdf:type rdf:resource="http://www.w3.org/2004/02/skos/core#Concept"/>
    <skos:definition>All dates are correct according to their month rules of probable number of days, e.g.  No 29 February in a non-leap year, no 31 April 31 are allowed values.</skos:definition>
  </rdf:Description>
  <rdf:Description rdf:about="https://standards.isotc211.org/19157/-3/1/dqc/content/measureDescription/MD41">
    <dqm:formula rdf:resource="https://standards.isotc211.org/19157/-3/1/dqc/content/formulaType/FT41_5"/>
    <dqm:formula rdf:resource="https://standards.isotc211.org/19157/-3/1/dqc/content/formulaType/FT41_1"/>
    <dqm:formula rdf:resource="https://standards.isotc211.org/19157/-3/1/dqc/content/formulaType/FT41_4"/>
    <dqm:formula rdf:resource="https://standards.isotc211.org/19157/-3/1/dqc/content/formulaType/FT41_3"/>
    <dqm:formula rdf:resource="https://standards.isotc211.org/19157/-3/1/dqc/content/formulaType/FT41_7"/>
    <dqm:formula rdf:resource="https://standards.isotc211.org/19157/-3/1/dqc/content/formulaType/FT41_8"/>
    <dqm:formula rdf:resource="https://standards.isotc211.org/19157/-3/1/dqc/content/formulaType/FT41_6"/>
    <dqm:formula rdf:resource="https://standards.isotc211.org/19157/-3/1/dqc/content/formulaType/FT41_2"/>
    <skos:prefLabel>MD41</skos:prefLabel>
    <skos:inScheme rdf:resource="https://standards.isotc211.org/19157/-3/1/dqc/content/measureDescription"/>
    <rdf:type rdf:resource="http://www.w3.org/2004/02/skos/core#Concept"/>
    <skos:definition>A manner of calculating the comparison of the data (source) and the control (reference).</skos:definition>
  </rdf:Description>
  <rdf:Description rdf:about="https://standards.isotc211.org/19157/-3/1/dqc/content/measureDescription/MDs1z">
    <dqm:formula rdf:resource="https://standards.isotc211.org/19157/-3/1/dqc/content/formulaType/FTsd1z"/>
    <skos:inScheme rdf:resource="https://standards.isotc211.org/19157/-3/1/dqc/content/measureDescription"/>
    <rdf:type rdf:resource="http://www.w3.org/2004/02/skos/core#Concept"/>
    <skos:prefLabel>MDs1z</skos:prefLabel>
    <skos:definition>Standard deviation 2D - true value known; direction z.</skos:definition>
  </rdf:Description>
  <rdf:Description rdf:about="https://standards.isotc211.org/19157/-3/1/dqc/content/measureDescription/MD205e">
    <skos:prefLabel>MD205e</skos:prefLabel>
    <skos:definition>It is ‘true’ if the value for an address has been updated in the database within user defined AQL (e.g. 5 days) since the decision on its change.</skos:definition>
    <rdf:type rdf:resource="http://www.w3.org/2004/02/skos/core#Concept"/>
    <skos:inScheme rdf:resource="https://standards.isotc211.org/19157/-3/1/dqc/content/measureDescription"/>
  </rdf:Description>
  <rdf:Description rdf:about="https://standards.isotc211.org/19157/-3/1/dqc/content/measureDescription/MD17e">
    <skos:prefLabel>MD17e</skos:prefLabel>
    <skos:definition>100 % (scope: attributes road width and speed limit for roads, are within the value domain).</skos:definition>
    <rdf:type rdf:resource="http://www.w3.org/2004/02/skos/core#Concept"/>
    <skos:inScheme rdf:resource="https://standards.isotc211.org/19157/-3/1/dqc/content/measureDescription"/>
  </rdf:Description>
  <rdf:Description rdf:about="https://standards.isotc211.org/19157/-3/1/dqc/content/measureDescription/MD12">
    <skos:prefLabel>MD12</skos:prefLabel>
    <rdf:type rdf:resource="http://www.w3.org/2004/02/skos/core#Concept"/>
    <skos:inScheme rdf:resource="https://standards.isotc211.org/19157/-3/1/dqc/content/measureDescription"/>
    <skos:definition>The value indicates number of items in the dataset that are not compliant with the rules of the conceptual schema in relation to the total number of these items supposed to be in the dataset.</skos:definition>
  </rdf:Description>
  <rdf:Description rdf:about="https://standards.isotc211.org/19157/-3/1/dqc/content/measureDescription/MD11e">
    <skos:prefLabel>MD11e</skos:prefLabel>
    <skos:definition>Search for surfaces that are not allowed to overlap according to the conceptual schema. In this case, forest and built-up-area are not allowed to overlap.</skos:definition>
    <skos:inScheme rdf:resource="https://standards.isotc211.org/19157/-3/1/dqc/content/measureDescription"/>
    <foaf:depiction rdf:resource="https://ogcincubator.github.io/iso19157-3-dqm-register/ISO19157-3/img/11e.PNG"/>
    <rdf:type rdf:resource="http://www.w3.org/2004/02/skos/core#Concept"/>
  </rdf:Description>
  <rdf:Description rdf:about="https://standards.isotc211.org/19157/-3/1/dqc/content/measureDescription/MD2">
    <skos:prefLabel>MD2</skos:prefLabel>
    <rdf:type rdf:resource="http://www.w3.org/2004/02/skos/core#Concept"/>
    <skos:inScheme rdf:resource="https://standards.isotc211.org/19157/-3/1/dqc/content/measureDescription"/>
    <skos:definition>Count number of item present in the dataset which does not exists in the universe of discourse.</skos:definition>
  </rdf:Description>
  <rdf:Description rdf:about="https://standards.isotc211.org/19157/-3/1/dqc/content/measureDescription/MDsd2_LE99r3">
    <skos:inScheme rdf:resource="https://standards.isotc211.org/19157/-3/1/dqc/content/measureDescription"/>
    <skos:definition>Standard deviation - true value unknown; significance level 99%; 3 redundant measurements.</skos:definition>
    <rdf:type rdf:resource="http://www.w3.org/2004/02/skos/core#Concept"/>
    <skos:prefLabel>MDsd2_LE99r3</skos:prefLabel>
    <dqm:formula rdf:resource="https://standards.isotc211.org/19157/-3/1/dqc/content/formulaType/FTsd2_LE99r3"/>
  </rdf:Description>
  <rdf:Description rdf:about="https://standards.isotc211.org/19157/-3/1/dqc/content/measureDescription/MDsd2_LE68.3r1">
    <skos:definition>Standard deviation - true value unknown; significance level 68.3%; 1 redundant measurement.</skos:definition>
    <skos:prefLabel>MDsd2_LE68.3r1</skos:prefLabel>
    <skos:inScheme rdf:resource="https://standards.isotc211.org/19157/-3/1/dqc/content/measureDescription"/>
    <rdf:type rdf:resource="http://www.w3.org/2004/02/skos/core#Concept"/>
    <dqm:formula rdf:resource="https://standards.isotc211.org/19157/-3/1/dqc/content/formulaType/FTsd2_LE68.3r1"/>
  </rdf:Description>
  <rdf:Description rdf:about="https://standards.isotc211.org/19157/-3/1/dqc/content/measureDescription/MDsd2_LE68.3r4">
    <skos:prefLabel>MDsd2_LE68.3r4</skos:prefLabel>
    <skos:definition>Standard deviation - true value unknown; significance level 68.3%; 4 redundant measurements.</skos:definition>
    <dqm:formula rdf:resource="https://standards.isotc211.org/19157/-3/1/dqc/content/formulaType/FTsd2_LE68.3r4"/>
    <rdf:type rdf:resource="http://www.w3.org/2004/02/skos/core#Concept"/>
    <skos:inScheme rdf:resource="https://standards.isotc211.org/19157/-3/1/dqc/content/measureDescription"/>
  </rdf:Description>
  <rdf:Description rdf:about="https://standards.isotc211.org/19157/-3/1/dqc/content/measureDescription/MD211e">
    <skos:definition>There are 15 street view images in the data. After running a computer vision algorithm to detect blurriness in images, three have been detected as blurry images. </skos:definition>
    <rdf:type rdf:resource="http://www.w3.org/2004/02/skos/core#Concept"/>
    <skos:inScheme rdf:resource="https://standards.isotc211.org/19157/-3/1/dqc/content/measureDescription"/>
    <skos:prefLabel>MD211e</skos:prefLabel>
    <foaf:depiction rdf:resource="https://ogcincubator.github.io/iso19157-3-dqm-register/ISO19157-3/img/MD211e.png"/>
  </rdf:Description>
  <rdf:Description rdf:about="https://standards.isotc211.org/19157/-3/1/dqc/content/measureDescription/MD28_1">
    <dqm:formula rdf:resource="https://standards.isotc211.org/19157/-3/1/dqc/content/formulaType/FT28_1"/>
    <skos:definition>For a number of points (N), the measured positions are given as xmi, ymi and zmi coordinates depending on the dimension in which the position of the point is measured. A corresponding coordinates xti, yti and zti are considered to represent true positions.</skos:definition>
    <rdf:type rdf:resource="http://www.w3.org/2004/02/skos/core#Concept"/>
    <skos:inScheme rdf:resource="https://standards.isotc211.org/19157/-3/1/dqc/content/measureDescription"/>
    <skos:prefLabel>MD28_1</skos:prefLabel>
    <dqm:sequence>1</dqm:sequence>
  </rdf:Description>
  <rdf:Description rdf:about="https://standards.isotc211.org/19157/-3/1/dqc/content/measureDescription/MDsd2_LE99.8r5">
    <dqm:formula rdf:resource="https://standards.isotc211.org/19157/-3/1/dqc/content/formulaType/FTsd2_LE99.8r5"/>
    <skos:definition>Standard deviation - true value unknown; significance level 99.8%; 5 redundant measurements.</skos:definition>
    <skos:prefLabel>MDsd2_LE99.8r5</skos:prefLabel>
    <rdf:type rdf:resource="http://www.w3.org/2004/02/skos/core#Concept"/>
    <skos:inScheme rdf:resource="https://standards.isotc211.org/19157/-3/1/dqc/content/measureDescription"/>
  </rdf:Description>
  <rdf:Description rdf:about="https://standards.isotc211.org/19157/-3/1/dqc/content/measureDescription/MD32_3">
    <skos:inScheme rdf:resource="https://standards.isotc211.org/19157/-3/1/dqc/content/measureDescription"/>
    <dqm:formula rdf:resource="https://standards.isotc211.org/19157/-3/1/dqc/content/formulaType/FT32_7"/>
    <dqm:formula rdf:resource="https://standards.isotc211.org/19157/-3/1/dqc/content/formulaType/FT32_8"/>
    <skos:definition>The covariance matrix generalizes the concept of variance from one to n dimensions, i.e. from scalar-valued random variables to vector-valued random variables (tuples of scalar random variables).</skos:definition>
    <skos:prefLabel>MD32_3</skos:prefLabel>
    <rdf:type rdf:resource="http://www.w3.org/2004/02/skos/core#Concept"/>
    <dqm:sequence>3</dqm:sequence>
  </rdf:Description>
  <rdf:Description rdf:about="https://standards.isotc211.org/19157/-3/1/dqc/content/measureDescription/MD32_4">
    <dqm:sequence>4</dqm:sequence>
    <skos:prefLabel>MD32_4</skos:prefLabel>
    <dqm:formula rdf:resource="https://standards.isotc211.org/19157/-3/1/dqc/content/formulaType/FT32_9"/>
    <dqm:formula rdf:resource="https://standards.isotc211.org/19157/-3/1/dqc/content/formulaType/FT32_10"/>
    <skos:definition>The covariance matrix generalizes the concept of variance from one to n dimensions, i.e. from scalar-valued random variables to vector-valued random variables (tuples of scalar random variables).</skos:definition>
    <rdf:type rdf:resource="http://www.w3.org/2004/02/skos/core#Concept"/>
    <skos:inScheme rdf:resource="https://standards.isotc211.org/19157/-3/1/dqc/content/measureDescription"/>
  </rdf:Description>
  <rdf:Description rdf:about="https://standards.isotc211.org/19157/-3/1/dqc/content/measureDescription/MDsd2_LE99r5">
    <skos:definition>Standard deviation - true value unknown; significance level 99%; 5 redundant measurements.</skos:definition>
    <skos:prefLabel>MDsd2_LE99r5</skos:prefLabel>
    <dqm:formula rdf:resource="https://standards.isotc211.org/19157/-3/1/dqc/content/formulaType/FTsd2_LE99r5"/>
    <rdf:type rdf:resource="http://www.w3.org/2004/02/skos/core#Concept"/>
    <skos:inScheme rdf:resource="https://standards.isotc211.org/19157/-3/1/dqc/content/measureDescription"/>
  </rdf:Description>
  <rdf:Description rdf:about="https://standards.isotc211.org/19157/-3/1/dqc/content/measureDescription/MD4e">
    <skos:definition>Features with identical attribution and identical coordinates representing the same real object, for example: two (or more) points collected on top of each other.
D13288RZ.EPS two (or more) curves collected on top of each other
D13288SZ.EPS two (or more) surfaces collected on top of each other.</skos:definition>
    <skos:prefLabel>MD4e</skos:prefLabel>
    <foaf:depiction rdf:resource="https://ogcincubator.github.io/iso19157-3-dqm-register/ISO19157-3/img/4e_2.PNG"/>
    <foaf:depiction rdf:resource="https://ogcincubator.github.io/iso19157-3-dqm-register/ISO19157-3/img/4e_1.PNG"/>
    <rdf:type rdf:resource="http://www.w3.org/2004/02/skos/core#Concept"/>
    <skos:inScheme rdf:resource="https://standards.isotc211.org/19157/-3/1/dqc/content/measureDescription"/>
  </rdf:Description>
  <rdf:Description rdf:about="https://standards.isotc211.org/19157/-3/1/dqc/content/measureDescription/MDsd2_LE95r3">
    <skos:definition>Standard deviation - true value unknown; significance level 95%; 3 redundant measurements.</skos:definition>
    <skos:inScheme rdf:resource="https://standards.isotc211.org/19157/-3/1/dqc/content/measureDescription"/>
    <rdf:type rdf:resource="http://www.w3.org/2004/02/skos/core#Concept"/>
    <skos:prefLabel>MDsd2_LE95r3</skos:prefLabel>
    <dqm:formula rdf:resource="https://standards.isotc211.org/19157/-3/1/dqc/content/formulaType/FTsd2_LE95r3"/>
  </rdf:Description>
  <rdf:Description rdf:nodeID="N4df3e8306032451892eef51fe2cba317">
    <rdfs:seeAlso rdf:resource="https://github.com/opengeospatial/ogc-na-tools"/>
    <rdf:type rdf:resource="http://www.w3.org/ns/prov#Agent"/>
    <rdf:type rdf:resource="https://schema.org/SoftwareApplication"/>
    <rdfs:label>OGC-NA tools</rdfs:label>
    <rdfs:comment>ogc.na.update_vocabs version 0.3.51</rdfs:comment>
    <dcterms:hasVersion>0.3.51</dcterms:hasVersion>
  </rdf:Description>
  <rdf:Description rdf:about="https://standards.isotc211.org/19157/-3/1/dqc/content/measureDescription/MD2e">
    <skos:definition>2 (12 houses are in the data set although only 10 exist within the universe of discourse).</skos:definition>
    <skos:prefLabel>MD2e</skos:prefLabel>
    <skos:inScheme rdf:resource="https://standards.isotc211.org/19157/-3/1/dqc/content/measureDescription"/>
    <rdf:type rdf:resource="http://www.w3.org/2004/02/skos/core#Concept"/>
  </rdf:Description>
  <rdf:Description rdf:about="https://standards.isotc211.org/19157/-3/1/dqc/content/measureDescription/MD3">
    <skos:inScheme rdf:resource="https://standards.isotc211.org/19157/-3/1/dqc/content/measureDescription"/>
    <rdf:type rdf:resource="http://www.w3.org/2004/02/skos/core#Concept"/>
    <skos:prefLabel>MD3</skos:prefLabel>
    <skos:definition>Divide excess items in relation to number of items in the universe of discourse.</skos:definition>
  </rdf:Description>
  <rdf:Description rdf:about="https://standards.isotc211.org/19157/-3/1/dqc/content/measureDescription/MD66">
    <skos:definition>Number of correct attribute values in relation to the total number of attribute values as described in the specification.</skos:definition>
    <skos:prefLabel>MD66</skos:prefLabel>
    <skos:inScheme rdf:resource="https://standards.isotc211.org/19157/-3/1/dqc/content/measureDescription"/>
    <rdf:type rdf:resource="http://www.w3.org/2004/02/skos/core#Concept"/>
  </rdf:Description>
  <rdf:Description rdf:about="https://standards.isotc211.org/19157/-3/1/dqc/content/measureDescription/MDsd2_LE99r10">
    <skos:definition>Standard deviation - true value unknown; significance level 99%; 10 redundant measurements.</skos:definition>
    <rdf:type rdf:resource="http://www.w3.org/2004/02/skos/core#Concept"/>
    <skos:inScheme rdf:resource="https://standards.isotc211.org/19157/-3/1/dqc/content/measureDescription"/>
    <dqm:formula rdf:resource="https://standards.isotc211.org/19157/-3/1/dqc/content/formulaType/FTsd2_LE99r10"/>
    <skos:prefLabel>MDsd2_LE99r10</skos:prefLabel>
  </rdf:Description>
  <rdf:Description rdf:about="https://standards.isotc211.org/19157/-3/1/dqc/content/measureDescription/MD50">
    <dqm:formula rdf:resource="https://standards.isotc211.org/19157/-3/1/dqc/content/formulaType/FT50_1"/>
    <dqm:formula rdf:resource="https://standards.isotc211.org/19157/-3/1/dqc/content/formulaType/FT50_2"/>
    <dqm:formula rdf:resource="https://standards.isotc211.org/19157/-3/1/dqc/content/formulaType/FT50_3"/>
    <rdf:type rdf:resource="http://www.w3.org/2004/02/skos/core#Concept"/>
    <skos:definition>Calculation of uncertainty ellipse parameters by eigenvalues from a given covariance matrix (https://standards.isotc211.org/19157/-1/1/dqc/content/qualityMeasure/32) of 2D point coordinates.</skos:definition>
    <skos:inScheme rdf:resource="https://standards.isotc211.org/19157/-3/1/dqc/content/measureDescription"/>
    <skos:prefLabel>MD50</skos:prefLabel>
  </rdf:Description>
  <rdf:Description rdf:about="https://standards.isotc211.org/19157/-3/1/dqc/content/measureDescription/MD25e_1">
    <foaf:depiction rdf:resource="https://ogcincubator.github.io/iso19157-3-dqm-register/ISO19157-3/img/25e_1.PNG"/>
    <skos:prefLabel>MD25e_1</skos:prefLabel>
    <rdf:type rdf:resource="http://www.w3.org/2004/02/skos/core#Concept"/>
    <skos:inScheme rdf:resource="https://standards.isotc211.org/19157/-3/1/dqc/content/measureDescription"/>
    <skos:definition>48 (count double line drain and slivers that do not fulfil the threshold values set by thinness ratio and maximum sliver area).
Key: 1) Single line drain
2) Double line drain
a) Maximum area parameter prevents correct double line drain portrayal from being flagged as an error</skos:definition>
  </rdf:Description>
  <rdf:Description rdf:about="https://standards.isotc211.org/19157/-3/1/dqc/content/measureDescription/MD102">
    <skos:prefLabel>MD102</skos:prefLabel>
    <skos:inScheme rdf:resource="https://standards.isotc211.org/19157/-3/1/dqc/content/measureDescription"/>
    <rdf:type rdf:resource="http://www.w3.org/2004/02/skos/core#Concept"/>
    <skos:definition>Indicator of the compliance with the data product specification.</skos:definition>
  </rdf:Description>
  <rdf:Description rdf:about="https://standards.isotc211.org/19157/-3/1/dqc/content/measureDescription/MDsd1xyz_SAS99">
    <skos:definition>Standard deviation 3D - true value known; spherical accuracy standard; significance level 99%.</skos:definition>
    <dqm:formula rdf:resource="https://standards.isotc211.org/19157/-3/1/dqc/content/formulaType/FTsd1xyz_SAS99"/>
    <rdf:type rdf:resource="http://www.w3.org/2004/02/skos/core#Concept"/>
    <skos:inScheme rdf:resource="https://standards.isotc211.org/19157/-3/1/dqc/content/measureDescription"/>
    <skos:prefLabel>MDsd1xyz_SAS99</skos:prefLabel>
  </rdf:Description>
  <rdf:Description rdf:about="https://standards.isotc211.org/19157/-3/1/dqc/content/measureDescription/MDsd1_CE99.8">
    <skos:definition>Standard deviation - true value known; significance level 99.8%.</skos:definition>
    <rdf:type rdf:resource="http://www.w3.org/2004/02/skos/core#Concept"/>
    <skos:inScheme rdf:resource="https://standards.isotc211.org/19157/-3/1/dqc/content/measureDescription"/>
    <dqm:formula rdf:resource="https://standards.isotc211.org/19157/-3/1/dqc/content/formulaType/FTsd1_LE99.8"/>
    <skos:prefLabel>MDsd1_CE99.8</skos:prefLabel>
  </rdf:Description>
  <rdf:Description rdf:about="https://standards.isotc211.org/19157/-3/1/dqc/content/measureDescription/MDsd2_LE90r3">
    <skos:definition>Standard deviation - true value unknown; significance level 90%; 3 redundant measurements.</skos:definition>
    <rdf:type rdf:resource="http://www.w3.org/2004/02/skos/core#Concept"/>
    <skos:inScheme rdf:resource="https://standards.isotc211.org/19157/-3/1/dqc/content/measureDescription"/>
    <dqm:formula rdf:resource="https://standards.isotc211.org/19157/-3/1/dqc/content/formulaType/FTsd2_LE90r3"/>
    <skos:prefLabel>MDsd2_LE90r3</skos:prefLabel>
  </rdf:Description>
  <rdf:Description rdf:about="https://standards.isotc211.org/19157/-3/1/dqc/content/measureDescription/MD212">
    <rdf:type rdf:resource="http://www.w3.org/2004/02/skos/core#Concept"/>
    <skos:inScheme rdf:resource="https://standards.isotc211.org/19157/-3/1/dqc/content/measureDescription"/>
    <skos:definition>The number of records with data present, divided by the total number of records that are supposed to be present.</skos:definition>
    <skos:prefLabel>MD212</skos:prefLabel>
  </rdf:Description>
  <rdf:Description rdf:about="https://standards.isotc211.org/19157/-3/1/dqc/content/measureDescription/MD213e">
    <skos:inScheme rdf:resource="https://standards.isotc211.org/19157/-3/1/dqc/content/measureDescription"/>
    <rdf:type rdf:resource="http://www.w3.org/2004/02/skos/core#Concept"/>
    <foaf:depiction rdf:resource="https://ogcincubator.github.io/iso19157-3-dqm-register/ISO19157-3/img/MD213e.png"/>
    <skos:definition>There are five street view images in the data. It is found in Image 3 that there is one unmasked human face, and in Image 2 that there are two unmasked car plate licences. The rate of occurrence of sensitive information in this data is thus calculated as n/N where n is the number of data instances with sensitive information found, and N is the total number of data instances.</skos:definition>
    <skos:prefLabel>MD213e</skos:prefLabel>
  </rdf:Description>
  <rdf:Description rdf:about="https://standards.isotc211.org/19157/-3/1/dqc/content/measureDescription/MDsd1xy_CE99.8">
    <rdf:type rdf:resource="http://www.w3.org/2004/02/skos/core#Concept"/>
    <skos:inScheme rdf:resource="https://standards.isotc211.org/19157/-3/1/dqc/content/measureDescription"/>
    <skos:prefLabel>MDsd1xy_CE99.8</skos:prefLabel>
    <dqm:formula rdf:resource="https://standards.isotc211.org/19157/-3/1/dqc/content/formulaType/FTsd1xy_CE99.8"/>
    <skos:definition>Standard deviation 2D - true value known; significance level 99.8%.</skos:definition>
  </rdf:Description>
  <rdf:Description rdf:nodeID="N85163b0296794a67b860b276db2c284c">
    <rdfs:seeAlso rdf:resource="https://raw.githubusercontent.com/ogcincubator/iso19157-3-dqm-register/master/sources/MeasureDescription.csv.ttl"/>
    <dcterms:hasVersion>git:4f17dcac9447f6d217612ec525843df2f94db721</dcterms:hasVersion>
    <rdf:type rdf:resource="http://www.w3.org/ns/prov#Entity"/>
    <dcterms:format>text/turtle</dcterms:format>
  </rdf:Description>
  <rdf:Description rdf:about="https://standards.isotc211.org/19157/-3/1/dqc/content/measureDescription/MDBM6">
    <skos:definition>The data product specification shall describe the features and which items shall be collected.</skos:definition>
    <skos:prefLabel>MDBM6</skos:prefLabel>
    <rdf:type rdf:resource="http://www.w3.org/2004/02/skos/core#Concept"/>
    <skos:inScheme rdf:resource="https://standards.isotc211.org/19157/-3/1/dqc/content/measureDescription"/>
  </rdf:Description>
  <rdf:Description rdf:about="https://standards.isotc211.org/19157/-3/1/dqc/content/measureDescription/MDsd1xyz_SEP">
    <dqm:formula rdf:resource="https://standards.isotc211.org/19157/-3/1/dqc/content/formulaType/FTsd1xyz_SEP"/>
    <skos:definition>Standard deviation 3D - true value known; Spherical error probable; significance level 50%.</skos:definition>
    <skos:prefLabel>MDsd1xyz_SEP</skos:prefLabel>
    <rdf:type rdf:resource="http://www.w3.org/2004/02/skos/core#Concept"/>
    <skos:inScheme rdf:resource="https://standards.isotc211.org/19157/-3/1/dqc/content/measureDescription"/>
  </rdf:Description>
  <rdf:Description rdf:about="https://standards.isotc211.org/19157/-3/1/dqc/content/measureDescription/MD25e_2">
    <foaf:depiction rdf:resource="https://ogcincubator.github.io/iso19157-3-dqm-register/ISO19157-3/img/25e_2.PNG"/>
    <skos:prefLabel>MD25e_2</skos:prefLabel>
    <rdf:type rdf:resource="http://www.w3.org/2004/02/skos/core#Concept"/>
    <skos:inScheme rdf:resource="https://standards.isotc211.org/19157/-3/1/dqc/content/measureDescription"/>
    <skos:definition>Key: 1) Sand
2) Sliver
3) Double line drain
b) The sliver is less than the maximum parameter and is flagged for evaluation of possible error.</skos:definition>
  </rdf:Description>
  <rdf:Description rdf:about="https://standards.isotc211.org/19157/-3/1/dqc/content/measureDescription/MDsd2_LE95r1">
    <skos:inScheme rdf:resource="https://standards.isotc211.org/19157/-3/1/dqc/content/measureDescription"/>
    <skos:definition>Standard deviation - true value unknown; significance level 95%; 1 redundant measurement.</skos:definition>
    <dqm:formula rdf:resource="https://standards.isotc211.org/19157/-3/1/dqc/content/formulaType/FTsd2_LE95r1"/>
    <skos:prefLabel>MDsd2_LE95r1</skos:prefLabel>
    <rdf:type rdf:resource="http://www.w3.org/2004/02/skos/core#Concept"/>
  </rdf:Description>
  <rdf:Description rdf:about="https://standards.isotc211.org/19157/-3/1/dqc/content/measureDescription/MD206e">
    <rdf:type rdf:resource="http://www.w3.org/2004/02/skos/core#Concept"/>
    <skos:inScheme rdf:resource="https://standards.isotc211.org/19157/-3/1/dqc/content/measureDescription"/>
    <skos:definition>Tests if a particular quality scope is updated according to its given maintenance and update frequency e.g. “Annually”. Value: yes or no.</skos:definition>
    <skos:prefLabel>MD206e</skos:prefLabel>
  </rdf:Description>
  <rdf:Description rdf:about="https://standards.isotc211.org/19157/-3/1/dqc/content/measureDescription/MDBM5">
    <skos:inScheme rdf:resource="https://standards.isotc211.org/19157/-3/1/dqc/content/measureDescription"/>
    <skos:prefLabel>MDBM5</skos:prefLabel>
    <rdf:type rdf:resource="http://www.w3.org/2004/02/skos/core#Concept"/>
    <skos:definition>The data product specification shall describe the features and how items shall be typed.</skos:definition>
  </rdf:Description>
  <rdf:Description rdf:about="https://standards.isotc211.org/19157/-3/1/dqc/content/measureDescription/MD211">
    <skos:prefLabel>MD211</skos:prefLabel>
    <rdf:type rdf:resource="http://www.w3.org/2004/02/skos/core#Concept"/>
    <skos:inScheme rdf:resource="https://standards.isotc211.org/19157/-3/1/dqc/content/measureDescription"/>
    <skos:definition>Quantity of data that suffers from imperfect coverage, divided by the total quantity of data.</skos:definition>
  </rdf:Description>
  <rdf:Description rdf:about="https://standards.isotc211.org/19157/-3/1/dqc/content/measureDescription/MD52">
    <dqm:formula rdf:resource="https://standards.isotc211.org/19157/-3/1/dqc/content/formulaType/FT52_1"/>
    <dqm:formula rdf:resource="https://standards.isotc211.org/19157/-3/1/dqc/content/formulaType/FT52_5"/>
    <dqm:formula rdf:resource="https://standards.isotc211.org/19157/-3/1/dqc/content/formulaType/FT52_3"/>
    <dqm:formula rdf:resource="https://standards.isotc211.org/19157/-3/1/dqc/content/formulaType/FT52_4"/>
    <dqm:formula rdf:resource="https://standards.isotc211.org/19157/-3/1/dqc/content/formulaType/FT52_2"/>
    <rdf:type rdf:resource="http://www.w3.org/2004/02/skos/core#Concept"/>
    <skos:prefLabel>MD52</skos:prefLabel>
    <skos:definition>A manner of calculating the comparison of the data (measured) and the control (true).</skos:definition>
    <skos:inScheme rdf:resource="https://standards.isotc211.org/19157/-3/1/dqc/content/measureDescription"/>
  </rdf:Description>
  <rdf:Description rdf:about="https://standards.isotc211.org/19157/-3/1/dqc/content/measureDescription/MD67">
    <skos:definition>Number of correct attribute values in relation to the total number of attribute values as described in the specification.</skos:definition>
    <rdf:type rdf:resource="http://www.w3.org/2004/02/skos/core#Concept"/>
    <skos:inScheme rdf:resource="https://standards.isotc211.org/19157/-3/1/dqc/content/measureDescription"/>
    <skos:prefLabel>MD67</skos:prefLabel>
  </rdf:Description>
  <rdf:Description rdf:about="https://standards.isotc211.org/19157/-3/1/dqc/content/measureDescription/MDsd2_LE50r10">
    <skos:definition>Standard deviation - true value unknown; significance level 50%; 10 redundant measurements.</skos:definition>
    <rdf:type rdf:resource="http://www.w3.org/2004/02/skos/core#Concept"/>
    <skos:inScheme rdf:resource="https://standards.isotc211.org/19157/-3/1/dqc/content/measureDescription"/>
    <skos:prefLabel>MDsd2_LE50r10</skos:prefLabel>
    <dqm:formula rdf:resource="https://standards.isotc211.org/19157/-3/1/dqc/content/formulaType/FTsd2_LE50r10"/>
  </rdf:Description>
  <rdf:Description rdf:nodeID="n5b05aa3326324313a7e7ca8d2cd849e5b3">
    <rdf:type rdf:resource="http://www.w3.org/ns/prov#Agent"/>
    <rdf:type rdf:resource="https://schema.org/SoftwareApplication"/>
    <dcterms:hasVersion>0.3.51</dcterms:hasVersion>
    <rdfs:label>OGC-NA tools</rdfs:label>
    <rdfs:seeAlso rdf:resource="https://github.com/opengeospatial/ogc-na-tools"/>
  </rdf:Description>
  <rdf:Description rdf:about="https://standards.isotc211.org/19157/-3/1/dqc/content/measureDescription/MDsd2_LE95r10">
    <dqm:formula rdf:resource="https://standards.isotc211.org/19157/-3/1/dqc/content/formulaType/FTsd2_LE95r10"/>
    <skos:definition>Standard deviation - true value unknown; significance level 95%; 10 redundant measurements.</skos:definition>
    <rdf:type rdf:resource="http://www.w3.org/2004/02/skos/core#Concept"/>
    <skos:prefLabel>MDsd2_LE95r10</skos:prefLabel>
    <skos:inScheme rdf:resource="https://standards.isotc211.org/19157/-3/1/dqc/content/measureDescription"/>
  </rdf:Description>
  <rdf:Description rdf:about="https://raw.githubusercontent.com/ogcincubator/iso19157-3-dqm-register/master/sources/entailed/MeasureDescription.csv.rdf">
    <dcterms:hasVersion>git:4f17dcac9447f6d217612ec525843df2f94db721</dcterms:hasVersion>
    <rdf:type rdf:resource="http://www.w3.org/ns/prov#Entity"/>
    <dcterms:format>application/rdf+xml</dcterms:format>
    <prov:wasGeneratedBy rdf:nodeID="Ne7f8011c60704c1eb0eba51720a78725"/>
    <prov:wasAttributedTo rdf:nodeID="N469a6b46769d4855b54ffff3e1e60b15"/>
  </rdf:Description>
  <rdf:Description rdf:about="https://standards.isotc211.org/19157/-3/1/dqc/content/measureDescription/MDsd1_LE90">
    <dqm:formula rdf:resource="https://standards.isotc211.org/19157/-3/1/dqc/content/formulaType/FTsd1_LE90"/>
    <skos:inScheme rdf:resource="https://standards.isotc211.org/19157/-3/1/dqc/content/measureDescription"/>
    <rdf:type rdf:resource="http://www.w3.org/2004/02/skos/core#Concept"/>
    <skos:definition>Standard deviation - true value known; significance level 90%.</skos:definition>
    <skos:prefLabel>MDsd1_LE90</skos:prefLabel>
  </rdf:Description>
  <rdf:Description rdf:about="https://standards.isotc211.org/19157/-3/1/dqc/content/measureDescription/MD23e">
    <rdf:type rdf:resource="http://www.w3.org/2004/02/skos/core#Concept"/>
    <foaf:depiction rdf:resource="https://ogcincubator.github.io/iso19157-3-dqm-register/ISO19157-3/img/23e.PNG"/>
    <skos:inScheme rdf:resource="https://standards.isotc211.org/19157/-3/1/dqc/content/measureDescription"/>
    <skos:prefLabel>MD23e</skos:prefLabel>
    <skos:definition>Key: 1) search distance = 3 m</skos:definition>
  </rdf:Description>
  <rdf:Description rdf:about="https://standards.isotc211.org/19157/-3/1/dqc/content/measureDescription/MD49">
    <skos:prefLabel>MD49</skos:prefLabel>
    <dqm:formula rdf:resource="https://standards.isotc211.org/19157/-3/1/dqc/content/formulaType/FT49_1"/>
    <dqm:formula rdf:resource="https://standards.isotc211.org/19157/-3/1/dqc/content/formulaType/FT49_8"/>
    <dqm:formula rdf:resource="https://standards.isotc211.org/19157/-3/1/dqc/content/formulaType/FT49_2"/>
    <dqm:formula rdf:resource="https://standards.isotc211.org/19157/-3/1/dqc/content/formulaType/FT49_6"/>
    <dqm:formula rdf:resource="https://standards.isotc211.org/19157/-3/1/dqc/content/formulaType/FT49_4"/>
    <dqm:formula rdf:resource="https://standards.isotc211.org/19157/-3/1/dqc/content/formulaType/FT49_5"/>
    <dqm:formula rdf:resource="https://standards.isotc211.org/19157/-3/1/dqc/content/formulaType/FT49_3"/>
    <dqm:formula rdf:resource="https://standards.isotc211.org/19157/-3/1/dqc/content/formulaType/FT49_7"/>
    <skos:inScheme rdf:resource="https://standards.isotc211.org/19157/-3/1/dqc/content/measureDescription"/>
    <rdf:type rdf:resource="http://www.w3.org/2004/02/skos/core#Concept"/>
    <skos:definition>Absolute horizontal accuracy of the data coordinates, expressed in terms of circular error at 90 % probability given that a bias is present. A manner of calculating the comparison of the data (source) and the control (reference).</skos:definition>
  </rdf:Description>
  <rdf:Description rdf:about="https://standards.isotc211.org/19157/-3/1/dqc/content/measureDescription/MD24e">
    <skos:definition>A road must have a length at least 3 meters. Key: 1) search distance = 3 m</skos:definition>
    <skos:prefLabel>MD24e</skos:prefLabel>
    <foaf:depiction rdf:resource="https://ogcincubator.github.io/iso19157-3-dqm-register/ISO19157-3/img/24e.PNG"/>
    <rdf:type rdf:resource="http://www.w3.org/2004/02/skos/core#Concept"/>
    <skos:inScheme rdf:resource="https://standards.isotc211.org/19157/-3/1/dqc/content/measureDescription"/>
  </rdf:Description>
  <rdf:Description rdf:about="https://standards.isotc211.org/19157/-3/1/dqc/content/measureDescription/MD60">
    <skos:prefLabel>MD60</skos:prefLabel>
    <skos:definition>Number of incorrectly classified features compared to the specification. Features and the classification method as defined in the specification.</skos:definition>
    <skos:inScheme rdf:resource="https://standards.isotc211.org/19157/-3/1/dqc/content/measureDescription"/>
    <rdf:type rdf:resource="http://www.w3.org/2004/02/skos/core#Concept"/>
  </rdf:Description>
  <rdf:Description rdf:about="https://standards.isotc211.org/19157/-3/1/dqc/content/measureDescription/MDsd1xy_CE90">
    <skos:prefLabel>MDsd1xy_CE90</skos:prefLabel>
    <skos:definition>Standard deviation 2D - true value known; significance level 90%.</skos:definition>
    <skos:inScheme rdf:resource="https://standards.isotc211.org/19157/-3/1/dqc/content/measureDescription"/>
    <rdf:type rdf:resource="http://www.w3.org/2004/02/skos/core#Concept"/>
    <dqm:formula rdf:resource="https://standards.isotc211.org/19157/-3/1/dqc/content/formulaType/FTsd1xy_CE90"/>
  </rdf:Description>
  <rdf:Description rdf:nodeID="Ne7f8011c60704c1eb0eba51720a78725">
    <prov:used rdf:nodeID="Nf7095029aaba4a9a838915a8d4aa2ea2"/>
    <prov:used rdf:nodeID="Nb31b7c799d2f441180f7235d2e01478a"/>
    <prov:used rdf:nodeID="Nbb155b54fc024684bf7e4df8eba1a3ce"/>
    <rdf:type rdf:resource="http://www.w3.org/ns/prov#Activity"/>
    <rdfs:label>Entailment and validation</rdfs:label>
    <prov:startedAtTime rdf:datatype="http://www.w3.org/2001/XMLSchema#dateTime">2024-09-11T12:20:22.049559</prov:startedAtTime>
    <prov:endedAtTime rdf:datatype="http://www.w3.org/2001/XMLSchema#dateTime">2024-09-11T12:20:25.485288</prov:endedAtTime>
    <prov:wasInformedBy rdf:nodeID="N6b0aa890b3f44184ab68539d5d3b19e6"/>
    <rdfs:comment>python ogc.na.update_vocabs -w . .ogc/catalog.ttl --batch --base-uri https://raw.githubusercontent.com/ogcincubator/iso19157-3-dqm-register/master --update --graph-store http://defs-dev.opengis.net:8061/fuseki-hosted/data</rdfs:comment>
    <prov:wasAssociatedWith rdf:nodeID="N469a6b46769d4855b54ffff3e1e60b15"/>
  </rdf:Description>
  <rdf:Description rdf:about="https://standards.isotc211.org/19157/-3/1/dqc/content/measureDescription/MDsd2_LE99r1">
    <skos:prefLabel>MDsd2_LE99r1</skos:prefLabel>
    <rdf:type rdf:resource="http://www.w3.org/2004/02/skos/core#Concept"/>
    <skos:inScheme rdf:resource="https://standards.isotc211.org/19157/-3/1/dqc/content/measureDescription"/>
    <skos:definition>Standard deviation - true value unknown; significance level 99%; 1 redundant measurement.</skos:definition>
    <dqm:formula rdf:resource="https://standards.isotc211.org/19157/-3/1/dqc/content/formulaType/FTsd2_LE99r1"/>
  </rdf:Description>
  <rdf:Description rdf:about="https://standards.isotc211.org/19157/-3/1/dqc/content/measureDescription/MD30">
    <skos:inScheme rdf:resource="https://standards.isotc211.org/19157/-3/1/dqc/content/measureDescription"/>
    <dqm:formula rdf:resource="https://standards.isotc211.org/19157/-3/1/dqc/content/formulaType/FT30"/>
    <rdf:type rdf:resource="http://www.w3.org/2004/02/skos/core#Concept"/>
    <skos:prefLabel>MD30</skos:prefLabel>
    <skos:definition>The calculation of ei is given by MD28_1, MD28_2 and MD28_3 in one, two and three dimensions.
A criterion for the establishing of correspondence should also be stated (e.g. allowing for correspondence to the closest position, correspondence on vertices or along lines). The criterion/criteria for finding the corresponding points shall be reported with the data quality evaluation result.</skos:definition>
  </rdf:Description>
  <rdf:Description rdf:about="https://standards.isotc211.org/19157/-3/1/dqc/content/measureDescription/MD7e">
    <rdf:type rdf:resource="http://www.w3.org/2004/02/skos/core#Concept"/>
    <skos:inScheme rdf:resource="https://standards.isotc211.org/19157/-3/1/dqc/content/measureDescription"/>
    <skos:definition>Example 1: 10 % (The data set has 10 % less houses than the universe of discourse).
Example 2: 6,6% of all pixels in the scene is clouded with no ground information.</skos:definition>
    <skos:prefLabel>MD7e</skos:prefLabel>
  </rdf:Description>
  <rdf:Description rdf:about="https://standards.isotc211.org/19157/-3/1/dqc/content/measureDescription/MD39">
    <dqm:formula rdf:resource="https://standards.isotc211.org/19157/-3/1/dqc/content/formulaType/FT39"/>
    <rdf:type rdf:resource="http://www.w3.org/2004/02/skos/core#Concept"/>
    <skos:inScheme rdf:resource="https://standards.isotc211.org/19157/-3/1/dqc/content/measureDescription"/>
    <skos:definition>Estimator of the true value of observable Z.</skos:definition>
    <skos:prefLabel>MD39</skos:prefLabel>
  </rdf:Description>
  <rdf:Description rdf:about="https://standards.isotc211.org/19157/-3/1/dqc/content/measureDescription/MDBM2">
    <rdf:type rdf:resource="http://www.w3.org/2004/02/skos/core#Concept"/>
    <skos:prefLabel>MDBM2</skos:prefLabel>
    <skos:inScheme rdf:resource="https://standards.isotc211.org/19157/-3/1/dqc/content/measureDescription"/>
    <skos:definition>The data product specification shall describe the features and which items shall be collected.</skos:definition>
  </rdf:Description>
  <rdf:Description rdf:about="https://standards.isotc211.org/19157/-3/1/dqc/content/measureDescription/MD105">
    <rdf:type rdf:resource="http://www.w3.org/2004/02/skos/core#Concept"/>
    <skos:inScheme rdf:resource="https://standards.isotc211.org/19157/-3/1/dqc/content/measureDescription"/>
    <skos:definition>Indicator of the compliance with the data product specification.</skos:definition>
    <skos:prefLabel>MD105</skos:prefLabel>
  </rdf:Description>
  <rdf:Description rdf:about="https://standards.isotc211.org/19157/-3/1/dqc/content/measureDescription/MDsd2_LE50r5">
    <rdf:type rdf:resource="http://www.w3.org/2004/02/skos/core#Concept"/>
    <skos:inScheme rdf:resource="https://standards.isotc211.org/19157/-3/1/dqc/content/measureDescription"/>
    <skos:prefLabel>MDsd2_LE50r5</skos:prefLabel>
    <dqm:formula rdf:resource="https://standards.isotc211.org/19157/-3/1/dqc/content/formulaType/FTsd2_LE50r5"/>
    <skos:definition>Standard deviation - true value unknown; significance level 50%; 5 redundant measurements.</skos:definition>
  </rdf:Description>
  <rdf:Description rdf:about="https://standards.isotc211.org/19157/-3/1/dqc/content/measureDescription/MD208_3">
    <dqm:formula rdf:resource="https://standards.isotc211.org/19157/-3/1/dqc/content/formulaType/FT208_A"/>
    <skos:prefLabel>MD208_3</skos:prefLabel>
    <dqm:sequence>3</dqm:sequence>
    <rdf:type rdf:resource="http://www.w3.org/2004/02/skos/core#Concept"/>
    <skos:inScheme rdf:resource="https://standards.isotc211.org/19157/-3/1/dqc/content/measureDescription"/>
    <skos:definition>If reference data is in polygon geometry:
Where a is the area of each segment of reference data that is not captured by the coverage of the source data, n is the total number of uncovered segments, and A is the total area of all reference polygon features.</skos:definition>
  </rdf:Description>
  <rdf:Description rdf:about="https://standards.isotc211.org/19157/-3/1/dqc/content/measureDescription/MDbm4">
    <skos:definition>Boolean value expressing the item is not indicated as an error.</skos:definition>
    <skos:prefLabel>MDbm4</skos:prefLabel>
    <rdf:type rdf:resource="http://www.w3.org/2004/02/skos/core#Concept"/>
    <skos:inScheme rdf:resource="https://standards.isotc211.org/19157/-3/1/dqc/content/measureDescription"/>
  </rdf:Description>
  <rdf:Description rdf:about="https://standards.isotc211.org/19157/-3/1/dqc/content/measureDescription/MDsd1_LE95">
    <skos:definition>Standard deviation - true value known; significance level 95%.</skos:definition>
    <skos:prefLabel>MDsd1_LE95</skos:prefLabel>
    <skos:inScheme rdf:resource="https://standards.isotc211.org/19157/-3/1/dqc/content/measureDescription"/>
    <rdf:type rdf:resource="http://www.w3.org/2004/02/skos/core#Concept"/>
    <dqm:formula rdf:resource="https://standards.isotc211.org/19157/-3/1/dqc/content/formulaType/FTsd1_LE95"/>
  </rdf:Description>
  <rdf:Description rdf:about="https://raw.githubusercontent.com/ogcincubator/iso19157-3-dqm-register/master/sources/entailed/MeasureDescription.csv.ttl">
    <rdf:type rdf:resource="http://www.w3.org/ns/prov#Entity"/>
    <prov:wasAttributedTo rdf:nodeID="N4df3e8306032451892eef51fe2cba317"/>
    <prov:wasGeneratedBy rdf:nodeID="N1eb0b1d7f55640ed87322f7fa3c19b95"/>
    <dcterms:hasVersion>git:4f17dcac9447f6d217612ec525843df2f94db721</dcterms:hasVersion>
    <dcterms:format>text/turtle</dcterms:format>
  </rdf:Description>
  <rdf:Description rdf:about="https://standards.isotc211.org/19157/-3/1/dqc/content/measureDescription/MD209">
    <foaf:depiction rdf:resource="https://ogcincubator.github.io/iso19157-3-dqm-register/ISO19157-3/img/MD209e"/>
    <skos:definition>The number of intervals with a distance longer than a certain threshold, divided by the total number of intervals present in the data. </skos:definition>
    <skos:prefLabel>MD209</skos:prefLabel>
    <rdf:type rdf:resource="http://www.w3.org/2004/02/skos/core#Concept"/>
    <skos:inScheme rdf:resource="https://standards.isotc211.org/19157/-3/1/dqc/content/measureDescription"/>
  </rdf:Description>
  <rdf:Description rdf:about="https://standards.isotc211.org/19157/-3/1/dqc/content/measureDescription/MDsd1xy_CE50">
    <rdf:type rdf:resource="http://www.w3.org/2004/02/skos/core#Concept"/>
    <skos:inScheme rdf:resource="https://standards.isotc211.org/19157/-3/1/dqc/content/measureDescription"/>
    <skos:definition>Standard deviation 2D - true value known; significance level 50%.</skos:definition>
    <dqm:formula rdf:resource="https://standards.isotc211.org/19157/-3/1/dqc/content/formulaType/FTsd1xy_CE50"/>
    <skos:prefLabel>MDsd1xy_CE50</skos:prefLabel>
  </rdf:Description>
  <rdf:Description rdf:about="https://standards.isotc211.org/19157/-3/1/dqc/content/measureDescription/MD14">
    <skos:prefLabel>MD14</skos:prefLabel>
    <rdf:type rdf:resource="http://www.w3.org/2004/02/skos/core#Concept"/>
    <skos:inScheme rdf:resource="https://standards.isotc211.org/19157/-3/1/dqc/content/measureDescription"/>
    <skos:definition>The value true indicates that an item is not in conformance with its value domain.</skos:definition>
  </rdf:Description>
  <rdf:Description rdf:about="https://standards.isotc211.org/19157/-3/1/dqc/content/measureDescription/MD212e">
    <rdf:type rdf:resource="http://www.w3.org/2004/02/skos/core#Concept"/>
    <skos:inScheme rdf:resource="https://standards.isotc211.org/19157/-3/1/dqc/content/measureDescription"/>
    <foaf:depiction rdf:resource="https://ogcincubator.github.io/iso19157-3-dqm-register/ISO19157-3/img/MD212e.png"/>
    <skos:prefLabel>MD212e</skos:prefLabel>
    <skos:definition>There are five instances in the data, and each of them is supposed to have three metadata attributes – Attributes A, B, and C. Symbol ‘x’ in the table indicates a certain metadata is available for the instance
In total, there are 5 empty records, out of 15 (5 × 3) records that are supposed to be available. The rate of metadata omission is thus calculated as 5/15 = 0.333.
The rate of omission can also be calculated for each metadata attribute A, B and C.</skos:definition>
  </rdf:Description>
  <rdf:Description rdf:about="https://standards.isotc211.org/19157/-3/1/dqc/content/measureDescription/MD119">
    <rdf:type rdf:resource="http://www.w3.org/2004/02/skos/core#Concept"/>
    <skos:inScheme rdf:resource="https://standards.isotc211.org/19157/-3/1/dqc/content/measureDescription"/>
    <skos:definition>The value true indicates physical structure conflict.</skos:definition>
    <skos:definition>Indicator of the compliance with the data product specification.</skos:definition>
    <skos:prefLabel>MD119</skos:prefLabel>
  </rdf:Description>
  <rdf:Description rdf:about="https://standards.isotc211.org/19157/-3/1/dqc/content/measureDescription/MD63">
    <skos:inScheme rdf:resource="https://standards.isotc211.org/19157/-3/1/dqc/content/measureDescription"/>
    <rdf:type rdf:resource="http://www.w3.org/2004/02/skos/core#Concept"/>
    <skos:prefLabel>MD63</skos:prefLabel>
    <skos:definition>The relative misclassification matrix (RMCM) is a quadratic matrix with n columns and n rows. n denotes the number of classes under consideration.
RMCM (i,j ) = [# items of class (i ) classified as class (j )] / (# items of class (i )] × 100 %</skos:definition>
  </rdf:Description>
  <rdf:Description rdf:about="https://standards.isotc211.org/19157/-3/1/dqc/content/measureDescription/MD53">
    <dqm:formula rdf:resource="https://standards.isotc211.org/19157/-3/1/dqc/content/formulaType/FT53_5"/>
    <dqm:formula rdf:resource="https://standards.isotc211.org/19157/-3/1/dqc/content/formulaType/FT53_3"/>
    <dqm:formula rdf:resource="https://standards.isotc211.org/19157/-3/1/dqc/content/formulaType/FT53_1"/>
    <dqm:formula rdf:resource="https://standards.isotc211.org/19157/-3/1/dqc/content/formulaType/FT53_4"/>
    <dqm:formula rdf:resource="https://standards.isotc211.org/19157/-3/1/dqc/content/formulaType/FT53_2"/>
    <dqm:formula rdf:resource="https://standards.isotc211.org/19157/-3/1/dqc/content/formulaType/FT53_6"/>
    <skos:prefLabel>MD53</skos:prefLabel>
    <rdf:type rdf:resource="http://www.w3.org/2004/02/skos/core#Concept"/>
    <skos:inScheme rdf:resource="https://standards.isotc211.org/19157/-3/1/dqc/content/measureDescription"/>
    <skos:definition>A manner of calculating the comparison of the data (measured) and the control (true).</skos:definition>
  </rdf:Description>
  <rdf:Description rdf:about="https://standards.isotc211.org/19157/-3/1/dqc/content/measureDescription/MD201e">
    <skos:definition>Rate of objects not in conformity to the tolerance.
In a common area for two datasets the coordinates compare to each other, an error is outside the tolerance.
Key: 1 Search tolerance 0,3 meter</skos:definition>
    <rdf:type rdf:resource="http://www.w3.org/2004/02/skos/core#Concept"/>
    <skos:prefLabel>MD201e</skos:prefLabel>
    <skos:inScheme rdf:resource="https://standards.isotc211.org/19157/-3/1/dqc/content/measureDescription"/>
    <foaf:depiction rdf:resource="https://ogcincubator.github.io/iso19157-3-dqm-register/ISO19157-3/img/201e.PNG"/>
  </rdf:Description>
  <rdf:Description rdf:about="https://standards.isotc211.org/19157/-3/1/dqc/content/measureDescription/MDsd2_LE68.3r3">
    <dqm:formula rdf:resource="https://standards.isotc211.org/19157/-3/1/dqc/content/formulaType/FTsd2_LE68.3r3"/>
    <rdf:type rdf:resource="http://www.w3.org/2004/02/skos/core#Concept"/>
    <skos:inScheme rdf:resource="https://standards.isotc211.org/19157/-3/1/dqc/content/measureDescription"/>
    <skos:definition>Standard deviation - true value unknown; significance level 68.3%; 3 redundant measurements.</skos:definition>
    <skos:prefLabel>MDsd2_LE68.3r3</skos:prefLabel>
  </rdf:Description>
  <rdf:Description rdf:about="https://standards.isotc211.org/19157/-3/1/dqc/content/measureDescription/MD62e">
    <skos:definition>Example misclassification matrix.</skos:definition>
    <rdf:type rdf:resource="http://www.w3.org/2004/02/skos/core#Concept"/>
    <skos:inScheme rdf:resource="https://standards.isotc211.org/19157/-3/1/dqc/content/measureDescription"/>
    <foaf:depiction rdf:resource="https://ogcincubator.github.io/iso19157-3-dqm-register/ISO19157-3/img/62e.PNG"/>
    <skos:prefLabel>MD62e</skos:prefLabel>
  </rdf:Description>
  <rdf:Description rdf:about="https://standards.isotc211.org/19157/-3/1/dqc/content/measureDescription/MDsd1y">
    <dqm:formula rdf:resource="https://standards.isotc211.org/19157/-3/1/dqc/content/formulaType/FTsd1y"/>
    <skos:prefLabel>MDsd1y</skos:prefLabel>
    <rdf:type rdf:resource="http://www.w3.org/2004/02/skos/core#Concept"/>
    <skos:inScheme rdf:resource="https://standards.isotc211.org/19157/-3/1/dqc/content/measureDescription"/>
    <skos:definition>Standard deviation 2D - true value known; direction y.</skos:definition>
  </rdf:Description>
  <rdf:Description rdf:about="https://standards.isotc211.org/19157/-3/1/dqc/content/measureDescription/MD14e">
    <skos:definition>True – a feature with attribute colour has the value ‘blau’, but it does not exist in the specified value domain: red, green, blue, yellow.</skos:definition>
    <rdf:type rdf:resource="http://www.w3.org/2004/02/skos/core#Concept"/>
    <skos:inScheme rdf:resource="https://standards.isotc211.org/19157/-3/1/dqc/content/measureDescription"/>
    <skos:prefLabel>MD14e</skos:prefLabel>
  </rdf:Description>
  <rdf:Description rdf:about="https://standards.isotc211.org/19157/-3/1/dqc/content/measureDescription/MD24">
    <skos:prefLabel>MD24</skos:prefLabel>
    <skos:definition>Search distance as defined in the specification.</skos:definition>
    <rdf:type rdf:resource="http://www.w3.org/2004/02/skos/core#Concept"/>
    <skos:inScheme rdf:resource="https://standards.isotc211.org/19157/-3/1/dqc/content/measureDescription"/>
  </rdf:Description>
  <rdf:Description rdf:about="https://standards.isotc211.org/19157/-3/1/dqc/content/measureDescription/MD128">
    <skos:definition>For a number of points (N), the measured positions are given as xmi, ymi and zmi coordinates depending on the dimension in which the position of the point is measured. A corresponding coordinates xti, yti and zti are considered to represent true positions. A criterion for the establishing of correspondence should also be stated (e.g. allowing for correspondence to the closest position, correspondence on vertices or along lines). The criterion/criteria for finding the corresponding points shall be reported with the data quality evaluation result.</skos:definition>
    <dqm:formula rdf:resource="https://standards.isotc211.org/19157/-3/1/dqc/content/formulaType/FT128_1"/>
    <dqm:formula rdf:resource="https://standards.isotc211.org/19157/-3/1/dqc/content/formulaType/FT128_2"/>
    <skos:inScheme rdf:resource="https://standards.isotc211.org/19157/-3/1/dqc/content/measureDescription"/>
    <rdf:type rdf:resource="http://www.w3.org/2004/02/skos/core#Concept"/>
    <skos:prefLabel>MD128</skos:prefLabel>
  </rdf:Description>
  <rdf:Description rdf:about="https://standards.isotc211.org/19157/-3/1/dqc/content/measureDescription/MDsd1_LE50">
    <dqm:formula rdf:resource="https://standards.isotc211.org/19157/-3/1/dqc/content/formulaType/FTsd1_LE50"/>
    <skos:prefLabel>MDsd1_LE50</skos:prefLabel>
    <rdf:type rdf:resource="http://www.w3.org/2004/02/skos/core#Concept"/>
    <skos:inScheme rdf:resource="https://standards.isotc211.org/19157/-3/1/dqc/content/measureDescription"/>
    <skos:definition>Standard deviation - true value known; significance level 50%.</skos:definition>
  </rdf:Description>
  <rdf:Description rdf:about="https://standards.isotc211.org/19157/-3/1/dqc/content/measureDescription/MD6">
    <skos:prefLabel>MD6</skos:prefLabel>
    <skos:definition>Count number of item not present in the dataset which exists in the universe of discourse.</skos:definition>
    <rdf:type rdf:resource="http://www.w3.org/2004/02/skos/core#Concept"/>
    <skos:inScheme rdf:resource="https://standards.isotc211.org/19157/-3/1/dqc/content/measureDescription"/>
  </rdf:Description>
  <rdf:Description rdf:about="https://standards.isotc211.org/19157/-3/1/dqc/content/measureDescription/MD65e">
    <rdf:type rdf:resource="http://www.w3.org/2004/02/skos/core#Concept"/>
    <skos:inScheme rdf:resource="https://standards.isotc211.org/19157/-3/1/dqc/content/measureDescription"/>
    <skos:definition>5 (5 geographical names are misspelled)</skos:definition>
    <skos:prefLabel>MD65e</skos:prefLabel>
  </rdf:Description>
  <rdf:Description rdf:about="https://standards.isotc211.org/19157/-3/1/dqc/content/measureDescription/MDsd2_LE99.8r10">
    <skos:prefLabel>MDsd2_LE99.8r10</skos:prefLabel>
    <dqm:formula rdf:resource="https://standards.isotc211.org/19157/-3/1/dqc/content/formulaType/FTsd2_LE99.8r10"/>
    <rdf:type rdf:resource="http://www.w3.org/2004/02/skos/core#Concept"/>
    <skos:inScheme rdf:resource="https://standards.isotc211.org/19157/-3/1/dqc/content/measureDescription"/>
    <skos:definition>Standard deviation - true value unknown; significance level 99.8%; 10 redundant measurements.</skos:definition>
  </rdf:Description>
  <rdf:Description rdf:about="https://standards.isotc211.org/19157/-3/1/dqc/content/measureDescription/MD104">
    <skos:prefLabel>MD104</skos:prefLabel>
    <skos:definition>Indicator of the compliance with the data product specification.</skos:definition>
    <rdf:type rdf:resource="http://www.w3.org/2004/02/skos/core#Concept"/>
    <skos:inScheme rdf:resource="https://standards.isotc211.org/19157/-3/1/dqc/content/measureDescription"/>
  </rdf:Description>
  <rdf:Description rdf:about="https://standards.isotc211.org/19157/-3/1/dqc/content/measureDescription/MDsd1xyz_MRSE">
    <skos:inScheme rdf:resource="https://standards.isotc211.org/19157/-3/1/dqc/content/measureDescription"/>
    <rdf:type rdf:resource="http://www.w3.org/2004/02/skos/core#Concept"/>
    <skos:prefLabel>MDsd1xyz_MRSE</skos:prefLabel>
    <dqm:formula rdf:resource="https://standards.isotc211.org/19157/-3/1/dqc/content/formulaType/FTsd1xyz_MRSE"/>
    <skos:definition>Standard deviation 3D - true value known; Mean spherical error; significance level 61%.</skos:definition>
  </rdf:Description>
  <rdf:Description rdf:about="https://standards.isotc211.org/19157/-3/1/dqc/content/measureDescription/MDsd2_LE99.8r2">
    <dqm:formula rdf:resource="https://standards.isotc211.org/19157/-3/1/dqc/content/formulaType/FTsd2_LE99.8r2"/>
    <skos:prefLabel>MDsd2_LE99.8r2</skos:prefLabel>
    <rdf:type rdf:resource="http://www.w3.org/2004/02/skos/core#Concept"/>
    <skos:inScheme rdf:resource="https://standards.isotc211.org/19157/-3/1/dqc/content/measureDescription"/>
    <skos:definition>Standard deviation - true value unknown; significance level 99.8%; 2 redundant measurements.</skos:definition>
  </rdf:Description>
  <rdf:Description rdf:nodeID="N469a6b46769d4855b54ffff3e1e60b15">
    <rdfs:seeAlso rdf:resource="https://github.com/opengeospatial/ogc-na-tools"/>
    <rdf:type rdf:resource="http://www.w3.org/ns/prov#Agent"/>
    <rdf:type rdf:resource="https://schema.org/SoftwareApplication"/>
    <rdfs:label>OGC-NA tools</rdfs:label>
    <rdfs:comment>ogc.na.update_vocabs version 0.3.51</rdfs:comment>
    <dcterms:hasVersion>0.3.51</dcterms:hasVersion>
  </rdf:Description>
  <rdf:Description rdf:about="https://standards.isotc211.org/19157/-3/1/dqc/content/measureDescription/MDsd1xy_CE39.4">
    <dqm:formula rdf:resource="https://standards.isotc211.org/19157/-3/1/dqc/content/formulaType/FTsd1xy_CE39.4"/>
    <skos:prefLabel>MDsd1xy_CE39.4</skos:prefLabel>
    <rdf:type rdf:resource="http://www.w3.org/2004/02/skos/core#Concept"/>
    <skos:inScheme rdf:resource="https://standards.isotc211.org/19157/-3/1/dqc/content/measureDescription"/>
    <skos:definition>Standard deviation 2D - true value known; significance level 39.4%.</skos:definition>
  </rdf:Description>
  <rdf:Description rdf:about="https://standards.isotc211.org/19157/-3/1/dqc/content/measureDescription/MDsd2_LE99.8r4">
    <dqm:formula rdf:resource="https://standards.isotc211.org/19157/-3/1/dqc/content/formulaType/FTsd2_LE99.8r4"/>
    <rdf:type rdf:resource="http://www.w3.org/2004/02/skos/core#Concept"/>
    <skos:inScheme rdf:resource="https://standards.isotc211.org/19157/-3/1/dqc/content/measureDescription"/>
    <skos:prefLabel>MDsd2_LE99.8r4</skos:prefLabel>
    <skos:definition>Standard deviation - true value unknown; significance level 99.8%; 4 redundant measurements.</skos:definition>
  </rdf:Description>
  <rdf:Description rdf:about="https://standards.isotc211.org/19157/-3/1/dqc/content/measureDescription/MD20">
    <skos:inScheme rdf:resource="https://standards.isotc211.org/19157/-3/1/dqc/content/measureDescription"/>
    <skos:definition>Conceptual schema describes the physical structure.</skos:definition>
    <skos:prefLabel>MD20</skos:prefLabel>
    <rdf:type rdf:resource="http://www.w3.org/2004/02/skos/core#Concept"/>
  </rdf:Description>
  <rdf:Description rdf:about="https://standards.isotc211.org/19157/-3/1/dqc/content/measureDescription/MDsd2_LE95r2">
    <skos:prefLabel>MDsd2_LE95r2</skos:prefLabel>
    <skos:definition>Standard deviation - true value unknown; significance level 95%; 2 redundant measurements.</skos:definition>
    <skos:inScheme rdf:resource="https://standards.isotc211.org/19157/-3/1/dqc/content/measureDescription"/>
    <dqm:formula rdf:resource="https://standards.isotc211.org/19157/-3/1/dqc/content/formulaType/FTsd2_LE95r2"/>
    <rdf:type rdf:resource="http://www.w3.org/2004/02/skos/core#Concept"/>
  </rdf:Description>
  <rdf:Description rdf:about="https://standards.isotc211.org/19157/-3/1/dqc/content/measureDescription/MD25">
    <skos:definition>Sliver is an unintended area that occurs when adjacent surfaces are not digitized properly. The borders of the adjacent surfaces may unintentionally gap or overlap by small amounts to cause a topological error.</skos:definition>
    <rdf:type rdf:resource="http://www.w3.org/2004/02/skos/core#Concept"/>
    <skos:inScheme rdf:resource="https://standards.isotc211.org/19157/-3/1/dqc/content/measureDescription"/>
    <skos:prefLabel>MD25</skos:prefLabel>
  </rdf:Description>
  <rdf:Description rdf:nodeID="Nb13b972d4e744b04a38526c2a2ae7942">
    <dcterms:identifier>fd69c946-3328-4566-8849-8d051541eb48</dcterms:identifier>
  </rdf:Description>
  <rdf:Description rdf:about="https://standards.isotc211.org/19157/-3/1/dqc/content/measureDescription/MD62">
    <skos:prefLabel>MD62</skos:prefLabel>
    <foaf:depiction rdf:resource="https://ogcincubator.github.io/iso19157-3-dqm-register/ISO19157-3/img/62.PNG"/>
    <skos:definition>The misclassification matrix (MCM) is a quadratic matrix with n columns and n rows. n denotes the number of classes under consideration.

MCM (i,j) = [# items of class (i) classified as class (j)] The diagonal elements of the misclassification matrix contain the correctly classified items, and the off diagonal elements contain the number of misclassification errors.</skos:definition>
    <rdf:type rdf:resource="http://www.w3.org/2004/02/skos/core#Concept"/>
    <skos:inScheme rdf:resource="https://standards.isotc211.org/19157/-3/1/dqc/content/measureDescription"/>
  </rdf:Description>
  <rdf:Description rdf:about="https://standards.isotc211.org/19157/-3/1/dqc/content/measureDescription/MD12e">
    <skos:definition>0.02 (in a test area there is 227 objects coded as living houses in the dataset but in the universe of discourse there are 231 objects that should be coded as living houses, 4 of them was coded as farm buildings).</skos:definition>
    <skos:prefLabel>MD12e</skos:prefLabel>
    <rdf:type rdf:resource="http://www.w3.org/2004/02/skos/core#Concept"/>
    <skos:inScheme rdf:resource="https://standards.isotc211.org/19157/-3/1/dqc/content/measureDescription"/>
  </rdf:Description>
  <rdf:Description rdf:about="https://standards.isotc211.org/19157/-3/1/dqc/content/measureDescription/MD1">
    <skos:definition>The value true indicates that the item is in excess.</skos:definition>
    <skos:inScheme rdf:resource="https://standards.isotc211.org/19157/-3/1/dqc/content/measureDescription"/>
    <rdf:type rdf:resource="http://www.w3.org/2004/02/skos/core#Concept"/>
    <skos:prefLabel>MD1</skos:prefLabel>
  </rdf:Description>
  <rdf:Description rdf:about="https://standards.isotc211.org/19157/-3/1/dqc/content/measureDescription/MD28_3">
    <dqm:sequence>3</dqm:sequence>
    <skos:prefLabel>MD28_3</skos:prefLabel>
    <dqm:formula rdf:resource="https://standards.isotc211.org/19157/-3/1/dqc/content/formulaType/FT28_3"/>
    <rdf:type rdf:resource="http://www.w3.org/2004/02/skos/core#Concept"/>
    <skos:inScheme rdf:resource="https://standards.isotc211.org/19157/-3/1/dqc/content/measureDescription"/>
    <skos:definition>For a number of points (N), the measured positions are given as xmi, ymi and zmi coordinates depending on the dimension in which the position of the point is measured. A corresponding coordinates xti, yti and zti are considered to represent true positions.</skos:definition>
  </rdf:Description>
  <rdf:Description rdf:about="https://standards.isotc211.org/19157/-3/1/dqc/content/measureDescription/MD3e">
    <skos:definition>10 % (The data set has 10 % more houses than the universe of discourse).</skos:definition>
    <skos:inScheme rdf:resource="https://standards.isotc211.org/19157/-3/1/dqc/content/measureDescription"/>
    <rdf:type rdf:resource="http://www.w3.org/2004/02/skos/core#Concept"/>
    <skos:prefLabel>MD3e</skos:prefLabel>
  </rdf:Description>
  <rdf:Description rdf:about="https://standards.isotc211.org/19157/-3/1/dqc/content/measureDescription/MDsd2">
    <rdf:type rdf:resource="http://www.w3.org/2004/02/skos/core#Concept"/>
    <skos:inScheme rdf:resource="https://standards.isotc211.org/19157/-3/1/dqc/content/measureDescription"/>
    <skos:definition>Standard deviation - true value unknown and it is estimated as the arithmetic mean of the observations.</skos:definition>
    <dqm:formula rdf:resource="https://standards.isotc211.org/19157/-3/1/dqc/content/formulaType/FTsd2"/>
    <skos:prefLabel>MDsd2</skos:prefLabel>
  </rdf:Description>
  <rdf:Description rdf:about="https://standards.isotc211.org/19157/-3/1/dqc/content/measureDescription/MD159">
    <skos:definition>True indicates that there are events incorrectly ordered.</skos:definition>
    <skos:prefLabel>MD159</skos:prefLabel>
    <skos:inScheme rdf:resource="https://standards.isotc211.org/19157/-3/1/dqc/content/measureDescription"/>
    <rdf:type rdf:resource="http://www.w3.org/2004/02/skos/core#Concept"/>
  </rdf:Description>
  <rdf:Description rdf:about="https://standards.isotc211.org/19157/-3/1/dqc/content/measureDescription/MD63e">
    <rdf:type rdf:resource="http://www.w3.org/2004/02/skos/core#Concept"/>
    <skos:inScheme rdf:resource="https://standards.isotc211.org/19157/-3/1/dqc/content/measureDescription"/>
    <skos:definition>Example relative misclassification matrix.</skos:definition>
    <skos:prefLabel>MD63e</skos:prefLabel>
    <foaf:depiction rdf:resource="https://ogcincubator.github.io/iso19157-3-dqm-register/ISO19157-3/img/63e.PNG"/>
  </rdf:Description>
  <rdf:Description rdf:about="https://standards.isotc211.org/19157/-3/1/dqc/content/measureDescription/MDBM4">
    <skos:prefLabel>MDBM4</skos:prefLabel>
    <skos:inScheme rdf:resource="https://standards.isotc211.org/19157/-3/1/dqc/content/measureDescription"/>
    <rdf:type rdf:resource="http://www.w3.org/2004/02/skos/core#Concept"/>
    <skos:definition>Boolean value expressing the item is correct.</skos:definition>
  </rdf:Description>
  <rdf:Description rdf:about="https://standards.isotc211.org/19157/-3/1/dqc/content/measureDescription/MD51">
    <rdf:type rdf:resource="http://www.w3.org/2004/02/skos/core#Concept"/>
    <skos:inScheme rdf:resource="https://standards.isotc211.org/19157/-3/1/dqc/content/measureDescription"/>
    <skos:prefLabel>MD51</skos:prefLabel>
    <dqm:formula rdf:resource="https://standards.isotc211.org/19157/-3/1/dqc/content/formulaType/FT51_1"/>
    <dqm:formula rdf:resource="https://standards.isotc211.org/19157/-3/1/dqc/content/formulaType/FT51_3"/>
    <dqm:formula rdf:resource="https://standards.isotc211.org/19157/-3/1/dqc/content/formulaType/FT51_2"/>
    <skos:definition>Calculation of uncertainty ellipse parameters by eigenvalues from a given covariance matrix (https://standards.isotc211.org/19157/-1/1/dqc/content/qualityMeasure/32) of 2D point coordinates. 
With values for the &lt;span class="inline-formula"&gt;&lt;math xmlns="http://www.w3.org/1998/Math/MathML"&gt; &lt;msubsup&gt; &lt;mi&gt;χ&lt;/mi&gt; &lt;mrow&gt; &lt;mn&gt;1&lt;/mn&gt; &lt;mo&gt;-&lt;/mo&gt; &lt;mi&gt;α&lt;/mi&gt; &lt;/mrow&gt; &lt;mn&gt;2&lt;/mn&gt; &lt;/msubsup&gt; &lt;mfenced&gt; &lt;mn&gt;2&lt;/mn&gt; &lt;/mfenced&gt;&lt;/math&gt;&lt;/span&gt;-distribution of a 2D-confidence ellipse&lt;/div&gt; &lt;div class="sts-p "&gt;&lt;span class="inline-formula"&gt;&lt;math id="id-870f1e92-7dac-44c3-964d-aaca5be575df"&gt; &lt;mi&gt;P&lt;/mi&gt; &lt;mo&gt;=&lt;/mo&gt; &lt;mn&gt;1&lt;/mn&gt; &lt;mo&gt;&lt;/mo&gt; &lt;mi&gt;α&lt;/mi&gt; &lt;mo&gt;=&lt;/mo&gt; &lt;mn&gt;95&lt;/mn&gt; &lt;mo&gt;&lt;/mo&gt; &lt;mo&gt;%&lt;/mo&gt;&lt;/math&gt;&lt;/span&gt;5,99&lt;/div&gt; &lt;div class="sts-p "&gt;&lt;span class="inline-formula"&gt;&lt;math id="id-297effe3-a0bb-4b80-ab4c-cf739b483a55"&gt; &lt;mi&gt;P&lt;/mi&gt; &lt;mo&gt;=&lt;/mo&gt; &lt;mn&gt;1&lt;/mn&gt; &lt;mo&gt;&lt;/mo&gt; &lt;mi&gt;α&lt;/mi&gt; &lt;mo&gt;=&lt;/mo&gt; &lt;mn&gt;99&lt;/mn&gt; &lt;mo&gt;&lt;/mo&gt; &lt;mo&gt;%&lt;/mo&gt;&lt;/math&gt;&lt;/span&gt;9,21</skos:definition>
  </rdf:Description>
  <rdf:Description rdf:about="https://standards.isotc211.org/19157/-3/1/dqc/content/measureDescription">
    <rdf:type rdf:resource="http://www.w3.org/2004/02/skos/core#ConceptScheme"/>
    <skos:prefLabel>ISO19157-3 Data Quality Measures (Extended Description Components)</skos:prefLabel>
    <skos:definition>ISO19157-3 Data Quality Measures (Extended Description Components)</skos:definition>
  </rdf:Description>
  <rdf:Description rdf:about="https://standards.isotc211.org/19157/-3/1/dqc/content/measureDescription/MD29_1">
    <dqm:formula rdf:resource="https://standards.isotc211.org/19157/-3/1/dqc/content/formulaType/FT29_1"/>
    <rdf:type rdf:resource="http://www.w3.org/2004/02/skos/core#Concept"/>
    <skos:inScheme rdf:resource="https://standards.isotc211.org/19157/-3/1/dqc/content/measureDescription"/>
    <skos:prefLabel>MD29_1</skos:prefLabel>
    <dqm:sequence>1</dqm:sequence>
    <skos:definition>The calculation of ei is given by MD28_1, MD28_2 and MD28_3 in one, two and three dimensions. </skos:definition>
  </rdf:Description>
  <rdf:Description rdf:about="https://standards.isotc211.org/19157/-3/1/dqc/content/measureDescription/MDsd2_LE99.8r1">
    <dqm:formula rdf:resource="https://standards.isotc211.org/19157/-3/1/dqc/content/formulaType/FTsd2_LE99.8r1"/>
    <skos:definition>Standard deviation - true value unknown; significance level 99.8%; 1 redundant measurement.</skos:definition>
    <skos:prefLabel>MDsd2_LE99.8r1</skos:prefLabel>
    <rdf:type rdf:resource="http://www.w3.org/2004/02/skos/core#Concept"/>
    <skos:inScheme rdf:resource="https://standards.isotc211.org/19157/-3/1/dqc/content/measureDescription"/>
  </rdf:Description>
  <rdf:Description rdf:about="https://standards.isotc211.org/19157/-3/1/dqc/content/measureDescription/MD4">
    <foaf:depiction rdf:resource="https://ogcincubator.github.io/iso19157-3-dqm-register/ISO19157-3/img/4_2.PNG"/>
    <foaf:depiction rdf:resource="https://ogcincubator.github.io/iso19157-3-dqm-register/ISO19157-3/img/4_1.PNG"/>
    <foaf:depiction rdf:resource="https://ogcincubator.github.io/iso19157-3-dqm-register/ISO19157-3/img/4_3.PNG"/>
    <rdf:type rdf:resource="http://www.w3.org/2004/02/skos/core#Concept"/>
    <skos:inScheme rdf:resource="https://standards.isotc211.org/19157/-3/1/dqc/content/measureDescription"/>
    <skos:prefLabel>MD4</skos:prefLabel>
    <skos:definition>Count of all items in the data that are incorrectly extracted with duplicate geometries.</skos:definition>
  </rdf:Description>
  <rdf:Description rdf:about="https://standards.isotc211.org/19157/-3/1/dqc/content/measureDescription/MDsd2_LE90r1">
    <dqm:formula rdf:resource="https://standards.isotc211.org/19157/-3/1/dqc/content/formulaType/FTsd2_LE90r1"/>
    <rdf:type rdf:resource="http://www.w3.org/2004/02/skos/core#Concept"/>
    <skos:inScheme rdf:resource="https://standards.isotc211.org/19157/-3/1/dqc/content/measureDescription"/>
    <skos:definition>Standard deviation - true value unknown; significance level 90%; 1 redundant measurement.</skos:definition>
    <skos:prefLabel>MDsd2_LE90r1</skos:prefLabel>
  </rdf:Description>
  <rdf:Description rdf:about="https://standards.isotc211.org/19157/-3/1/dqc/content/measureDescription/MD21">
    <skos:prefLabel>MD21</skos:prefLabel>
    <skos:definition>A point-curve connection exists where different curves touch. These curves have an intrinsic topological relationship that shall reflect the true constellation. If the point-curve connection contradicts the universe of discourse, the point-curve connection is faulty with respect to this data quality measure. The data quality measure counts the number of errors of this kind.</skos:definition>
    <rdf:type rdf:resource="http://www.w3.org/2004/02/skos/core#Concept"/>
    <skos:inScheme rdf:resource="https://standards.isotc211.org/19157/-3/1/dqc/content/measureDescription"/>
  </rdf:Description>
  <rdf:Description rdf:about="https://standards.isotc211.org/19157/-3/1/dqc/content/measureDescription/MD103">
    <skos:definition>Indicator of the compliance with the data product specification.</skos:definition>
    <skos:inScheme rdf:resource="https://standards.isotc211.org/19157/-3/1/dqc/content/measureDescription"/>
    <rdf:type rdf:resource="http://www.w3.org/2004/02/skos/core#Concept"/>
    <skos:prefLabel>MD103</skos:prefLabel>
  </rdf:Description>
  <rdf:Description rdf:about="https://standards.isotc211.org/19157/-3/1/dqc/content/measureDescription/MD209e">
    <skos:definition>In this example, there are three sequences of data, S1, S2, and S3. There are eight points in S1 and the interval distance between each pair of consecutive points is measured as d1, d2, … d7. Similarly, d8 and d9 are measured for S2 and d10, d11, and d12 for S3. Among these distances, d3, d5, and d6 are above a specified threshold (e.g. 50 m) indicating lack of continuity in spatial coverage.
The rate of spatial discontinuity in this example is thus calculated as:
where n is the number of intervals with a distance above the threshold, and N is the total number of intervals in the data.</skos:definition>
    <rdf:type rdf:resource="http://www.w3.org/2004/02/skos/core#Concept"/>
    <skos:inScheme rdf:resource="https://standards.isotc211.org/19157/-3/1/dqc/content/measureDescription"/>
    <skos:prefLabel>MD209e</skos:prefLabel>
    <dqm:formula rdf:resource="https://standards.isotc211.org/19157/-3/1/dqc/content/formulaType/FT208_P"/>
  </rdf:Description>
  <rdf:Description rdf:about="https://standards.isotc211.org/19157/-3/1/dqc/content/measureDescription/MD5e">
    <skos:definition>A data product specification requires all towers higher than 300 m to be captured. The data quality measure “missing item” allows a data quality evaluator or a data user to report that a specific item, in this case a feature of type “tower” (name depends on the application schema), is missing.
Data quality scope: all towers with height &gt; 300
Example result of a completeness evaluation of a particular data set:
missing item = true for
tower.name = “Eiffel Tower, Paris, France"
tower.name = “Beijing Tower, Beijing, China”</skos:definition>
    <rdf:type rdf:resource="http://www.w3.org/2004/02/skos/core#Concept"/>
    <skos:prefLabel>MD5e</skos:prefLabel>
    <skos:inScheme rdf:resource="https://standards.isotc211.org/19157/-3/1/dqc/content/measureDescription"/>
  </rdf:Description>
  <rdf:Description rdf:about="https://standards.isotc211.org/19157/-3/1/dqc/content/measureDescription/MD2bme">
    <skos:definition>0.0189</skos:definition>
    <skos:prefLabel>MD2bme</skos:prefLabel>
    <rdf:type rdf:resource="http://www.w3.org/2004/02/skos/core#Concept"/>
    <skos:inScheme rdf:resource="https://standards.isotc211.org/19157/-3/1/dqc/content/measureDescription"/>
  </rdf:Description>
  <rdf:Description rdf:about="https://standards.isotc211.org/19157/-3/1/dqc/content/measureDescription/MD5">
    <skos:prefLabel>MD5</skos:prefLabel>
    <skos:definition>The value true indicates that an item is missing.</skos:definition>
    <skos:inScheme rdf:resource="https://standards.isotc211.org/19157/-3/1/dqc/content/measureDescription"/>
    <rdf:type rdf:resource="http://www.w3.org/2004/02/skos/core#Concept"/>
  </rdf:Description>
  <rdf:Description rdf:about="https://standards.isotc211.org/19157/-3/1/dqc/content/measureDescription/MD18e">
    <skos:prefLabel>MD18e</skos:prefLabel>
    <rdf:type rdf:resource="http://www.w3.org/2004/02/skos/core#Concept"/>
    <skos:inScheme rdf:resource="https://standards.isotc211.org/19157/-3/1/dqc/content/measureDescription"/>
    <skos:definition>10% (Domain of a ‘buildingType’ attribute is defined as the following set of values {1,2,0}; 10 out of 100 ‘building’ objects contain value ‘X’ in ‘buildingType’ attribute).</skos:definition>
  </rdf:Description>
  <rdf:Description rdf:about="https://standards.isotc211.org/19157/-3/1/dqc/content/measureDescription/MD27">
    <skos:prefLabel>MD27</skos:prefLabel>
    <skos:inScheme rdf:resource="https://standards.isotc211.org/19157/-3/1/dqc/content/measureDescription"/>
    <rdf:type rdf:resource="http://www.w3.org/2004/02/skos/core#Concept"/>
    <skos:definition>Topological rules as defined in the specification.</skos:definition>
  </rdf:Description>
  <rdf:Description rdf:about="https://standards.isotc211.org/19157/-3/1/dqc/content/measureDescription/MD31e">
    <skos:definition>The calculation of ei is given by MD28_1, MD28_2 and MD28_3 in one, two and three dimensions.
A criterion for the establishing of correspondence should also be stated (e.g. allowing for correspondence to the closest position, correspondence on vertices or along lines). The criterion/criteria for finding the corresponding points shall be reported with the data quality evaluation result.</skos:definition>
    <skos:definition>25 % of the nodes within the data quality scope have error distance greater than 1 m.</skos:definition>
    <skos:prefLabel>MD31e</skos:prefLabel>
    <rdf:type rdf:resource="http://www.w3.org/2004/02/skos/core#Concept"/>
    <skos:inScheme rdf:resource="https://standards.isotc211.org/19157/-3/1/dqc/content/measureDescription"/>
    <dqm:formula rdf:resource="https://standards.isotc211.org/19157/-3/1/dqc/content/formulaType/FT31"/>
  </rdf:Description>
  <rdf:Description rdf:about="https://standards.isotc211.org/19157/-3/1/dqc/content/measureDescription/MD11">
    <skos:prefLabel>MD11</skos:prefLabel>
    <rdf:type rdf:resource="http://www.w3.org/2004/02/skos/core#Concept"/>
    <skos:inScheme rdf:resource="https://standards.isotc211.org/19157/-3/1/dqc/content/measureDescription"/>
    <skos:definition>Which surfaces may overlap and which shall not is application dependent. Not all overlapping surfaces are necessarily erroneous. When reporting this data quality measure, the types of feature classes corresponding to the illegal overlapping surfaces shall be reported as well. 
See also Complete tessellation: https://standards.isotc211.org/19157/-3/1/dqc/content/measureDescription/MD204</skos:definition>
  </rdf:Description>
  <rdf:Description rdf:about="https://standards.isotc211.org/19157/-3/1/dqc/content/measureDescription/MDsd1_LE68.3">
    <rdf:type rdf:resource="http://www.w3.org/2004/02/skos/core#Concept"/>
    <skos:inScheme rdf:resource="https://standards.isotc211.org/19157/-3/1/dqc/content/measureDescription"/>
    <dqm:formula rdf:resource="https://standards.isotc211.org/19157/-3/1/dqc/content/formulaType/FTsd1_LE68.3"/>
    <skos:definition>Standard deviation - true value known; significance level 68.3%.</skos:definition>
    <skos:prefLabel>MDsd1_LE68.3</skos:prefLabel>
  </rdf:Description>
  <rdf:Description rdf:about="https://standards.isotc211.org/19157/-3/1/dqc/content/measureDescription/MDsd2_LE99r">
    <rdf:type rdf:resource="http://www.w3.org/2004/02/skos/core#Concept"/>
    <skos:inScheme rdf:resource="https://standards.isotc211.org/19157/-3/1/dqc/content/measureDescription"/>
    <skos:definition>Standard deviation - true value unknown; significance level 99%; 2 redundant measurements.</skos:definition>
    <dqm:formula rdf:resource="https://standards.isotc211.org/19157/-3/1/dqc/content/formulaType/FTsd2_LE99r2"/>
    <skos:prefLabel>MDsd2_LE99r</skos:prefLabel>
  </rdf:Description>
  <rdf:Description rdf:about="https://standards.isotc211.org/19157/-3/1/dqc/content/measureDescription/MDsd2_LE68.3r5">
    <dqm:formula rdf:resource="https://standards.isotc211.org/19157/-3/1/dqc/content/formulaType/FTsd2_LE68.3r5"/>
    <skos:prefLabel>MDsd2_LE68.3r5</skos:prefLabel>
    <rdf:type rdf:resource="http://www.w3.org/2004/02/skos/core#Concept"/>
    <skos:inScheme rdf:resource="https://standards.isotc211.org/19157/-3/1/dqc/content/measureDescription"/>
    <skos:definition>Standard deviation - true value unknown; significance level 68.3%; 5 redundant measurements.</skos:definition>
  </rdf:Description>
  <rdf:Description rdf:about="https://standards.isotc211.org/19157/-3/1/dqc/content/measureDescription/MDsd1xyz_SAS90">
    <skos:definition>Standard deviation 3D - true value known; spherical accuracy standard; significance level 90%.</skos:definition>
    <rdf:type rdf:resource="http://www.w3.org/2004/02/skos/core#Concept"/>
    <skos:inScheme rdf:resource="https://standards.isotc211.org/19157/-3/1/dqc/content/measureDescription"/>
    <skos:prefLabel>MDsd1xyz_SAS90</skos:prefLabel>
    <dqm:formula rdf:resource="https://standards.isotc211.org/19157/-3/1/dqc/content/formulaType/FTsd1xyz_SAS90"/>
  </rdf:Description>
  <rdf:Description rdf:nodeID="n5b05aa3326324313a7e7ca8d2cd849e5b2">
    <rdf:type rdf:resource="http://www.w3.org/ns/prov#Entity"/>
    <dcterms:format>application/json</dcterms:format>
    <dcterms:hasVersion>git:57794f311633719a6690d7986204bd7c6f8c06f7</dcterms:hasVersion>
    <rdfs:seeAlso rdf:resource="file:///home/runner/work/iso19157-3-dqm-register/iso19157-3-dqm-register/sources/MeasureDescription.csv.json"/>
  </rdf:Description>
  <rdf:Description rdf:about="https://standards.isotc211.org/19157/-3/1/dqc/content/measureDescription/MDsd2_LE95r5">
    <skos:prefLabel>MDsd2_LE95r5</skos:prefLabel>
    <skos:definition>Standard deviation - true value unknown; significance level 95%; 5 redundant measurements.</skos:definition>
    <dqm:formula rdf:resource="https://standards.isotc211.org/19157/-3/1/dqc/content/formulaType/FTsd2_LE95r5"/>
    <skos:inScheme rdf:resource="https://standards.isotc211.org/19157/-3/1/dqc/content/measureDescription"/>
    <rdf:type rdf:resource="http://www.w3.org/2004/02/skos/core#Concept"/>
  </rdf:Description>
  <rdf:Description rdf:about="https://standards.isotc211.org/19157/-3/1/dqc/content/measureDescription/MDsd2_LE50r2">
    <rdf:type rdf:resource="http://www.w3.org/2004/02/skos/core#Concept"/>
    <dqm:formula rdf:resource="https://standards.isotc211.org/19157/-3/1/dqc/content/formulaType/FTsd2_LE50r2"/>
    <skos:inScheme rdf:resource="https://standards.isotc211.org/19157/-3/1/dqc/content/measureDescription"/>
    <skos:definition>Standard deviation - true value unknown; significance level 50%; 2 redundant measurements.</skos:definition>
    <skos:prefLabel>MDsd2_LE50r2</skos:prefLabel>
  </rdf:Description>
  <rdf:Description rdf:about="https://standards.isotc211.org/19157/-3/1/dqc/content/measureDescription/MDsd2_LE50r3">
    <skos:definition>Standard deviation - true value unknown; significance level 50%; 3 redundant measurements.</skos:definition>
    <dqm:formula rdf:resource="https://standards.isotc211.org/19157/-3/1/dqc/content/formulaType/FTsd2_LE50r3"/>
    <skos:prefLabel>MDsd2_LE50r3</skos:prefLabel>
    <rdf:type rdf:resource="http://www.w3.org/2004/02/skos/core#Concept"/>
    <skos:inScheme rdf:resource="https://standards.isotc211.org/19157/-3/1/dqc/content/measureDescription"/>
  </rdf:Description>
  <rdf:Description rdf:about="https://standards.isotc211.org/19157/-3/1/dqc/content/measureDescription/MD101">
    <rdf:type rdf:resource="http://www.w3.org/2004/02/skos/core#Concept"/>
    <skos:inScheme rdf:resource="https://standards.isotc211.org/19157/-3/1/dqc/content/measureDescription"/>
    <skos:prefLabel>MD101</skos:prefLabel>
    <skos:definition>The measure will take the value true if all the requirements in the referred data product specification are fulfilled.</skos:definition>
  </rdf:Description>
  <rdf:Description rdf:nodeID="N54101fafc1ba44c2aa5e49528e77a94c">
    <dcterms:hasVersion>git:4f17dcac9447f6d217612ec525843df2f94db721</dcterms:hasVersion>
    <rdfs:seeAlso rdf:resource="https://raw.githubusercontent.com/ogcincubator/iso19157-3-dqm-register/master/.ogc/catalog.ttl"/>
    <rdf:type rdf:resource="http://www.w3.org/ns/prov#Entity"/>
    <dcterms:format>text/turtle</dcterms:format>
  </rdf:Description>
  <rdf:Description rdf:about="https://standards.isotc211.org/19157/-3/1/dqc/content/measureDescription/MD28e">
    <rdf:type rdf:resource="http://www.w3.org/2004/02/skos/core#Concept"/>
    <skos:inScheme rdf:resource="https://standards.isotc211.org/19157/-3/1/dqc/content/measureDescription"/>
    <skos:definition>0.054 meter</skos:definition>
    <skos:prefLabel>MD28e</skos:prefLabel>
  </rdf:Description>
  <rdf:Description rdf:about="https://standards.isotc211.org/19157/-3/1/dqc/content/measureDescription/MD22">
    <skos:definition>A point-curve connection exists where different curves touch. These curves have an intrinsic topological relationship that shall reflect the true constellation. If the point-curve connection contradicts the universe of discourse, the point-curve connection is faulty with respect to this data quality measure. This data quality measure gives the erroneous point-curve connections in relation to the total number of point-curve connections.</skos:definition>
    <skos:prefLabel>MD22</skos:prefLabel>
    <skos:inScheme rdf:resource="https://standards.isotc211.org/19157/-3/1/dqc/content/measureDescription"/>
    <rdf:type rdf:resource="http://www.w3.org/2004/02/skos/core#Concept"/>
  </rdf:Description>
  <rdf:Description rdf:about="https://standards.isotc211.org/19157/-3/1/dqc/content/measureDescription/MD65">
    <skos:prefLabel>MD65</skos:prefLabel>
    <rdf:type rdf:resource="http://www.w3.org/2004/02/skos/core#Concept"/>
    <skos:inScheme rdf:resource="https://standards.isotc211.org/19157/-3/1/dqc/content/measureDescription"/>
    <skos:definition>Count of all attribute values where the value is incorrect.</skos:definition>
  </rdf:Description>
  <rdf:Description rdf:about="https://standards.isotc211.org/19157/-3/1/dqc/content/measureDescription/MD26">
    <rdf:type rdf:resource="http://www.w3.org/2004/02/skos/core#Concept"/>
    <skos:inScheme rdf:resource="https://standards.isotc211.org/19157/-3/1/dqc/content/measureDescription"/>
    <skos:definition>Topological rules as defined in the specification.</skos:definition>
    <skos:prefLabel>MD26</skos:prefLabel>
  </rdf:Description>
  <rdf:Description rdf:about="https://standards.isotc211.org/19157/-3/1/dqc/content/measureDescription/MDsd2_LE68.3r10">
    <skos:prefLabel>MDsd2_LE68.3r10</skos:prefLabel>
    <dqm:formula rdf:resource="https://standards.isotc211.org/19157/-3/1/dqc/content/formulaType/FTsd2_LE68.3r10"/>
    <skos:definition>Standard deviation - true value unknown; significance level 68.3%; 10 redundant measurements.</skos:definition>
    <rdf:type rdf:resource="http://www.w3.org/2004/02/skos/core#Concept"/>
    <skos:inScheme rdf:resource="https://standards.isotc211.org/19157/-3/1/dqc/content/measureDescription"/>
  </rdf:Description>
  <rdf:Description rdf:about="https://standards.isotc211.org/19157/-3/1/dqc/content/measureDescription/MDsd2_LE99r4">
    <dqm:formula rdf:resource="https://standards.isotc211.org/19157/-3/1/dqc/content/formulaType/FTsd2_LE99r4"/>
    <skos:prefLabel>MDsd2_LE99r4</skos:prefLabel>
    <skos:definition>Standard deviation - true value unknown; significance level 99%; 4 redundant measurements.</skos:definition>
    <rdf:type rdf:resource="http://www.w3.org/2004/02/skos/core#Concept"/>
    <skos:inScheme rdf:resource="https://standards.isotc211.org/19157/-3/1/dqc/content/measureDescription"/>
  </rdf:Description>
  <rdf:Description rdf:about="https://standards.isotc211.org/19157/-3/1/dqc/content/measureDescription/MD10e">
    <foaf:depiction rdf:resource="https://ogcincubator.github.io/iso19157-3-dqm-register/ISO19157-3/img/10e_4.PNG"/>
    <foaf:depiction rdf:resource="https://ogcincubator.github.io/iso19157-3-dqm-register/ISO19157-3/img/10e_3.PNG"/>
    <foaf:depiction rdf:resource="https://ogcincubator.github.io/iso19157-3-dqm-register/ISO19157-3/img/10e_2.PNG"/>
    <foaf:depiction rdf:resource="https://ogcincubator.github.io/iso19157-3-dqm-register/ISO19157-3/img/10e_1.PNG"/>
    <skos:definition>If the conceptual schema explicitly or implicitly describes rules, these rules shall be followed. Violations against such rules can be, for example, invalid placement of features within a defined tolerance, duplication of features and invalid overlap of features.</skos:definition>
    <skos:definition>Example 1: Towers with identical attribution and within search tolerance (search tolerance = 10 m)
Example 2: Bridge has invalid Transportation. Use Category of Road
Example 3: Invalid placement of Airport inside a Lake
Example 4: Invalid overlap of area feature Lake within line feature Railroad
Key: 1. Bridge 2.  Railroad 3. Lake 4. Airport</skos:definition>
    <rdf:type rdf:resource="http://www.w3.org/2004/02/skos/core#Concept"/>
    <skos:inScheme rdf:resource="https://standards.isotc211.org/19157/-3/1/dqc/content/measureDescription"/>
    <skos:prefLabel>MD10e</skos:prefLabel>
  </rdf:Description>
  <rdf:Description rdf:about="https://standards.isotc211.org/19157/-3/1/dqc/content/measureDescription/MD42">
    <skos:definition>Radius describing a circle, in which the true point location lies with the probability of 39.4%.</skos:definition>
    <skos:prefLabel>MD42</skos:prefLabel>
    <rdf:type rdf:resource="http://www.w3.org/2004/02/skos/core#Concept"/>
    <skos:inScheme rdf:resource="https://standards.isotc211.org/19157/-3/1/dqc/content/measureDescription"/>
  </rdf:Description>
  <rdf:Description rdf:about="https://standards.isotc211.org/19157/-3/1/dqc/content/measureDescription/MD202e">
    <skos:definition>Count error not in compliance with the definition of feature type in the Data Product Specification, DPS In the specification a house shall be stored with perpendicular corners if the real world house is perpendicular.</skos:definition>
    <skos:prefLabel>MD202e</skos:prefLabel>
    <foaf:depiction rdf:resource="https://ogcincubator.github.io/iso19157-3-dqm-register/ISO19157-3/img/202e.PNG"/>
    <rdf:type rdf:resource="http://www.w3.org/2004/02/skos/core#Concept"/>
    <skos:inScheme rdf:resource="https://standards.isotc211.org/19157/-3/1/dqc/content/measureDescription"/>
  </rdf:Description>
  <rdf:Description rdf:about="https://standards.isotc211.org/19157/-3/1/dqc/content/measureDescription/MD64">
    <skos:definition>With the elements of the misclassification matrix (https://standards.isotc211.org/19157/-1/1/dqc/content/qualityMeasure/62).</skos:definition>
    <skos:inScheme rdf:resource="https://standards.isotc211.org/19157/-3/1/dqc/content/measureDescription"/>
    <rdf:type rdf:resource="http://www.w3.org/2004/02/skos/core#Concept"/>
    <dqm:formula rdf:resource="https://standards.isotc211.org/19157/-3/1/dqc/content/formulaType/FT64"/>
    <skos:prefLabel>MD64</skos:prefLabel>
  </rdf:Description>
  <rdf:Description rdf:about="https://standards.isotc211.org/19157/-3/1/dqc/content/measureDescription/MDsd2_LE90r4">
    <skos:definition>Standard deviation - true value unknown; significance level 90%; 4 redundant measurements.</skos:definition>
    <dqm:formula rdf:resource="https://standards.isotc211.org/19157/-3/1/dqc/content/formulaType/FTsd2_LE90r4"/>
    <skos:inScheme rdf:resource="https://standards.isotc211.org/19157/-3/1/dqc/content/measureDescription"/>
    <rdf:type rdf:resource="http://www.w3.org/2004/02/skos/core#Concept"/>
    <skos:prefLabel>MDsd2_LE90r4</skos:prefLabel>
  </rdf:Description>
  <rdf:Description rdf:about="https://standards.isotc211.org/19157/-3/1/dqc/content/measureDescription/MDsd2_LE90r2">
    <skos:inScheme rdf:resource="https://standards.isotc211.org/19157/-3/1/dqc/content/measureDescription"/>
    <rdf:type rdf:resource="http://www.w3.org/2004/02/skos/core#Concept"/>
    <skos:definition>Standard deviation - true value unknown; significance level 90%; 2 redundant measurements.</skos:definition>
    <skos:prefLabel>MDsd2_LE90r2</skos:prefLabel>
    <dqm:formula rdf:resource="https://standards.isotc211.org/19157/-3/1/dqc/content/formulaType/FTsd2_LE90r2"/>
  </rdf:Description>
  <rdf:Description rdf:about="https://standards.isotc211.org/19157/-3/1/dqc/content/measureDescription/MD13e">
    <skos:definition>99.8 % (in the dataset there is 1005 items of 1007 items correct stored in compliance with the conceptual schema).</skos:definition>
    <skos:prefLabel>MD13e</skos:prefLabel>
    <skos:inScheme rdf:resource="https://standards.isotc211.org/19157/-3/1/dqc/content/measureDescription"/>
    <rdf:type rdf:resource="http://www.w3.org/2004/02/skos/core#Concept"/>
  </rdf:Description>
  <rdf:Description rdf:about="https://standards.isotc211.org/19157/-3/1/dqc/content/measureDescription/MD17">
    <skos:prefLabel>MD17</skos:prefLabel>
    <rdf:type rdf:resource="http://www.w3.org/2004/02/skos/core#Concept"/>
    <skos:inScheme rdf:resource="https://standards.isotc211.org/19157/-3/1/dqc/content/measureDescription"/>
    <skos:definition>Conceptual schema describes valid values in the domain.</skos:definition>
  </rdf:Description>
  <rdf:Description rdf:nodeID="n5b05aa3326324313a7e7ca8d2cd849e5b1">
    <prov:used rdf:nodeID="n5b05aa3326324313a7e7ca8d2cd849e5b2"/>
    <prov:wasAssociatedWith rdf:nodeID="n5b05aa3326324313a7e7ca8d2cd849e5b3"/>
    <prov:endedAtTime rdf:datatype="http://www.w3.org/2001/XMLSchema#dateTime">2024-09-10T13:09:31.784619</prov:endedAtTime>
    <prov:startedAtTime rdf:datatype="http://www.w3.org/2001/XMLSchema#dateTime">2024-09-10T13:09:31.533130</prov:startedAtTime>
    <prov:wasInformedBy rdf:nodeID="n5b05aa3326324313a7e7ca8d2cd849e5b4"/>
    <rdf:type rdf:resource="http://www.w3.org/ns/prov#Activity"/>
  </rdf:Description>
  <rdf:Description rdf:about="https://standards.isotc211.org/19157/-3/1/dqc/content/measureDescription/MDsd2_LE50r1">
    <dqm:formula rdf:resource="https://standards.isotc211.org/19157/-3/1/dqc/content/formulaType/FTsd2_LE50r1"/>
    <skos:definition>Standard deviation - true value unknown; significance level 50%; 1 redundant measurement.</skos:definition>
    <rdf:type rdf:resource="http://www.w3.org/2004/02/skos/core#Concept"/>
    <skos:inScheme rdf:resource="https://standards.isotc211.org/19157/-3/1/dqc/content/measureDescription"/>
    <skos:prefLabel>MDsd2_LE50r1</skos:prefLabel>
  </rdf:Description>
  <rdf:Description rdf:about="https://standards.isotc211.org/19157/-3/1/dqc/content/measureDescription/MD8">
    <skos:definition>The value true indicates that an item is not compliant with the rules of the conceptual schema.</skos:definition>
    <skos:prefLabel>MD8</skos:prefLabel>
    <rdf:type rdf:resource="http://www.w3.org/2004/02/skos/core#Concept"/>
    <skos:inScheme rdf:resource="https://standards.isotc211.org/19157/-3/1/dqc/content/measureDescription"/>
  </rdf:Description>
  <rdf:Description rdf:about="https://standards.isotc211.org/19157/-3/1/dqc/content/measureDescription/MDsd2_LE90r10">
    <skos:definition>Standard deviation - true value unknown; significance level 90%; 10 redundant measurements.</skos:definition>
    <dqm:formula rdf:resource="https://standards.isotc211.org/19157/-3/1/dqc/content/formulaType/FTsd2_LE90r10"/>
    <rdf:type rdf:resource="http://www.w3.org/2004/02/skos/core#Concept"/>
    <skos:inScheme rdf:resource="https://standards.isotc211.org/19157/-3/1/dqc/content/measureDescription"/>
    <skos:prefLabel>MDsd2_LE90r10</skos:prefLabel>
  </rdf:Description>
  <rdf:Description rdf:about="https://standards.isotc211.org/19157/-3/1/dqc/content/measureDescription/MDsd1">
    <dqm:formula rdf:resource="https://standards.isotc211.org/19157/-3/1/dqc/content/formulaType/FTsd1"/>
    <rdf:type rdf:resource="http://www.w3.org/2004/02/skos/core#Concept"/>
    <skos:inScheme rdf:resource="https://standards.isotc211.org/19157/-3/1/dqc/content/measureDescription"/>
    <skos:prefLabel>MDsd1</skos:prefLabel>
    <skos:definition>Standard deviation - true value known.</skos:definition>
  </rdf:Description>
  <rdf:Description rdf:about="https://standards.isotc211.org/19157/-3/1/dqc/content/measureDescription/MD207">
    <skos:definition>User defined acceptance quality level.</skos:definition>
    <skos:inScheme rdf:resource="https://standards.isotc211.org/19157/-3/1/dqc/content/measureDescription"/>
    <rdf:type rdf:resource="http://www.w3.org/2004/02/skos/core#Concept"/>
    <skos:prefLabel>MD207</skos:prefLabel>
  </rdf:Description>
  <rdf:Description rdf:about="https://standards.isotc211.org/19157/-3/1/dqc/content/measureDescription/MD47">
    <rdf:type rdf:resource="http://www.w3.org/2004/02/skos/core#Concept"/>
    <skos:inScheme rdf:resource="https://standards.isotc211.org/19157/-3/1/dqc/content/measureDescription"/>
    <skos:definition>Root mean square error of planimetry.</skos:definition>
    <dqm:formula rdf:resource="https://standards.isotc211.org/19157/-3/1/dqc/content/formulaType/FT47"/>
    <skos:prefLabel>MD47</skos:prefLabel>
  </rdf:Description>
  <rdf:Description rdf:about="https://standards.isotc211.org/19157/-3/1/dqc/content/measureDescription/MD204e">
    <skos:definition>Parent polygon dashed (quadrat) filled currently with child polygons (colored) Reporting by parent polygons.</skos:definition>
    <rdf:type rdf:resource="http://www.w3.org/2004/02/skos/core#Concept"/>
    <skos:inScheme rdf:resource="https://standards.isotc211.org/19157/-3/1/dqc/content/measureDescription"/>
    <skos:prefLabel>MD204e</skos:prefLabel>
    <foaf:depiction rdf:resource="https://ogcincubator.github.io/iso19157-3-dqm-register/ISO19157-3/img/204e.PNG"/>
  </rdf:Description>
  <rdf:Description rdf:about="https://standards.isotc211.org/19157/-3/1/dqc/content/measureDescription/MD204">
    <skos:definition>All child polygons must be located inside the parent polygon. Reports the number of child polygons not inside the parent polygon. A set of features instances (set of child’s) which completely, covers the testbed feature.</skos:definition>
    <skos:prefLabel>MD204</skos:prefLabel>
    <skos:inScheme rdf:resource="https://standards.isotc211.org/19157/-3/1/dqc/content/measureDescription"/>
    <rdf:type rdf:resource="http://www.w3.org/2004/02/skos/core#Concept"/>
  </rdf:Description>
  <rdf:Description rdf:about="https://standards.isotc211.org/19157/-3/1/dqc/content/measureDescription/MDsd2_LE68.3r2">
    <dqm:formula rdf:resource="https://standards.isotc211.org/19157/-3/1/dqc/content/formulaType/FTsd2_LE68.3r2"/>
    <skos:prefLabel>MDsd2_LE68.3r2</skos:prefLabel>
    <skos:definition>Standard deviation - true value unknown; significance level 68.3%; 2 redundant measurements.</skos:definition>
    <rdf:type rdf:resource="http://www.w3.org/2004/02/skos/core#Concept"/>
    <skos:inScheme rdf:resource="https://standards.isotc211.org/19157/-3/1/dqc/content/measureDescription"/>
  </rdf:Description>
  <rdf:Description rdf:about="https://standards.isotc211.org/19157/-3/1/dqc/content/measureDescription/MD203">
    <skos:inScheme rdf:resource="https://standards.isotc211.org/19157/-3/1/dqc/content/measureDescription"/>
    <rdf:type rdf:resource="http://www.w3.org/2004/02/skos/core#Concept"/>
    <skos:prefLabel>MD203</skos:prefLabel>
    <skos:definition>The principle of geometric fidelity is that any real world alignment or shape, when viewed at the source survey scale, shall be accurately reflected in the data to the required specification.</skos:definition>
  </rdf:Description>
  <rdf:Description rdf:about="https://standards.isotc211.org/19157/-3/1/dqc/content/measureDescription/MD208_1">
    <dqm:formula rdf:resource="https://standards.isotc211.org/19157/-3/1/dqc/content/formulaType/FT208_P"/>
    <dqm:sequence>1</dqm:sequence>
    <skos:prefLabel>MD208_1</skos:prefLabel>
    <skos:definition>If reference data is in point geometry:
Where n is the total number of reference point features that are not captured by the coverage of source data, and N is the total number of reference point features.</skos:definition>
    <rdf:type rdf:resource="http://www.w3.org/2004/02/skos/core#Concept"/>
    <skos:inScheme rdf:resource="https://standards.isotc211.org/19157/-3/1/dqc/content/measureDescription"/>
  </rdf:Description>
  <rdf:Description rdf:about="https://standards.isotc211.org/19157/-3/1/dqc/content/measureDescription/MD159e">
    <skos:definition>True (5 historical events are present in the dataset but are not ordered correctly).</skos:definition>
    <skos:prefLabel>MD159e</skos:prefLabel>
    <rdf:type rdf:resource="http://www.w3.org/2004/02/skos/core#Concept"/>
    <skos:inScheme rdf:resource="https://standards.isotc211.org/19157/-3/1/dqc/content/measureDescription"/>
  </rdf:Description>
  <rdf:Description rdf:about="https://standards.isotc211.org/19157/-3/1/dqc/content/measureDescription/MD119e">
    <rdf:type rdf:resource="http://www.w3.org/2004/02/skos/core#Concept"/>
    <skos:definition>True (the dataset is stored in wrong file format, a shape file instead of gml).</skos:definition>
    <skos:inScheme rdf:resource="https://standards.isotc211.org/19157/-3/1/dqc/content/measureDescription"/>
    <skos:prefLabel>MD119e</skos:prefLabel>
  </rdf:Description>
  <rdf:Description rdf:about="https://standards.isotc211.org/19157/-3/1/dqc/content/measureDescription/MD6e">
    <skos:definition>2 (10 houses are in the data set although 12 exist within the universe of discourse).</skos:definition>
    <rdf:type rdf:resource="http://www.w3.org/2004/02/skos/core#Concept"/>
    <skos:inScheme rdf:resource="https://standards.isotc211.org/19157/-3/1/dqc/content/measureDescription"/>
    <skos:prefLabel>MD6e</skos:prefLabel>
  </rdf:Description>
  <rdf:Description rdf:about="https://standards.isotc211.org/19157/-3/1/dqc/content/measureDescription/MD201">
    <skos:prefLabel>MD201</skos:prefLabel>
    <skos:definition>Rate of items in a common area representing the same real world object with different coordinates in two different datasets according to a specified tolerance.</skos:definition>
    <skos:inScheme rdf:resource="https://standards.isotc211.org/19157/-3/1/dqc/content/measureDescription"/>
    <rdf:type rdf:resource="http://www.w3.org/2004/02/skos/core#Concept"/>
  </rdf:Description>
  <rdf:Description rdf:nodeID="Ndd11de545b8f4594afde58b69b5ba57d">
    <rdfs:seeAlso rdf:resource="entailments.shapes.ttl"/>
    <rdf:type rdf:resource="http://www.w3.org/ns/prov#Entity"/>
  </rdf:Description>
  <rdf:Description rdf:about="https://standards.isotc211.org/19157/-3/1/dqc/content/measureDescription/MD210">
    <skos:prefLabel>MD210</skos:prefLabel>
    <skos:inScheme rdf:resource="https://standards.isotc211.org/19157/-3/1/dqc/content/measureDescription"/>
    <rdf:type rdf:resource="http://www.w3.org/2004/02/skos/core#Concept"/>
    <skos:definition>The amount of time (e.g. number of years, number of months, number of days, number of hours etc.) during which no data is present, divided by the total amount of time during which data is supposed to be present.</skos:definition>
  </rdf:Description>
  <rdf:Description rdf:about="https://standards.isotc211.org/19157/-3/1/dqc/content/measureDescription/MD18">
    <rdf:type rdf:resource="http://www.w3.org/2004/02/skos/core#Concept"/>
    <skos:inScheme rdf:resource="https://standards.isotc211.org/19157/-3/1/dqc/content/measureDescription"/>
    <skos:definition>Conceptual schema describes valid values in the domain.</skos:definition>
    <skos:prefLabel>MD18</skos:prefLabel>
  </rdf:Description>
  <rdf:Description rdf:about="https://standards.isotc211.org/19157/-3/1/dqc/content/measureDescription/MD28_2">
    <skos:inScheme rdf:resource="https://standards.isotc211.org/19157/-3/1/dqc/content/measureDescription"/>
    <rdf:type rdf:resource="http://www.w3.org/2004/02/skos/core#Concept"/>
    <skos:definition>For a number of points (N), the measured positions are given as xmi, ymi and zmi coordinates depending on the dimension in which the position of the point is measured. A corresponding coordinates xti, yti and zti are considered to represent true positions.</skos:definition>
    <skos:prefLabel>MD28_2</skos:prefLabel>
    <dqm:formula rdf:resource="https://standards.isotc211.org/19157/-3/1/dqc/content/formulaType/FT28_2"/>
    <dqm:sequence>2</dqm:sequence>
  </rdf:Description>
  <rdf:Description rdf:about="https://standards.isotc211.org/19157/-3/1/dqc/content/measureDescription/MD9">
    <skos:prefLabel>MD9</skos:prefLabel>
    <skos:definition>True indicates that an item is in compliance with the rules of the conceptual schema.</skos:definition>
    <rdf:type rdf:resource="http://www.w3.org/2004/02/skos/core#Concept"/>
    <skos:inScheme rdf:resource="https://standards.isotc211.org/19157/-3/1/dqc/content/measureDescription"/>
  </rdf:Description>
  <rdf:Description rdf:about="https://standards.isotc211.org/19157/-3/1/dqc/content/measureDescription/MD27e">
    <foaf:depiction rdf:resource="https://ogcincubator.github.io/iso19157-3-dqm-register/ISO19157-3/img/27e.PNG"/>
    <skos:prefLabel>MD27e</skos:prefLabel>
    <skos:inScheme rdf:resource="https://standards.isotc211.org/19157/-3/1/dqc/content/measureDescription"/>
    <rdf:type rdf:resource="http://www.w3.org/2004/02/skos/core#Concept"/>
    <skos:definition>324 (count road segment with overlap by other road segment)
Key: a) vertices</skos:definition>
  </rdf:Description>
  <rdf:Description rdf:nodeID="n5b05aa3326324313a7e7ca8d2cd849e5b4">
    <dcterms:identifier>8a487b7b-3e4a-4497-9a66-83a6075bf59a</dcterms:identifier>
  </rdf:Description>
  <rdf:Description rdf:about="https://standards.isotc211.org/19157/-3/1/dqc/content/measureDescription/MD19">
    <rdf:type rdf:resource="http://www.w3.org/2004/02/skos/core#Concept"/>
    <skos:inScheme rdf:resource="https://standards.isotc211.org/19157/-3/1/dqc/content/measureDescription"/>
    <skos:definition>Conceptual schema describes the physical structure.</skos:definition>
    <skos:prefLabel>MD19</skos:prefLabel>
  </rdf:Description>
  <rdf:Description rdf:nodeID="Nbb155b54fc024684bf7e4df8eba1a3ce">
    <rdfs:seeAlso rdf:resource="entailments.shapes.ttl"/>
    <rdf:type rdf:resource="http://www.w3.org/ns/prov#Entity"/>
  </rdf:Description>
  <rdf:Description rdf:about="https://standards.isotc211.org/19157/-3/1/dqc/content/measureDescription/MD16">
    <rdf:type rdf:resource="http://www.w3.org/2004/02/skos/core#Concept"/>
    <skos:inScheme rdf:resource="https://standards.isotc211.org/19157/-3/1/dqc/content/measureDescription"/>
    <skos:prefLabel>MD16</skos:prefLabel>
    <skos:definition>Conceptual schema describes valid values in the domain.</skos:definition>
  </rdf:Description>
</rdf:RDF>
