@prefix dcterms: <http://purl.org/dc/terms/> .
@prefix dqm: <http://www.opengis.net/def/metamodel/isodqm/> .
@prefix ns1: <http://www.opengis.net/ogc-na#> .
@prefix prov: <http://www.w3.org/ns/prov#> .
@prefix rdfs: <http://www.w3.org/2000/01/rdf-schema#> .
@prefix schema: <https://schema.org/> .
@prefix skos: <http://www.w3.org/2004/02/skos/core#> .
@prefix xsd: <http://www.w3.org/2001/XMLSchema#> .

<https://raw.githubusercontent.com/ogcincubator/iso19157-3-dqm-register/master/sources/entailed/MeasureParameter.csv.ttl> a prov:Entity ;
    dcterms:format "text/turtle" ;
    dcterms:hasVersion "git:2ee5a3a93f258ce6da3f28b1054485bf73027dd1" ;
    prov:wasAttributedTo _:N555945c9d533410b9bb00bc134ff5ef4 ;
    prov:wasGeneratedBy [ a prov:Activity ;
            rdfs:label "Entailment and validation" ;
            rdfs:comment "python ogc.na.update_vocabs -w . .ogc/catalog.ttl --batch --base-uri https://raw.githubusercontent.com/ogcincubator/iso19157-3-dqm-register/master --update --graph-store http://defs-dev.opengis.net:8061/fuseki-hosted/data" ;
            prov:endedAtTime "2024-09-25T12:25:17.898383"^^xsd:dateTime ;
            prov:startedAtTime "2024-09-25T12:25:17.732798"^^xsd:dateTime ;
            prov:used [ a prov:Entity ;
                    dcterms:format "text/turtle" ;
                    dcterms:hasVersion "git:2ee5a3a93f258ce6da3f28b1054485bf73027dd1" ;
                    rdfs:seeAlso <https://raw.githubusercontent.com/ogcincubator/iso19157-3-dqm-register/master/.ogc/catalog.ttl> ],
                [ a prov:Entity ;
                    rdfs:seeAlso <entailments.shapes.ttl> ],
                [ a prov:Entity ;
                    dcterms:format "text/turtle" ;
                    dcterms:hasVersion "git:2ee5a3a93f258ce6da3f28b1054485bf73027dd1" ;
                    rdfs:seeAlso <https://raw.githubusercontent.com/ogcincubator/iso19157-3-dqm-register/master/sources/MeasureParameter.csv.ttl> ] ;
            prov:wasAssociatedWith _:N555945c9d533410b9bb00bc134ff5ef4 ;
            prov:wasInformedBy [ dcterms:identifier "adfc8266-a8a0-40fd-8a76-23c26fd7be7c" ] ] .

<https://standards.isotc211.org/19157/-3/1/dqc/content/measureParameter/MP1> a dqm:MeasureParameter ;
    dqm:valueType "Real" ;
    skos:broader <https://standards.isotc211.org/19157/-3/1/dqc/content/qualityMeasure/Param> ;
    skos:definition "Minimum of 30 points is normally used but may not always be possible depending on identifiable control points. For feature level attribution sample 10 % of the feature population." ;
    skos:inScheme <https://standards.isotc211.org/19157/-3/1/dqc/content/qualityMeasure> ;
    skos:prefLabel "Sample size" .

<https://standards.isotc211.org/19157/-3/1/dqc/content/measureParameter/MP2> a dqm:MeasureParameter ;
    dqm:valueType "Integer" ;
    skos:broader <https://standards.isotc211.org/19157/-3/1/dqc/content/qualityMeasure/Param> ;
    skos:definition "Number of items." ;
    skos:inScheme <https://standards.isotc211.org/19157/-3/1/dqc/content/qualityMeasure> ;
    skos:prefLabel "n" .

<https://standards.isotc211.org/19157/-3/1/dqc/content/measureParameter/MP201> a dqm:MeasureParameter ;
    skos:broader <https://standards.isotc211.org/19157/-3/1/dqc/content/qualityMeasure/Param> ;
    skos:definition "Tolerance of differences in the coordinates for two datasets." ;
    skos:inScheme <https://standards.isotc211.org/19157/-3/1/dqc/content/qualityMeasure> ;
    skos:prefLabel "Tolerance" .

<https://standards.isotc211.org/19157/-3/1/dqc/content/measureParameter/MP204> a dqm:MeasureParameter ;
    dqm:valueType "Percentage" ;
    skos:broader <https://standards.isotc211.org/19157/-3/1/dqc/content/qualityMeasure/Param> ;
    skos:definition "Identification of child polygons." ;
    skos:inScheme <https://standards.isotc211.org/19157/-3/1/dqc/content/qualityMeasure> ;
    skos:prefLabel "Polygon ID" .

<https://standards.isotc211.org/19157/-3/1/dqc/content/measureParameter/MP205> a dqm:MeasureParameter ;
    skos:broader <https://standards.isotc211.org/19157/-3/1/dqc/content/qualityMeasure/Param> ;
    skos:definition "TM_PeriodDuration described with at least one of the parameters described in ISO 19108:2005." ;
    skos:inScheme <https://standards.isotc211.org/19157/-3/1/dqc/content/qualityMeasure> ;
    skos:prefLabel "User defined maintenance" .

<https://standards.isotc211.org/19157/-3/1/dqc/content/measureParameter/MP206> a dqm:MeasureParameter ;
    dqm:valueType "MD_MaintenanceFrequencyCode" ;
    skos:broader <https://standards.isotc211.org/19157/-3/1/dqc/content/qualityMeasure/Param> ;
    skos:definition "Frequency with which modifications and deletions are made to the data after it is first produced." ;
    skos:inScheme <https://standards.isotc211.org/19157/-3/1/dqc/content/qualityMeasure> ;
    skos:prefLabel "Maintenance and update frequency" .

<https://standards.isotc211.org/19157/-3/1/dqc/content/measureParameter/MP207> a dqm:MeasureParameter ;
    dqm:valueType "Integer" ;
    skos:broader <https://standards.isotc211.org/19157/-3/1/dqc/content/qualityMeasure/Param> ;
    skos:definition "Maximum permitted age as defined in the data product specification." ;
    skos:inScheme <https://standards.isotc211.org/19157/-3/1/dqc/content/qualityMeasure> ;
    skos:prefLabel "Maximum permitted age" .

<https://standards.isotc211.org/19157/-3/1/dqc/content/measureParameter/MP23> a dqm:MeasureParameter ;
    dqm:valueType "Real" ;
    skos:broader <https://standards.isotc211.org/19157/-3/1/dqc/content/qualityMeasure/Param> ;
    skos:definition "Search distance from the end of a dangling line." ;
    skos:inScheme <https://standards.isotc211.org/19157/-3/1/dqc/content/qualityMeasure> ;
    skos:prefLabel "Search distance" .

<https://standards.isotc211.org/19157/-3/1/dqc/content/measureParameter/MP24> a dqm:MeasureParameter ;
    dqm:valueType "Real" ;
    skos:broader <https://standards.isotc211.org/19157/-3/1/dqc/content/qualityMeasure/Param> ;
    skos:definition "Search tolerance of minimum allowable length in the dataset." ;
    skos:inScheme <https://standards.isotc211.org/19157/-3/1/dqc/content/qualityMeasure> ;
    skos:prefLabel "Search tolerance " .

<https://standards.isotc211.org/19157/-3/1/dqc/content/measureParameter/MP25_1> a dqm:MeasureParameter ;
    dqm:valueType "Real" ;
    skos:broader <https://standards.isotc211.org/19157/-3/1/dqc/content/qualityMeasure/Param> ;
    skos:definition "The maximum area determines the upper limit of a sliver. This is to prevent surfaces with sinuous perimeters and large areas from being mistaken as slivers." ;
    skos:inScheme <https://standards.isotc211.org/19157/-3/1/dqc/content/qualityMeasure> ;
    skos:prefLabel "Maximum sliver area size" .

<https://standards.isotc211.org/19157/-3/1/dqc/content/measureParameter/MP25_2> a dqm:MeasureParameter ;
    dcterms:description "MD25" ;
    dqm:valueType "Real" ;
    skos:broader <https://standards.isotc211.org/19157/-3/1/dqc/content/qualityMeasure/Param> ;
    skos:definition """The thickness quotient shall be a real number between 0 and 1. This quotient is determined by the following formula:
T is the thickness quotient
T= 4 Ï€ [area]/[perimeter] 2
T= 1 value corresponds to a circle that has the largest area/perimeter 2 value.
T= 0 value corresponds to a line that has the smallest area/perimeter 2 value""" ;
    skos:inScheme <https://standards.isotc211.org/19157/-3/1/dqc/content/qualityMeasure> ;
    skos:prefLabel "Thickness quotient" .

<https://standards.isotc211.org/19157/-3/1/dqc/content/measureParameter/MP29> a dqm:MeasureParameter ;
    dqm:valueType "Real" ;
    skos:broader <https://standards.isotc211.org/19157/-3/1/dqc/content/qualityMeasure/Param> ;
    skos:definition "Threshold for accepted positional uncertainties." ;
    skos:inScheme <https://standards.isotc211.org/19157/-3/1/dqc/content/qualityMeasure> ;
    skos:prefLabel "emax" .

<https://standards.isotc211.org/19157/-3/1/dqc/content/measureParameter/MP30> a dqm:MeasureParameter ;
    dqm:valueType "Integer" ;
    skos:broader <https://standards.isotc211.org/19157/-3/1/dqc/content/qualityMeasure/Param> ;
    skos:definition "Threshold for accepted positional discrepancy." ;
    skos:inScheme <https://standards.isotc211.org/19157/-3/1/dqc/content/qualityMeasure> ;
    skos:prefLabel "emax" .

<https://standards.isotc211.org/19157/-3/1/dqc/content/measureParameter/MP31> a dqm:MeasureParameter ;
    dqm:valueType "Integer" ;
    skos:broader <https://standards.isotc211.org/19157/-3/1/dqc/content/qualityMeasure/Param> ;
    skos:definition "Threshold above which the positional discrepancies are counted." ;
    skos:inScheme <https://standards.isotc211.org/19157/-3/1/dqc/content/qualityMeasure> ;
    skos:prefLabel "emax" .

<https://standards.isotc211.org/19157/-3/1/dqc/content/measureParameter/MP33> a dqm:MeasureParameter ;
    dcterms:description "50" ;
    dqm:valueType "Percentage" ;
    skos:broader <https://standards.isotc211.org/19157/-3/1/dqc/content/qualityMeasure/Param> ;
    skos:definition "Measure 50%" ;
    skos:inScheme <https://standards.isotc211.org/19157/-3/1/dqc/content/qualityMeasure> ;
    skos:prefLabel "Significance level" .

<https://standards.isotc211.org/19157/-3/1/dqc/content/measureParameter/MP34> a dqm:MeasureParameter ;
    dcterms:description "68.3" ;
    dqm:valueType "Percentage" ;
    skos:broader <https://standards.isotc211.org/19157/-3/1/dqc/content/qualityMeasure/Param> ;
    skos:definition "Measure 68.3%" ;
    skos:inScheme <https://standards.isotc211.org/19157/-3/1/dqc/content/qualityMeasure> ;
    skos:prefLabel "Significance level" .

<https://standards.isotc211.org/19157/-3/1/dqc/content/measureParameter/MP35> a dqm:MeasureParameter ;
    dcterms:description "90" ;
    dqm:valueType "Percentage" ;
    skos:broader <https://standards.isotc211.org/19157/-3/1/dqc/content/qualityMeasure/Param> ;
    skos:definition "Measure 90%" ;
    skos:inScheme <https://standards.isotc211.org/19157/-3/1/dqc/content/qualityMeasure> ;
    skos:prefLabel "Significance level" .

<https://standards.isotc211.org/19157/-3/1/dqc/content/measureParameter/MP36> a dqm:MeasureParameter ;
    dcterms:description "95" ;
    dqm:valueType "Percentage" ;
    skos:broader <https://standards.isotc211.org/19157/-3/1/dqc/content/qualityMeasure/Param> ;
    skos:definition "Measure 95%" ;
    skos:inScheme <https://standards.isotc211.org/19157/-3/1/dqc/content/qualityMeasure> ;
    skos:prefLabel "Significance level" .

<https://standards.isotc211.org/19157/-3/1/dqc/content/measureParameter/MP37> a dqm:MeasureParameter ;
    dcterms:description "99" ;
    dqm:valueType "Percentage" ;
    skos:broader <https://standards.isotc211.org/19157/-3/1/dqc/content/qualityMeasure/Param> ;
    skos:definition "Measure 99%" ;
    skos:inScheme <https://standards.isotc211.org/19157/-3/1/dqc/content/qualityMeasure> ;
    skos:prefLabel "Significance level" .

<https://standards.isotc211.org/19157/-3/1/dqc/content/measureParameter/MP38> a dqm:MeasureParameter ;
    dcterms:description "99.8" ;
    dqm:valueType "Percentage" ;
    skos:broader <https://standards.isotc211.org/19157/-3/1/dqc/content/qualityMeasure/Param> ;
    skos:definition "Measure 99.8%" ;
    skos:inScheme <https://standards.isotc211.org/19157/-3/1/dqc/content/qualityMeasure> ;
    skos:prefLabel "Significance level" .

<https://standards.isotc211.org/19157/-3/1/dqc/content/measureParameter/MP41> a dqm:MeasureParameter ;
    dqm:valueType "Real" ;
    skos:broader <https://standards.isotc211.org/19157/-3/1/dqc/content/qualityMeasure/Param> ;
    skos:definition "Minimum of 30 points is normally used but may not always be possible depending on identifiable control points. For feature level attribution sample 10Â % of the feature population." ;
    skos:inScheme <https://standards.isotc211.org/19157/-3/1/dqc/content/qualityMeasure> ;
    skos:prefLabel "Sample size" .

<https://standards.isotc211.org/19157/-3/1/dqc/content/measureParameter/MP49> a dqm:MeasureParameter ;
    dqm:valueType "Real" ;
    skos:broader <https://standards.isotc211.org/19157/-3/1/dqc/content/qualityMeasure/Param> ;
    skos:definition "Minimum of 30 points is normally used but may not always be possible depending on identifiable control points. For feature level attribution sample 10Â % of the feature population." ;
    skos:inScheme <https://standards.isotc211.org/19157/-3/1/dqc/content/qualityMeasure> ;
    skos:prefLabel "Sample size" .

<https://standards.isotc211.org/19157/-3/1/dqc/content/measureParameter/MP51> a dqm:MeasureParameter ;
    dqm:valueType "Integer" ;
    skos:broader <https://standards.isotc211.org/19157/-3/1/dqc/content/qualityMeasure/Param> ;
    skos:definition "1Î±" ;
    skos:inScheme <https://standards.isotc211.org/19157/-3/1/dqc/content/qualityMeasure> ;
    skos:prefLabel "Significance level" .

<https://standards.isotc211.org/19157/-3/1/dqc/content/measureParameter/MP63_1> a dqm:MeasureParameter ;
    dqm:valueType "Real" ;
    skos:broader <https://standards.isotc211.org/19157/-3/1/dqc/content/qualityMeasure/Param> ;
    skos:definition "Number of classes under consideration." ;
    skos:inScheme <https://standards.isotc211.org/19157/-3/1/dqc/content/qualityMeasure> ;
    skos:prefLabel "n" .

<https://standards.isotc211.org/19157/-3/1/dqc/content/measureParameter/MP63_2> a dqm:MeasureParameter ;
    dqm:valueType "Ratio" ;
    skos:broader <https://standards.isotc211.org/19157/-3/1/dqc/content/qualityMeasure/Param> ;
    skos:definition "Number of classes under consideration." ;
    skos:inScheme <https://standards.isotc211.org/19157/-3/1/dqc/content/qualityMeasure> ;
    skos:prefLabel "n" .

<https://standards.isotc211.org/19157/-3/1/dqc/content/measureParameter/MP63_3> a dqm:MeasureParameter ;
    dqm:valueType "Percentage" ;
    skos:broader <https://standards.isotc211.org/19157/-3/1/dqc/content/qualityMeasure/Param> ;
    skos:definition "Number of classes under consideration." ;
    skos:inScheme <https://standards.isotc211.org/19157/-3/1/dqc/content/qualityMeasure> ;
    skos:prefLabel "n" .

<https://standards.isotc211.org/19157/-3/1/dqc/content/measureParameter/MP68> a dqm:MeasureParameter ;
    dqm:valueType "Percentage" ;
    skos:broader <https://standards.isotc211.org/19157/-3/1/dqc/content/qualityMeasure/Param> ;
    skos:definition "Measure 68.3%" ;
    skos:inScheme <https://standards.isotc211.org/19157/-3/1/dqc/content/qualityMeasure> ;
    skos:prefLabel "Significance level" .

<https://standards.isotc211.org/19157/-3/1/dqc/content/measureParameter/MP69> a dqm:MeasureParameter ;
    dqm:valueType "Percentage" ;
    skos:broader <https://standards.isotc211.org/19157/-3/1/dqc/content/qualityMeasure/Param> ;
    skos:definition "Measure 50%" ;
    skos:inScheme <https://standards.isotc211.org/19157/-3/1/dqc/content/qualityMeasure> ;
    skos:prefLabel "Significance level" .

<https://standards.isotc211.org/19157/-3/1/dqc/content/qualityMeasure> a skos:ConceptScheme ;
    ns1:targetGraph "https://standards.isotc211.org/19157/-3/1/dqc/content/measureParameter" ;
    skos:definition "ISO19157-3 quality measure Parameters" ;
    skos:prefLabel "ISO19157-3 quality measure Parameters" .

[] a prov:Activity ;
    prov:endedAtTime "2024-09-25T04:42:29.009059"^^xsd:dateTime ;
    prov:startedAtTime "2024-09-25T04:42:28.926309"^^xsd:dateTime ;
    prov:used [ a prov:Entity ;
            dcterms:format "application/json" ;
            dcterms:hasVersion "git:8905abaf759b215933ee907f77a56f2a4d68d28b" ;
            rdfs:seeAlso <file:///home/runner/work/iso19157-3-dqm-register/iso19157-3-dqm-register/sources/MeasureParameter.csv.json> ] ;
    prov:wasAssociatedWith [ a prov:Agent,
                schema:SoftwareApplication ;
            rdfs:label "OGC-NA tools" ;
            dcterms:hasVersion "0.3.53" ;
            rdfs:seeAlso <https://github.com/opengeospatial/ogc-na-tools> ] ;
    prov:wasInformedBy [ dcterms:identifier "3c7b094c-0e86-491c-81a7-a371b9ddda0f" ] .

_:N555945c9d533410b9bb00bc134ff5ef4 a prov:Agent,
        schema:SoftwareApplication ;
    rdfs:label "OGC-NA tools" ;
    dcterms:hasVersion "0.3.53" ;
    rdfs:comment "ogc.na.update_vocabs version 0.3.53" ;
    rdfs:seeAlso <https://github.com/opengeospatial/ogc-na-tools> .

