@prefix dcterms: <http://purl.org/dc/terms/> .
@prefix dqm: <http://www.opengis.net/def/metamodel/isodqm/> .
@prefix policy: <http://www.opengis.net/def/metamodel/ogc-na/> .
@prefix prov: <http://www.w3.org/ns/prov#> .
@prefix rdfs: <http://www.w3.org/2000/01/rdf-schema#> .
@prefix schema: <https://schema.org/> .
@prefix skos: <http://www.w3.org/2004/02/skos/core#> .
@prefix xsd: <http://www.w3.org/2001/XMLSchema#> .

<https://raw.githubusercontent.com/ogcincubator/iso19157-3-dqm-register/master/sources/entailed/QualityMeasure.csv.ttl> a prov:Entity ;
    dcterms:format "text/turtle" ;
    prov:wasAttributedTo _:Nf3b2d4a831374ec1a14aef2d4c4cac7f ;
    prov:wasGeneratedBy [ a prov:Activity ;
            rdfs:label "Entailment and validation" ;
            rdfs:comment "python ogc.na.update_vocabs -w . .ogc/catalog.ttl --batch --base-uri https://raw.githubusercontent.com/ogcincubator/iso19157-3-dqm-register/master --update --graph-store http://defs-dev.opengis.net:8061/fuseki-hosted/data" ;
            prov:endedAtTime "2024-09-10T03:30:36.399463"^^xsd:dateTime ;
            prov:startedAtTime "2024-09-10T03:30:36.335815"^^xsd:dateTime ;
            prov:used [ a prov:Entity ;
                    dcterms:format "text/turtle" ;
                    dcterms:hasVersion "git:d4382313268168ee2a17aa1d0e7c97b24668a5ac" ;
                    rdfs:seeAlso <https://raw.githubusercontent.com/ogcincubator/iso19157-3-dqm-register/master/sources/QualityMeasure.csv.ttl> ],
                [ a prov:Entity ;
                    dcterms:format "text/turtle" ;
                    dcterms:hasVersion "git:d4382313268168ee2a17aa1d0e7c97b24668a5ac" ;
                    rdfs:seeAlso <https://raw.githubusercontent.com/ogcincubator/iso19157-3-dqm-register/master/.ogc/catalog.ttl> ] ;
            prov:wasAssociatedWith _:Nf3b2d4a831374ec1a14aef2d4c4cac7f ;
            prov:wasInformedBy [ dcterms:identifier "4bd7d1eb-d699-46c2-960f-12468eb9594d" ] ] .

<https://standards.isotc211.org/19157/-3/1/dqc/content/basicQualityMeasure/> dqm:usedBy _:n61346038c5d14cc38e028ccb9d3332f8b1,
        _:n61346038c5d14cc38e028ccb9d3332f8b2,
        _:n61346038c5d14cc38e028ccb9d3332f8b3,
        _:n61346038c5d14cc38e028ccb9d3332f8b4,
        _:n61346038c5d14cc38e028ccb9d3332f8b5,
        _:n61346038c5d14cc38e028ccb9d3332f8b6 .

<https://standards.isotc211.org/19157/-3/1/dqc/content/basicQualityMeasure/BM1> dqm:usedBy _:n61346038c5d14cc38e028ccb9d3332f8b10,
        _:n61346038c5d14cc38e028ccb9d3332f8b11,
        _:n61346038c5d14cc38e028ccb9d3332f8b12,
        _:n61346038c5d14cc38e028ccb9d3332f8b7,
        _:n61346038c5d14cc38e028ccb9d3332f8b8,
        _:n61346038c5d14cc38e028ccb9d3332f8b9 .

<https://standards.isotc211.org/19157/-3/1/dqc/content/basicQualityMeasure/BM2> dqm:usedBy _:n61346038c5d14cc38e028ccb9d3332f8b13,
        _:n61346038c5d14cc38e028ccb9d3332f8b14,
        _:n61346038c5d14cc38e028ccb9d3332f8b15,
        _:n61346038c5d14cc38e028ccb9d3332f8b16,
        _:n61346038c5d14cc38e028ccb9d3332f8b17,
        _:n61346038c5d14cc38e028ccb9d3332f8b18,
        _:n61346038c5d14cc38e028ccb9d3332f8b19,
        _:n61346038c5d14cc38e028ccb9d3332f8b20,
        _:n61346038c5d14cc38e028ccb9d3332f8b21,
        _:n61346038c5d14cc38e028ccb9d3332f8b22,
        _:n61346038c5d14cc38e028ccb9d3332f8b23,
        _:n61346038c5d14cc38e028ccb9d3332f8b24 .

<https://standards.isotc211.org/19157/-3/1/dqc/content/basicQualityMeasure/BM3> dqm:usedBy _:n61346038c5d14cc38e028ccb9d3332f8b25,
        _:n61346038c5d14cc38e028ccb9d3332f8b26,
        _:n61346038c5d14cc38e028ccb9d3332f8b27,
        _:n61346038c5d14cc38e028ccb9d3332f8b28,
        _:n61346038c5d14cc38e028ccb9d3332f8b29,
        _:n61346038c5d14cc38e028ccb9d3332f8b30,
        _:n61346038c5d14cc38e028ccb9d3332f8b31,
        _:n61346038c5d14cc38e028ccb9d3332f8b32,
        _:n61346038c5d14cc38e028ccb9d3332f8b33,
        _:n61346038c5d14cc38e028ccb9d3332f8b34,
        _:n61346038c5d14cc38e028ccb9d3332f8b35,
        _:n61346038c5d14cc38e028ccb9d3332f8b36,
        _:n61346038c5d14cc38e028ccb9d3332f8b37,
        _:n61346038c5d14cc38e028ccb9d3332f8b38,
        _:n61346038c5d14cc38e028ccb9d3332f8b39,
        _:n61346038c5d14cc38e028ccb9d3332f8b40,
        _:n61346038c5d14cc38e028ccb9d3332f8b41,
        _:n61346038c5d14cc38e028ccb9d3332f8b42 .

<https://standards.isotc211.org/19157/-3/1/dqc/content/basicQualityMeasure/BM4> dqm:usedBy _:n61346038c5d14cc38e028ccb9d3332f8b43,
        _:n61346038c5d14cc38e028ccb9d3332f8b44,
        _:n61346038c5d14cc38e028ccb9d3332f8b45,
        _:n61346038c5d14cc38e028ccb9d3332f8b46,
        _:n61346038c5d14cc38e028ccb9d3332f8b47 .

<https://standards.isotc211.org/19157/-3/1/dqc/content/basicQualityMeasure/BM5> dqm:usedBy _:n61346038c5d14cc38e028ccb9d3332f8b48 .

<https://standards.isotc211.org/19157/-3/1/dqc/content/basicQualityMeasure/BM6> dqm:usedBy _:n61346038c5d14cc38e028ccb9d3332f8b49,
        _:n61346038c5d14cc38e028ccb9d3332f8b50,
        _:n61346038c5d14cc38e028ccb9d3332f8b51,
        _:n61346038c5d14cc38e028ccb9d3332f8b52,
        _:n61346038c5d14cc38e028ccb9d3332f8b53 .

<https://standards.isotc211.org/19157/-3/1/dqc/content/basicQualityMeasure/CE39.4> dqm:usedBy _:n61346038c5d14cc38e028ccb9d3332f8b54 .

<https://standards.isotc211.org/19157/-3/1/dqc/content/basicQualityMeasure/CE50> dqm:usedBy _:n61346038c5d14cc38e028ccb9d3332f8b55 .

<https://standards.isotc211.org/19157/-3/1/dqc/content/basicQualityMeasure/CE90> dqm:usedBy _:n61346038c5d14cc38e028ccb9d3332f8b56 .

<https://standards.isotc211.org/19157/-3/1/dqc/content/basicQualityMeasure/CE95> dqm:usedBy _:n61346038c5d14cc38e028ccb9d3332f8b57 .

<https://standards.isotc211.org/19157/-3/1/dqc/content/basicQualityMeasure/CE99.8> dqm:usedBy _:n61346038c5d14cc38e028ccb9d3332f8b58 .

<https://standards.isotc211.org/19157/-3/1/dqc/content/basicQualityMeasure/LE50LE50r> dqm:usedBy _:n61346038c5d14cc38e028ccb9d3332f8b59,
        _:n61346038c5d14cc38e028ccb9d3332f8b60,
        _:n61346038c5d14cc38e028ccb9d3332f8b61 .

<https://standards.isotc211.org/19157/-3/1/dqc/content/basicQualityMeasure/LE68.3LE68.3r> dqm:usedBy _:n61346038c5d14cc38e028ccb9d3332f8b62,
        _:n61346038c5d14cc38e028ccb9d3332f8b63,
        _:n61346038c5d14cc38e028ccb9d3332f8b64 .

<https://standards.isotc211.org/19157/-3/1/dqc/content/basicQualityMeasure/LE90LE90r> dqm:usedBy _:n61346038c5d14cc38e028ccb9d3332f8b65,
        _:n61346038c5d14cc38e028ccb9d3332f8b66 .

<https://standards.isotc211.org/19157/-3/1/dqc/content/basicQualityMeasure/LE95LE95r> dqm:usedBy _:n61346038c5d14cc38e028ccb9d3332f8b67,
        _:n61346038c5d14cc38e028ccb9d3332f8b68 .

<https://standards.isotc211.org/19157/-3/1/dqc/content/basicQualityMeasure/LE99LE99r> dqm:usedBy _:n61346038c5d14cc38e028ccb9d3332f8b69,
        _:n61346038c5d14cc38e028ccb9d3332f8b70 .

<https://standards.isotc211.org/19157/-3/1/dqc/content/measureDescription/MD1> dqm:describes _:n61346038c5d14cc38e028ccb9d3332f8b8 .

<https://standards.isotc211.org/19157/-3/1/dqc/content/measureDescription/MD10> dqm:describes _:n61346038c5d14cc38e028ccb9d3332f8b41 .

<https://standards.isotc211.org/19157/-3/1/dqc/content/measureDescription/MD101> dqm:describes _:n61346038c5d14cc38e028ccb9d3332f8b44 .

<https://standards.isotc211.org/19157/-3/1/dqc/content/measureDescription/MD102> dqm:describes _:n61346038c5d14cc38e028ccb9d3332f8b33 .

<https://standards.isotc211.org/19157/-3/1/dqc/content/measureDescription/MD103> dqm:describes _:n61346038c5d14cc38e028ccb9d3332f8b48 .

<https://standards.isotc211.org/19157/-3/1/dqc/content/measureDescription/MD104> dqm:describes _:n61346038c5d14cc38e028ccb9d3332f8b17 .

<https://standards.isotc211.org/19157/-3/1/dqc/content/measureDescription/MD105> dqm:describes _:n61346038c5d14cc38e028ccb9d3332f8b49 .

<https://standards.isotc211.org/19157/-3/1/dqc/content/measureDescription/MD11> dqm:describes _:n61346038c5d14cc38e028ccb9d3332f8b29 .

<https://standards.isotc211.org/19157/-3/1/dqc/content/measureDescription/MD119> dqm:describes _:n61346038c5d14cc38e028ccb9d3332f8b11 .

<https://standards.isotc211.org/19157/-3/1/dqc/content/measureDescription/MD12> dqm:describes _:n61346038c5d14cc38e028ccb9d3332f8b23 .

<https://standards.isotc211.org/19157/-3/1/dqc/content/measureDescription/MD128> dqm:describes _:n61346038c5d14cc38e028ccb9d3332f8b71 .

<https://standards.isotc211.org/19157/-3/1/dqc/content/measureDescription/MD13> dqm:describes _:n61346038c5d14cc38e028ccb9d3332f8b53 .

<https://standards.isotc211.org/19157/-3/1/dqc/content/measureDescription/MD14> dqm:describes _:n61346038c5d14cc38e028ccb9d3332f8b12 .

<https://standards.isotc211.org/19157/-3/1/dqc/content/measureDescription/MD15> dqm:describes _:n61346038c5d14cc38e028ccb9d3332f8b46 .

<https://standards.isotc211.org/19157/-3/1/dqc/content/measureDescription/MD159> dqm:describes _:n61346038c5d14cc38e028ccb9d3332f8b9 .

<https://standards.isotc211.org/19157/-3/1/dqc/content/measureDescription/MD16> dqm:describes _:n61346038c5d14cc38e028ccb9d3332f8b28 .

<https://standards.isotc211.org/19157/-3/1/dqc/content/measureDescription/MD17> dqm:describes _:n61346038c5d14cc38e028ccb9d3332f8b51 .

<https://standards.isotc211.org/19157/-3/1/dqc/content/measureDescription/MD18> dqm:describes _:n61346038c5d14cc38e028ccb9d3332f8b18 .

<https://standards.isotc211.org/19157/-3/1/dqc/content/measureDescription/MD19> dqm:describes _:n61346038c5d14cc38e028ccb9d3332f8b34 .

<https://standards.isotc211.org/19157/-3/1/dqc/content/measureDescription/MD2> dqm:describes _:n61346038c5d14cc38e028ccb9d3332f8b36 .

<https://standards.isotc211.org/19157/-3/1/dqc/content/measureDescription/MD20> dqm:describes _:n61346038c5d14cc38e028ccb9d3332f8b16 .

<https://standards.isotc211.org/19157/-3/1/dqc/content/measureDescription/MD201> dqm:describes _:n61346038c5d14cc38e028ccb9d3332f8b13 .

<https://standards.isotc211.org/19157/-3/1/dqc/content/measureDescription/MD202> dqm:describes _:n61346038c5d14cc38e028ccb9d3332f8b40 .

<https://standards.isotc211.org/19157/-3/1/dqc/content/measureDescription/MD203> dqm:describes _:n61346038c5d14cc38e028ccb9d3332f8b19 .

<https://standards.isotc211.org/19157/-3/1/dqc/content/measureDescription/MD204> dqm:describes _:n61346038c5d14cc38e028ccb9d3332f8b22 .

<https://standards.isotc211.org/19157/-3/1/dqc/content/measureDescription/MD205> dqm:describes _:n61346038c5d14cc38e028ccb9d3332f8b47 .

<https://standards.isotc211.org/19157/-3/1/dqc/content/measureDescription/MD206> dqm:describes _:n61346038c5d14cc38e028ccb9d3332f8b43 .

<https://standards.isotc211.org/19157/-3/1/dqc/content/measureDescription/MD207> dqm:describes _:n61346038c5d14cc38e028ccb9d3332f8b52 .

<https://standards.isotc211.org/19157/-3/1/dqc/content/measureDescription/MD208> dqm:describes _:n61346038c5d14cc38e028ccb9d3332f8b72 .

<https://standards.isotc211.org/19157/-3/1/dqc/content/measureDescription/MD209> dqm:describes _:n61346038c5d14cc38e028ccb9d3332f8b73 .

<https://standards.isotc211.org/19157/-3/1/dqc/content/measureDescription/MD21> dqm:describes _:n61346038c5d14cc38e028ccb9d3332f8b42 .

<https://standards.isotc211.org/19157/-3/1/dqc/content/measureDescription/MD210> dqm:describes _:n61346038c5d14cc38e028ccb9d3332f8b74 .

<https://standards.isotc211.org/19157/-3/1/dqc/content/measureDescription/MD211> dqm:describes _:n61346038c5d14cc38e028ccb9d3332f8b75 .

<https://standards.isotc211.org/19157/-3/1/dqc/content/measureDescription/MD212> dqm:describes _:n61346038c5d14cc38e028ccb9d3332f8b76 .

<https://standards.isotc211.org/19157/-3/1/dqc/content/measureDescription/MD213> dqm:describes _:n61346038c5d14cc38e028ccb9d3332f8b77 .

<https://standards.isotc211.org/19157/-3/1/dqc/content/measureDescription/MD22> dqm:describes _:n61346038c5d14cc38e028ccb9d3332f8b15 .

<https://standards.isotc211.org/19157/-3/1/dqc/content/measureDescription/MD23> dqm:describes _:n61346038c5d14cc38e028ccb9d3332f8b39 .

<https://standards.isotc211.org/19157/-3/1/dqc/content/measureDescription/MD24> dqm:describes _:n61346038c5d14cc38e028ccb9d3332f8b26 .

<https://standards.isotc211.org/19157/-3/1/dqc/content/measureDescription/MD25> dqm:describes _:n61346038c5d14cc38e028ccb9d3332f8b30 .

<https://standards.isotc211.org/19157/-3/1/dqc/content/measureDescription/MD26> dqm:describes _:n61346038c5d14cc38e028ccb9d3332f8b31 .

<https://standards.isotc211.org/19157/-3/1/dqc/content/measureDescription/MD27> dqm:describes _:n61346038c5d14cc38e028ccb9d3332f8b27 .

<https://standards.isotc211.org/19157/-3/1/dqc/content/measureDescription/MD28_1> dqm:describes _:n61346038c5d14cc38e028ccb9d3332f8b78 .

<https://standards.isotc211.org/19157/-3/1/dqc/content/measureDescription/MD28_2> dqm:describes _:n61346038c5d14cc38e028ccb9d3332f8b78 .

<https://standards.isotc211.org/19157/-3/1/dqc/content/measureDescription/MD28_3> dqm:describes _:n61346038c5d14cc38e028ccb9d3332f8b78 .

<https://standards.isotc211.org/19157/-3/1/dqc/content/measureDescription/MD29_1> dqm:describes _:n61346038c5d14cc38e028ccb9d3332f8b79 .

<https://standards.isotc211.org/19157/-3/1/dqc/content/measureDescription/MD29_2> dqm:describes _:n61346038c5d14cc38e028ccb9d3332f8b79 .

<https://standards.isotc211.org/19157/-3/1/dqc/content/measureDescription/MD3> dqm:describes _:n61346038c5d14cc38e028ccb9d3332f8b20 .

<https://standards.isotc211.org/19157/-3/1/dqc/content/measureDescription/MD30> dqm:describes _:n61346038c5d14cc38e028ccb9d3332f8b25 .

<https://standards.isotc211.org/19157/-3/1/dqc/content/measureDescription/MD31> dqm:describes _:n61346038c5d14cc38e028ccb9d3332f8b80 .

<https://standards.isotc211.org/19157/-3/1/dqc/content/measureDescription/MD32_1> dqm:describes _:n61346038c5d14cc38e028ccb9d3332f8b81 .

<https://standards.isotc211.org/19157/-3/1/dqc/content/measureDescription/MD32_2> dqm:describes _:n61346038c5d14cc38e028ccb9d3332f8b81 .

<https://standards.isotc211.org/19157/-3/1/dqc/content/measureDescription/MD32_3> dqm:describes _:n61346038c5d14cc38e028ccb9d3332f8b81 .

<https://standards.isotc211.org/19157/-3/1/dqc/content/measureDescription/MD32_4> dqm:describes _:n61346038c5d14cc38e028ccb9d3332f8b81 .

<https://standards.isotc211.org/19157/-3/1/dqc/content/measureDescription/MD39> dqm:describes _:n61346038c5d14cc38e028ccb9d3332f8b82 .

<https://standards.isotc211.org/19157/-3/1/dqc/content/measureDescription/MD4> dqm:describes _:n61346038c5d14cc38e028ccb9d3332f8b37 .

<https://standards.isotc211.org/19157/-3/1/dqc/content/measureDescription/MD40> dqm:describes _:n61346038c5d14cc38e028ccb9d3332f8b83 .

<https://standards.isotc211.org/19157/-3/1/dqc/content/measureDescription/MD41> dqm:describes _:n61346038c5d14cc38e028ccb9d3332f8b84 .

<https://standards.isotc211.org/19157/-3/1/dqc/content/measureDescription/MD42> dqm:describes _:n61346038c5d14cc38e028ccb9d3332f8b54,
        _:n61346038c5d14cc38e028ccb9d3332f8b55,
        _:n61346038c5d14cc38e028ccb9d3332f8b56,
        _:n61346038c5d14cc38e028ccb9d3332f8b57,
        _:n61346038c5d14cc38e028ccb9d3332f8b58 .

<https://standards.isotc211.org/19157/-3/1/dqc/content/measureDescription/MD47> dqm:describes _:n61346038c5d14cc38e028ccb9d3332f8b85 .

<https://standards.isotc211.org/19157/-3/1/dqc/content/measureDescription/MD48> dqm:describes _:n61346038c5d14cc38e028ccb9d3332f8b86 .

<https://standards.isotc211.org/19157/-3/1/dqc/content/measureDescription/MD49> dqm:describes _:n61346038c5d14cc38e028ccb9d3332f8b87 .

<https://standards.isotc211.org/19157/-3/1/dqc/content/measureDescription/MD5> dqm:describes _:n61346038c5d14cc38e028ccb9d3332f8b7 .

<https://standards.isotc211.org/19157/-3/1/dqc/content/measureDescription/MD50> dqm:describes _:n61346038c5d14cc38e028ccb9d3332f8b88 .

<https://standards.isotc211.org/19157/-3/1/dqc/content/measureDescription/MD51> dqm:describes _:n61346038c5d14cc38e028ccb9d3332f8b89 .

<https://standards.isotc211.org/19157/-3/1/dqc/content/measureDescription/MD52> dqm:describes _:n61346038c5d14cc38e028ccb9d3332f8b90 .

<https://standards.isotc211.org/19157/-3/1/dqc/content/measureDescription/MD53> dqm:describes _:n61346038c5d14cc38e028ccb9d3332f8b91 .

<https://standards.isotc211.org/19157/-3/1/dqc/content/measureDescription/MD6> dqm:describes _:n61346038c5d14cc38e028ccb9d3332f8b32 .

<https://standards.isotc211.org/19157/-3/1/dqc/content/measureDescription/MD60> dqm:describes _:n61346038c5d14cc38e028ccb9d3332f8b38 .

<https://standards.isotc211.org/19157/-3/1/dqc/content/measureDescription/MD61> dqm:describes _:n61346038c5d14cc38e028ccb9d3332f8b21 .

<https://standards.isotc211.org/19157/-3/1/dqc/content/measureDescription/MD62> dqm:describes _:n61346038c5d14cc38e028ccb9d3332f8b92 .

<https://standards.isotc211.org/19157/-3/1/dqc/content/measureDescription/MD63> dqm:describes _:n61346038c5d14cc38e028ccb9d3332f8b93 .

<https://standards.isotc211.org/19157/-3/1/dqc/content/measureDescription/MD64> dqm:describes _:n61346038c5d14cc38e028ccb9d3332f8b94 .

<https://standards.isotc211.org/19157/-3/1/dqc/content/measureDescription/MD65> dqm:describes _:n61346038c5d14cc38e028ccb9d3332f8b35 .

<https://standards.isotc211.org/19157/-3/1/dqc/content/measureDescription/MD66> dqm:describes _:n61346038c5d14cc38e028ccb9d3332f8b50 .

<https://standards.isotc211.org/19157/-3/1/dqc/content/measureDescription/MD67> dqm:describes _:n61346038c5d14cc38e028ccb9d3332f8b24 .

<https://standards.isotc211.org/19157/-3/1/dqc/content/measureDescription/MD7> dqm:describes _:n61346038c5d14cc38e028ccb9d3332f8b14 .

<https://standards.isotc211.org/19157/-3/1/dqc/content/measureDescription/MD8> dqm:describes _:n61346038c5d14cc38e028ccb9d3332f8b10 .

<https://standards.isotc211.org/19157/-3/1/dqc/content/measureDescription/MD9> dqm:describes _:n61346038c5d14cc38e028ccb9d3332f8b45 .

<https://standards.isotc211.org/19157/-3/1/dqc/content/measureDescription/MDsd1_LE50> dqm:describes _:n61346038c5d14cc38e028ccb9d3332f8b59,
        _:n61346038c5d14cc38e028ccb9d3332f8b60,
        _:n61346038c5d14cc38e028ccb9d3332f8b61 .

<https://standards.isotc211.org/19157/-3/1/dqc/content/measureDescription/MDsd1_LE68.3> dqm:describes _:n61346038c5d14cc38e028ccb9d3332f8b62,
        _:n61346038c5d14cc38e028ccb9d3332f8b63,
        _:n61346038c5d14cc38e028ccb9d3332f8b64 .

<https://standards.isotc211.org/19157/-3/1/dqc/content/measureDescription/MDsd1_LE90> dqm:describes _:n61346038c5d14cc38e028ccb9d3332f8b4,
        _:n61346038c5d14cc38e028ccb9d3332f8b65,
        _:n61346038c5d14cc38e028ccb9d3332f8b66 .

<https://standards.isotc211.org/19157/-3/1/dqc/content/measureDescription/MDsd1_LE95> dqm:describes _:n61346038c5d14cc38e028ccb9d3332f8b2,
        _:n61346038c5d14cc38e028ccb9d3332f8b67,
        _:n61346038c5d14cc38e028ccb9d3332f8b68 .

<https://standards.isotc211.org/19157/-3/1/dqc/content/measureDescription/MDsd1_LE99> dqm:describes _:n61346038c5d14cc38e028ccb9d3332f8b1,
        _:n61346038c5d14cc38e028ccb9d3332f8b69,
        _:n61346038c5d14cc38e028ccb9d3332f8b70 .

<https://standards.isotc211.org/19157/-3/1/dqc/content/measureDescription/MDsd1_LE99.8> dqm:describes _:n61346038c5d14cc38e028ccb9d3332f8b3,
        _:n61346038c5d14cc38e028ccb9d3332f8b5,
        _:n61346038c5d14cc38e028ccb9d3332f8b6 .

<https://standards.isotc211.org/19157/-3/1/dqc/content/measureDescription/MDsd2_LE50r1> dqm:describes _:n61346038c5d14cc38e028ccb9d3332f8b59,
        _:n61346038c5d14cc38e028ccb9d3332f8b60,
        _:n61346038c5d14cc38e028ccb9d3332f8b61 .

<https://standards.isotc211.org/19157/-3/1/dqc/content/measureDescription/MDsd2_LE50r10> dqm:describes _:n61346038c5d14cc38e028ccb9d3332f8b59,
        _:n61346038c5d14cc38e028ccb9d3332f8b60,
        _:n61346038c5d14cc38e028ccb9d3332f8b61 .

<https://standards.isotc211.org/19157/-3/1/dqc/content/measureDescription/MDsd2_LE50r2> dqm:describes _:n61346038c5d14cc38e028ccb9d3332f8b59,
        _:n61346038c5d14cc38e028ccb9d3332f8b60,
        _:n61346038c5d14cc38e028ccb9d3332f8b61 .

<https://standards.isotc211.org/19157/-3/1/dqc/content/measureDescription/MDsd2_LE50r3> dqm:describes _:n61346038c5d14cc38e028ccb9d3332f8b59,
        _:n61346038c5d14cc38e028ccb9d3332f8b60,
        _:n61346038c5d14cc38e028ccb9d3332f8b61 .

<https://standards.isotc211.org/19157/-3/1/dqc/content/measureDescription/MDsd2_LE50r4> dqm:describes _:n61346038c5d14cc38e028ccb9d3332f8b59,
        _:n61346038c5d14cc38e028ccb9d3332f8b60,
        _:n61346038c5d14cc38e028ccb9d3332f8b61 .

<https://standards.isotc211.org/19157/-3/1/dqc/content/measureDescription/MDsd2_LE50r5> dqm:describes _:n61346038c5d14cc38e028ccb9d3332f8b59,
        _:n61346038c5d14cc38e028ccb9d3332f8b60,
        _:n61346038c5d14cc38e028ccb9d3332f8b61 .

<https://standards.isotc211.org/19157/-3/1/dqc/content/measureDescription/MDsd2_LE68.3r1> dqm:describes _:n61346038c5d14cc38e028ccb9d3332f8b62,
        _:n61346038c5d14cc38e028ccb9d3332f8b63,
        _:n61346038c5d14cc38e028ccb9d3332f8b64 .

<https://standards.isotc211.org/19157/-3/1/dqc/content/measureDescription/MDsd2_LE68.3r10> dqm:describes _:n61346038c5d14cc38e028ccb9d3332f8b62,
        _:n61346038c5d14cc38e028ccb9d3332f8b63,
        _:n61346038c5d14cc38e028ccb9d3332f8b64 .

<https://standards.isotc211.org/19157/-3/1/dqc/content/measureDescription/MDsd2_LE68.3r2> dqm:describes _:n61346038c5d14cc38e028ccb9d3332f8b62,
        _:n61346038c5d14cc38e028ccb9d3332f8b63,
        _:n61346038c5d14cc38e028ccb9d3332f8b64 .

<https://standards.isotc211.org/19157/-3/1/dqc/content/measureDescription/MDsd2_LE68.3r3> dqm:describes _:n61346038c5d14cc38e028ccb9d3332f8b62,
        _:n61346038c5d14cc38e028ccb9d3332f8b63,
        _:n61346038c5d14cc38e028ccb9d3332f8b64 .

<https://standards.isotc211.org/19157/-3/1/dqc/content/measureDescription/MDsd2_LE68.3r4> dqm:describes _:n61346038c5d14cc38e028ccb9d3332f8b62,
        _:n61346038c5d14cc38e028ccb9d3332f8b63,
        _:n61346038c5d14cc38e028ccb9d3332f8b64 .

<https://standards.isotc211.org/19157/-3/1/dqc/content/measureDescription/MDsd2_LE68.3r5> dqm:describes _:n61346038c5d14cc38e028ccb9d3332f8b62,
        _:n61346038c5d14cc38e028ccb9d3332f8b63,
        _:n61346038c5d14cc38e028ccb9d3332f8b64 .

<https://standards.isotc211.org/19157/-3/1/dqc/content/measureDescription/MDsd2_LE90r1> dqm:describes _:n61346038c5d14cc38e028ccb9d3332f8b4,
        _:n61346038c5d14cc38e028ccb9d3332f8b65,
        _:n61346038c5d14cc38e028ccb9d3332f8b66 .

<https://standards.isotc211.org/19157/-3/1/dqc/content/measureDescription/MDsd2_LE90r10> dqm:describes _:n61346038c5d14cc38e028ccb9d3332f8b4,
        _:n61346038c5d14cc38e028ccb9d3332f8b65,
        _:n61346038c5d14cc38e028ccb9d3332f8b66 .

<https://standards.isotc211.org/19157/-3/1/dqc/content/measureDescription/MDsd2_LE90r2> dqm:describes _:n61346038c5d14cc38e028ccb9d3332f8b4,
        _:n61346038c5d14cc38e028ccb9d3332f8b65,
        _:n61346038c5d14cc38e028ccb9d3332f8b66 .

<https://standards.isotc211.org/19157/-3/1/dqc/content/measureDescription/MDsd2_LE90r3> dqm:describes _:n61346038c5d14cc38e028ccb9d3332f8b4,
        _:n61346038c5d14cc38e028ccb9d3332f8b65,
        _:n61346038c5d14cc38e028ccb9d3332f8b66 .

<https://standards.isotc211.org/19157/-3/1/dqc/content/measureDescription/MDsd2_LE90r4> dqm:describes _:n61346038c5d14cc38e028ccb9d3332f8b4,
        _:n61346038c5d14cc38e028ccb9d3332f8b65,
        _:n61346038c5d14cc38e028ccb9d3332f8b66 .

<https://standards.isotc211.org/19157/-3/1/dqc/content/measureDescription/MDsd2_LE90r5> dqm:describes _:n61346038c5d14cc38e028ccb9d3332f8b4,
        _:n61346038c5d14cc38e028ccb9d3332f8b65,
        _:n61346038c5d14cc38e028ccb9d3332f8b66 .

<https://standards.isotc211.org/19157/-3/1/dqc/content/measureDescription/MDsd2_LE95r1> dqm:describes _:n61346038c5d14cc38e028ccb9d3332f8b2,
        _:n61346038c5d14cc38e028ccb9d3332f8b67,
        _:n61346038c5d14cc38e028ccb9d3332f8b68 .

<https://standards.isotc211.org/19157/-3/1/dqc/content/measureDescription/MDsd2_LE95r10> dqm:describes _:n61346038c5d14cc38e028ccb9d3332f8b2,
        _:n61346038c5d14cc38e028ccb9d3332f8b67,
        _:n61346038c5d14cc38e028ccb9d3332f8b68 .

<https://standards.isotc211.org/19157/-3/1/dqc/content/measureDescription/MDsd2_LE95r2> dqm:describes _:n61346038c5d14cc38e028ccb9d3332f8b2,
        _:n61346038c5d14cc38e028ccb9d3332f8b67,
        _:n61346038c5d14cc38e028ccb9d3332f8b68 .

<https://standards.isotc211.org/19157/-3/1/dqc/content/measureDescription/MDsd2_LE95r3> dqm:describes _:n61346038c5d14cc38e028ccb9d3332f8b2,
        _:n61346038c5d14cc38e028ccb9d3332f8b67,
        _:n61346038c5d14cc38e028ccb9d3332f8b68 .

<https://standards.isotc211.org/19157/-3/1/dqc/content/measureDescription/MDsd2_LE95r4> dqm:describes _:n61346038c5d14cc38e028ccb9d3332f8b2,
        _:n61346038c5d14cc38e028ccb9d3332f8b67,
        _:n61346038c5d14cc38e028ccb9d3332f8b68 .

<https://standards.isotc211.org/19157/-3/1/dqc/content/measureDescription/MDsd2_LE95r5> dqm:describes _:n61346038c5d14cc38e028ccb9d3332f8b2,
        _:n61346038c5d14cc38e028ccb9d3332f8b67,
        _:n61346038c5d14cc38e028ccb9d3332f8b68 .

<https://standards.isotc211.org/19157/-3/1/dqc/content/measureDescription/MDsd2_LE99.8r1> dqm:describes _:n61346038c5d14cc38e028ccb9d3332f8b3,
        _:n61346038c5d14cc38e028ccb9d3332f8b5,
        _:n61346038c5d14cc38e028ccb9d3332f8b6 .

<https://standards.isotc211.org/19157/-3/1/dqc/content/measureDescription/MDsd2_LE99.8r10> dqm:describes _:n61346038c5d14cc38e028ccb9d3332f8b3,
        _:n61346038c5d14cc38e028ccb9d3332f8b5,
        _:n61346038c5d14cc38e028ccb9d3332f8b6 .

<https://standards.isotc211.org/19157/-3/1/dqc/content/measureDescription/MDsd2_LE99.8r2> dqm:describes _:n61346038c5d14cc38e028ccb9d3332f8b3,
        _:n61346038c5d14cc38e028ccb9d3332f8b5,
        _:n61346038c5d14cc38e028ccb9d3332f8b6 .

<https://standards.isotc211.org/19157/-3/1/dqc/content/measureDescription/MDsd2_LE99.8r3> dqm:describes _:n61346038c5d14cc38e028ccb9d3332f8b3,
        _:n61346038c5d14cc38e028ccb9d3332f8b5,
        _:n61346038c5d14cc38e028ccb9d3332f8b6 .

<https://standards.isotc211.org/19157/-3/1/dqc/content/measureDescription/MDsd2_LE99.8r4> dqm:describes _:n61346038c5d14cc38e028ccb9d3332f8b3,
        _:n61346038c5d14cc38e028ccb9d3332f8b5,
        _:n61346038c5d14cc38e028ccb9d3332f8b6 .

<https://standards.isotc211.org/19157/-3/1/dqc/content/measureDescription/MDsd2_LE99.8r5> dqm:describes _:n61346038c5d14cc38e028ccb9d3332f8b3,
        _:n61346038c5d14cc38e028ccb9d3332f8b5,
        _:n61346038c5d14cc38e028ccb9d3332f8b6 .

<https://standards.isotc211.org/19157/-3/1/dqc/content/measureDescription/MDsd2_LE99r1> dqm:describes _:n61346038c5d14cc38e028ccb9d3332f8b1,
        _:n61346038c5d14cc38e028ccb9d3332f8b69,
        _:n61346038c5d14cc38e028ccb9d3332f8b70 .

<https://standards.isotc211.org/19157/-3/1/dqc/content/measureDescription/MDsd2_LE99r10> dqm:describes _:n61346038c5d14cc38e028ccb9d3332f8b1,
        _:n61346038c5d14cc38e028ccb9d3332f8b69,
        _:n61346038c5d14cc38e028ccb9d3332f8b70 .

<https://standards.isotc211.org/19157/-3/1/dqc/content/measureDescription/MDsd2_LE99r2> dqm:describes _:n61346038c5d14cc38e028ccb9d3332f8b1,
        _:n61346038c5d14cc38e028ccb9d3332f8b69,
        _:n61346038c5d14cc38e028ccb9d3332f8b70 .

<https://standards.isotc211.org/19157/-3/1/dqc/content/measureDescription/MDsd2_LE99r3> dqm:describes _:n61346038c5d14cc38e028ccb9d3332f8b1,
        _:n61346038c5d14cc38e028ccb9d3332f8b69,
        _:n61346038c5d14cc38e028ccb9d3332f8b70 .

<https://standards.isotc211.org/19157/-3/1/dqc/content/measureDescription/MDsd2_LE99r4> dqm:describes _:n61346038c5d14cc38e028ccb9d3332f8b1,
        _:n61346038c5d14cc38e028ccb9d3332f8b69,
        _:n61346038c5d14cc38e028ccb9d3332f8b70 .

<https://standards.isotc211.org/19157/-3/1/dqc/content/measureDescription/MDsd2_LE99r5> dqm:describes _:n61346038c5d14cc38e028ccb9d3332f8b1,
        _:n61346038c5d14cc38e028ccb9d3332f8b69,
        _:n61346038c5d14cc38e028ccb9d3332f8b70 .

<https://standards.isotc211.org/19157/-3/1/dqc/content/qualityMeasure/QC1> skos:narrower _:n61346038c5d14cc38e028ccb9d3332f8b1,
        _:n61346038c5d14cc38e028ccb9d3332f8b2,
        _:n61346038c5d14cc38e028ccb9d3332f8b25,
        _:n61346038c5d14cc38e028ccb9d3332f8b4,
        _:n61346038c5d14cc38e028ccb9d3332f8b5,
        _:n61346038c5d14cc38e028ccb9d3332f8b54,
        _:n61346038c5d14cc38e028ccb9d3332f8b55,
        _:n61346038c5d14cc38e028ccb9d3332f8b56,
        _:n61346038c5d14cc38e028ccb9d3332f8b57,
        _:n61346038c5d14cc38e028ccb9d3332f8b58,
        _:n61346038c5d14cc38e028ccb9d3332f8b61,
        _:n61346038c5d14cc38e028ccb9d3332f8b63,
        _:n61346038c5d14cc38e028ccb9d3332f8b71,
        _:n61346038c5d14cc38e028ccb9d3332f8b78,
        _:n61346038c5d14cc38e028ccb9d3332f8b79,
        _:n61346038c5d14cc38e028ccb9d3332f8b80,
        _:n61346038c5d14cc38e028ccb9d3332f8b81,
        _:n61346038c5d14cc38e028ccb9d3332f8b82,
        _:n61346038c5d14cc38e028ccb9d3332f8b83,
        _:n61346038c5d14cc38e028ccb9d3332f8b84,
        _:n61346038c5d14cc38e028ccb9d3332f8b85,
        _:n61346038c5d14cc38e028ccb9d3332f8b86,
        _:n61346038c5d14cc38e028ccb9d3332f8b87,
        _:n61346038c5d14cc38e028ccb9d3332f8b88,
        _:n61346038c5d14cc38e028ccb9d3332f8b89,
        _:n61346038c5d14cc38e028ccb9d3332f8b90,
        _:n61346038c5d14cc38e028ccb9d3332f8b91 .

<https://standards.isotc211.org/19157/-3/1/dqc/content/qualityMeasure/QC2> skos:narrower _:n61346038c5d14cc38e028ccb9d3332f8b21,
        _:n61346038c5d14cc38e028ccb9d3332f8b24,
        _:n61346038c5d14cc38e028ccb9d3332f8b3,
        _:n61346038c5d14cc38e028ccb9d3332f8b35,
        _:n61346038c5d14cc38e028ccb9d3332f8b38,
        _:n61346038c5d14cc38e028ccb9d3332f8b50,
        _:n61346038c5d14cc38e028ccb9d3332f8b59,
        _:n61346038c5d14cc38e028ccb9d3332f8b64,
        _:n61346038c5d14cc38e028ccb9d3332f8b66,
        _:n61346038c5d14cc38e028ccb9d3332f8b68,
        _:n61346038c5d14cc38e028ccb9d3332f8b70,
        _:n61346038c5d14cc38e028ccb9d3332f8b92,
        _:n61346038c5d14cc38e028ccb9d3332f8b93,
        _:n61346038c5d14cc38e028ccb9d3332f8b94 .

<https://standards.isotc211.org/19157/-3/1/dqc/content/qualityMeasure/QC3> skos:narrower _:n61346038c5d14cc38e028ccb9d3332f8b43,
        _:n61346038c5d14cc38e028ccb9d3332f8b47,
        _:n61346038c5d14cc38e028ccb9d3332f8b52,
        _:n61346038c5d14cc38e028ccb9d3332f8b6,
        _:n61346038c5d14cc38e028ccb9d3332f8b60,
        _:n61346038c5d14cc38e028ccb9d3332f8b62,
        _:n61346038c5d14cc38e028ccb9d3332f8b65,
        _:n61346038c5d14cc38e028ccb9d3332f8b67,
        _:n61346038c5d14cc38e028ccb9d3332f8b69 .

<https://standards.isotc211.org/19157/-3/1/dqc/content/qualityMeasure/QC4> skos:narrower _:n61346038c5d14cc38e028ccb9d3332f8b14,
        _:n61346038c5d14cc38e028ccb9d3332f8b20,
        _:n61346038c5d14cc38e028ccb9d3332f8b32,
        _:n61346038c5d14cc38e028ccb9d3332f8b36,
        _:n61346038c5d14cc38e028ccb9d3332f8b37,
        _:n61346038c5d14cc38e028ccb9d3332f8b7,
        _:n61346038c5d14cc38e028ccb9d3332f8b72,
        _:n61346038c5d14cc38e028ccb9d3332f8b73,
        _:n61346038c5d14cc38e028ccb9d3332f8b74,
        _:n61346038c5d14cc38e028ccb9d3332f8b75,
        _:n61346038c5d14cc38e028ccb9d3332f8b76,
        _:n61346038c5d14cc38e028ccb9d3332f8b77,
        _:n61346038c5d14cc38e028ccb9d3332f8b8 .

<https://standards.isotc211.org/19157/-3/1/dqc/content/qualityMeasure/QC5> skos:narrower _:n61346038c5d14cc38e028ccb9d3332f8b10,
        _:n61346038c5d14cc38e028ccb9d3332f8b11,
        _:n61346038c5d14cc38e028ccb9d3332f8b12,
        _:n61346038c5d14cc38e028ccb9d3332f8b13,
        _:n61346038c5d14cc38e028ccb9d3332f8b15,
        _:n61346038c5d14cc38e028ccb9d3332f8b16,
        _:n61346038c5d14cc38e028ccb9d3332f8b17,
        _:n61346038c5d14cc38e028ccb9d3332f8b18,
        _:n61346038c5d14cc38e028ccb9d3332f8b19,
        _:n61346038c5d14cc38e028ccb9d3332f8b22,
        _:n61346038c5d14cc38e028ccb9d3332f8b23,
        _:n61346038c5d14cc38e028ccb9d3332f8b26,
        _:n61346038c5d14cc38e028ccb9d3332f8b27,
        _:n61346038c5d14cc38e028ccb9d3332f8b28,
        _:n61346038c5d14cc38e028ccb9d3332f8b29,
        _:n61346038c5d14cc38e028ccb9d3332f8b30,
        _:n61346038c5d14cc38e028ccb9d3332f8b31,
        _:n61346038c5d14cc38e028ccb9d3332f8b33,
        _:n61346038c5d14cc38e028ccb9d3332f8b34,
        _:n61346038c5d14cc38e028ccb9d3332f8b39,
        _:n61346038c5d14cc38e028ccb9d3332f8b40,
        _:n61346038c5d14cc38e028ccb9d3332f8b41,
        _:n61346038c5d14cc38e028ccb9d3332f8b42,
        _:n61346038c5d14cc38e028ccb9d3332f8b44,
        _:n61346038c5d14cc38e028ccb9d3332f8b45,
        _:n61346038c5d14cc38e028ccb9d3332f8b46,
        _:n61346038c5d14cc38e028ccb9d3332f8b48,
        _:n61346038c5d14cc38e028ccb9d3332f8b49,
        _:n61346038c5d14cc38e028ccb9d3332f8b51,
        _:n61346038c5d14cc38e028ccb9d3332f8b53,
        _:n61346038c5d14cc38e028ccb9d3332f8b9 .

<https://standards.isotc211.org/19157/-3/1/dqc/content/qualityMeasureParameter/> dqm:hasParameter _:n61346038c5d14cc38e028ccb9d3332f8b19,
        _:n61346038c5d14cc38e028ccb9d3332f8b40 .

<https://standards.isotc211.org/19157/-3/1/dqc/content/qualityMeasureParameter/MP2> dqm:hasParameter _:n61346038c5d14cc38e028ccb9d3332f8b90,
        _:n61346038c5d14cc38e028ccb9d3332f8b91,
        _:n61346038c5d14cc38e028ccb9d3332f8b92,
        _:n61346038c5d14cc38e028ccb9d3332f8b94 .

<https://standards.isotc211.org/19157/-3/1/dqc/content/qualityMeasureParameter/MP201> dqm:hasParameter _:n61346038c5d14cc38e028ccb9d3332f8b13 .

<https://standards.isotc211.org/19157/-3/1/dqc/content/qualityMeasureParameter/MP204> dqm:hasParameter _:n61346038c5d14cc38e028ccb9d3332f8b22 .

<https://standards.isotc211.org/19157/-3/1/dqc/content/qualityMeasureParameter/MP205> dqm:hasParameter _:n61346038c5d14cc38e028ccb9d3332f8b47 .

<https://standards.isotc211.org/19157/-3/1/dqc/content/qualityMeasureParameter/MP206> dqm:hasParameter _:n61346038c5d14cc38e028ccb9d3332f8b43 .

<https://standards.isotc211.org/19157/-3/1/dqc/content/qualityMeasureParameter/MP207> dqm:hasParameter _:n61346038c5d14cc38e028ccb9d3332f8b52 .

<https://standards.isotc211.org/19157/-3/1/dqc/content/qualityMeasureParameter/MP23> dqm:hasParameter _:n61346038c5d14cc38e028ccb9d3332f8b39 .

<https://standards.isotc211.org/19157/-3/1/dqc/content/qualityMeasureParameter/MP24> dqm:hasParameter _:n61346038c5d14cc38e028ccb9d3332f8b26 .

<https://standards.isotc211.org/19157/-3/1/dqc/content/qualityMeasureParameter/MP25_1MP25_2> dqm:hasParameter _:n61346038c5d14cc38e028ccb9d3332f8b30 .

<https://standards.isotc211.org/19157/-3/1/dqc/content/qualityMeasureParameter/MP29> dqm:hasParameter _:n61346038c5d14cc38e028ccb9d3332f8b79 .

<https://standards.isotc211.org/19157/-3/1/dqc/content/qualityMeasureParameter/MP30> dqm:hasParameter _:n61346038c5d14cc38e028ccb9d3332f8b25 .

<https://standards.isotc211.org/19157/-3/1/dqc/content/qualityMeasureParameter/MP31> dqm:hasParameter _:n61346038c5d14cc38e028ccb9d3332f8b80 .

<https://standards.isotc211.org/19157/-3/1/dqc/content/qualityMeasureParameter/MP35> dqm:hasParameter _:n61346038c5d14cc38e028ccb9d3332f8b4,
        _:n61346038c5d14cc38e028ccb9d3332f8b65,
        _:n61346038c5d14cc38e028ccb9d3332f8b66,
        _:n61346038c5d14cc38e028ccb9d3332f8b67,
        _:n61346038c5d14cc38e028ccb9d3332f8b69 .

<https://standards.isotc211.org/19157/-3/1/dqc/content/qualityMeasureParameter/MP36> dqm:hasParameter _:n61346038c5d14cc38e028ccb9d3332f8b2,
        _:n61346038c5d14cc38e028ccb9d3332f8b68 .

<https://standards.isotc211.org/19157/-3/1/dqc/content/qualityMeasureParameter/MP37> dqm:hasParameter _:n61346038c5d14cc38e028ccb9d3332f8b1,
        _:n61346038c5d14cc38e028ccb9d3332f8b70 .

<https://standards.isotc211.org/19157/-3/1/dqc/content/qualityMeasureParameter/MP38> dqm:hasParameter _:n61346038c5d14cc38e028ccb9d3332f8b3,
        _:n61346038c5d14cc38e028ccb9d3332f8b5 .

<https://standards.isotc211.org/19157/-3/1/dqc/content/qualityMeasureParameter/MP41> dqm:hasParameter _:n61346038c5d14cc38e028ccb9d3332f8b84 .

<https://standards.isotc211.org/19157/-3/1/dqc/content/qualityMeasureParameter/MP49> dqm:hasParameter _:n61346038c5d14cc38e028ccb9d3332f8b87 .

<https://standards.isotc211.org/19157/-3/1/dqc/content/qualityMeasureParameter/MP51> dqm:hasParameter _:n61346038c5d14cc38e028ccb9d3332f8b89 .

<https://standards.isotc211.org/19157/-3/1/dqc/content/qualityMeasureParameter/MP63_1MP63_2MP63_3> dqm:hasParameter _:n61346038c5d14cc38e028ccb9d3332f8b93 .

<https://standards.isotc211.org/19157/-3/1/dqc/content/qualityMeasureParameter/MP68> dqm:hasParameter _:n61346038c5d14cc38e028ccb9d3332f8b64 .

<https://standards.isotc211.org/19157/-3/1/dqc/content/qualityMeasureParameter/MP69> dqm:hasParameter _:n61346038c5d14cc38e028ccb9d3332f8b59 .

<https://standards.isotc211.org/19157/-3/1/dqc/content/qualityMeasure> a skos:ConceptScheme ;
    skos:prefLabel "ISO19157-3 quality measures" .

[] a prov:Activity ;
    prov:endedAtTime "2024-09-10T03:27:15.912020"^^xsd:dateTime ;
    prov:startedAtTime "2024-09-10T03:27:15.595457"^^xsd:dateTime ;
    prov:used [ a prov:Entity ;
            dcterms:format "application/json" ;
            dcterms:hasVersion "git:920217be7835f2f560e248763da2138c9f935863" ;
            rdfs:seeAlso <file:///home/runner/work/iso19157-3-dqm-register/iso19157-3-dqm-register/sources/QualityMeasure.csv.json> ] ;
    prov:wasAssociatedWith [ a prov:Agent,
                schema:SoftwareApplication ;
            rdfs:label "OGC-NA tools" ;
            dcterms:hasVersion "0.3.51" ;
            rdfs:seeAlso <https://github.com/opengeospatial/ogc-na-tools> ] ;
    prov:wasInformedBy [ dcterms:identifier "fef6e3ff-1b3f-49f7-bf09-fb273b03ea41" ] .

_:Nf3b2d4a831374ec1a14aef2d4c4cac7f a prov:Agent,
        schema:SoftwareApplication ;
    rdfs:label "OGC-NA tools" ;
    dcterms:hasVersion "0.3.51" ;
    rdfs:comment "ogc.na.update_vocabs version 0.3.51" ;
    rdfs:seeAlso <https://github.com/opengeospatial/ogc-na-tools> .

_:n61346038c5d14cc38e028ccb9d3332f8b71 a skos:Concept ;
    dcterms:date "2024-09-09 14:41:43.660" ;
    dcterms:hasVersion "1.0" ;
    dqm:elementName "absolute or external accuracy" ;
    dqm:valueType "Real" ;
    policy:status <http://www.opengis.net/def/status/valid> ;
    skos:definition "Bias of the positions for a set of positions where the positional uncertainties are defined as the deviation between a measured position and what is accepted as the corresponding true position." ;
    skos:inScheme <https://standards.isotc211.org/19157/-3/1/dqc/content/qualityMeasure> ;
    skos:prefLabel "bias of positions (1D, 2D and 3D)" .

_:n61346038c5d14cc38e028ccb9d3332f8b72 a skos:Concept ;
    dcterms:date "2024-09-09 14:41:43.660" ;
    dcterms:hasVersion "0.1" ;
    dcterms:source <https://standards.isotc211.org/19157/-3/1/dqc/content/onlineResource/SR5> ;
    dqm:elementName "omission" ;
    dqm:valueType "Real" ;
    policy:status <http://www.opengis.net/def/status/submitted> ;
    skos:definition "Percentage of reference feature geometry where data is absent." ;
    skos:example """MD208e
MD208e2""" ;
    skos:inScheme <https://standards.isotc211.org/19157/-3/1/dqc/content/qualityMeasure> ;
    skos:prefLabel "rate of omission for spatial coverage" .

_:n61346038c5d14cc38e028ccb9d3332f8b73 a skos:Concept ;
    dcterms:date "2024-09-09 14:41:43.660" ;
    dcterms:hasVersion "0.1" ;
    dcterms:source <https://standards.isotc211.org/19157/-3/1/dqc/content/onlineResource/SR5> ;
    dqm:elementName "omission" ;
    dqm:valueType "Real" ;
    policy:status <http://www.opengis.net/def/status/submitted> ;
    skos:definition "Quantity of spatially discontinuous data in relation to the total quantity of data." ;
    skos:example "MD209e" ;
    skos:inScheme <https://standards.isotc211.org/19157/-3/1/dqc/content/qualityMeasure> ;
    skos:prefLabel "rate of spatial discontinuity" .

_:n61346038c5d14cc38e028ccb9d3332f8b74 a skos:Concept ;
    dcterms:date "2024-09-09 14:41:43.660" ;
    dcterms:hasVersion "0.1" ;
    dcterms:source <https://standards.isotc211.org/19157/-3/1/dqc/content/onlineResource/SR5> ;
    dqm:elementName "omission" ;
    dqm:valueType "Real" ;
    policy:status <http://www.opengis.net/def/status/submitted> ;
    skos:definition "Temporal duration without data in relation to the total temporal duration in which data is supposed to be present ." ;
    skos:inScheme <https://standards.isotc211.org/19157/-3/1/dqc/content/qualityMeasure> ;
    skos:prefLabel "rate of omission for temporal coverage" .

_:n61346038c5d14cc38e028ccb9d3332f8b75 a skos:Concept ;
    dcterms:date "2024-09-09 14:41:43.660" ;
    dcterms:hasVersion "0.1" ;
    dcterms:source <https://standards.isotc211.org/19157/-3/1/dqc/content/onlineResource/SR5> ;
    dqm:elementName "omission" ;
    dqm:valueType "Real" ;
    policy:status <http://www.opengis.net/def/status/submitted> ;
    skos:definition "Percentage of data that fails to provide full coverage due to certain quality issues." ;
    skos:example "MD211e" ;
    skos:inScheme <https://standards.isotc211.org/19157/-3/1/dqc/content/qualityMeasure> ;
    skos:prefLabel "rate of imperfect coverage" .

_:n61346038c5d14cc38e028ccb9d3332f8b76 a skos:Concept ;
    dcterms:date "2024-09-09 14:41:43.660" ;
    dcterms:hasVersion "0.1" ;
    dcterms:source <https://standards.isotc211.org/19157/-3/1/dqc/content/onlineResource/SR5> ;
    dqm:elementName "omission" ;
    dqm:valueType "Real" ;
    policy:status <http://www.opengis.net/def/status/submitted> ;
    skos:definition "Quantity of missing metadata in relation to the total quantity of metadata that are supposed to be present." ;
    skos:inScheme <https://standards.isotc211.org/19157/-3/1/dqc/content/qualityMeasure> ;
    skos:prefLabel "rate of omission for metadata" .

_:n61346038c5d14cc38e028ccb9d3332f8b77 a skos:Concept ;
    dcterms:date "2024-09-09 14:41:43.660" ;
    dcterms:hasVersion "0.1" ;
    dcterms:source <https://standards.isotc211.org/19157/-3/1/dqc/content/onlineResource/SR5> ;
    dqm:elementName "omission" ;
    dqm:valueType "Real" ;
    policy:status <http://www.opengis.net/def/status/submitted> ;
    skos:definition "Percentage of data where sensitive information is present." ;
    skos:example "MD213e" ;
    skos:inScheme <https://standards.isotc211.org/19157/-3/1/dqc/content/qualityMeasure> ;
    skos:prefLabel "rate of occurrence of sensitive information" .

_:n61346038c5d14cc38e028ccb9d3332f8b82 a skos:Concept ;
    dcterms:date "2024-09-09 14:41:43.660" ;
    dcterms:hasVersion "1.0" ;
    dqm:elementName "absolute or external accuracy" ;
    dqm:valueType "Measure" ;
    policy:status <http://www.opengis.net/def/status/valid> ;
    skos:altLabel "RMSE" ;
    skos:definition "Radius of a circle around a given point, in which the true value lies with probability P." ;
    skos:inScheme <https://standards.isotc211.org/19157/-3/1/dqc/content/qualityMeasure> ;
    skos:prefLabel "root mean square error" .

_:n61346038c5d14cc38e028ccb9d3332f8b83 a skos:Concept ;
    dcterms:date "2024-09-09 14:41:43.660" ;
    dcterms:hasVersion "1.0" ;
    dcterms:source <https://standards.isotc211.org/19157/-3/1/dqc/content/onlineResource/SR1> ;
    dqm:elementName "absolute or external accuracy" ;
    dqm:valueType "Measure" ;
    policy:status <http://www.opengis.net/def/status/valid> ;
    skos:altLabel "LMAS" ;
    skos:definition "Absolute vertical accuracy of the data’s coordinates, expressed in terms of linear error at 90 % probability given that a bias is present." ;
    skos:inScheme <https://standards.isotc211.org/19157/-3/1/dqc/content/qualityMeasure> ;
    skos:prefLabel "absolute linear error at 90 % significance level of biased vertical data (Alternative 1)" .

_:n61346038c5d14cc38e028ccb9d3332f8b85 a skos:Concept ;
    dcterms:date "2024-09-09 14:41:43.660" ;
    dcterms:hasVersion "1.0" ;
    dqm:elementName "absolute or external accuracy" ;
    dqm:valueType "Measure" ;
    policy:status <http://www.opengis.net/def/status/valid> ;
    skos:altLabel "RMSEP" ;
    skos:definition "Radius of a circle around the given point, in which the true value lies with probability P." ;
    skos:inScheme <https://standards.isotc211.org/19157/-3/1/dqc/content/qualityMeasure> ;
    skos:prefLabel "root mean square error of planimetry" .

_:n61346038c5d14cc38e028ccb9d3332f8b86 a skos:Concept ;
    dcterms:date "2024-09-09 14:41:43.660" ;
    dcterms:hasVersion "1.0" ;
    dcterms:source <https://standards.isotc211.org/19157/-3/1/dqc/content/onlineResource/SR1> ;
    dqm:elementName "absolute or external accuracy" ;
    dqm:valueType "Measure" ;
    policy:status <http://www.opengis.net/def/status/valid> ;
    skos:altLabel "CMAS" ;
    skos:definition "Absolute horizontal accuracy of the data’s coordinates, expressed in terms of circular error at 90 % probability given that a bias is present." ;
    skos:inScheme <https://standards.isotc211.org/19157/-3/1/dqc/content/qualityMeasure> ;
    skos:prefLabel "absolute circular error at 90 % significance level of biased data" .

_:n61346038c5d14cc38e028ccb9d3332f8b88 a skos:Concept ;
    dcterms:date "2024-09-09 14:41:43.660" ;
    dcterms:hasVersion "1.0" ;
    dqm:elementName "absolute or external accuracy" ;
    dqm:valueStructure """Sequence
formula (a, b, φ) """ ;
    dqm:valueType "Real" ;
    policy:status <http://www.opengis.net/def/status/valid> ;
    skos:altLabel "standard point error ellipse" ;
    skos:definition "2D ellipse with the two main axes indicating the direction and magnitude of the highest and the lowest uncertainty of a 2D point." ;
    skos:inScheme <https://standards.isotc211.org/19157/-3/1/dqc/content/qualityMeasure> ;
    skos:prefLabel "uncertainty ellipse" .

_:n61346038c5d14cc38e028ccb9d3332f8b10 a skos:Concept ;
    dcterms:date "2024-09-09 14:41:43.660" ;
    dcterms:hasVersion "1.0" ;
    dqm:elementName "conceptual consistency" ;
    dqm:valueType "Boolean" ;
    policy:status <http://www.opengis.net/def/status/valid> ;
    skos:definition "Indication that an item is not compliant to the rules of the relevant conceptual schema." ;
    skos:example "MD8e" ;
    skos:inScheme <https://standards.isotc211.org/19157/-3/1/dqc/content/qualityMeasure> ;
    skos:prefLabel "conceptual schema non-compliance" .

_:n61346038c5d14cc38e028ccb9d3332f8b11 a skos:Concept ;
    dcterms:date "2024-09-09 14:41:43.660" ;
    dcterms:hasVersion "1.0" ;
    dqm:elementName "format consistency" ;
    dqm:valueType "Boolean" ;
    policy:status <http://www.opengis.net/def/status/retired> ;
    skos:definition "Indication that items are stored in conflict with the physical structure of the dataset." ;
    skos:example "MD119e" ;
    skos:inScheme <https://standards.isotc211.org/19157/-3/1/dqc/content/qualityMeasure> ;
    skos:prefLabel "physical structure conflicts" .

_:n61346038c5d14cc38e028ccb9d3332f8b12 a skos:Concept ;
    dcterms:date "2024-09-09 14:41:43.660" ;
    dcterms:hasVersion "1.0" ;
    dqm:elementName "domain consistency" ;
    dqm:valueType "Boolean" ;
    policy:status <http://www.opengis.net/def/status/valid> ;
    skos:definition "Indication of if an item is not in conformance with its value domain." ;
    skos:example "MD14e" ;
    skos:inScheme <https://standards.isotc211.org/19157/-3/1/dqc/content/qualityMeasure> ;
    skos:prefLabel "value domain non-conformance" .

_:n61346038c5d14cc38e028ccb9d3332f8b14 a skos:Concept ;
    dcterms:date "2024-09-09 14:41:43.660" ;
    dcterms:hasVersion "1.0" ;
    dqm:elementName "omission" ;
    dqm:valueType "Real" ;
    policy:status <http://www.opengis.net/def/status/valid> ;
    skos:definition "Number of missing items in the data set or sample in relation to the number of items that should have been present." ;
    skos:example "MD7e" ;
    skos:inScheme <https://standards.isotc211.org/19157/-3/1/dqc/content/qualityMeasure> ;
    skos:prefLabel "rate of missing items" .

_:n61346038c5d14cc38e028ccb9d3332f8b15 a skos:Concept ;
    dcterms:date "2024-09-09 14:41:43.660" ;
    dcterms:hasVersion "1.0" ;
    dqm:elementName "topological consistency" ;
    dqm:valueType "Real" ;
    policy:status <http://www.opengis.net/def/status/valid> ;
    skos:definition "Number of faulty link node connections in relation to the number of link node connections in the universe of discourse." ;
    skos:inScheme <https://standards.isotc211.org/19157/-3/1/dqc/content/qualityMeasure> ;
    skos:prefLabel "rate of faulty point-curve connections" .

_:n61346038c5d14cc38e028ccb9d3332f8b16 a skos:Concept ;
    dcterms:date "2024-09-09 14:41:43.660" ;
    dcterms:hasVersion "1.0" ;
    dqm:elementName "format consistency" ;
    dqm:valueType "Real" ;
    policy:status <http://www.opengis.net/def/status/valid> ;
    skos:definition "Number of items in the data set that are stored in conflict with the physical structure of the data set divided by the total number of items." ;
    skos:inScheme <https://standards.isotc211.org/19157/-3/1/dqc/content/qualityMeasure> ;
    skos:prefLabel "physical structure conflict rate" .

_:n61346038c5d14cc38e028ccb9d3332f8b17 a skos:Concept ;
    dcterms:date "2024-09-09 14:41:43.660" ;
    dcterms:hasVersion "1.0" ;
    dqm:elementName "conceptual consistency" ;
    dqm:valueType "Real" ;
    policy:status <http://www.opengis.net/def/status/valid> ;
    skos:definition "Number of the data product specification requirements that are not fulfilled by the current product/dataset in relation to the total number of data product specification requirements." ;
    skos:inScheme <https://standards.isotc211.org/19157/-3/1/dqc/content/qualityMeasure> ;
    skos:prefLabel "data product specification fail rate" .

_:n61346038c5d14cc38e028ccb9d3332f8b18 a skos:Concept ;
    dcterms:date "2024-09-09 14:41:43.660" ;
    dcterms:hasVersion "1.0" ;
    dqm:elementName "domain consistency" ;
    dqm:valueType "Real" ;
    policy:status <http://www.opengis.net/def/status/valid> ;
    skos:definition "Number of items in the data set that are not in conformance with their value domain in relation to the total number of items." ;
    skos:example "MD18e" ;
    skos:inScheme <https://standards.isotc211.org/19157/-3/1/dqc/content/qualityMeasure> ;
    skos:prefLabel "value domain non-conformance rate" .

_:n61346038c5d14cc38e028ccb9d3332f8b20 a skos:Concept ;
    dcterms:date "2024-09-09 14:41:43.660" ;
    dcterms:hasVersion "1.0" ;
    dqm:elementName "commission" ;
    dqm:valueType "Real" ;
    policy:status <http://www.opengis.net/def/status/valid> ;
    skos:definition "Number of excess items in the data set or sample in relation to the number of items that should have been present." ;
    skos:example "MD3e" ;
    skos:inScheme <https://standards.isotc211.org/19157/-3/1/dqc/content/qualityMeasure> ;
    skos:prefLabel "rate of excess items" .

_:n61346038c5d14cc38e028ccb9d3332f8b21 a skos:Concept ;
    dcterms:date "2024-09-09 14:41:43.660" ;
    dcterms:hasVersion "1.0" ;
    dqm:elementName "classification correctness" ;
    dqm:valueType "Real" ;
    policy:status <http://www.opengis.net/def/status/valid> ;
    skos:definition "Number of incorrectly classified features relative to the number of features that should be there." ;
    skos:inScheme <https://standards.isotc211.org/19157/-3/1/dqc/content/qualityMeasure> ;
    skos:prefLabel "misclassification rate" .

_:n61346038c5d14cc38e028ccb9d3332f8b23 a skos:Concept ;
    dcterms:date "2024-09-09 14:41:43.660" ;
    dcterms:hasVersion "1.0" ;
    dqm:elementName "conceptual consistency" ;
    dqm:valueType "Real" ;
    policy:status <http://www.opengis.net/def/status/draft> ;
    skos:definition "Number of items in the dataset that are not compliant with the rules of the conceptual schema in relation to the total number of these items supposed to be in the dataset." ;
    skos:example "MD12e" ;
    skos:inScheme <https://standards.isotc211.org/19157/-3/1/dqc/content/qualityMeasure> ;
    skos:prefLabel "non-compliance rate with respect to the rules of the conceptual schema" .

_:n61346038c5d14cc38e028ccb9d3332f8b24 a skos:Concept ;
    dcterms:date "2024-09-09 14:41:43.660" ;
    dcterms:hasVersion "1.0" ;
    dqm:elementName "non-quantitative attribute correctness" ;
    dqm:valueType "Real" ;
    policy:status <http://www.opengis.net/def/status/valid> ;
    skos:definition "Number of attribute values where incorrect values are assigned in relation to the total number of attribute values." ;
    skos:inScheme <https://standards.isotc211.org/19157/-3/1/dqc/content/qualityMeasure> ;
    skos:prefLabel "rate of incorrect attribute values" .

_:n61346038c5d14cc38e028ccb9d3332f8b27 a skos:Concept ;
    dcterms:date "2024-09-09 14:41:43.660" ;
    dcterms:hasVersion "1.0" ;
    dqm:elementName "topological consistency" ;
    dqm:valueType "Integer" ;
    policy:status <http://www.opengis.net/def/status/valid> ;
    skos:altLabel "kickbacks" ;
    skos:definition "Count of all items in the data that illegally self-overlap." ;
    skos:example "MD27e" ;
    skos:inScheme <https://standards.isotc211.org/19157/-3/1/dqc/content/qualityMeasure> ;
    skos:prefLabel "number of invalid self-overlap errors" .

_:n61346038c5d14cc38e028ccb9d3332f8b28 a skos:Concept ;
    dcterms:date "2024-09-09 14:41:43.660" ;
    dcterms:hasVersion "1.0" ;
    dqm:elementName "domain consistency" ;
    dqm:valueType "Integer" ;
    policy:status <http://www.opengis.net/def/status/valid> ;
    skos:definition "Count of all items in the data set that are not in conformance with their value domain." ;
    skos:inScheme <https://standards.isotc211.org/19157/-3/1/dqc/content/qualityMeasure> ;
    skos:prefLabel "number of items not in conformance with their value domain" .

_:n61346038c5d14cc38e028ccb9d3332f8b29 a skos:Concept ;
    dcterms:date "2024-09-09 14:41:43.660" ;
    dcterms:hasVersion "1.0" ;
    dqm:elementName "conceptual consistency" ;
    dqm:valueType "Integer" ;
    policy:status <http://www.opengis.net/def/status/valid> ;
    skos:altLabel "overlapping surfaces" ;
    skos:definition "Total number of erroneous overlaps within the data." ;
    skos:example "MD11e" ;
    skos:inScheme <https://standards.isotc211.org/19157/-3/1/dqc/content/qualityMeasure> ;
    skos:prefLabel "number of invalid overlaps of surfaces" .

_:n61346038c5d14cc38e028ccb9d3332f8b31 a skos:Concept ;
    dcterms:date "2024-09-09 14:41:43.660" ;
    dcterms:hasVersion "1.0" ;
    dqm:elementName "topological consistency" ;
    dqm:valueType "Integer" ;
    policy:status <http://www.opengis.net/def/status/valid> ;
    skos:altLabel "loops" ;
    skos:definition "Count of all items in the data that illegally intersect with themselves." ;
    skos:example "MD26e" ;
    skos:inScheme <https://standards.isotc211.org/19157/-3/1/dqc/content/qualityMeasure> ;
    skos:prefLabel "number of invalid self-intersect errors" .

_:n61346038c5d14cc38e028ccb9d3332f8b32 a skos:Concept ;
    dcterms:date "2024-09-09 14:41:43.660" ;
    dcterms:hasVersion "1.0" ;
    dqm:elementName "omission" ;
    dqm:valueType "Integer" ;
    policy:status <http://www.opengis.net/def/status/valid> ;
    skos:definition "Count of all items that should have been in the data set or sample and are missing." ;
    skos:example "MD6e" ;
    skos:inScheme <https://standards.isotc211.org/19157/-3/1/dqc/content/qualityMeasure> ;
    skos:prefLabel "number of missing items" .

_:n61346038c5d14cc38e028ccb9d3332f8b33 a skos:Concept ;
    dcterms:date "2024-09-09 14:41:43.660" ;
    dcterms:hasVersion "1.0" ;
    dqm:elementName "conceptual consistency" ;
    dqm:valueType "Integer" ;
    policy:status <http://www.opengis.net/def/status/valid> ;
    skos:definition "Number of data product specification requirements that are not fulfilled by the current product/dataset." ;
    skos:inScheme <https://standards.isotc211.org/19157/-3/1/dqc/content/qualityMeasure> ;
    skos:prefLabel "data product specification fail count" .

_:n61346038c5d14cc38e028ccb9d3332f8b34 a skos:Concept ;
    dcterms:date "2024-09-09 14:41:43.660" ;
    dcterms:hasVersion "1.0" ;
    dqm:elementName "format consistency" ;
    dqm:valueType "Integer" ;
    policy:status <http://www.opengis.net/def/status/valid> ;
    skos:definition "Count of all items in the data set that are stored in conflict with the physical structure of the data set." ;
    skos:example "MD19e" ;
    skos:inScheme <https://standards.isotc211.org/19157/-3/1/dqc/content/qualityMeasure> ;
    skos:prefLabel "number of physical structure conflicts" .

_:n61346038c5d14cc38e028ccb9d3332f8b35 a skos:Concept ;
    dcterms:date "2024-09-09 14:41:43.660" ;
    dcterms:hasVersion "1.0" ;
    dqm:elementName "non-quantitative attribute correctness" ;
    dqm:valueType "Integer" ;
    policy:status <http://www.opengis.net/def/status/valid> ;
    skos:definition "Total number of erroneous attribute values within the relevant part of the dataset." ;
    skos:example "MD65e" ;
    skos:inScheme <https://standards.isotc211.org/19157/-3/1/dqc/content/qualityMeasure> ;
    skos:prefLabel "number of incorrect attribute values" .

_:n61346038c5d14cc38e028ccb9d3332f8b36 a skos:Concept ;
    dcterms:date "2024-09-09 14:41:43.660" ;
    dcterms:hasVersion "1.0" ;
    dqm:elementName "commission" ;
    dqm:valueType "Integer" ;
    policy:status <http://www.opengis.net/def/status/valid> ;
    skos:definition "Number of items within the data set or sample that should not have been present." ;
    skos:example "MD2e" ;
    skos:inScheme <https://standards.isotc211.org/19157/-3/1/dqc/content/qualityMeasure> ;
    skos:prefLabel "number of excess items" .

_:n61346038c5d14cc38e028ccb9d3332f8b37 a skos:Concept ;
    dcterms:date "2024-09-09 14:41:43.660" ;
    dcterms:hasVersion "1.0" ;
    dqm:elementName "commission" ;
    dqm:valueType "Integer" ;
    policy:status <http://www.opengis.net/def/status/valid> ;
    skos:definition "Total number of exact duplications of feature instances within the data." ;
    skos:example "MD4e" ;
    skos:inScheme <https://standards.isotc211.org/19157/-3/1/dqc/content/qualityMeasure> ;
    skos:prefLabel "number of duplicate feature instances" .

_:n61346038c5d14cc38e028ccb9d3332f8b38 a skos:Concept ;
    dcterms:date "2024-09-09 14:41:43.660" ;
    dcterms:hasVersion "1.0" ;
    dqm:elementName "classification correctness" ;
    dqm:valueType "Integer" ;
    policy:status <http://www.opengis.net/def/status/valid> ;
    skos:definition "Number of incorrectly classified features." ;
    skos:inScheme <https://standards.isotc211.org/19157/-3/1/dqc/content/qualityMeasure> ;
    skos:prefLabel "number of incorrectly classified features" .

_:n61346038c5d14cc38e028ccb9d3332f8b41 a skos:Concept ;
    dcterms:date "2024-09-09 14:41:43.660" ;
    dcterms:hasVersion "1.0" ;
    dqm:elementName "conceptual consistency" ;
    dqm:valueType "Integer" ;
    skos:definition "Count of all items in the data set that are not compliant with the rules of the conceptual schema." ;
    skos:example "MD10e" ;
    skos:inScheme <https://standards.isotc211.org/19157/-3/1/dqc/content/qualityMeasure> ;
    skos:prefLabel "Number of items not compliant with the rules of the conceptual schema" .

_:n61346038c5d14cc38e028ccb9d3332f8b42 a skos:Concept ;
    dcterms:date "2024-09-09 14:41:43.660" ;
    dcterms:hasVersion "1.0" ;
    dqm:elementName "topological consistency" ;
    dqm:valueType "Integer" ;
    policy:status <http://www.opengis.net/def/status/valid> ;
    skos:altLabel "extraneous nodes" ;
    skos:definition "Number of faulty point-curve connections in the dataset." ;
    skos:example "MD21e" ;
    skos:inScheme <https://standards.isotc211.org/19157/-3/1/dqc/content/qualityMeasure> ;
    skos:prefLabel "number of faulty point-curve connections" .

_:n61346038c5d14cc38e028ccb9d3332f8b44 a skos:Concept ;
    dcterms:date "2024-09-09 14:41:43.660" ;
    dcterms:hasVersion "1.0" ;
    dqm:elementName "conceptual consistency" ;
    dqm:valueType "Boolean " ;
    policy:status <http://www.opengis.net/def/status/valid> ;
    skos:definition "Indication that all requirements in the referred data product specification are fulfilled." ;
    skos:inScheme <https://standards.isotc211.org/19157/-3/1/dqc/content/qualityMeasure> ;
    skos:prefLabel "data product specification passed" .

_:n61346038c5d14cc38e028ccb9d3332f8b45 a skos:Concept ;
    dcterms:date "2024-09-09 14:41:43.660" ;
    dcterms:hasVersion "1.0" ;
    dqm:elementName "conceptual consistency" ;
    dqm:valueType "Boolean" ;
    policy:status <http://www.opengis.net/def/status/valid> ;
    skos:definition "Indication that an item complies with the rules of the relevant conceptual schema." ;
    skos:inScheme <https://standards.isotc211.org/19157/-3/1/dqc/content/qualityMeasure> ;
    skos:prefLabel "conceptual schema compliance" .

_:n61346038c5d14cc38e028ccb9d3332f8b46 a skos:Concept ;
    dcterms:date "2024-09-09 14:41:43.660" ;
    dcterms:hasVersion "1.0" ;
    dqm:elementName "domain consistency" ;
    dqm:valueType "Boolean" ;
    policy:status <http://www.opengis.net/def/status/valid> ;
    skos:definition "Indication that an item is conforming to its value domain." ;
    skos:example "MD15e" ;
    skos:inScheme <https://standards.isotc211.org/19157/-3/1/dqc/content/qualityMeasure> ;
    skos:prefLabel "value domain conformance" .

_:n61346038c5d14cc38e028ccb9d3332f8b48 a skos:Concept ;
    dcterms:date "2024-09-09 14:41:43.660" ;
    dcterms:hasVersion "1.0" ;
    dqm:elementName "conceptual consistency" ;
    dqm:valueType "Integer" ;
    policy:status <http://www.opengis.net/def/status/valid> ;
    skos:definition "Number of the data product specification requirements that are fulfilled by the current product/dataset." ;
    skos:inScheme <https://standards.isotc211.org/19157/-3/1/dqc/content/qualityMeasure> ;
    skos:prefLabel "data product specification pass count" .

_:n61346038c5d14cc38e028ccb9d3332f8b49 a skos:Concept ;
    dcterms:date "2024-09-09 14:41:43.660" ;
    dcterms:hasVersion "1.0" ;
    dqm:elementName "conceptual consistency" ;
    dqm:valueType "Real" ;
    policy:status <http://www.opengis.net/def/status/valid> ;
    skos:definition "Number of the data product specification requirements that are fulfilled by the current product/dataset in relation to the total number of data product specification requirements." ;
    skos:inScheme <https://standards.isotc211.org/19157/-3/1/dqc/content/qualityMeasure> ;
    skos:prefLabel "data product specification pass rate" .

_:n61346038c5d14cc38e028ccb9d3332f8b50 a skos:Concept ;
    dcterms:date "2024-09-09 14:41:43.660" ;
    dcterms:hasVersion "1.0" ;
    dqm:elementName "non-quantitative attribute correctness" ;
    dqm:valueType "Real" ;
    policy:status <http://www.opengis.net/def/status/valid> ;
    skos:definition "Number of correct attribute values in relation to the total number of attribute values." ;
    skos:inScheme <https://standards.isotc211.org/19157/-3/1/dqc/content/qualityMeasure> ;
    skos:prefLabel "rate of correct attribute values" .

_:n61346038c5d14cc38e028ccb9d3332f8b51 a skos:Concept ;
    dcterms:date "2024-09-09 14:41:43.660" ;
    dcterms:hasVersion "1.0" ;
    dqm:elementName "domain consistency" ;
    dqm:valueType "Real" ;
    policy:status <http://www.opengis.net/def/status/valid> ;
    skos:definition "Number of items in the data set that are in conformance with their value domain in relation to the total number of items in the data set." ;
    skos:example "MD17e" ;
    skos:inScheme <https://standards.isotc211.org/19157/-3/1/dqc/content/qualityMeasure> ;
    skos:prefLabel "value domain conformance rate" .

_:n61346038c5d14cc38e028ccb9d3332f8b53 a skos:Concept ;
    dcterms:date "2024-09-09 14:41:43.660" ;
    dcterms:hasVersion "1.0" ;
    dqm:elementName "conceptual consistency" ;
    dqm:valueType "Real" ;
    policy:status <http://www.opengis.net/def/status/valid> ;
    skos:definition "Number of items in the data set in compliance with the rules of the conceptual schema in relation to the total number of items supposed to be in the data set." ;
    skos:example "MD13e" ;
    skos:inScheme <https://standards.isotc211.org/19157/-3/1/dqc/content/qualityMeasure> ;
    skos:prefLabel "compliance rate with the rules of the conceptual schema" .

_:n61346038c5d14cc38e028ccb9d3332f8b54 a skos:Concept ;
    dcterms:date "2024-09-09 14:41:43.660" ;
    dcterms:hasVersion "1.0" ;
    dqm:elementName "absolute or external accuracy" ;
    dqm:valueType "Measure" ;
    policy:status <http://www.opengis.net/def/status/valid> ;
    skos:altLabel "circular standard error, Helmert’s point error, CSE" ;
    skos:definition "Radius describing a circle, in which the true point location lies with the probability of a normal distribution at 39.4 %." ;
    skos:inScheme <https://standards.isotc211.org/19157/-3/1/dqc/content/qualityMeasure> ;
    skos:prefLabel "circular standard deviation" .

_:n61346038c5d14cc38e028ccb9d3332f8b55 a skos:Concept ;
    dcterms:date "2024-09-09 14:41:43.660" ;
    dcterms:hasVersion "1.0" ;
    dqm:elementName "absolute or external accuracy" ;
    dqm:valueType "Measure" ;
    policy:status <http://www.opengis.net/def/status/valid> ;
    skos:altLabel "CEP" ;
    skos:definition "Radius describing a circle, in which the true point location lies with the probability of 50 %." ;
    skos:inScheme <https://standards.isotc211.org/19157/-3/1/dqc/content/qualityMeasure> ;
    skos:prefLabel "circular error probable" .

_:n61346038c5d14cc38e028ccb9d3332f8b56 a skos:Concept ;
    dcterms:date "2024-09-09 14:41:43.660" ;
    dcterms:hasVersion "1.0" ;
    dqm:elementName "absolute or external accuracy" ;
    dqm:valueType "Measure" ;
    policy:status <http://www.opengis.net/def/status/valid> ;
    skos:altLabel "circular map accuracy standard (CMAS)" ;
    skos:definition "Radius describing a circle, in which the true point location lies with the probability of 90 %." ;
    skos:inScheme <https://standards.isotc211.org/19157/-3/1/dqc/content/qualityMeasure> ;
    skos:prefLabel "circular error at 90 % significant level" .

_:n61346038c5d14cc38e028ccb9d3332f8b57 a skos:Concept ;
    dcterms:date "2024-09-09 14:41:43.660" ;
    dcterms:hasVersion "1.0" ;
    dqm:elementName "absolute or external accuracy" ;
    dqm:valueType "Measure" ;
    policy:status <http://www.opengis.net/def/status/valid> ;
    skos:altLabel "navigation accuracy" ;
    skos:definition "Radius describing a circle, in which the true point location lies with the probability of 95 %." ;
    skos:inScheme <https://standards.isotc211.org/19157/-3/1/dqc/content/qualityMeasure> ;
    skos:prefLabel "circular error at 95 % significance level" .

_:n61346038c5d14cc38e028ccb9d3332f8b58 a skos:Concept ;
    dcterms:date "2024-09-09 14:41:43.660" ;
    dcterms:hasVersion "1.0" ;
    dqm:elementName "absolute or external accuracy" ;
    dqm:valueType "Measure" ;
    policy:status <http://www.opengis.net/def/status/valid> ;
    skos:altLabel "CNCE" ;
    skos:definition "Radius describing a circle, in which the true point location lies with the probability of 99.8 %." ;
    skos:inScheme <https://standards.isotc211.org/19157/-3/1/dqc/content/qualityMeasure> ;
    skos:prefLabel "circular near certainty error" .

_:n61346038c5d14cc38e028ccb9d3332f8b7 a skos:Concept ;
    dcterms:date "2024-09-09 14:41:43.660" ;
    dcterms:hasVersion "1.0" ;
    dqm:elementName "omission" ;
    dqm:valueType "Boolean" ;
    policy:status <http://www.opengis.net/def/status/valid> ;
    skos:definition "Indicator that shows a specific item is missing in the data." ;
    skos:example "MD5e" ;
    skos:inScheme <https://standards.isotc211.org/19157/-3/1/dqc/content/qualityMeasure> ;
    skos:prefLabel "missing item" .

_:n61346038c5d14cc38e028ccb9d3332f8b8 a skos:Concept ;
    dcterms:date "2024-09-09 14:41:43.660" ;
    dcterms:hasVersion "1.0" ;
    dqm:elementName "commission" ;
    dqm:valueType "Boolean" ;
    policy:status <http://www.opengis.net/def/status/valid> ;
    skos:definition "Indication that an item is incorrectly present in the data." ;
    skos:example "MD1e" ;
    skos:inScheme <https://standards.isotc211.org/19157/-3/1/dqc/content/qualityMeasure> ;
    skos:prefLabel "excess item" .

_:n61346038c5d14cc38e028ccb9d3332f8b80 a skos:Concept ;
    dcterms:date "2024-09-09 14:41:43.660" ;
    dcterms:hasVersion "1.0" ;
    dqm:elementName "absolute or external accuracy" ;
    dqm:valueType "Number" ;
    policy:status <http://www.opengis.net/def/status/valid> ;
    skos:definition """Number of positional discrepancies above a given threshold for a set of positions in relation to the total number of measured positions.
The discrepancies are defined as the distance between a measured position and what is accepted as the corresponding true position.""" ;
    skos:example "MD31e" ;
    skos:inScheme <https://standards.isotc211.org/19157/-3/1/dqc/content/qualityMeasure> ;
    skos:prefLabel "rate of positional uncertainties above a given threshold" .

_:n61346038c5d14cc38e028ccb9d3332f8b84 a skos:Concept ;
    dcterms:date "2024-09-09 14:41:43.660" ;
    dcterms:hasVersion "1.0" ;
    dcterms:source <https://standards.isotc211.org/19157/-3/1/dqc/content/onlineResource/SR1> ;
    dqm:elementName "absolute or external accuracy" ;
    dqm:valueType "Measure" ;
    policy:status <http://www.opengis.net/def/status/valid> ;
    skos:altLabel "ALE" ;
    skos:definition "Absolute vertical accuracy of the data’s coordinates, expressed in terms of linear error at 90 % probability given that a bias is present." ;
    skos:inScheme <https://standards.isotc211.org/19157/-3/1/dqc/content/qualityMeasure> ;
    skos:prefLabel "absolute linear error at 90 % significance level of biased vertical data (Alternative 2)" .

_:n61346038c5d14cc38e028ccb9d3332f8b87 a skos:Concept ;
    dcterms:date "2024-09-09 14:41:43.660" ;
    dcterms:hasVersion "1.0" ;
    dcterms:source <https://standards.isotc211.org/19157/-3/1/dqc/content/onlineResource/SR1> ;
    dqm:elementName "absolute or external accuracy" ;
    dqm:valueType "Measure" ;
    policy:status <http://www.opengis.net/def/status/valid> ;
    skos:altLabel "ACE" ;
    skos:definition "Absolute horizontal accuracy of the data’s coordinates, expressed in terms of circular error at 90 % probability given that a bias is present." ;
    skos:inScheme <https://standards.isotc211.org/19157/-3/1/dqc/content/qualityMeasure> ;
    skos:prefLabel "absolute circular error at 90 % significance level of biased data" .

_:n61346038c5d14cc38e028ccb9d3332f8b89 a skos:Concept ;
    dcterms:date "2024-09-09 14:41:43.660" ;
    dcterms:hasVersion "1.0" ;
    dqm:elementName "absolute or external accuracy" ;
    dqm:valueStructure """Sequence
formula (a, b, φ) """ ;
    dqm:valueType "Measure" ;
    policy:status <http://www.opengis.net/def/status/valid> ;
    skos:altLabel "confidence point error ellipse" ;
    skos:definition "2D ellipse with the two main axes indicating the direction and magnitude of the highest and the lowest uncertainty of a 2D point." ;
    skos:inScheme <https://standards.isotc211.org/19157/-3/1/dqc/content/qualityMeasure> ;
    skos:prefLabel "confidence ellipse" .

_:n61346038c5d14cc38e028ccb9d3332f8b9 a skos:Concept ;
    dcterms:date "2024-09-09 14:41:43.660" ;
    dcterms:hasVersion "1.0" ;
    dqm:elementName "conceptual consistency" ;
    dqm:valueType "Boolean " ;
    policy:status <http://www.opengis.net/def/status/valid> ;
    skos:definition "Indication that events is incorrectly ordered against the other events." ;
    skos:example "MD159e" ;
    skos:inScheme <https://standards.isotc211.org/19157/-3/1/dqc/content/qualityMeasure> ;
    skos:prefLabel "chronological disorder" .

_:n61346038c5d14cc38e028ccb9d3332f8b90 a skos:Concept ;
    dcterms:date "2024-09-09 14:41:43.660" ;
    dcterms:hasVersion "1.0" ;
    dcterms:source <https://standards.isotc211.org/19157/-3/1/dqc/content/onlineResource/SR1> ;
    dqm:elementName "relative or internal accuracy" ;
    dqm:valueType "Measure" ;
    policy:status <http://www.opengis.net/def/status/valid> ;
    skos:altLabel "Rel LE90" ;
    skos:definition """Evaluation of the random errors of one relief feature to another in the same dataset or on the same map/chart.
It is a function of the random errors in the two elevations with respect to a common vertical datum.""" ;
    skos:inScheme <https://standards.isotc211.org/19157/-3/1/dqc/content/qualityMeasure> ;
    skos:prefLabel "relative vertical error" .

_:n61346038c5d14cc38e028ccb9d3332f8b91 a skos:Concept ;
    dcterms:date "2024-09-09 14:41:43.660" ;
    dcterms:hasVersion "1.0" ;
    dcterms:source <https://standards.isotc211.org/19157/-3/1/dqc/content/onlineResource/SR1> ;
    dqm:elementName "relative or internal accuracy" ;
    dqm:valueType "Measure" ;
    policy:status <http://www.opengis.net/def/status/valid> ;
    skos:altLabel "Rel CE90" ;
    skos:definition "Evaluation of the random errors in the horizontal position of one feature to another in the same dataset or on the same map/chart." ;
    skos:inScheme <https://standards.isotc211.org/19157/-3/1/dqc/content/qualityMeasure> ;
    skos:prefLabel "relative horizontal error" .

_:n61346038c5d14cc38e028ccb9d3332f8b92 a skos:Concept ;
    dcterms:date "2024-09-09 14:41:43.660" ;
    dcterms:hasVersion "1.0" ;
    dqm:elementName "classification correctness" ;
    dqm:valueStructure "Matrix (n × n)" ;
    dqm:valueType "Integer" ;
    policy:status <http://www.opengis.net/def/status/valid> ;
    skos:altLabel "confusion matrix" ;
    skos:definition "Matrix that indicates the number of items of class (i) classified as class (j)." ;
    skos:example "MD62e" ;
    skos:inScheme <https://standards.isotc211.org/19157/-3/1/dqc/content/qualityMeasure> ;
    skos:prefLabel "misclassification matrix" .

_:n61346038c5d14cc38e028ccb9d3332f8b93 a skos:Concept ;
    dcterms:date "2024-09-09 14:41:43.660" ;
    dcterms:hasVersion "1.0" ;
    dqm:elementName "classification correctness" ;
    dqm:valueStructure "Matrix (n × n)" ;
    dqm:valueType "Real" ;
    policy:status <http://www.opengis.net/def/status/valid> ;
    skos:definition "Matrix that indicates the number of items of class (i ) classified as class (j ) divided by the number of items of class (i )." ;
    skos:example "MD63e" ;
    skos:inScheme <https://standards.isotc211.org/19157/-3/1/dqc/content/qualityMeasure> ;
    skos:prefLabel "relative misclassification matrix" .

_:n61346038c5d14cc38e028ccb9d3332f8b94 a skos:Concept ;
    dcterms:date "2024-09-09 14:41:43.660" ;
    dcterms:hasVersion "1.0" ;
    dqm:elementName "classification correctness" ;
    dqm:valueType "Real" ;
    skos:definition "Coefficient to quantify the proportion of agreement of assignments to classes by removing misclassifications." ;
    skos:inScheme <https://standards.isotc211.org/19157/-3/1/dqc/content/qualityMeasure> ;
    skos:prefLabel "kappa coefficient" .

_:n61346038c5d14cc38e028ccb9d3332f8b13 a skos:Concept ;
    dcterms:date "2024-09-09 14:41:43.660" ;
    dcterms:hasVersion "0.1" ;
    dqm:elementName "conceptual consistency" ;
    dqm:valueType "Real" ;
    policy:status <http://www.opengis.net/def/status/submitted> ;
    skos:definition "Rate of items in a common area representing the same real world object with different coordinates in two different datasets according to a tolerance." ;
    skos:inScheme <https://standards.isotc211.org/19157/-3/1/dqc/content/qualityMeasure> ;
    skos:prefLabel "rate of geometric inconsistency" .

_:n61346038c5d14cc38e028ccb9d3332f8b19 a skos:Concept ;
    dcterms:date "2024-09-09 14:41:43.660" ;
    dcterms:hasVersion "0.1" ;
    dcterms:source <https://standards.isotc211.org/19157/-3/1/dqc/content/onlineResource/SR2> ;
    dqm:elementName "conceptual consistency" ;
    dqm:valueType "Rate" ;
    policy:status <http://www.opengis.net/def/status/submitted> ;
    skos:definition "Error rate of difference between registered geometry in the dataset and the actual geometry of the real world object." ;
    skos:inScheme <https://standards.isotc211.org/19157/-3/1/dqc/content/qualityMeasure> ;
    skos:prefLabel "rate of geometric fidelity failure" .

_:n61346038c5d14cc38e028ccb9d3332f8b22 a skos:Concept ;
    dcterms:date "2024-09-09 14:41:43.660" ;
    dcterms:hasVersion "0.1" ;
    dcterms:source <https://standards.isotc211.org/19157/-3/1/dqc/content/onlineResource/SR3> ;
    dqm:elementName "topological consistency" ;
    dqm:valueType "Real" ;
    policy:status <http://www.opengis.net/def/status/submitted> ;
    skos:altLabel "Tessellation complete" ;
    skos:definition "Total number of erroneous polygons within the data." ;
    skos:example "MD204e" ;
    skos:inScheme <https://standards.isotc211.org/19157/-3/1/dqc/content/qualityMeasure> ;
    skos:prefLabel "Complete tessellation" .

_:n61346038c5d14cc38e028ccb9d3332f8b25 a skos:Concept ;
    dcterms:date "2024-09-09 14:41:43.660" ;
    dcterms:hasVersion "1.0" ;
    dqm:elementName "absolute or external accuracy" ;
    dqm:valueType "Integer" ;
    policy:status <http://www.opengis.net/def/status/valid> ;
    skos:definition """Number of positional discrepancies above a given threshold for a set of positions.
The discrepancies are defined as the distance between a measured position and what is accepted as the corresponding true position.""" ;
    skos:inScheme <https://standards.isotc211.org/19157/-3/1/dqc/content/qualityMeasure> ;
    skos:prefLabel "number of positional uncertainties above a given threshold" .

_:n61346038c5d14cc38e028ccb9d3332f8b26 a skos:Concept ;
    dcterms:date "2024-09-09 14:41:43.660" ;
    dcterms:hasVersion "1.0" ;
    dqm:elementName "topological consistency" ;
    dqm:valueType "Integer" ;
    policy:status <http://www.opengis.net/def/status/valid> ;
    skos:altLabel "overshoots" ;
    skos:definition "Count of items in the dataset, within the parameter tolerance, that are mismatched due to overshoots." ;
    skos:example "MD24e" ;
    skos:inScheme <https://standards.isotc211.org/19157/-3/1/dqc/content/qualityMeasure> ;
    skos:prefLabel "number of missing connections due to overshoots" .

_:n61346038c5d14cc38e028ccb9d3332f8b30 a skos:Concept ;
    dcterms:date "2024-09-09 14:41:43.660" ;
    dcterms:hasVersion "1.0" ;
    dcterms:source <https://standards.isotc211.org/19157/-3/1/dqc/content/onlineResource/SR6> ;
    dqm:elementName "topological consistency" ;
    dqm:valueType "Integer" ;
    policy:status <http://www.opengis.net/def/status/valid> ;
    skos:altLabel "slivers" ;
    skos:definition "Count of all items in the dataset that are invalid sliver surfaces." ;
    skos:example """MD25e_1
MD25e_2""" ;
    skos:inScheme <https://standards.isotc211.org/19157/-3/1/dqc/content/qualityMeasure> ;
    skos:prefLabel "number of invalid slivers" .

_:n61346038c5d14cc38e028ccb9d3332f8b39 a skos:Concept ;
    dcterms:date "2024-09-09 14:41:43.660" ;
    dcterms:hasVersion "1.0" ;
    dqm:elementName "topological consistency" ;
    dqm:valueType "Integer" ;
    policy:status <http://www.opengis.net/def/status/valid> ;
    skos:altLabel "undershoots" ;
    skos:definition "Count of items in the dataset, within the parameter tolerance, that are mismatched due to undershoots." ;
    skos:example "MD23e" ;
    skos:inScheme <https://standards.isotc211.org/19157/-3/1/dqc/content/qualityMeasure> ;
    skos:prefLabel "number of missing connections due to undershoot" .

_:n61346038c5d14cc38e028ccb9d3332f8b40 a skos:Concept ;
    dcterms:date "2024-09-09 14:41:43.660" ;
    dcterms:hasVersion "0.1" ;
    dqm:elementName "conceptual consistency" ;
    dqm:valueType "Integer" ;
    policy:status <http://www.opengis.net/def/status/submitted> ;
    skos:definition "Number of differences between registered geometry in the dataset and the actual geometry of the real world object." ;
    skos:example "MD202e" ;
    skos:inScheme <https://standards.isotc211.org/19157/-3/1/dqc/content/qualityMeasure> ;
    skos:prefLabel "count of geometric fidelity failure" .

_:n61346038c5d14cc38e028ccb9d3332f8b43 a skos:Concept ;
    dcterms:date "2024-09-09 14:41:43.660" ;
    dcterms:hasVersion "0.1" ;
    dcterms:source <https://standards.isotc211.org/19157/-3/1/dqc/content/onlineResource/SR4> ;
    dqm:elementName "temporal validity" ;
    dqm:valueType "Boolean" ;
    policy:status <http://www.opengis.net/def/status/submitted> ;
    skos:definition "Evaluation if a dataset is maintained as set by maintenance frequency." ;
    skos:example "MD206e" ;
    skos:inScheme <https://standards.isotc211.org/19157/-3/1/dqc/content/qualityMeasure> ;
    skos:prefLabel "maintenance frequency" .

_:n61346038c5d14cc38e028ccb9d3332f8b47 a skos:Concept ;
    dcterms:date "2024-09-09 14:41:43.660" ;
    dcterms:hasVersion "0.1" ;
    dqm:elementName "temporal validity" ;
    dqm:valueType "Boolean" ;
    policy:status <http://www.opengis.net/def/status/submitted> ;
    skos:definition "Evaluation of acceptance quality limit, AQL for user defined maintenance frequency from a feature has changed in the real world until it is updated in the database." ;
    skos:example "MD205e" ;
    skos:inScheme <https://standards.isotc211.org/19157/-3/1/dqc/content/qualityMeasure> ;
    skos:prefLabel "user defined maintenance frequency" .

_:n61346038c5d14cc38e028ccb9d3332f8b52 a skos:Concept ;
    dcterms:date "2024-09-09 14:41:43.660" ;
    dcterms:hasVersion "0.1" ;
    dcterms:source <https://standards.isotc211.org/19157/-3/1/dqc/content/onlineResource/SR7> ;
    dqm:elementName "temporal validity" ;
    dqm:valueType "Real" ;
    policy:status <http://www.opengis.net/def/status/submitted> ;
    skos:definition "Degree to which data has attributes that are of the right age in a specific context of use." ;
    skos:example "M207e" ;
    skos:inScheme <https://standards.isotc211.org/19157/-3/1/dqc/content/qualityMeasure> ;
    skos:prefLabel "currentness" .

_:n61346038c5d14cc38e028ccb9d3332f8b78 a skos:Concept ;
    dcterms:date "2024-09-09 14:41:43.660" ;
    dcterms:hasVersion "1.0" ;
    dqm:elementName "absolute or external accuracy" ;
    policy:status <http://www.opengis.net/def/status/valid> ;
    skos:definition "Mean value of the positional uncertainties for a set of positions where the positional uncertainties are defined as the distance between a measured position and what is accepted as the corresponding true position." ;
    skos:example "MD28e" ;
    skos:inScheme <https://standards.isotc211.org/19157/-3/1/dqc/content/qualityMeasure> ;
    skos:prefLabel "mean value of positional uncertainties (1D, 2D and 3D)" .

_:n61346038c5d14cc38e028ccb9d3332f8b79 a skos:Concept ;
    dcterms:date "2024-09-09 14:41:43.660" ;
    dcterms:hasVersion "1.0" ;
    dqm:elementName "absolute or external accuracy" ;
    dqm:valueType "Real" ;
    policy:status <http://www.opengis.net/def/status/valid> ;
    skos:definition "For a set of points where the discrepancy does not exceed a defined threshold, the arithmetical average of discrepancies between their measured positions and what is accepted as the corresponding true positions." ;
    skos:inScheme <https://standards.isotc211.org/19157/-3/1/dqc/content/qualityMeasure> ;
    skos:prefLabel "mean value of positional uncertainties excluding outliers (1D, 2D, 3D)" .

_:n61346038c5d14cc38e028ccb9d3332f8b81 a skos:Concept ;
    dcterms:date "2024-09-09 14:41:43.660" ;
    dcterms:hasVersion "1.0" ;
    dqm:elementName "absolute or external accuracy" ;
    dqm:valueStructure "Matrix" ;
    dqm:valueType "Real" ;
    policy:status <http://www.opengis.net/def/status/valid> ;
    skos:altLabel "variance-covariance matrix" ;
    skos:definition "Symmetrical square matrix with variances of point discrepancies on the main diagonal and covariance between these discrepancies as off-diagonal elements." ;
    skos:inScheme <https://standards.isotc211.org/19157/-3/1/dqc/content/qualityMeasure> ;
    skos:prefLabel "covariance matrix" .

_:n61346038c5d14cc38e028ccb9d3332f8b6 a skos:Concept ;
    dcterms:date "2024-09-09 14:41:43.660" ;
    dcterms:hasVersion "1.0" ;
    dqm:elementName "accuracy of a time measurement" ;
    dqm:valueType "Measure" ;
    policy:status <http://www.opengis.net/def/status/valid> ;
    skos:definition "Half length of the interval defined by an upper and a lower limit, in which the true value for the time instance lies with probability 99.8 %." ;
    skos:inScheme <https://standards.isotc211.org/19157/-3/1/dqc/content/qualityMeasure> ;
    skos:prefLabel "time accuracy at 99,8 % significance level" .

_:n61346038c5d14cc38e028ccb9d3332f8b60 a skos:Concept ;
    dcterms:date "2024-09-09 14:41:43.660" ;
    dcterms:hasVersion "1.0" ;
    dqm:elementName "accuracy of a time measurement" ;
    dqm:valueType "Measure" ;
    policy:status <http://www.opengis.net/def/status/valid> ;
    skos:definition "Half length of the interval defined by an upper and a lower limit, in which the true value for the time instance lies with probability 50 %." ;
    skos:inScheme <https://standards.isotc211.org/19157/-3/1/dqc/content/qualityMeasure> ;
    skos:prefLabel "time accuracy at 50 % significance level" .

_:n61346038c5d14cc38e028ccb9d3332f8b61 a skos:Concept ;
    dcterms:date "2024-09-09 14:41:43.660" ;
    dcterms:hasVersion "1.0" ;
    dqm:elementName "absolute or external accuracy" ;
    dqm:valueType "Measure" ;
    policy:status <http://www.opengis.net/def/status/valid> ;
    skos:altLabel "LEP" ;
    skos:definition "Half length of the interval defined by an upper and a lower limit, in which the true value lies with probability 50 %." ;
    skos:inScheme <https://standards.isotc211.org/19157/-3/1/dqc/content/qualityMeasure> ;
    skos:prefLabel "linear error probable" .

_:n61346038c5d14cc38e028ccb9d3332f8b62 a skos:Concept ;
    dcterms:date "2024-09-09 14:41:43.660" ;
    dcterms:hasVersion "1.0" ;
    dqm:elementName "accuracy of a time measurement" ;
    dqm:valueType "Measure" ;
    policy:status <http://www.opengis.net/def/status/valid> ;
    skos:definition "Half length of the interval defined by an upper and a lower limit, in which the true value for the time instance lies with probability 68.3 %." ;
    skos:inScheme <https://standards.isotc211.org/19157/-3/1/dqc/content/qualityMeasure> ;
    skos:prefLabel "time accuracy at 68,3 % significance level" .

_:n61346038c5d14cc38e028ccb9d3332f8b63 a skos:Concept ;
    dcterms:date "2024-09-09 14:41:43.660" ;
    dcterms:hasVersion "1.0" ;
    dqm:elementName "absolute or external accuracy" ;
    dqm:valueType "Measure" ;
    policy:status <http://www.opengis.net/def/status/valid> ;
    skos:altLabel "SLE" ;
    skos:definition "Half length of the interval defined by an upper and a lower limit, in which the true value lies with probability 68.3 %." ;
    skos:inScheme <https://standards.isotc211.org/19157/-3/1/dqc/content/qualityMeasure> ;
    skos:prefLabel "standard linear error" .

_:n61346038c5d14cc38e028ccb9d3332f8b1 a skos:Concept ;
    dcterms:date "2024-09-09 14:41:43.660" ;
    dcterms:hasVersion "1.0" ;
    dqm:elementName "absolute or external accuracy" ;
    dqm:valueType "Measure" ;
    policy:status <http://www.opengis.net/def/status/valid> ;
    skos:altLabel "LMAS 99 %" ;
    skos:definition "Half length of the interval defined by an upper and a lower limit, in which the true value lies with probability 99 %." ;
    skos:inScheme <https://standards.isotc211.org/19157/-3/1/dqc/content/qualityMeasure> ;
    skos:prefLabel "linear map accuracy at 99 % significance level" .

_:n61346038c5d14cc38e028ccb9d3332f8b2 a skos:Concept ;
    dcterms:date "2024-09-09 14:41:43.660" ;
    dcterms:hasVersion "1.0" ;
    dqm:elementName "absolute or external accuracy" ;
    dqm:valueType "Measure" ;
    policy:status <http://www.opengis.net/def/status/valid> ;
    skos:altLabel "LMAS 95 %" ;
    skos:definition "Half length of the interval defined by an upper and a lower limit, in which the true value lies with probability 95 %." ;
    skos:inScheme <https://standards.isotc211.org/19157/-3/1/dqc/content/qualityMeasure> ;
    skos:prefLabel "linear map accuracy at 95 % significance level" .

_:n61346038c5d14cc38e028ccb9d3332f8b3 a skos:Concept ;
    dcterms:date "2024-09-09 14:41:43.660" ;
    dcterms:hasVersion "1.0" ;
    dqm:elementName "quantitative attribute accuracy" ;
    dqm:valueType "Measure" ;
    policy:status <http://www.opengis.net/def/status/valid> ;
    skos:definition "Half length of the interval defined by an upper and a lower limit, in which the true value for the quantitative attribute lies with probability 99.8 %." ;
    skos:inScheme <https://standards.isotc211.org/19157/-3/1/dqc/content/qualityMeasure> ;
    skos:prefLabel "Attribute value uncertainty at 99,8 % significance level" .

_:n61346038c5d14cc38e028ccb9d3332f8b4 a skos:Concept ;
    dcterms:date "2024-09-09 14:41:43.660" ;
    dcterms:hasVersion "1.0" ;
    dqm:elementName "absolute or external accuracy" ;
    dqm:valueType "Measure" ;
    policy:status <http://www.opengis.net/def/status/valid> ;
    skos:altLabel "LMAS 90 %" ;
    skos:definition "Half length of the interval defined by an upper and a lower limit, in which the true value lies with probability 90 %." ;
    skos:inScheme <https://standards.isotc211.org/19157/-3/1/dqc/content/qualityMeasure> ;
    skos:prefLabel "linear map accuracy at 90 % significance level" .

_:n61346038c5d14cc38e028ccb9d3332f8b5 a skos:Concept ;
    dcterms:date "2024-09-09 14:41:43.660" ;
    dcterms:hasVersion "1.0" ;
    dqm:elementName "absolute or external accuracy" ;
    dqm:valueType "Measure" ;
    policy:status <http://www.opengis.net/def/status/valid> ;
    skos:definition "Half length of the interval defined by an upper and a lower limit, in which the true value lies with probability 99.8 %." ;
    skos:inScheme <https://standards.isotc211.org/19157/-3/1/dqc/content/qualityMeasure> ;
    skos:prefLabel "near certainty linear error" .

_:n61346038c5d14cc38e028ccb9d3332f8b59 a skos:Concept ;
    dcterms:date "2024-09-09 14:41:43.660" ;
    dcterms:hasVersion "1.0" ;
    dqm:elementName "quantitative attribute accuracy" ;
    dqm:valueType "Measure" ;
    policy:status <http://www.opengis.net/def/status/valid> ;
    skos:definition "Half length of the interval defined by an upper and a lower limit, in which the true value for the quantitative attribute lies with probability 50 %." ;
    skos:inScheme <https://standards.isotc211.org/19157/-3/1/dqc/content/qualityMeasure> ;
    skos:prefLabel "attribute value uncertainty at 50 % significance level" .

_:n61346038c5d14cc38e028ccb9d3332f8b64 a skos:Concept ;
    dcterms:date "2024-09-09 14:41:43.660" ;
    dcterms:hasVersion "1.0" ;
    dqm:elementName "quantitative attribute accuracy" ;
    dqm:valueType "Measure" ;
    policy:status <http://www.opengis.net/def/status/valid> ;
    skos:definition "Half length of the interval defined by an upper and a lower limit, in which the true value for the quantitative attribute lies with probability 68.3 %." ;
    skos:inScheme <https://standards.isotc211.org/19157/-3/1/dqc/content/qualityMeasure> ;
    skos:prefLabel "attribute value uncertainty at 68,3 % significance level" .

_:n61346038c5d14cc38e028ccb9d3332f8b65 a skos:Concept ;
    dcterms:date "2024-09-09 14:41:43.660" ;
    dcterms:hasVersion "1.0" ;
    dqm:elementName "accuracy of a time measurement" ;
    dqm:valueType "Measure" ;
    policy:status <http://www.opengis.net/def/status/valid> ;
    skos:definition "Half length of the interval defined by an upper and a lower limit, in which the true value for the time instance lies with probability 90 %." ;
    skos:inScheme <https://standards.isotc211.org/19157/-3/1/dqc/content/qualityMeasure> ;
    skos:prefLabel "time accuracy at 90 % significance level" .

_:n61346038c5d14cc38e028ccb9d3332f8b66 a skos:Concept ;
    dcterms:date "2024-09-09 14:41:43.660" ;
    dcterms:hasVersion "1.0" ;
    dqm:elementName "quantitative attribute accuracy" ;
    dqm:valueType "Measure" ;
    policy:status <http://www.opengis.net/def/status/valid> ;
    skos:definition "Half length of the interval defined by an upper and a lower limit, in which the true value for the quantitative attribute lies with probability 90 %." ;
    skos:inScheme <https://standards.isotc211.org/19157/-3/1/dqc/content/qualityMeasure> ;
    skos:prefLabel "attribute value uncertainty at 90 % significance level" .

_:n61346038c5d14cc38e028ccb9d3332f8b67 a skos:Concept ;
    dcterms:date "2024-09-09 14:41:43.660" ;
    dcterms:hasVersion "1.0" ;
    dqm:elementName "accuracy of a time measurement" ;
    dqm:valueType "Measure" ;
    policy:status <http://www.opengis.net/def/status/valid> ;
    skos:definition "Half length of the interval defined by an upper and a lower limit, in which the true value for the time instance lies with probability 95 %." ;
    skos:inScheme <https://standards.isotc211.org/19157/-3/1/dqc/content/qualityMeasure> ;
    skos:prefLabel "time accuracy at 95 % significance level" .

_:n61346038c5d14cc38e028ccb9d3332f8b68 a skos:Concept ;
    dcterms:date "2024-09-09 14:41:43.660" ;
    dcterms:hasVersion "1.0" ;
    dqm:elementName "quantitative attribute accuracy" ;
    dqm:valueType "Measure" ;
    policy:status <http://www.opengis.net/def/status/valid> ;
    skos:definition "Half length of the interval defined by an upper and a lower limit, in which the true value for the quantitative attribute lies with probability 95 %." ;
    skos:inScheme <https://standards.isotc211.org/19157/-3/1/dqc/content/qualityMeasure> ;
    skos:prefLabel "attribute value uncertainty at 95 % significance level" .

_:n61346038c5d14cc38e028ccb9d3332f8b69 a skos:Concept ;
    dcterms:date "2024-09-09 14:41:43.660" ;
    dcterms:hasVersion "1.0" ;
    dqm:elementName "accuracy of a time measurement" ;
    dqm:valueType "Measure" ;
    policy:status <http://www.opengis.net/def/status/valid> ;
    skos:definition "Half length of the interval defined by an upper and a lower limit, in which the true value for the time instance lies with probability 99 %." ;
    skos:inScheme <https://standards.isotc211.org/19157/-3/1/dqc/content/qualityMeasure> ;
    skos:prefLabel "time accuracy at 99 % significance level" .

_:n61346038c5d14cc38e028ccb9d3332f8b70 a skos:Concept ;
    dcterms:date "2024-09-09 14:41:43.660" ;
    dcterms:hasVersion "1.0" ;
    dqm:elementName "quantitative attribute accuracy" ;
    dqm:valueType "Measure" ;
    policy:status <http://www.opengis.net/def/status/valid> ;
    skos:definition "Half length of the interval defined by an upper and a lower limit, in which the true value for the quantitative attribute lies with probability 99 %." ;
    skos:inScheme <https://standards.isotc211.org/19157/-3/1/dqc/content/qualityMeasure> ;
    skos:prefLabel "attribute value uncertainty at 99 % significance level" .

