@prefix dcterms: <http://purl.org/dc/terms/> .
@prefix prov: <http://www.w3.org/ns/prov#> .
@prefix rdfs: <http://www.w3.org/2000/01/rdf-schema#> .
@prefix schema: <https://schema.org/> .
@prefix skos: <http://www.w3.org/2004/02/skos/core#> .
@prefix xsd: <http://www.w3.org/2001/XMLSchema#> .

<https://raw.githubusercontent.com/ogcincubator/iso19157-3-dqm-register/master/sources/entailed/SourceReference.csv.ttl> a prov:Entity ;
    dcterms:format "text/turtle" ;
    dcterms:hasVersion "git:6f93445715758528e2bb5810810e23ae07990368" ;
    prov:wasAttributedTo _:N1c3c0dc7e67e43269add3f23fbfa5b37 ;
    prov:wasGeneratedBy [ a prov:Activity ;
            rdfs:label "Entailment and validation" ;
            rdfs:comment "python ogc.na.update_vocabs -w . .ogc/catalog.ttl --batch --base-uri https://raw.githubusercontent.com/ogcincubator/iso19157-3-dqm-register/master --update --graph-store http://defs-dev.opengis.net:8061/fuseki-hosted/data" ;
            prov:endedAtTime "2024-09-24T02:18:08.331437"^^xsd:dateTime ;
            prov:startedAtTime "2024-09-24T02:18:08.161927"^^xsd:dateTime ;
            prov:used [ a prov:Entity ;
                    dcterms:format "text/turtle" ;
                    dcterms:hasVersion "git:6f93445715758528e2bb5810810e23ae07990368" ;
                    rdfs:seeAlso <https://raw.githubusercontent.com/ogcincubator/iso19157-3-dqm-register/master/.ogc/catalog.ttl> ],
                [ a prov:Entity ;
                    rdfs:seeAlso <entailments.shapes.ttl> ],
                [ a prov:Entity ;
                    dcterms:format "text/turtle" ;
                    dcterms:hasVersion "git:6f93445715758528e2bb5810810e23ae07990368" ;
                    rdfs:seeAlso <https://raw.githubusercontent.com/ogcincubator/iso19157-3-dqm-register/master/sources/SourceReference.csv.ttl> ] ;
            prov:wasAssociatedWith _:N1c3c0dc7e67e43269add3f23fbfa5b37 ;
            prov:wasInformedBy [ dcterms:identifier "754bb239-028c-44cd-a661-8f6cc1963c94" ] ] .

<https://standards.isotc211.org/19157/-3/1/dqc/content/onlineResource/SR1> a skos:Concept ;
    dcterms:source "https://standards.globalspec.com/std/1296998/stanag-2215" ;
    skos:definition "NATO STANAG 2215 IGEO" ;
    skos:inScheme <https://standards.isotc211.org/19157/-3/1/dqc/content/onlineResource> ;
    skos:prefLabel "NATO STANAG 2215 IGEO" .

<https://standards.isotc211.org/19157/-3/1/dqc/content/onlineResource/SR2> a skos:Concept ;
    dcterms:source "https://www.ordnancesurvey.co.uk/documents/os-mastermap-real-world-object-catalogue.pdf" ;
    skos:definition """Ordnance Survey topo-96 (2007), redefined
""" ;
    skos:inScheme <https://standards.isotc211.org/19157/-3/1/dqc/content/onlineResource> ;
    skos:prefLabel """Ordnance Survey topo-96 (2007), redefined
""" .

<https://standards.isotc211.org/19157/-3/1/dqc/content/onlineResource/SR3> a skos:Concept ;
    dcterms:source "https://doi.org/10.5593/sgem2017/21/S08.112" ;
    skos:definition "Exploring subset profile and validation procedures of geographical markup language (GML) for 3D areal plan information. " ;
    skos:inScheme <https://standards.isotc211.org/19157/-3/1/dqc/content/onlineResource> ;
    skos:prefLabel "Exploring subset profile and validation procedures of geographical markup language (GML) for 3D areal plan information. " .

<https://standards.isotc211.org/19157/-3/1/dqc/content/onlineResource/SR4> a skos:Concept ;
    dcterms:source "https://schemas.isotc211.org/19115/-1/mmi/1.3.0/" ;
    skos:definition "ISO 19115-1 Geographic information - Metadata - Part 1: Fundamentals" ;
    skos:inScheme <https://standards.isotc211.org/19157/-3/1/dqc/content/onlineResource> ;
    skos:prefLabel "ISO 19115-1 Geographic information - Metadata - Part 1: Fundamentals" .

<https://standards.isotc211.org/19157/-3/1/dqc/content/onlineResource/SR5> a skos:Concept ;
    dcterms:source "https://doi.org/10.1016/j.jag.2022.103094" ;
    skos:definition "Yujun Hou and Filip Biljecki (2022). A comprehensive framework for evaluating the quality of street view imagery" ;
    skos:inScheme <https://standards.isotc211.org/19157/-3/1/dqc/content/onlineResource> ;
    skos:prefLabel "Yujun Hou and Filip Biljecki (2022). A comprehensive framework for evaluating the quality of street view imagery" .

<https://standards.isotc211.org/19157/-3/1/dqc/content/onlineResource/SR6> a skos:Concept ;
    dcterms:source "https://support.esri.com/en-us/technical-paper/plts-gis-data-reviewer-4-2-528" ;
    skos:definition "Environmental Systems Research Institute, Inc (ERSI) GSI Data ReViewer 4.2 User Guide" ;
    skos:inScheme <https://standards.isotc211.org/19157/-3/1/dqc/content/onlineResource> ;
    skos:prefLabel "Environmental Systems Research Institute, Inc (ERSI) GSI Data ReViewer 4.2 User Guide" .

<https://standards.isotc211.org/19157/-3/1/dqc/content/onlineResource/SR7> a skos:Concept ;
    dcterms:source "https://www.iso.org/standard/35736.html" ;
    skos:definition "ISO/IEC 25012:2008 Software engineering — Software product Quality Requirements and Evaluation (SQuaRE) — Data quality model" ;
    skos:inScheme <https://standards.isotc211.org/19157/-3/1/dqc/content/onlineResource> ;
    skos:prefLabel "ISO/IEC 25012:2008 Software engineering — Software product Quality Requirements and Evaluation (SQuaRE) — Data quality model" .

<https://standards.isotc211.org/19157/-3/1/dqc/content/onlineResource> a skos:ConceptScheme ;
    skos:definition "ISO19157-3 Quality Source References" ;
    skos:prefLabel "ISO19157-3 Quality Source References" .

[] a prov:Activity ;
    prov:endedAtTime "2024-09-24T02:16:43.908785"^^xsd:dateTime ;
    prov:startedAtTime "2024-09-24T02:16:43.854003"^^xsd:dateTime ;
    prov:used [ a prov:Entity ;
            dcterms:format "application/json" ;
            dcterms:hasVersion "git:660e477c7d570211a32a80451ec03fe2909a0676" ;
            rdfs:seeAlso <file:///home/runner/work/iso19157-3-dqm-register/iso19157-3-dqm-register/sources/SourceReference.csv.json> ] ;
    prov:wasAssociatedWith [ a prov:Agent,
                schema:SoftwareApplication ;
            rdfs:label "OGC-NA tools" ;
            dcterms:hasVersion "0.3.53" ;
            rdfs:seeAlso <https://github.com/opengeospatial/ogc-na-tools> ] ;
    prov:wasInformedBy [ dcterms:identifier "e724770a-e4ee-42b6-9b62-2d4052686b0b" ] .

_:N1c3c0dc7e67e43269add3f23fbfa5b37 a prov:Agent,
        schema:SoftwareApplication ;
    rdfs:label "OGC-NA tools" ;
    dcterms:hasVersion "0.3.53" ;
    rdfs:comment "ogc.na.update_vocabs version 0.3.53" ;
    rdfs:seeAlso <https://github.com/opengeospatial/ogc-na-tools> .

